<?xml version="1.0"?>
<rdf:RDF xmlns="http://www.semanticweb.org/bbucher/ontologies/2025/9/geodata#"
     xml:base="http://www.semanticweb.org/bbucher/ontologies/2025/9/geodata"
     xmlns:dc="http://purl.org/dc/elements/1.1/"
     xmlns:ns="http://creativecommons.org/ns#"
     xmlns:org="http://www.w3.org/ns/org#"
     xmlns:owl="http://www.w3.org/2002/07/owl#"
     xmlns:pav="http://purl.org/pav/"
     xmlns:rdf="http://www.w3.org/1999/02/22-rdf-syntax-ns#"
     xmlns:xml="http://www.w3.org/XML/1998/namespace"
     xmlns:xsd="http://www.w3.org/2001/XMLSchema#"
     xmlns:adms="http://www.w3.org/ns/adms#"
     xmlns:bibo="http://purl.org/ontology/bibo/"
     xmlns:dcam="http://purl.org/dc/dcam/"
     xmlns:dcat="http://www.w3.org/ns/dcat#"
     xmlns:foaf="http://xmlns.com/foaf/0.1/"
     xmlns:prov="http://www.w3.org/ns/prov#"
     xmlns:rdfs="http://www.w3.org/2000/01/rdf-schema#"
     xmlns:skos="http://www.w3.org/2004/02/skos/core#"
     xmlns:time="http://www.w3.org/2006/time#"
     xmlns:vann="http://purl.org/vocab/vann/"
     xmlns:terms="http://purl.org/dc/terms/"
     xmlns:vocab="http://www.w3.org/1999/xhtml/vocab#"
     xmlns:schema="http://schema.org/">
    <owl:Ontology rdf:about="http://www.semanticweb.org/bbucher/ontologies/2025/9/geodata">
        <owl:imports rdf:resource="http://data.ign.fr/def/topo#"/>
        <owl:imports rdf:resource="http://www.w3.org/2004/02/skos/core"/>
        <owl:imports rdf:resource="http://www.w3.org/ns/dcat3"/>
        <owl:imports rdf:resource="http://www.w3.org/ns/prov#"/>
        <terms:title xml:lang="fr">Ontologie des jeux de données géospatiales</terms:title>
        <terms:title xml:lang="en">Ontology for Geospatial Datasets</terms:title>
        <vann:preferredNamespacePrefix>geodata</vann:preferredNamespacePrefix>
        <vann:preferredNamespaceUri rdf:resource="https://intforout.github.io/geodata#"/>
        <rdfs:comment>Ontology to describe geodatasets in support of knowledge production and transfer</rdfs:comment>
    </owl:Ontology>
    


    <!-- 
    ///////////////////////////////////////////////////////////////////////////////////////
    //
    // Annotation properties
    //
    ///////////////////////////////////////////////////////////////////////////////////////
     -->


    


    <!-- http://creativecommons.org/ns#license -->


    <owl:AnnotationProperty rdf:about="http://creativecommons.org/ns#license"/>
    


    <!-- http://purl.org/dc/terms/abstract -->


    <rdf:Description rdf:about="http://purl.org/dc/terms/abstract">
        <rdfs:subPropertyOf rdf:resource="http://purl.org/dc/elements/1.1/description"/>
        <rdfs:subPropertyOf rdf:resource="http://purl.org/dc/terms/description"/>
    </rdf:Description>
    


    <!-- http://purl.org/dc/terms/accessRights -->


    <rdf:Description rdf:about="http://purl.org/dc/terms/accessRights">
        <rdfs:subPropertyOf rdf:resource="http://purl.org/dc/elements/1.1/rights"/>
        <rdfs:subPropertyOf rdf:resource="http://purl.org/dc/terms/rights"/>
    </rdf:Description>
    


    <!-- http://purl.org/dc/terms/accrualMethod -->


    <rdf:Description rdf:about="http://purl.org/dc/terms/accrualMethod">
        <rdfs:domain rdf:resource="http://purl.org/dc/dcmitype/Collection"/>
    </rdf:Description>
    


    <!-- http://purl.org/dc/terms/accrualPeriodicity -->


    <rdf:Description rdf:about="http://purl.org/dc/terms/accrualPeriodicity">
        <rdfs:domain rdf:resource="http://purl.org/dc/dcmitype/Collection"/>
    </rdf:Description>
    


    <!-- http://purl.org/dc/terms/accrualPolicy -->


    <rdf:Description rdf:about="http://purl.org/dc/terms/accrualPolicy">
        <rdfs:domain rdf:resource="http://purl.org/dc/dcmitype/Collection"/>
    </rdf:Description>
    


    <!-- http://purl.org/dc/terms/alternative -->


    <rdf:Description rdf:about="http://purl.org/dc/terms/alternative">
        <rdfs:subPropertyOf rdf:resource="http://purl.org/dc/elements/1.1/title"/>
    </rdf:Description>
    


    <!-- http://purl.org/dc/terms/available -->


    <rdf:Description rdf:about="http://purl.org/dc/terms/available">
        <rdfs:subPropertyOf rdf:resource="http://purl.org/dc/elements/1.1/date"/>
    </rdf:Description>
    


    <!-- http://purl.org/dc/terms/bibliographicCitation -->


    <rdf:Description rdf:about="http://purl.org/dc/terms/bibliographicCitation">
        <rdfs:subPropertyOf rdf:resource="http://purl.org/dc/elements/1.1/identifier"/>
    </rdf:Description>
    


    <!-- http://purl.org/dc/terms/conformsTo -->


    <rdf:Description rdf:about="http://purl.org/dc/terms/conformsTo">
        <rdfs:subPropertyOf rdf:resource="http://purl.org/dc/elements/1.1/relation"/>
        <rdfs:subPropertyOf rdf:resource="http://purl.org/dc/terms/relation"/>
    </rdf:Description>
    


    <!-- http://purl.org/dc/terms/contributor -->


    <owl:AnnotationProperty rdf:about="http://purl.org/dc/terms/contributor">
        <rdfs:subPropertyOf rdf:resource="http://purl.org/dc/elements/1.1/contributor"/>
    </owl:AnnotationProperty>
    


    <!-- http://purl.org/dc/terms/coverage -->


    <rdf:Description rdf:about="http://purl.org/dc/terms/coverage">
        <rdfs:subPropertyOf rdf:resource="http://purl.org/dc/elements/1.1/coverage"/>
    </rdf:Description>
    


    <!-- http://purl.org/dc/terms/created -->


    <rdf:Description rdf:about="http://purl.org/dc/terms/created">
        <rdfs:subPropertyOf rdf:resource="http://purl.org/dc/elements/1.1/date"/>
    </rdf:Description>
    


    <!-- http://purl.org/dc/terms/creator -->


    <owl:AnnotationProperty rdf:about="http://purl.org/dc/terms/creator">
        <rdfs:subPropertyOf rdf:resource="http://purl.org/dc/elements/1.1/creator"/>
        <rdfs:subPropertyOf rdf:resource="http://purl.org/dc/terms/contributor"/>
    </owl:AnnotationProperty>
    


    <!-- http://purl.org/dc/terms/date -->


    <rdf:Description rdf:about="http://purl.org/dc/terms/date">
        <rdfs:subPropertyOf rdf:resource="http://purl.org/dc/elements/1.1/date"/>
    </rdf:Description>
    


    <!-- http://purl.org/dc/terms/dateAccepted -->


    <rdf:Description rdf:about="http://purl.org/dc/terms/dateAccepted">
        <rdfs:subPropertyOf rdf:resource="http://purl.org/dc/elements/1.1/date"/>
    </rdf:Description>
    


    <!-- http://purl.org/dc/terms/dateCopyrighted -->


    <rdf:Description rdf:about="http://purl.org/dc/terms/dateCopyrighted">
        <rdfs:subPropertyOf rdf:resource="http://purl.org/dc/elements/1.1/date"/>
    </rdf:Description>
    


    <!-- http://purl.org/dc/terms/dateSubmitted -->


    <rdf:Description rdf:about="http://purl.org/dc/terms/dateSubmitted">
        <rdfs:subPropertyOf rdf:resource="http://purl.org/dc/elements/1.1/date"/>
    </rdf:Description>
    


    <!-- http://purl.org/dc/terms/description -->


    <owl:AnnotationProperty rdf:about="http://purl.org/dc/terms/description">
        <rdfs:subPropertyOf rdf:resource="http://purl.org/dc/elements/1.1/description"/>
    </owl:AnnotationProperty>
    


    <!-- http://purl.org/dc/terms/educationLevel -->


    <rdf:Description rdf:about="http://purl.org/dc/terms/educationLevel">
        <rdfs:subPropertyOf rdf:resource="http://purl.org/dc/terms/audience"/>
    </rdf:Description>
    


    <!-- http://purl.org/dc/terms/extent -->


    <rdf:Description rdf:about="http://purl.org/dc/terms/extent">
        <rdfs:subPropertyOf rdf:resource="http://purl.org/dc/elements/1.1/format"/>
        <rdfs:subPropertyOf rdf:resource="http://purl.org/dc/terms/format"/>
    </rdf:Description>
    


    <!-- http://purl.org/dc/terms/format -->


    <rdf:Description rdf:about="http://purl.org/dc/terms/format">
        <rdfs:subPropertyOf rdf:resource="http://purl.org/dc/elements/1.1/format"/>
    </rdf:Description>
    


    <!-- http://purl.org/dc/terms/hasFormat -->


    <rdf:Description rdf:about="http://purl.org/dc/terms/hasFormat">
        <rdfs:subPropertyOf rdf:resource="http://purl.org/dc/elements/1.1/relation"/>
        <rdfs:subPropertyOf rdf:resource="http://purl.org/dc/terms/relation"/>
    </rdf:Description>
    


    <!-- http://purl.org/dc/terms/hasPart -->


    <rdf:Description rdf:about="http://purl.org/dc/terms/hasPart">
        <rdfs:subPropertyOf rdf:resource="http://purl.org/dc/elements/1.1/relation"/>
        <rdfs:subPropertyOf rdf:resource="http://purl.org/dc/terms/relation"/>
    </rdf:Description>
    


    <!-- http://purl.org/dc/terms/hasVersion -->


    <rdf:Description rdf:about="http://purl.org/dc/terms/hasVersion">
        <rdfs:subPropertyOf rdf:resource="http://purl.org/dc/elements/1.1/relation"/>
        <rdfs:subPropertyOf rdf:resource="http://purl.org/dc/terms/relation"/>
    </rdf:Description>
    


    <!-- http://purl.org/dc/terms/identifier -->


    <rdf:Description rdf:about="http://purl.org/dc/terms/identifier">
        <rdfs:subPropertyOf rdf:resource="http://purl.org/dc/elements/1.1/identifier"/>
    </rdf:Description>
    


    <!-- http://purl.org/dc/terms/isFormatOf -->


    <rdf:Description rdf:about="http://purl.org/dc/terms/isFormatOf">
        <rdfs:subPropertyOf rdf:resource="http://purl.org/dc/elements/1.1/relation"/>
        <rdfs:subPropertyOf rdf:resource="http://purl.org/dc/terms/relation"/>
    </rdf:Description>
    


    <!-- http://purl.org/dc/terms/isPartOf -->


    <rdf:Description rdf:about="http://purl.org/dc/terms/isPartOf">
        <rdfs:subPropertyOf rdf:resource="http://purl.org/dc/elements/1.1/relation"/>
        <rdfs:subPropertyOf rdf:resource="http://purl.org/dc/terms/relation"/>
    </rdf:Description>
    


    <!-- http://purl.org/dc/terms/isReferencedBy -->


    <rdf:Description rdf:about="http://purl.org/dc/terms/isReferencedBy">
        <rdfs:subPropertyOf rdf:resource="http://purl.org/dc/elements/1.1/relation"/>
        <rdfs:subPropertyOf rdf:resource="http://purl.org/dc/terms/relation"/>
    </rdf:Description>
    


    <!-- http://purl.org/dc/terms/isReplacedBy -->


    <rdf:Description rdf:about="http://purl.org/dc/terms/isReplacedBy">
        <rdfs:subPropertyOf rdf:resource="http://purl.org/dc/elements/1.1/relation"/>
        <rdfs:subPropertyOf rdf:resource="http://purl.org/dc/terms/relation"/>
    </rdf:Description>
    


    <!-- http://purl.org/dc/terms/isRequiredBy -->


    <rdf:Description rdf:about="http://purl.org/dc/terms/isRequiredBy">
        <rdfs:subPropertyOf rdf:resource="http://purl.org/dc/elements/1.1/relation"/>
        <rdfs:subPropertyOf rdf:resource="http://purl.org/dc/terms/relation"/>
    </rdf:Description>
    


    <!-- http://purl.org/dc/terms/isVersionOf -->


    <rdf:Description rdf:about="http://purl.org/dc/terms/isVersionOf">
        <rdfs:subPropertyOf rdf:resource="http://purl.org/dc/elements/1.1/relation"/>
        <rdfs:subPropertyOf rdf:resource="http://purl.org/dc/terms/relation"/>
    </rdf:Description>
    


    <!-- http://purl.org/dc/terms/issued -->


    <owl:AnnotationProperty rdf:about="http://purl.org/dc/terms/issued">
        <rdfs:subPropertyOf rdf:resource="http://purl.org/dc/elements/1.1/date"/>
    </owl:AnnotationProperty>
    


    <!-- http://purl.org/dc/terms/language -->


    <rdf:Description rdf:about="http://purl.org/dc/terms/language">
        <rdfs:subPropertyOf rdf:resource="http://purl.org/dc/elements/1.1/language"/>
    </rdf:Description>
    


    <!-- http://purl.org/dc/terms/license -->


    <rdf:Description rdf:about="http://purl.org/dc/terms/license">
        <rdfs:subPropertyOf rdf:resource="http://purl.org/dc/elements/1.1/rights"/>
        <rdfs:subPropertyOf rdf:resource="http://purl.org/dc/terms/rights"/>
    </rdf:Description>
    


    <!-- http://purl.org/dc/terms/mediator -->


    <rdf:Description rdf:about="http://purl.org/dc/terms/mediator">
        <rdfs:subPropertyOf rdf:resource="http://purl.org/dc/terms/audience"/>
    </rdf:Description>
    


    <!-- http://purl.org/dc/terms/medium -->


    <rdf:Description rdf:about="http://purl.org/dc/terms/medium">
        <rdfs:subPropertyOf rdf:resource="http://purl.org/dc/elements/1.1/format"/>
        <rdfs:subPropertyOf rdf:resource="http://purl.org/dc/terms/format"/>
    </rdf:Description>
    


    <!-- http://purl.org/dc/terms/modified -->


    <owl:AnnotationProperty rdf:about="http://purl.org/dc/terms/modified">
        <rdfs:subPropertyOf rdf:resource="http://purl.org/dc/elements/1.1/date"/>
    </owl:AnnotationProperty>
    


    <!-- http://purl.org/dc/terms/publisher -->


    <owl:AnnotationProperty rdf:about="http://purl.org/dc/terms/publisher">
        <rdfs:subPropertyOf rdf:resource="http://purl.org/dc/elements/1.1/publisher"/>
    </owl:AnnotationProperty>
    


    <!-- http://purl.org/dc/terms/references -->


    <rdf:Description rdf:about="http://purl.org/dc/terms/references">
        <rdfs:subPropertyOf rdf:resource="http://purl.org/dc/elements/1.1/relation"/>
        <rdfs:subPropertyOf rdf:resource="http://purl.org/dc/terms/relation"/>
    </rdf:Description>
    


    <!-- http://purl.org/dc/terms/relation -->


    <rdf:Description rdf:about="http://purl.org/dc/terms/relation">
        <rdfs:subPropertyOf rdf:resource="http://purl.org/dc/elements/1.1/relation"/>
    </rdf:Description>
    


    <!-- http://purl.org/dc/terms/replaces -->


    <rdf:Description rdf:about="http://purl.org/dc/terms/replaces">
        <rdfs:subPropertyOf rdf:resource="http://purl.org/dc/elements/1.1/relation"/>
        <rdfs:subPropertyOf rdf:resource="http://purl.org/dc/terms/relation"/>
    </rdf:Description>
    


    <!-- http://purl.org/dc/terms/requires -->


    <rdf:Description rdf:about="http://purl.org/dc/terms/requires">
        <rdfs:subPropertyOf rdf:resource="http://purl.org/dc/elements/1.1/relation"/>
        <rdfs:subPropertyOf rdf:resource="http://purl.org/dc/terms/relation"/>
    </rdf:Description>
    


    <!-- http://purl.org/dc/terms/rights -->


    <owl:AnnotationProperty rdf:about="http://purl.org/dc/terms/rights">
        <rdfs:subPropertyOf rdf:resource="http://purl.org/dc/elements/1.1/rights"/>
    </owl:AnnotationProperty>
    


    <!-- http://purl.org/dc/terms/source -->


    <rdf:Description rdf:about="http://purl.org/dc/terms/source">
        <rdfs:subPropertyOf rdf:resource="http://purl.org/dc/elements/1.1/source"/>
        <rdfs:subPropertyOf rdf:resource="http://purl.org/dc/terms/relation"/>
    </rdf:Description>
    


    <!-- http://purl.org/dc/terms/spatial -->


    <rdf:Description rdf:about="http://purl.org/dc/terms/spatial">
        <rdfs:subPropertyOf rdf:resource="http://purl.org/dc/elements/1.1/coverage"/>
        <rdfs:subPropertyOf rdf:resource="http://purl.org/dc/terms/coverage"/>
    </rdf:Description>
    


    <!-- http://purl.org/dc/terms/subject -->


    <rdf:Description rdf:about="http://purl.org/dc/terms/subject">
        <rdfs:subPropertyOf rdf:resource="http://purl.org/dc/elements/1.1/subject"/>
    </rdf:Description>
    


    <!-- http://purl.org/dc/terms/tableOfContents -->


    <rdf:Description rdf:about="http://purl.org/dc/terms/tableOfContents">
        <rdfs:subPropertyOf rdf:resource="http://purl.org/dc/elements/1.1/description"/>
        <rdfs:subPropertyOf rdf:resource="http://purl.org/dc/terms/description"/>
    </rdf:Description>
    


    <!-- http://purl.org/dc/terms/temporal -->


    <rdf:Description rdf:about="http://purl.org/dc/terms/temporal">
        <rdfs:subPropertyOf rdf:resource="http://purl.org/dc/elements/1.1/coverage"/>
        <rdfs:subPropertyOf rdf:resource="http://purl.org/dc/terms/coverage"/>
    </rdf:Description>
    


    <!-- http://purl.org/dc/terms/title -->


    <owl:AnnotationProperty rdf:about="http://purl.org/dc/terms/title">
        <rdfs:subPropertyOf rdf:resource="http://purl.org/dc/elements/1.1/title"/>
    </owl:AnnotationProperty>
    


    <!-- http://purl.org/dc/terms/type -->


    <rdf:Description rdf:about="http://purl.org/dc/terms/type">
        <rdfs:subPropertyOf rdf:resource="http://purl.org/dc/elements/1.1/type"/>
    </rdf:Description>
    


    <!-- http://purl.org/dc/terms/valid -->


    <rdf:Description rdf:about="http://purl.org/dc/terms/valid">
        <rdfs:subPropertyOf rdf:resource="http://purl.org/dc/elements/1.1/date"/>
    </rdf:Description>
    


    <!-- http://purl.org/vocab/vann/preferredNamespacePrefix -->


    <owl:AnnotationProperty rdf:about="http://purl.org/vocab/vann/preferredNamespacePrefix"/>
    


    <!-- http://purl.org/vocab/vann/preferredNamespaceUri -->


    <owl:AnnotationProperty rdf:about="http://purl.org/vocab/vann/preferredNamespaceUri"/>
    


    <!-- http://www.w3.org/2004/02/skos/core#altLabel -->


    <owl:AnnotationProperty rdf:about="http://www.w3.org/2004/02/skos/core#altLabel">
        <rdfs:comment xml:lang="en">The range of skos:altLabel is the class of RDF plain literals.</rdfs:comment>
        <rdfs:comment xml:lang="en">skos:prefLabel, skos:altLabel and skos:hiddenLabel are pairwise disjoint properties.</rdfs:comment>
        <rdfs:isDefinedBy rdf:resource="http://www.w3.org/2004/02/skos/core"/>
        <rdfs:label xml:lang="en">alternative label</rdfs:label>
        <skos:definition xml:lang="en">An alternative lexical label for a resource.</skos:definition>
        <skos:example xml:lang="en">Acronyms, abbreviations, spelling variants, and irregular plural/singular forms may be included among the alternative labels for a concept. Mis-spelled terms are normally included as hidden labels (see skos:hiddenLabel).</skos:example>
        <rdfs:subPropertyOf rdf:resource="http://www.w3.org/2000/01/rdf-schema#label"/>
    </owl:AnnotationProperty>
    


    <!-- http://www.w3.org/2004/02/skos/core#broadMatch -->


    <owl:AnnotationProperty rdf:about="http://www.w3.org/2004/02/skos/core#broadMatch"/>
    


    <!-- http://www.w3.org/2004/02/skos/core#broader -->


    <owl:AnnotationProperty rdf:about="http://www.w3.org/2004/02/skos/core#broader"/>
    


    <!-- http://www.w3.org/2004/02/skos/core#changeNote -->


    <owl:AnnotationProperty rdf:about="http://www.w3.org/2004/02/skos/core#changeNote">
        <rdfs:isDefinedBy rdf:resource="http://www.w3.org/2004/02/skos/core"/>
        <rdfs:label xml:lang="en">change note</rdfs:label>
        <skos:definition xml:lang="en">A note about a modification to a concept.</skos:definition>
        <rdfs:subPropertyOf rdf:resource="http://www.w3.org/2004/02/skos/core#note"/>
    </owl:AnnotationProperty>
    


    <!-- http://www.w3.org/2004/02/skos/core#definition -->


    <owl:AnnotationProperty rdf:about="http://www.w3.org/2004/02/skos/core#definition">
        <rdfs:isDefinedBy rdf:resource="http://www.w3.org/2004/02/skos/core"/>
        <rdfs:label xml:lang="en">definition</rdfs:label>
        <skos:definition xml:lang="en">A statement or formal explanation of the meaning of a concept.</skos:definition>
        <rdfs:subPropertyOf rdf:resource="http://www.w3.org/2004/02/skos/core#note"/>
    </owl:AnnotationProperty>
    


    <!-- http://www.w3.org/2004/02/skos/core#editorialNote -->


    <owl:AnnotationProperty rdf:about="http://www.w3.org/2004/02/skos/core#editorialNote">
        <rdfs:isDefinedBy rdf:resource="http://www.w3.org/2004/02/skos/core"/>
        <rdfs:label xml:lang="en">editorial note</rdfs:label>
        <skos:definition xml:lang="en">A note for an editor, translator or maintainer of the vocabulary.</skos:definition>
        <rdfs:subPropertyOf rdf:resource="http://www.w3.org/2004/02/skos/core#note"/>
    </owl:AnnotationProperty>
    


    <!-- http://www.w3.org/2004/02/skos/core#example -->


    <owl:AnnotationProperty rdf:about="http://www.w3.org/2004/02/skos/core#example">
        <rdfs:isDefinedBy rdf:resource="http://www.w3.org/2004/02/skos/core"/>
        <rdfs:label xml:lang="en">example</rdfs:label>
        <skos:definition xml:lang="en">An example of the use of a concept.</skos:definition>
        <rdfs:subPropertyOf rdf:resource="http://www.w3.org/2004/02/skos/core#note"/>
    </owl:AnnotationProperty>
    


    <!-- http://www.w3.org/2004/02/skos/core#hasTopConcept -->


    <owl:AnnotationProperty rdf:about="http://www.w3.org/2004/02/skos/core#hasTopConcept"/>
    


    <!-- http://www.w3.org/2004/02/skos/core#hiddenLabel -->


    <owl:AnnotationProperty rdf:about="http://www.w3.org/2004/02/skos/core#hiddenLabel">
        <rdfs:comment xml:lang="en">The range of skos:hiddenLabel is the class of RDF plain literals.</rdfs:comment>
        <rdfs:comment xml:lang="en">skos:prefLabel, skos:altLabel and skos:hiddenLabel are pairwise disjoint properties.</rdfs:comment>
        <rdfs:isDefinedBy rdf:resource="http://www.w3.org/2004/02/skos/core"/>
        <rdfs:label xml:lang="en">hidden label</rdfs:label>
        <skos:definition xml:lang="en">A lexical label for a resource that should be hidden when generating visual displays of the resource, but should still be accessible to free text search operations.</skos:definition>
        <rdfs:subPropertyOf rdf:resource="http://www.w3.org/2000/01/rdf-schema#label"/>
    </owl:AnnotationProperty>
    


    <!-- http://www.w3.org/2004/02/skos/core#historyNote -->


    <owl:AnnotationProperty rdf:about="http://www.w3.org/2004/02/skos/core#historyNote">
        <rdfs:isDefinedBy rdf:resource="http://www.w3.org/2004/02/skos/core"/>
        <rdfs:label xml:lang="en">history note</rdfs:label>
        <skos:definition xml:lang="en">A note about the past state/use/meaning of a concept.</skos:definition>
        <rdfs:subPropertyOf rdf:resource="http://www.w3.org/2004/02/skos/core#note"/>
    </owl:AnnotationProperty>
    


    <!-- http://www.w3.org/2004/02/skos/core#narrowMatch -->


    <owl:AnnotationProperty rdf:about="http://www.w3.org/2004/02/skos/core#narrowMatch"/>
    


    <!-- http://www.w3.org/2004/02/skos/core#note -->


    <owl:AnnotationProperty rdf:about="http://www.w3.org/2004/02/skos/core#note">
        <rdfs:isDefinedBy rdf:resource="http://www.w3.org/2004/02/skos/core"/>
        <rdfs:label xml:lang="en">note</rdfs:label>
        <skos:definition xml:lang="en">A general note, for any purpose.</skos:definition>
        <skos:scopeNote xml:lang="en">This property may be used directly, or as a super-property for more specific note types.</skos:scopeNote>
    </owl:AnnotationProperty>
    


    <!-- http://www.w3.org/2004/02/skos/core#prefLabel -->


    <owl:AnnotationProperty rdf:about="http://www.w3.org/2004/02/skos/core#prefLabel">
        <rdfs:comment xml:lang="en">A resource has no more than one value of skos:prefLabel per language tag, and no more than one value of skos:prefLabel without language tag.</rdfs:comment>
        <rdfs:comment xml:lang="en">The range of skos:prefLabel is the class of RDF plain literals.</rdfs:comment>
        <rdfs:comment xml:lang="en">skos:prefLabel, skos:altLabel and skos:hiddenLabel are pairwise
      disjoint properties.</rdfs:comment>
        <rdfs:isDefinedBy rdf:resource="http://www.w3.org/2004/02/skos/core"/>
        <rdfs:label xml:lang="en">preferred label</rdfs:label>
        <skos:definition xml:lang="en">The preferred lexical label for a resource, in a given language.</skos:definition>
        <rdfs:subPropertyOf rdf:resource="http://www.w3.org/2000/01/rdf-schema#label"/>
    </owl:AnnotationProperty>
    


    <!-- http://www.w3.org/2004/02/skos/core#relatedMatch -->


    <owl:AnnotationProperty rdf:about="http://www.w3.org/2004/02/skos/core#relatedMatch"/>
    


    <!-- http://www.w3.org/2004/02/skos/core#scopeNote -->


    <owl:AnnotationProperty rdf:about="http://www.w3.org/2004/02/skos/core#scopeNote">
        <rdfs:isDefinedBy rdf:resource="http://www.w3.org/2004/02/skos/core"/>
        <rdfs:label xml:lang="en">scope note</rdfs:label>
        <skos:definition xml:lang="en">A note that helps to clarify the meaning and/or the use of a concept.</skos:definition>
        <rdfs:subPropertyOf rdf:resource="http://www.w3.org/2004/02/skos/core#note"/>
    </owl:AnnotationProperty>
    


    <!-- http://www.w3.org/2006/time#hasBeginning -->


    <owl:AnnotationProperty rdf:about="http://www.w3.org/2006/time#hasBeginning"/>
    


    <!-- http://www.w3.org/2006/time#inXSDDateTimeStamp -->


    <owl:AnnotationProperty rdf:about="http://www.w3.org/2006/time#inXSDDateTimeStamp"/>
    


    <!-- http://www.w3.org/ns/dcat#distribution -->


    <rdf:Description rdf:about="http://www.w3.org/ns/dcat#distribution">
        <rdfs:subPropertyOf rdf:resource="http://purl.org/dc/terms/relation"/>
    </rdf:Description>
    


    <!-- http://www.w3.org/ns/dcat#hasCurrentVersion -->


    <rdf:Description rdf:about="http://www.w3.org/ns/dcat#hasCurrentVersion">
        <rdfs:subPropertyOf rdf:resource="http://purl.org/pav/hasVersion"/>
    </rdf:Description>
    


    <!-- http://www.w3.org/ns/dcat#last -->


    <rdf:Description rdf:about="http://www.w3.org/ns/dcat#last">
        <rdfs:subPropertyOf rdf:resource="http://www.w3.org/1999/xhtml/vocab#last"/>
    </rdf:Description>
    


    <!-- http://www.w3.org/ns/org#hasMembership -->


    <owl:AnnotationProperty rdf:about="http://www.w3.org/ns/org#hasMembership"/>
    


    <!-- http://www.w3.org/ns/org#memberDuring -->


    <owl:AnnotationProperty rdf:about="http://www.w3.org/ns/org#memberDuring"/>
    


    <!-- http://www.w3.org/ns/org#organization -->


    <owl:AnnotationProperty rdf:about="http://www.w3.org/ns/org#organization"/>
    


    <!-- http://www.w3.org/ns/org#role -->


    <owl:AnnotationProperty rdf:about="http://www.w3.org/ns/org#role"/>
    


    <!-- http://xmlns.com/foaf/0.1/family_name -->


    <owl:AnnotationProperty rdf:about="http://xmlns.com/foaf/0.1/family_name"/>
    


    <!-- http://xmlns.com/foaf/0.1/firstName -->


    <owl:AnnotationProperty rdf:about="http://xmlns.com/foaf/0.1/firstName"/>
    


    <!-- http://xmlns.com/foaf/0.1/givenname -->


    <owl:AnnotationProperty rdf:about="http://xmlns.com/foaf/0.1/givenname"/>
    


    <!-- http://xmlns.com/foaf/0.1/homepage -->


    <owl:AnnotationProperty rdf:about="http://xmlns.com/foaf/0.1/homepage"/>
    


    <!-- http://xmlns.com/foaf/0.1/mbox -->


    <owl:AnnotationProperty rdf:about="http://xmlns.com/foaf/0.1/mbox"/>
    


    <!-- http://xmlns.com/foaf/0.1/member -->


    <owl:AnnotationProperty rdf:about="http://xmlns.com/foaf/0.1/member"/>
    


    <!-- http://xmlns.com/foaf/0.1/name -->


    <owl:AnnotationProperty rdf:about="http://xmlns.com/foaf/0.1/name"/>
    


    <!-- http://xmlns.com/foaf/0.1/title -->


    <owl:AnnotationProperty rdf:about="http://xmlns.com/foaf/0.1/title"/>
    


    <!-- http://xmlns.com/foaf/0.1/workInfoHomepage -->


    <owl:AnnotationProperty rdf:about="http://xmlns.com/foaf/0.1/workInfoHomepage"/>
    


    <!-- 
    ///////////////////////////////////////////////////////////////////////////////////////
    //
    // Datatypes
    //
    ///////////////////////////////////////////////////////////////////////////////////////
     -->


    


    <!-- http://purl.org/dc/terms/Box -->


    <rdfs:Datatype rdf:about="http://purl.org/dc/terms/Box"/>
    


    <!-- http://purl.org/dc/terms/ISO3166 -->


    <rdfs:Datatype rdf:about="http://purl.org/dc/terms/ISO3166"/>
    


    <!-- http://purl.org/dc/terms/ISO639-2 -->


    <rdfs:Datatype rdf:about="http://purl.org/dc/terms/ISO639-2"/>
    


    <!-- http://purl.org/dc/terms/ISO639-3 -->


    <rdfs:Datatype rdf:about="http://purl.org/dc/terms/ISO639-3"/>
    


    <!-- http://purl.org/dc/terms/Period -->


    <rdfs:Datatype rdf:about="http://purl.org/dc/terms/Period"/>
    


    <!-- http://purl.org/dc/terms/Point -->


    <rdfs:Datatype rdf:about="http://purl.org/dc/terms/Point"/>
    


    <!-- http://purl.org/dc/terms/RFC1766 -->


    <rdfs:Datatype rdf:about="http://purl.org/dc/terms/RFC1766"/>
    


    <!-- http://purl.org/dc/terms/RFC3066 -->


    <rdfs:Datatype rdf:about="http://purl.org/dc/terms/RFC3066"/>
    


    <!-- http://purl.org/dc/terms/RFC4646 -->


    <rdfs:Datatype rdf:about="http://purl.org/dc/terms/RFC4646"/>
    


    <!-- http://purl.org/dc/terms/RFC5646 -->


    <rdfs:Datatype rdf:about="http://purl.org/dc/terms/RFC5646"/>
    


    <!-- http://purl.org/dc/terms/URI -->


    <rdfs:Datatype rdf:about="http://purl.org/dc/terms/URI"/>
    


    <!-- http://purl.org/dc/terms/W3CDTF -->


    <rdfs:Datatype rdf:about="http://purl.org/dc/terms/W3CDTF"/>
    


    <!-- xsd:date -->


    <rdfs:Datatype rdf:about="xsd:date"/>
    


    <!-- 
    ///////////////////////////////////////////////////////////////////////////////////////
    //
    // Object Properties
    //
    ///////////////////////////////////////////////////////////////////////////////////////
     -->


    


    <!-- http://data.ign.fr/def/geometrie#geometry -->


    <owl:ObjectProperty rdf:about="http://data.ign.fr/def/geometrie#geometry"/>
    


    <!-- http://data.ign.fr/def/topo#borneFin -->


    <owl:ObjectProperty rdf:about="http://data.ign.fr/def/topo#borneFin">
        <rdfs:domain rdf:resource="http://data.ign.fr/def/topo#Route"/>
        <rdfs:range rdf:resource="http://data.ign.fr/def/topo#BornePostale"/>
        <rdfs:comment xml:lang="fr">Relation entre un tronçon de route et la borne postale correspondant à son point final.</rdfs:comment>
        <rdfs:comment xml:lang="en">Relationship between a section of road and the post office terminal corresponding to its end point.</rdfs:comment>
        <rdfs:isDefinedBy rdf:resource="http://data.ign.fr/def/topo"/>
        <rdfs:label xml:lang="fr">borne finale</rdfs:label>
        <rdfs:label xml:lang="en">final civic number marker</rdfs:label>
    </owl:ObjectProperty>
    


    <!-- http://data.ign.fr/def/topo#borneIni -->


    <owl:ObjectProperty rdf:about="http://data.ign.fr/def/topo#borneIni">
        <rdfs:domain rdf:resource="http://data.ign.fr/def/topo#Route"/>
        <rdfs:range rdf:resource="http://data.ign.fr/def/topo#BornePostale"/>
        <rdfs:comment xml:lang="fr">Relation entre un tronçon de route et la borne postale correspondant à son point initial.</rdfs:comment>
        <rdfs:comment xml:lang="en">Relationship between a section of road and the post office terminal corresponding to its initial point.</rdfs:comment>
        <rdfs:isDefinedBy rdf:resource="http://data.ign.fr/def/topo"/>
        <rdfs:label xml:lang="fr">borne initiale</rdfs:label>
        <rdfs:label xml:lang="en">initial civic number marker</rdfs:label>
    </owl:ObjectProperty>
    


    <!-- http://data.ign.fr/def/topo#clAdmin -->


    <owl:ObjectProperty rdf:about="http://data.ign.fr/def/topo#clAdmin">
        <rdfs:domain rdf:resource="http://data.ign.fr/def/topo#Route"/>
        <rdfs:range>
            <owl:Restriction>
                <owl:onProperty rdf:resource="http://www.w3.org/2004/02/skos/core#inScheme"/>
                <owl:hasValue rdf:resource="http://data.ign.fr/id/codes/topo/typederoute/liste"/>
            </owl:Restriction>
        </rdfs:range>
        <rdfs:comment xml:lang="en">Administrative classification. Status of a numbered or named road.</rdfs:comment>
        <rdfs:comment xml:lang="fr">Classement administratif. Statut d’une route numérotée ou nommée.</rdfs:comment>
        <rdfs:isDefinedBy rdf:resource="http://data.ign.fr/def/topo"/>
        <rdfs:label xml:lang="en">administrative status</rdfs:label>
        <rdfs:label xml:lang="fr">classement administratif</rdfs:label>
    </owl:ObjectProperty>
    


    <!-- http://data.ign.fr/def/topo#concerne -->


    <owl:ObjectProperty rdf:about="http://data.ign.fr/def/topo#concerne">
        <rdfs:domain rdf:resource="http://data.ign.fr/def/topo#BornePostale"/>
        <rdfs:range rdf:resource="http://data.ign.fr/def/topo#Voie"/>
        <rdfs:comment xml:lang="fr">Relation entre une borne postale et la voie à laquelle elle se rapporte.</rdfs:comment>
        <rdfs:comment xml:lang="en">Relationship between a postal station and the route to which it relates.</rdfs:comment>
        <rdfs:isDefinedBy rdf:resource="http://data.ign.fr/def/topo"/>
        <rdfs:label xml:lang="fr">concerne</rdfs:label>
        <rdfs:label xml:lang="en">related to</rdfs:label>
    </owl:ObjectProperty>
    


    <!-- http://data.ign.fr/def/topo#gestionVoie -->


    <owl:ObjectProperty rdf:about="http://data.ign.fr/def/topo#gestionVoie">
        <rdfs:domain rdf:resource="http://data.ign.fr/def/topo#Voie"/>
        <rdfs:range rdf:resource="http://data.ign.fr/def/geofla#Commune"/>
        <rdfs:comment xml:lang="fr">Relation entre une voie nommée et la commune dont elle dépend.</rdfs:comment>
        <rdfs:comment xml:lang="en">Relationship between a named path and the municipality on which it depends.</rdfs:comment>
        <rdfs:isDefinedBy rdf:resource="http://data.ign.fr/def/topo"/>
        <rdfs:label xml:lang="fr">commune gestionnaire de la voie nommée</rdfs:label>
        <rdfs:label xml:lang="en">manager of the nammed street</rdfs:label>
    </owl:ObjectProperty>
    


    <!-- http://data.ign.fr/def/topo#nature -->


    <owl:ObjectProperty rdf:about="http://data.ign.fr/def/topo#nature">
        <rdfs:domain rdf:resource="http://data.ign.fr/def/topo#EntiteTopographique"/>
        <rdfs:range rdf:resource="http://www.w3.org/2004/02/skos/core#Concept"/>
        <rdfs:comment xml:lang="en">Link a topographic entity to the concept that specifies its nature.</rdfs:comment>
        <rdfs:comment xml:lang="fr">Relie une entité topographique au concept qui précise sa nature.</rdfs:comment>
        <rdfs:isDefinedBy rdf:resource="http://data.ign.fr/def/topo"/>
        <rdfs:label xml:lang="en">nature</rdfs:label>
        <rdfs:label xml:lang="fr">nature</rdfs:label>
    </owl:ObjectProperty>
    


    <!-- http://data.ign.fr/def/topo#origine -->


    <owl:ObjectProperty rdf:about="http://data.ign.fr/def/topo#origine">
        <rdfs:subPropertyOf rdf:resource="http://www.w3.org/ns/prov#wasDerivedFrom"/>
        <rdfs:domain rdf:resource="http://data.ign.fr/def/topo#EntiteTopographique"/>
        <rdfs:range rdf:resource="http://www.w3.org/ns/prov#Entity"/>
        <rdfs:comment xml:lang="fr">Source de l&apos;information.</rdfs:comment>
        <rdfs:comment xml:lang="en">Source of information.</rdfs:comment>
        <rdfs:isDefinedBy rdf:resource="http://data.ign.fr/def/topo"/>
        <rdfs:label xml:lang="en">origine</rdfs:label>
        <rdfs:label xml:lang="fr">origine</rdfs:label>
    </owl:ObjectProperty>
    


    <!-- http://data.ign.fr/def/topo#typeDeBatiment -->


    <owl:ObjectProperty rdf:about="http://data.ign.fr/def/topo#typeDeBatiment">
        <rdfs:subPropertyOf rdf:resource="http://data.ign.fr/def/topo#nature"/>
        <rdfs:domain rdf:resource="http://data.ign.fr/def/topo#Batiment"/>
        <rdfs:range>
            <owl:Restriction>
                <owl:onProperty rdf:resource="http://www.w3.org/2004/02/skos/core#inScheme"/>
                <owl:hasValue rdf:resource="http://data.ign.fr/id/codes/topo/typedebatiment/liste"/>
            </owl:Restriction>
        </rdfs:range>
        <rdfs:comment xml:lang="en">Links a building instance to an instance of skos: Concept defined in the list &apos;building&apos; which specifies its nature.</rdfs:comment>
        <rdfs:comment xml:lang="fr">Relie une instance de bâtiment à une instance de skos:Concept définie dans la liste &apos;bati&apos; qui précise sa nature.</rdfs:comment>
        <rdfs:isDefinedBy rdf:resource="http://data.ign.fr/def/topo"/>
        <rdfs:label xml:lang="fr">type de bâtiment</rdfs:label>
        <rdfs:label xml:lang="en">type of building </rdfs:label>
    </owl:ObjectProperty>
    


    <!-- http://data.ign.fr/def/topo#typeDeConstruction -->


    <owl:ObjectProperty rdf:about="http://data.ign.fr/def/topo#typeDeConstruction">
        <rdfs:subPropertyOf rdf:resource="http://data.ign.fr/def/topo#nature"/>
        <rdfs:domain rdf:resource="http://data.ign.fr/def/topo#Construction"/>
        <rdfs:range>
            <owl:Restriction>
                <owl:onProperty rdf:resource="http://www.w3.org/2004/02/skos/core#inScheme"/>
                <owl:hasValue rdf:resource="http://data.ign.fr/id/codes/topo/typedeconstruction/liste"/>
            </owl:Restriction>
        </rdfs:range>
        <rdfs:comment xml:lang="en">Links a build instance to an instance of skos: Concept defined in the list &apos;cnstr&apos; which specifies its nature.</rdfs:comment>
        <rdfs:comment xml:lang="fr">Relie une instance de construction à une instance de skos:Concept définie dans la liste &apos;cnstr&apos; qui précise sa nature.</rdfs:comment>
        <rdfs:isDefinedBy rdf:resource="http://data.ign.fr/def/topo"/>
        <rdfs:label xml:lang="fr">type de construction</rdfs:label>
        <rdfs:label xml:lang="en">type of structure</rdfs:label>
    </owl:ObjectProperty>
    


    <!-- http://data.ign.fr/def/topo#typeDeFranchissement -->


    <owl:ObjectProperty rdf:about="http://data.ign.fr/def/topo#typeDeFranchissement">
        <rdfs:domain>
            <owl:Class>
                <owl:unionOf rdf:parseType="Collection">
                    <rdf:Description rdf:about="http://data.ign.fr/def/topo#Route"/>
                    <rdf:Description rdf:about="http://data.ign.fr/def/topo#VoieFerree"/>
                </owl:unionOf>
            </owl:Class>
        </rdfs:domain>
        <rdfs:range>
            <owl:Restriction>
                <owl:onProperty rdf:resource="http://www.w3.org/2004/02/skos/core#inScheme"/>
                <owl:hasValue rdf:resource="http://data.ign.fr/id/codes/topo/typedefranchissement/liste"/>
            </owl:Restriction>
        </rdfs:range>
        <rdfs:comment xml:lang="en">Links the elements of the transport networks to the type of crossing structure to which they correspond.</rdfs:comment>
        <rdfs:comment xml:lang="fr">Relie les éléments de réseaux de transport au type d&apos;ouvrage de franchissement auquel ils correspondent.</rdfs:comment>
        <rdfs:isDefinedBy rdf:resource="http://data.ign.fr/def/topo"/>
        <rdfs:label xml:lang="fr">type de franchissement</rdfs:label>
        <rdfs:label xml:lang="en">type of crossing</rdfs:label>
    </owl:ObjectProperty>
    


    <!-- http://data.ign.fr/def/topo#typeDeLaisse -->


    <owl:ObjectProperty rdf:about="http://data.ign.fr/def/topo#typeDeLaisse">
        <rdfs:subPropertyOf rdf:resource="http://data.ign.fr/def/topo#nature"/>
        <rdfs:domain rdf:resource="http://data.ign.fr/def/topo#Laisse"/>
        <rdfs:range>
            <owl:Restriction>
                <owl:onProperty rdf:resource="http://www.w3.org/2004/02/skos/core#inScheme"/>
                <owl:hasValue rdf:resource="http://data.ign.fr/id/codes/topo/typedelaisse/liste"/>
            </owl:Restriction>
        </rdfs:range>
        <rdfs:comment xml:lang="en">Links an instance of leash to an instance of skos: Concept defined in the list &apos;tdl&apos; which specifies its nature.</rdfs:comment>
        <rdfs:comment xml:lang="fr">Relie une instance de laisse à une instance de skos:Concept définie dans la liste &apos;tdl&apos; qui précise sa nature.</rdfs:comment>
        <rdfs:isDefinedBy rdf:resource="http://data.ign.fr/def/topo"/>
        <rdfs:label xml:lang="fr">type de laisse</rdfs:label>
        <rdfs:label xml:lang="en">type of tide line</rdfs:label>
    </owl:ObjectProperty>
    


    <!-- http://data.ign.fr/def/topo#typeDePointDEau -->


    <owl:ObjectProperty rdf:about="http://data.ign.fr/def/topo#typeDePointDEau">
        <rdfs:subPropertyOf rdf:resource="http://data.ign.fr/def/topo#nature"/>
        <rdfs:domain rdf:resource="http://data.ign.fr/def/topo#PointDEau"/>
        <rdfs:range>
            <owl:Restriction>
                <owl:onProperty rdf:resource="http://www.w3.org/2004/02/skos/core#inScheme"/>
                <owl:hasValue rdf:resource="http://data.ign.fr/id/codes/topo/typedepointdeau/liste"/>
            </owl:Restriction>
        </rdfs:range>
        <rdfs:comment xml:lang="en">Links an instance of water point to an instance of skos: Concept defined in the list &apos;pte&apos; which specifies its nature.</rdfs:comment>
        <rdfs:comment xml:lang="fr">Relie une instance de point d&apos;eau à une instance de skos:Concept définie dans la liste &apos;pte&apos; qui précise sa nature.</rdfs:comment>
        <rdfs:isDefinedBy rdf:resource="http://data.ign.fr/def/topo"/>
        <rdfs:label xml:lang="fr">type de point d&apos;eau</rdfs:label>
        <rdfs:label xml:lang="en">type of waterhole</rdfs:label>
    </owl:ObjectProperty>
    


    <!-- http://data.ign.fr/def/topo#typeDeRelief -->


    <owl:ObjectProperty rdf:about="http://data.ign.fr/def/topo#typeDeRelief">
        <rdfs:subPropertyOf rdf:resource="http://data.ign.fr/def/topo#nature"/>
        <rdfs:domain rdf:resource="http://data.ign.fr/def/topo#ElementDuRelief"/>
        <rdfs:range>
            <owl:Restriction>
                <owl:onProperty rdf:resource="http://www.w3.org/2004/02/skos/core#inScheme"/>
                <owl:hasValue rdf:resource="http://data.ign.fr/id/codes/topo/typederelief/liste"/>
            </owl:Restriction>
        </rdfs:range>
        <rdfs:comment xml:lang="en">Links a terrain element instance to an instance of skos: Concept defined in the &apos;rel&apos; list that specifies its nature.</rdfs:comment>
        <rdfs:comment xml:lang="fr">Relie une instance d&apos;élément du relief à une instance de skos:Concept définie dans la liste &apos;rel&apos; qui précise sa nature.</rdfs:comment>
        <rdfs:isDefinedBy rdf:resource="http://data.ign.fr/def/topo"/>
        <rdfs:label xml:lang="fr">type d&apos;élément du relief</rdfs:label>
        <rdfs:label xml:lang="en">type of relief feature</rdfs:label>
    </owl:ObjectProperty>
    


    <!-- http://data.ign.fr/def/topo#typeDeReservoir -->


    <owl:ObjectProperty rdf:about="http://data.ign.fr/def/topo#typeDeReservoir">
        <rdfs:subPropertyOf rdf:resource="http://data.ign.fr/def/topo#nature"/>
        <rdfs:domain rdf:resource="http://data.ign.fr/def/topo#Reservoir"/>
        <rdfs:range>
            <owl:Restriction>
                <owl:onProperty rdf:resource="http://www.w3.org/2004/02/skos/core#inScheme"/>
                <owl:hasValue rdf:resource="http://data.ign.fr/id/codes/topo/typedereservoir/liste"/>
            </owl:Restriction>
        </rdfs:range>
        <rdfs:comment xml:lang="en">Links a tank instance to an instance of skos: Concept defined in the &apos;rsv&apos; list which specifies its nature.</rdfs:comment>
        <rdfs:comment xml:lang="fr">Relie une instance de réservoir à une instance de skos:Concept définie dans la liste &apos;rsv&apos; qui précise sa nature.</rdfs:comment>
        <rdfs:isDefinedBy rdf:resource="http://data.ign.fr/def/topo"/>
        <rdfs:label xml:lang="fr">type de réservoir</rdfs:label>
        <rdfs:label xml:lang="en">type of tank</rdfs:label>
    </owl:ObjectProperty>
    


    <!-- http://data.ign.fr/def/topo#typeDeRoute -->


    <owl:ObjectProperty rdf:about="http://data.ign.fr/def/topo#typeDeRoute">
        <rdfs:subPropertyOf rdf:resource="http://data.ign.fr/def/topo#nature"/>
        <rdfs:domain rdf:resource="http://data.ign.fr/def/topo#Route"/>
        <rdfs:range>
            <owl:Restriction>
                <owl:onProperty rdf:resource="http://www.w3.org/2004/02/skos/core#inScheme"/>
                <owl:hasValue rdf:resource="http://data.ign.fr/id/codes/topo/typederoute/liste"/>
            </owl:Restriction>
        </rdfs:range>
        <rdfs:comment xml:lang="en">Links a route instance to an instance of skos: Concept defined in the list &apos;rte&apos; which specifies its nature.</rdfs:comment>
        <rdfs:comment xml:lang="fr">Relie une instance de route à une instance de skos:Concept définie dans la liste &apos;rte&apos; qui précise sa nature.</rdfs:comment>
        <rdfs:isDefinedBy rdf:resource="http://data.ign.fr/def/topo"/>
        <rdfs:label xml:lang="fr">type de route</rdfs:label>
        <rdfs:label xml:lang="en">type of road</rdfs:label>
    </owl:ObjectProperty>
    


    <!-- http://data.ign.fr/def/topo#typeDeTerrainDeSport -->


    <owl:ObjectProperty rdf:about="http://data.ign.fr/def/topo#typeDeTerrainDeSport">
        <rdfs:subPropertyOf rdf:resource="http://data.ign.fr/def/topo#nature"/>
        <rdfs:domain rdf:resource="http://data.ign.fr/def/topo#TerrainDeSport"/>
        <rdfs:range>
            <owl:Restriction>
                <owl:onProperty rdf:resource="http://www.w3.org/2004/02/skos/core#inScheme"/>
                <owl:hasValue rdf:resource="http://data.ign.fr/id/codes/topo/typedeterraindesport/liste"/>
            </owl:Restriction>
        </rdfs:range>
        <rdfs:comment xml:lang="en">Links a sport field instance to an instance of skos: Concept defined in the &apos;tds&apos; list which specifies its nature.</rdfs:comment>
        <rdfs:comment xml:lang="fr">Relie une instance de terrain de sport à une instance de skos:Concept définie dans la liste &apos;tds&apos; qui précise sa nature.</rdfs:comment>
        <rdfs:isDefinedBy rdf:resource="http://data.ign.fr/def/topo"/>
        <rdfs:label xml:lang="fr">type de terrain de sport</rdfs:label>
        <rdfs:label xml:lang="en">type of sports ground</rdfs:label>
    </owl:ObjectProperty>
    


    <!-- http://data.ign.fr/def/topo#typeDeTransportCable -->


    <owl:ObjectProperty rdf:about="http://data.ign.fr/def/topo#typeDeTransportCable">
        <rdfs:subPropertyOf rdf:resource="http://data.ign.fr/def/topo#nature"/>
        <rdfs:domain rdf:resource="http://data.ign.fr/def/topo#LigneTransportCable"/>
        <rdfs:range>
            <owl:Restriction>
                <owl:onProperty rdf:resource="http://www.w3.org/2004/02/skos/core#inScheme"/>
                <owl:hasValue rdf:resource="http://data.ign.fr/id/codes/topo/typedetransportcable/liste"/>
            </owl:Restriction>
        </rdfs:range>
        <rdfs:comment xml:lang="en">Links a cable transport infrastructure instance to an instance of skos: Concept defined in the &apos;tpc&apos; list which specifies its nature.</rdfs:comment>
        <rdfs:comment xml:lang="fr">Relie une instance d&apos;infrastructure de transport par câble à une instance de skos:Concept définie dans la liste &apos;tpc&apos; qui précise sa nature.</rdfs:comment>
        <rdfs:isDefinedBy rdf:resource="http://data.ign.fr/def/topo"/>
        <rdfs:label xml:lang="fr">type de ligne de transport par câble</rdfs:label>
        <rdfs:label xml:lang="en">type of cableway transport line</rdfs:label>
    </owl:ObjectProperty>
    


    <!-- http://data.ign.fr/def/topo#typeDeVegetation -->


    <owl:ObjectProperty rdf:about="http://data.ign.fr/def/topo#typeDeVegetation">
        <rdfs:subPropertyOf rdf:resource="http://data.ign.fr/def/topo#nature"/>
        <rdfs:domain rdf:resource="http://data.ign.fr/def/topo#ZoneDeVegetation"/>
        <rdfs:range>
            <owl:Restriction>
                <owl:onProperty rdf:resource="http://www.w3.org/2004/02/skos/core#inScheme"/>
                <owl:hasValue rdf:resource="http://data.ign.fr/id/codes/topo/typedevegetation/liste"/>
            </owl:Restriction>
        </rdfs:range>
        <rdfs:comment xml:lang="en">Links an instance of a vegetation zone to an instance of skos: Concept defined in the &apos;veg&apos; list which specifies its nature.</rdfs:comment>
        <rdfs:comment xml:lang="fr">Relie une instance de zone de végétation à une instance de skos:Concept définie dans la liste &apos;veg&apos; qui précise sa nature.</rdfs:comment>
        <rdfs:isDefinedBy rdf:resource="http://data.ign.fr/def/topo"/>
        <rdfs:label xml:lang="fr">type de végétation</rdfs:label>
        <rdfs:label xml:lang="en">type of vegetation </rdfs:label>
    </owl:ObjectProperty>
    


    <!-- http://data.ign.fr/def/topo#typeDeVoieFerree -->


    <owl:ObjectProperty rdf:about="http://data.ign.fr/def/topo#typeDeVoieFerree">
        <rdfs:subPropertyOf rdf:resource="http://data.ign.fr/def/topo#nature"/>
        <rdfs:domain rdf:resource="http://data.ign.fr/def/topo#VoieFerree"/>
        <rdfs:range>
            <owl:Restriction>
                <owl:onProperty rdf:resource="http://www.w3.org/2004/02/skos/core#inScheme"/>
                <owl:hasValue rdf:resource="http://data.ign.fr/id/codes/topo/typedevoieferree/liste"/>
            </owl:Restriction>
        </rdfs:range>
        <rdfs:comment xml:lang="en">Links a railroad instance to an instance of skos: Concept defined in the &apos;vfr&apos; list which specifies its nature.</rdfs:comment>
        <rdfs:comment xml:lang="fr">Relie une instance de voie ferrée à une instance de skos:Concept définie dans la liste &apos;vfr&apos; qui précise sa nature.</rdfs:comment>
        <rdfs:isDefinedBy rdf:resource="http://data.ign.fr/def/topo"/>
        <rdfs:label xml:lang="fr">type de voie ferrée</rdfs:label>
        <rdfs:label xml:lang="en">type of railway track</rdfs:label>
    </owl:ObjectProperty>
    


    <!-- http://data.ign.fr/def/topo#typeDeZAI -->


    <owl:ObjectProperty rdf:about="http://data.ign.fr/def/topo#typeDeZAI">
        <rdfs:subPropertyOf rdf:resource="http://data.ign.fr/def/topo#nature"/>
        <rdfs:domain rdf:resource="http://data.ign.fr/def/topo#ZoneActiviteInteret"/>
        <rdfs:range>
            <owl:Restriction>
                <owl:onProperty rdf:resource="http://www.w3.org/2004/02/skos/core#inScheme"/>
                <owl:hasValue rdf:resource="http://data.ign.fr/id/codes/topo/typedezai/liste"/>
            </owl:Restriction>
        </rdfs:range>
        <rdfs:comment xml:lang="en">Links an instance of activity and interest zone to an instance of skos: Concept defined in the list &apos;zai&apos; which specifies its nature.</rdfs:comment>
        <rdfs:comment xml:lang="fr">Relie une instance de zone d&apos;activité et d&apos;intérêt à une instance de skos:Concept définie dans la liste &apos;zai&apos; qui précise sa nature.</rdfs:comment>
        <rdfs:isDefinedBy rdf:resource="http://data.ign.fr/def/topo"/>
        <rdfs:label xml:lang="fr">type de ZAI</rdfs:label>
        <rdfs:label xml:lang="en">type of Area Of Interest (AOI)</rdfs:label>
    </owl:ObjectProperty>
    


    <!-- http://purl.org/dc/terms/isPartOf -->


    <owl:ObjectProperty rdf:about="http://purl.org/dc/terms/isPartOf"/>
    


    <!-- http://www.semanticweb.org/bbucher/ontologies/2025/9/geodata#hasConcept -->


    <owl:ObjectProperty rdf:about="http://www.semanticweb.org/bbucher/ontologies/2025/9/geodata#hasConcept">
        <rdfs:domain rdf:resource="http://www.semanticweb.org/bbucher/ontologies/2025/9/geodata#Representation"/>
        <rdfs:range rdf:resource="http://www.w3.org/2004/02/skos/core#Concept"/>
    </owl:ObjectProperty>
    


    <!-- http://www.semanticweb.org/bbucher/ontologies/2025/9/geodata#hasData -->


    <owl:ObjectProperty rdf:about="http://www.semanticweb.org/bbucher/ontologies/2025/9/geodata#hasData">
        <rdfs:domain rdf:resource="http://www.semanticweb.org/bbucher/ontologies/2025/9/geodata#Representation"/>
        <rdfs:range rdf:resource="http://www.w3.org/ns/dcat#Resource"/>
    </owl:ObjectProperty>
    


    <!-- http://www.semanticweb.org/bbucher/ontologies/2025/9/geodata#hasMethodOfInstruction -->


    <owl:ObjectProperty rdf:about="http://www.semanticweb.org/bbucher/ontologies/2025/9/geodata#hasMethodOfInstruction">
        <rdfs:domain rdf:resource="http://www.semanticweb.org/bbucher/ontologies/2025/9/geodata#Collection"/>
        <rdfs:range rdf:resource="http://purl.org/dc/terms/MethodOfInstruction"/>
    </owl:ObjectProperty>
    


    <!-- http://www.semanticweb.org/bbucher/ontologies/2025/9/geodata#has_member -->


    <owl:ObjectProperty rdf:about="http://www.semanticweb.org/bbucher/ontologies/2025/9/geodata#has_member">
        <rdfs:domain rdf:resource="http://www.semanticweb.org/bbucher/ontologies/2025/9/geodata#Collection"/>
        <rdfs:range rdf:resource="http://www.semanticweb.org/bbucher/ontologies/2025/9/geodata#CollectionItem"/>
    </owl:ObjectProperty>
    


    <!-- http://www.w3.org/2004/02/skos/core#broadMatch -->


    <owl:ObjectProperty rdf:about="http://www.w3.org/2004/02/skos/core#broadMatch">
        <rdfs:subPropertyOf rdf:resource="http://www.w3.org/2004/02/skos/core#broader"/>
        <rdfs:subPropertyOf rdf:resource="http://www.w3.org/2004/02/skos/core#mappingRelation"/>
        <owl:inverseOf rdf:resource="http://www.w3.org/2004/02/skos/core#narrowMatch"/>
    </owl:ObjectProperty>
    


    <!-- http://www.w3.org/2004/02/skos/core#broader -->


    <owl:ObjectProperty rdf:about="http://www.w3.org/2004/02/skos/core#broader">
        <rdfs:subPropertyOf rdf:resource="http://www.w3.org/2004/02/skos/core#broaderTransitive"/>
    </owl:ObjectProperty>
    


    <!-- http://www.w3.org/2004/02/skos/core#broaderTransitive -->


    <owl:ObjectProperty rdf:about="http://www.w3.org/2004/02/skos/core#broaderTransitive">
        <rdfs:subPropertyOf rdf:resource="http://www.w3.org/2004/02/skos/core#semanticRelation"/>
        <owl:inverseOf rdf:resource="http://www.w3.org/2004/02/skos/core#narrowerTransitive"/>
        <rdf:type rdf:resource="http://www.w3.org/2002/07/owl#TransitiveProperty"/>
        <rdfs:isDefinedBy rdf:resource="http://www.w3.org/2004/02/skos/core"/>
        <rdfs:label xml:lang="en">has broader transitive</rdfs:label>
        <skos:definition>skos:broaderTransitive is a transitive superproperty of skos:broader.</skos:definition>
        <skos:scopeNote xml:lang="en">By convention, skos:broaderTransitive is not used to make assertions. Rather, the properties can be used to draw inferences about the transitive closure of the hierarchical relation, which is useful e.g. when implementing a simple query expansion algorithm in a search application.</skos:scopeNote>
    </owl:ObjectProperty>
    


    <!-- http://www.w3.org/2004/02/skos/core#closeMatch -->


    <owl:ObjectProperty rdf:about="http://www.w3.org/2004/02/skos/core#closeMatch">
        <rdfs:subPropertyOf rdf:resource="http://www.w3.org/2004/02/skos/core#mappingRelation"/>
        <rdf:type rdf:resource="http://www.w3.org/2002/07/owl#SymmetricProperty"/>
        <rdfs:isDefinedBy rdf:resource="http://www.w3.org/2004/02/skos/core"/>
        <rdfs:label xml:lang="en">has close match</rdfs:label>
        <skos:definition xml:lang="en">skos:closeMatch is used to link two concepts that are sufficiently similar that they can be used interchangeably in some information retrieval applications. In order to avoid the possibility of &quot;compound errors&quot; when combining mappings across more than two concept schemes, skos:closeMatch is not declared to be a transitive property.</skos:definition>
    </owl:ObjectProperty>
    


    <!-- http://www.w3.org/2004/02/skos/core#exactMatch -->


    <owl:ObjectProperty rdf:about="http://www.w3.org/2004/02/skos/core#exactMatch">
        <rdfs:subPropertyOf rdf:resource="http://www.w3.org/2004/02/skos/core#closeMatch"/>
        <rdf:type rdf:resource="http://www.w3.org/2002/07/owl#SymmetricProperty"/>
        <rdf:type rdf:resource="http://www.w3.org/2002/07/owl#TransitiveProperty"/>
        <rdfs:comment xml:lang="en">skos:exactMatch is disjoint with each of the properties skos:broadMatch and skos:relatedMatch.</rdfs:comment>
        <rdfs:isDefinedBy rdf:resource="http://www.w3.org/2004/02/skos/core"/>
        <rdfs:label xml:lang="en">has exact match</rdfs:label>
        <skos:definition xml:lang="en">skos:exactMatch is used to link two concepts, indicating a high degree of confidence that the concepts can be used interchangeably across a wide range of information retrieval applications. skos:exactMatch is a transitive property, and is a sub-property of skos:closeMatch.</skos:definition>
    </owl:ObjectProperty>
    


    <!-- http://www.w3.org/2004/02/skos/core#hasTopConcept -->


    <owl:ObjectProperty rdf:about="http://www.w3.org/2004/02/skos/core#hasTopConcept">
        <owl:inverseOf rdf:resource="http://www.w3.org/2004/02/skos/core#topConceptOf"/>
        <rdfs:domain rdf:resource="http://www.w3.org/2004/02/skos/core#ConceptScheme"/>
        <rdfs:range rdf:resource="http://www.w3.org/2004/02/skos/core#Concept"/>
    </owl:ObjectProperty>
    


    <!-- http://www.w3.org/2004/02/skos/core#inScheme -->


    <owl:ObjectProperty rdf:about="http://www.w3.org/2004/02/skos/core#inScheme">
        <rdfs:range rdf:resource="http://www.w3.org/2004/02/skos/core#ConceptScheme"/>
        <rdfs:isDefinedBy rdf:resource="http://www.w3.org/2004/02/skos/core"/>
        <rdfs:label xml:lang="en">is in scheme</rdfs:label>
        <skos:definition xml:lang="en">Relates a resource (for example a concept) to a concept scheme in which it is included.</skos:definition>
        <skos:scopeNote xml:lang="en">A concept may be a member of more than one concept scheme.</skos:scopeNote>
    </owl:ObjectProperty>
    


    <!-- http://www.w3.org/2004/02/skos/core#mappingRelation -->


    <owl:ObjectProperty rdf:about="http://www.w3.org/2004/02/skos/core#mappingRelation">
        <rdfs:subPropertyOf rdf:resource="http://www.w3.org/2004/02/skos/core#semanticRelation"/>
        <rdfs:comment xml:lang="en">These concept mapping relations mirror semantic relations, and the data model defined below is similar (with the exception of skos:exactMatch) to the data model defined for semantic relations. A distinct vocabulary is provided for concept mapping relations, to provide a convenient way to differentiate links within a concept scheme from links between concept schemes. However, this pattern of usage is not a formal requirement of the SKOS data model, and relies on informal definitions of best practice.</rdfs:comment>
        <rdfs:isDefinedBy rdf:resource="http://www.w3.org/2004/02/skos/core"/>
        <rdfs:label xml:lang="en">is in mapping relation with</rdfs:label>
        <skos:definition xml:lang="en">Relates two concepts coming, by convention, from different schemes, and that have comparable meanings</skos:definition>
    </owl:ObjectProperty>
    


    <!-- http://www.w3.org/2004/02/skos/core#member -->


    <owl:ObjectProperty rdf:about="http://www.w3.org/2004/02/skos/core#member">
        <rdfs:domain rdf:resource="http://www.w3.org/2004/02/skos/core#Collection"/>
        <rdfs:range>
            <owl:Class>
                <owl:unionOf rdf:parseType="Collection">
                    <rdf:Description rdf:about="http://www.w3.org/2004/02/skos/core#Collection"/>
                    <rdf:Description rdf:about="http://www.w3.org/2004/02/skos/core#Concept"/>
                </owl:unionOf>
            </owl:Class>
        </rdfs:range>
        <rdfs:isDefinedBy rdf:resource="http://www.w3.org/2004/02/skos/core"/>
        <rdfs:label xml:lang="en">has member</rdfs:label>
        <skos:definition xml:lang="en">Relates a collection to one of its members.</skos:definition>
    </owl:ObjectProperty>
    


    <!-- http://www.w3.org/2004/02/skos/core#memberList -->


    <owl:ObjectProperty rdf:about="http://www.w3.org/2004/02/skos/core#memberList">
        <rdf:type rdf:resource="http://www.w3.org/2002/07/owl#FunctionalProperty"/>
        <rdfs:domain rdf:resource="http://www.w3.org/2004/02/skos/core#OrderedCollection"/>
        <rdfs:range rdf:resource="http://www.w3.org/1999/02/22-rdf-syntax-ns#List"/>
        <rdfs:comment xml:lang="en">For any resource, every item in the list given as the value of the
      skos:memberList property is also a value of the skos:member property.</rdfs:comment>
        <rdfs:isDefinedBy rdf:resource="http://www.w3.org/2004/02/skos/core"/>
        <rdfs:label xml:lang="en">has member list</rdfs:label>
        <skos:definition xml:lang="en">Relates an ordered collection to the RDF list containing its members.</skos:definition>
    </owl:ObjectProperty>
    


    <!-- http://www.w3.org/2004/02/skos/core#narrowMatch -->


    <owl:ObjectProperty rdf:about="http://www.w3.org/2004/02/skos/core#narrowMatch">
        <rdfs:subPropertyOf rdf:resource="http://www.w3.org/2004/02/skos/core#mappingRelation"/>
        <rdfs:subPropertyOf rdf:resource="http://www.w3.org/2004/02/skos/core#narrower"/>
    </owl:ObjectProperty>
    


    <!-- http://www.w3.org/2004/02/skos/core#narrower -->


    <owl:ObjectProperty rdf:about="http://www.w3.org/2004/02/skos/core#narrower">
        <rdfs:subPropertyOf rdf:resource="http://www.w3.org/2004/02/skos/core#narrowerTransitive"/>
        <owl:inverseOf rdf:resource="http://www.w3.org/2004/02/skos/core#broader"/>
        <rdfs:comment xml:lang="en">Narrower concepts are typically rendered as children in a concept hierarchy (tree).</rdfs:comment>
        <rdfs:isDefinedBy rdf:resource="http://www.w3.org/2004/02/skos/core"/>
        <rdfs:label xml:lang="en">has narrower</rdfs:label>
        <skos:definition xml:lang="en">Relates a concept to a concept that is more specific in meaning.</skos:definition>
        <skos:scopeNote xml:lang="en">By convention, skos:broader is only used to assert an immediate (i.e. direct) hierarchical link between two conceptual resources.</skos:scopeNote>
    </owl:ObjectProperty>
    


    <!-- http://www.w3.org/2004/02/skos/core#narrowerTransitive -->


    <owl:ObjectProperty rdf:about="http://www.w3.org/2004/02/skos/core#narrowerTransitive">
        <rdfs:subPropertyOf rdf:resource="http://www.w3.org/2004/02/skos/core#semanticRelation"/>
        <rdf:type rdf:resource="http://www.w3.org/2002/07/owl#TransitiveProperty"/>
        <rdfs:isDefinedBy rdf:resource="http://www.w3.org/2004/02/skos/core"/>
        <rdfs:label xml:lang="en">has narrower transitive</rdfs:label>
        <skos:definition>skos:narrowerTransitive is a transitive superproperty of skos:narrower.</skos:definition>
        <skos:scopeNote xml:lang="en">By convention, skos:narrowerTransitive is not used to make assertions. Rather, the properties can be used to draw inferences about the transitive closure of the hierarchical relation, which is useful e.g. when implementing a simple query expansion algorithm in a search application.</skos:scopeNote>
    </owl:ObjectProperty>
    


    <!-- http://www.w3.org/2004/02/skos/core#related -->


    <owl:ObjectProperty rdf:about="http://www.w3.org/2004/02/skos/core#related">
        <rdfs:subPropertyOf rdf:resource="http://www.w3.org/2004/02/skos/core#semanticRelation"/>
        <rdf:type rdf:resource="http://www.w3.org/2002/07/owl#SymmetricProperty"/>
        <rdfs:comment xml:lang="en">skos:related is disjoint with skos:broaderTransitive</rdfs:comment>
        <rdfs:isDefinedBy rdf:resource="http://www.w3.org/2004/02/skos/core"/>
        <rdfs:label xml:lang="en">has related</rdfs:label>
        <skos:definition xml:lang="en">Relates a concept to a concept with which there is an associative semantic relationship.</skos:definition>
    </owl:ObjectProperty>
    


    <!-- http://www.w3.org/2004/02/skos/core#relatedMatch -->


    <owl:ObjectProperty rdf:about="http://www.w3.org/2004/02/skos/core#relatedMatch">
        <rdfs:subPropertyOf rdf:resource="http://www.w3.org/2004/02/skos/core#mappingRelation"/>
        <rdfs:subPropertyOf rdf:resource="http://www.w3.org/2004/02/skos/core#related"/>
        <rdf:type rdf:resource="http://www.w3.org/2002/07/owl#SymmetricProperty"/>
    </owl:ObjectProperty>
    


    <!-- http://www.w3.org/2004/02/skos/core#semanticRelation -->


    <owl:ObjectProperty rdf:about="http://www.w3.org/2004/02/skos/core#semanticRelation">
        <rdfs:domain rdf:resource="http://www.w3.org/2004/02/skos/core#Concept"/>
        <rdfs:range rdf:resource="http://www.w3.org/2004/02/skos/core#Concept"/>
        <rdfs:isDefinedBy rdf:resource="http://www.w3.org/2004/02/skos/core"/>
        <rdfs:label xml:lang="en">is in semantic relation with</rdfs:label>
        <skos:definition xml:lang="en">Links a concept to a concept related by meaning.</skos:definition>
        <skos:scopeNote xml:lang="en">This property should not be used directly, but as a super-property for all properties denoting a relationship of meaning between concepts.</skos:scopeNote>
    </owl:ObjectProperty>
    


    <!-- http://www.w3.org/2004/02/skos/core#topConceptOf -->


    <owl:ObjectProperty rdf:about="http://www.w3.org/2004/02/skos/core#topConceptOf">
        <rdfs:subPropertyOf rdf:resource="http://www.w3.org/2004/02/skos/core#inScheme"/>
        <rdfs:domain rdf:resource="http://www.w3.org/2004/02/skos/core#Concept"/>
        <rdfs:range rdf:resource="http://www.w3.org/2004/02/skos/core#ConceptScheme"/>
        <rdfs:isDefinedBy rdf:resource="http://www.w3.org/2004/02/skos/core"/>
        <rdfs:label xml:lang="en">is top concept in scheme</rdfs:label>
        <skos:definition xml:lang="en">Relates a concept to the concept scheme that it is a top level concept of.</skos:definition>
    </owl:ObjectProperty>
    


    <!-- http://www.w3.org/ns/dcat#accessService -->


    <owl:ObjectProperty rdf:about="http://www.w3.org/ns/dcat#accessService">
        <rdfs:range rdf:resource="http://www.w3.org/ns/dcat#DataService"/>
        <rdfs:comment xml:lang="en">A site or end-point that gives access to the distribution of the dataset.</rdfs:comment>
        <rdfs:comment xml:lang="da">Et websted eller endpoint der giver adgang til en repræsentation af datasættet.</rdfs:comment>
        <rdfs:comment xml:lang="cs">Umístění či přístupový bod zpřístupňující distribuci datové sady.</rdfs:comment>
        <rdfs:comment xml:lang="es">Un sitio o end-point que da acceso a la distribución de un conjunto de datos.</rdfs:comment>
        <rdfs:comment xml:lang="it">Un sito o end-point che dà accesso alla distribuzione del set di dati.</rdfs:comment>
        <rdfs:isDefinedBy rdf:resource="https://www.w3.org/TR/vocab-dcat-2/"/>
        <rdfs:label xml:lang="en">data access service</rdfs:label>
        <rdfs:label xml:lang="da">dataadgangstjeneste</rdfs:label>
        <rdfs:label xml:lang="es">servicio de acceso de datos</rdfs:label>
        <rdfs:label xml:lang="it">servizio di accesso ai dati</rdfs:label>
        <rdfs:label xml:lang="cs">služba pro přístup k datům</rdfs:label>
        <skos:changeNote xml:lang="en">New property added in DCAT 2.</skos:changeNote>
        <skos:changeNote xml:lang="cs">Nová vlastnost přidaná ve verzi DCAT 2.</skos:changeNote>
        <skos:changeNote xml:lang="es">Nueva propiedad agregada en DCAT 2.</skos:changeNote>
        <skos:changeNote xml:lang="it">Nuova proprietà aggiunta in DCAT 2.</skos:changeNote>
        <skos:changeNote xml:lang="da">Ny egenskab tilføjet i DCAT 2.</skos:changeNote>
        <skos:definition xml:lang="en">A site or end-point that gives access to the distribution of the dataset.</skos:definition>
        <skos:definition xml:lang="da">Et websted eller endpoint der giver adgang til en repræsentation af datasættet.</skos:definition>
        <skos:definition xml:lang="cs">Umístění či přístupový bod zpřístupňující distribuci datové sady.</skos:definition>
        <skos:definition xml:lang="es">Un sitio o end-point que da acceso a la distribución de un conjunto de datos.</skos:definition>
        <skos:definition xml:lang="it">Un sito o end-point che dà accesso alla distribuzione del set di dati.</skos:definition>
    </owl:ObjectProperty>
    


    <!-- http://www.w3.org/ns/dcat#accessURL -->


    <owl:ObjectProperty rdf:about="http://www.w3.org/ns/dcat#accessURL">
        <rdfs:domain rdf:resource="http://www.w3.org/ns/dcat#Distribution"/>
        <rdfs:range rdf:resource="http://www.w3.org/2000/01/rdf-schema#Resource"/>
        <owl:propertyChainAxiom rdf:parseType="Collection">
            <rdf:Description rdf:about="http://www.w3.org/ns/dcat#accessService"/>
            <rdf:Description rdf:about="http://www.w3.org/ns/dcat#endpointURL"/>
        </owl:propertyChainAxiom>
        <rdfs:comment xml:lang="en">A URL of a resource that gives access to a distribution of the dataset. E.g. landing page, feed, SPARQL endpoint. Use for all cases except a simple download link, in which case downloadURL is preferred.</rdfs:comment>
        <rdfs:comment xml:lang="fr">Ceci peut être tout type d&apos;URL qui donne accès à une distribution du jeu de données. Par exemple, un lien à une page HTML contenant un lien au jeu de données, un Flux RSS, un point d&apos;accès SPARQL. Utilisez le lorsque votre catalogue ne contient pas d&apos;information sur quoi il est ou quand ce n&apos;est pas téléchargeable.</rdfs:comment>
        <rdfs:comment xml:lang="da">En URL for en ressource som giver adgang til en repræsentation af datsættet. Fx destinationsside, feed, SPARQL-endpoint. Anvendes i alle sammenhænge undtagen til angivelse af et simpelt download link hvor anvendelse af egenskaben downloadURL foretrækkes.</rdfs:comment>
        <rdfs:comment xml:lang="es">Puede ser cualquier tipo de URL que de acceso a una distribución del conjunto de datos, e.g., página de destino, descarga, URL feed, punto de acceso SPARQL. Esta propriedad se debe usar cuando su catálogo de datos no tiene información sobre donde está o cuando no se puede descargar.</rdfs:comment>
        <rdfs:comment xml:lang="cs">URL zdroje, přes které je přístupná distribuce datové sady. Příkladem může být vstupní stránka, RSS kanál či SPARQL endpoint. Použijte ve všech případech kromě URL souboru ke stažení, pro které je lepší použít dcat:downloadURL.</rdfs:comment>
        <rdfs:comment xml:lang="it">Un URL di una risorsa che consente di accedere a una distribuzione del set di dati. Per esempio, pagina di destinazione, feed, endpoint SPARQL. Da utilizzare per tutti i casi, tranne  quando  si tratta di un semplice link per il download nel qual caso è preferito downloadURL.</rdfs:comment>
        <rdfs:comment xml:lang="el">Μπορεί να είναι οποιουδήποτε είδους URL που δίνει πρόσβαση στη διανομή ενός συνόλου δεδομένων. Π.χ. ιστοσελίδα αρχικής πρόσβασης, μεταφόρτωση, feed URL, σημείο διάθεσης SPARQL. Να χρησιμοποιείται όταν ο κατάλογος δεν περιέχει πληροφορίες εαν πρόκειται ή όχι για μεταφορτώσιμο αρχείο.</rdfs:comment>
        <rdfs:comment xml:lang="ar">أي رابط يتيح الوصول إلى البيانات. إذا كان الرابط هو ربط مباشر لملف يمكن تحميله استخدم الخاصية downloadURL</rdfs:comment>
        <rdfs:comment xml:lang="ja">データセットの配信にアクセス権を与えるランディング・ページ、フィード、SPARQLエンドポイント、その他の種類の資源。</rdfs:comment>
        <rdfs:isDefinedBy rdf:resource="http://www.w3.org/TR/vocab-dcat/"/>
        <rdfs:label xml:lang="fr">URL d&apos;accès</rdfs:label>
        <rdfs:label xml:lang="es">URL de acceso</rdfs:label>
        <rdfs:label xml:lang="el">URL πρόσβασης</rdfs:label>
        <rdfs:label xml:lang="en">access address</rdfs:label>
        <rdfs:label xml:lang="da">adgangsadresse</rdfs:label>
        <rdfs:label xml:lang="it">indirizzo di accesso</rdfs:label>
        <rdfs:label xml:lang="cs">přístupová adresa</rdfs:label>
        <rdfs:label xml:lang="ar">رابط وصول</rdfs:label>
        <rdfs:label xml:lang="ja">アクセスURL</rdfs:label>
        <skos:altLabel xml:lang="da">adgangsURL</skos:altLabel>
        <skos:definition xml:lang="en">A URL of a resource that gives access to a distribution of the dataset. E.g. landing page, feed, SPARQL endpoint. Use for all cases except a simple download link, in which case downloadURL is preferred.</skos:definition>
        <skos:definition xml:lang="fr">Ceci peut être tout type d&apos;URL qui donne accès à une distribution du jeu de données. Par exemple, un lien à une page HTML contenant un lien au jeu de données, un Flux RSS, un point d&apos;accès SPARQL. Utilisez le lorsque votre catalogue ne contient pas d&apos;information sur quoi il est ou quand ce n&apos;est pas téléchargeable.</skos:definition>
        <skos:definition xml:lang="da">En URL for en ressource som giver adgang til en repræsentation af datsættet. Fx destinationsside, feed, SPARQL-endpoint. Anvendes i alle sammenhænge undtagen til angivelse af et simpelt download link hvor anvendelse af egenskaben downloadURL foretrækkes.</skos:definition>
        <skos:definition xml:lang="es">Puede ser cualquier tipo de URL que de acceso a una distribución del conjunto de datos, e.g., página de destino, descarga, URL feed, punto de acceso SPARQL. Esta propriedad se debe usar cuando su catálogo de datos no tiene información sobre donde está o cuando no se puede descargar.</skos:definition>
        <skos:definition xml:lang="cs">URL zdroje, přes které je přístupná distribuce datové sady. Příkladem může být vstupní stránka, RSS kanál či SPARQL endpoint. Použijte ve všech případech kromě URL souboru ke stažení, pro které je lepší použít dcat:downloadURL.</skos:definition>
        <skos:definition xml:lang="it">Un URL di una risorsa che consente di accedere a una distribuzione del set di dati. Per esempio, pagina di destinazione, feed, endpoint SPARQL. Da utilizzare per tutti i casi, tranne  quando  si tratta di un semplice link per il download nel qual caso è preferito downloadURL.</skos:definition>
        <skos:definition xml:lang="el">Μπορεί να είναι οποιουδήποτε είδους URL που δίνει πρόσβαση στη διανομή ενός συνόλου δεδομένων. Π.χ. ιστοσελίδα αρχικής πρόσβασης, μεταφόρτωση, feed URL, σημείο διάθεσης SPARQL. Να χρησιμοποιείται όταν ο κατάλογος δεν περιέχει πληροφορίες εαν πρόκειται ή όχι για μεταφορτώσιμο αρχείο.</skos:definition>
        <skos:definition xml:lang="ar">أي رابط يتيح الوصول إلى البيانات. إذا كان الرابط هو ربط مباشر لملف يمكن تحميله استخدم الخاصية downloadURL</skos:definition>
        <skos:definition xml:lang="ja">データセットの配信にアクセス権を与えるランディング・ページ、フィード、SPARQLエンドポイント、その他の種類の資源。</skos:definition>
        <skos:editorialNote xml:lang="en">Status: English Definition text modified by DCAT revision team, updated Italian and Czech translation provided, translations for other languages pending.</skos:editorialNote>
        <skos:editorialNote xml:lang="en">rdfs:label, rdfs:comment and skos:scopeNote have been modified. Non-english versions except for Italian must be updated.</skos:editorialNote>
        <skos:scopeNote xml:lang="es">El rango es una URL. Si la distribución es accesible solamente través de una página de destino (es decir, si no se conoce una URL de descarga directa), entonces el enlance a la página de destino debe ser duplicado como accessURL en la distribución.</skos:scopeNote>
        <skos:scopeNote xml:lang="da">Hvis en eller flere distributioner kun er tilgængelige via en destinationsside (dvs. en URL til direkte download er ikke kendt), så bør destinationssidelinket gentages som adgangsadresse for distributionen.</skos:scopeNote>
        <skos:scopeNote xml:lang="en">If the distribution(s) are accessible only through a landing page (i.e. direct download URLs are not known), then the landing page link should be duplicated as accessURL on a distribution.</skos:scopeNote>
        <skos:scopeNote xml:lang="fr">La valeur est une URL. Si la distribution est accessible seulement au travers d&apos;une page d&apos;atterrissage (c-à-dire on n&apos;ignore une URL de téléchargement direct), alors le lien à la page d&apos;atterrissage doit être dupliqué comee accessURL sur la distribution.</skos:scopeNote>
        <skos:scopeNote xml:lang="cs">Pokud jsou distribuce přístupné pouze přes vstupní stránku (tj. URL pro přímé stažení nejsou známa), pak by URL přístupové stránky mělo být duplikováno ve vlastnosti distribuce accessURL.</skos:scopeNote>
        <skos:scopeNote xml:lang="it">Se le distribuzioni sono accessibili solo attraverso una pagina web (ad esempio, gli URL per il download diretto non sono noti), allora il link della pagina web deve essere duplicato come accessURL sulla distribuzione.</skos:scopeNote>
        <skos:scopeNote xml:lang="el">Η τιμή είναι ένα URL. Αν η/οι διανομή/ές είναι προσβάσιμη/ες μόνο μέσω μίας ιστοσελίδας αρχικής πρόσβασης (δηλαδή αν δεν υπάρχουν γνωστές διευθύνσεις άμεσης μεταφόρτωσης), τότε ο σύνδεσμος της ιστοσελίδας αρχικής πρόσβασης πρέπει να αναπαραχθεί ως accessURL σε μία διανομή.</skos:scopeNote>
        <skos:scopeNote xml:lang="ja">確実にダウンロードでない場合や、ダウンロードかどうかが不明である場合は、downloadURLではなく、accessURLを用いてください。ランディング・ページを通じてしか配信にアクセスできない場合（つまり、直接的なダウンロードURLが不明）は、配信におけるaccessURLとしてランディング・ページのリンクをコピーすべきです（SHOULD）。</skos:scopeNote>
    </owl:ObjectProperty>
    


    <!-- http://www.w3.org/ns/dcat#catalog -->


    <owl:ObjectProperty rdf:about="http://www.w3.org/ns/dcat#catalog">
        <rdfs:subPropertyOf rdf:resource="http://www.w3.org/ns/dcat#resource"/>
        <rdfs:domain rdf:resource="http://www.w3.org/ns/dcat#Catalog"/>
        <rdfs:range rdf:resource="http://www.w3.org/ns/dcat#Catalog"/>
        <rdfs:comment xml:lang="en">A catalog that is listed in the catalog.</rdfs:comment>
        <rdfs:comment xml:lang="da">Et katalog hvis indhold er relevant i forhold til det aktuelle katalog.</rdfs:comment>
        <rdfs:comment xml:lang="cs">Katalog, jehož obsah je v kontextu tohoto katalogu zajímavý.</rdfs:comment>
        <rdfs:comment xml:lang="it">Un catalogo i cui contenuti sono di interesse nel contesto di questo catalogo.</rdfs:comment>
        <rdfs:comment xml:lang="es">Un catálogo cuyo contenido es de interés en el contexto del catálogo que está siendo descripto.</rdfs:comment>
        <rdfs:isDefinedBy rdf:resource="https://www.w3.org/TR/vocab-dcat-2/"/>
        <rdfs:label xml:lang="en">catalog</rdfs:label>
        <rdfs:label xml:lang="it">catalogo</rdfs:label>
        <rdfs:label xml:lang="es">catálogo</rdfs:label>
        <rdfs:label xml:lang="cs">katalog</rdfs:label>
        <rdfs:label xml:lang="da">katalog</rdfs:label>
        <skos:altLabel xml:lang="da">har delkatalog</skos:altLabel>
        <skos:altLabel xml:lang="en">has catalog</skos:altLabel>
        <skos:changeNote xml:lang="en">New property added in DCAT 2.</skos:changeNote>
        <skos:changeNote xml:lang="cs">Nová vlastnost přidaná ve verzi DCAT 2.</skos:changeNote>
        <skos:changeNote xml:lang="es">Nueva propiedad agregada en DCAT 2.</skos:changeNote>
        <skos:changeNote xml:lang="it">Nuova proprietà aggiunta in DCAT 2.</skos:changeNote>
        <skos:definition xml:lang="en">A catalog that is listed in the catalog.</skos:definition>
        <skos:definition xml:lang="da">Et katalog hvis indhold er relevant i forhold til det aktuelle katalog.</skos:definition>
        <skos:definition xml:lang="cs">Katalog, jehož obsah je v kontextu tohoto katalogu zajímavý.</skos:definition>
        <skos:definition xml:lang="it">Un catalogo i cui contenuti sono di interesse nel contesto di questo catalogo.</skos:definition>
        <skos:definition xml:lang="es">Un catálogo cuyo contenido es de interés en el contexto del catálogo que está siendo descripto.</skos:definition>
        <skos:editorialNote xml:lang="en">Status: English Definition text modified by DCAT 3 revision team, translations pending.</skos:editorialNote>
    </owl:ObjectProperty>
    


    <!-- http://www.w3.org/ns/dcat#compressFormat -->


    <owl:ObjectProperty rdf:about="http://www.w3.org/ns/dcat#compressFormat">
        <rdfs:subPropertyOf rdf:resource="http://purl.org/dc/terms/format"/>
        <rdfs:domain rdf:resource="http://www.w3.org/ns/dcat#Distribution"/>
        <rdfs:range rdf:resource="http://purl.org/dc/terms/MediaType"/>
        <rdfs:comment xml:lang="es">El formato de la distribución en el que los datos están en forma comprimida, e.g. para reducir el tamaño del archivo a bajar.</rdfs:comment>
        <rdfs:comment xml:lang="cs">Formát komprese souboru, ve kterém jsou data poskytována v komprimované podobě, např. ke snížení velikosti souboru ke stažení.</rdfs:comment>
        <rdfs:comment xml:lang="it">Il formato di compressione della distribuzione nel quale i dati sono in forma compressa, ad es. per ridurre le dimensioni del file da scaricare.</rdfs:comment>
        <rdfs:comment xml:lang="da">Kompressionsformatet for distributionen som indeholder data i et komprimeret format, fx for at reducere størrelsen af downloadfilen.</rdfs:comment>
        <rdfs:comment xml:lang="en">The compression format of the distribution in which the data is contained in a compressed form, e.g. to reduce the size of the downloadable file.</rdfs:comment>
        <rdfs:isDefinedBy rdf:resource="https://www.w3.org/TR/vocab-dcat-2/"/>
        <rdfs:label xml:lang="en">compression format</rdfs:label>
        <rdfs:label xml:lang="es">formato de compresión</rdfs:label>
        <rdfs:label xml:lang="it">formato di compressione</rdfs:label>
        <rdfs:label xml:lang="cs">formát komprese</rdfs:label>
        <rdfs:label xml:lang="da">kompressionsformat</rdfs:label>
        <skos:changeNote xml:lang="en">New property added in DCAT 2.</skos:changeNote>
        <skos:changeNote xml:lang="cs">Nová vlastnost přidaná ve verzi DCAT 2.</skos:changeNote>
        <skos:changeNote xml:lang="es">Nueva propiedad agregada en DCAT 2.</skos:changeNote>
        <skos:changeNote xml:lang="it">Nuova proprietà aggiunta in DCAT 2.</skos:changeNote>
        <skos:changeNote xml:lang="da">Ny egenskab tilføjet i DCAT 2.</skos:changeNote>
        <skos:definition xml:lang="es">El formato de la distribución en el que los datos están en forma comprimida, e.g. para reducir el tamaño del archivo a bajar.</skos:definition>
        <skos:definition xml:lang="cs">Formát komprese souboru, ve kterém jsou data poskytována v komprimované podobě, např. ke snížení velikosti souboru ke stažení.</skos:definition>
        <skos:definition xml:lang="it">Il formato di compressione della distribuzione nel quale i dati sono in forma compressa, ad es. per ridurre le dimensioni del file da scaricare.</skos:definition>
        <skos:definition xml:lang="da">Kompressionsformatet for distributionen som indeholder data i et komprimeret format, fx for at reducere størrelsen af downloadfilen.</skos:definition>
        <skos:definition xml:lang="en">The compression format of the distribution in which the data is contained in a compressed form, e.g. to reduce the size of the downloadable file.</skos:definition>
        <skos:scopeNote xml:lang="da">Denne egenskab kan anvendes når filerne i en distribution er blevet komprimeret, fx i en ZIP-fil. Formatet BØR udtrykkes ved en medietype som defineret i &apos;IANA media types registry&apos;, hvis der optræder en relevant medietype dér: https://www.iana.org/assignments/media-types/.</skos:scopeNote>
        <skos:scopeNote xml:lang="es">Esta propiedad se debe usar cuando los archivos de la distribución están comprimidos, por ejemplo en un archivo ZIP. El formato DEBERÍA expresarse usando un &apos;media type&apos;, tales como los definidos en el registro IANA de &apos;media types&apos; https://www.iana.org/assignments/media-types/, si está disponibles.</skos:scopeNote>
        <skos:scopeNote xml:lang="it">Questa proprietà deve essere utilizzata quando i file nella distribuzione sono compressi, ad es. in un file ZIP. Il formato DOVREBBE essere espresso usando un tipo di media come definito dal registro dei tipi di media IANA https://www.iana.org/assignments/media-types/, se disponibile.</skos:scopeNote>
        <skos:scopeNote xml:lang="cs">Tato vlastnost se použije, když jsou soubory v distribuci komprimovány, např. v ZIP souboru. Formát BY MĚL být vyjádřen pomocí typu média definovaného v registru IANA https://www.iana.org/assignments/media-types/, pokud existuje.</skos:scopeNote>
        <skos:scopeNote xml:lang="en">This property is to be used when the files in the distribution are compressed, e.g. in a ZIP file. The format SHOULD be expressed using a media type as defined by IANA media types registry https://www.iana.org/assignments/media-types/, if available.</skos:scopeNote>
    </owl:ObjectProperty>
    


    <!-- http://www.w3.org/ns/dcat#contactPoint -->


    <owl:ObjectProperty rdf:about="http://www.w3.org/ns/dcat#contactPoint">
        <rdfs:range rdf:resource="http://www.w3.org/2006/vcard/ns#Kind"/>
        <rdfs:comment xml:lang="es">Información relevante de contacto para el recurso catalogado. Se recomienda el uso de vCard.</rdfs:comment>
        <rdfs:comment xml:lang="it">Informazioni di contatto rilevanti per la risorsa catalogata. Si raccomanda l&apos;uso di vCard.</rdfs:comment>
        <rdfs:comment xml:lang="en">Relevant contact information for the catalogued resource. Use of vCard is recommended.</rdfs:comment>
        <rdfs:comment xml:lang="da">Relevante kontaktoplysninger for den katalogiserede ressource. Anvendelse af vCard anbefales.</rdfs:comment>
        <rdfs:comment xml:lang="cs">Relevantní kontaktní informace pro katalogizovaný zdroj. Doporučuje se použít slovník VCard.</rdfs:comment>
        <rdfs:comment xml:lang="fr">Relie un jeu de données à une information de contact utile en utilisant VCard.</rdfs:comment>
        <rdfs:comment xml:lang="el">Συνδέει ένα σύνολο δεδομένων με ένα σχετικό σημείο επικοινωνίας, μέσω VCard.</rdfs:comment>
        <rdfs:comment xml:lang="ar">تربط قائمة البيانات بعنوان اتصال موصف  باستخدام VCard</rdfs:comment>
        <rdfs:comment xml:lang="ja">データセットを、VCardを用いて提供されている適切な連絡先情報にリンクします。</rdfs:comment>
        <rdfs:isDefinedBy rdf:resource="http://www.w3.org/TR/vocab-dcat/"/>
        <rdfs:label xml:lang="es">Punto de contacto</rdfs:label>
        <rdfs:label xml:lang="en">contact point</rdfs:label>
        <rdfs:label xml:lang="cs">kontaktní bod</rdfs:label>
        <rdfs:label xml:lang="da">kontaktpunkt</rdfs:label>
        <rdfs:label xml:lang="fr">point de contact</rdfs:label>
        <rdfs:label xml:lang="it">punto di contatto</rdfs:label>
        <rdfs:label xml:lang="el">σημείο επικοινωνίας</rdfs:label>
        <rdfs:label xml:lang="ar">عنوان اتصال</rdfs:label>
        <rdfs:label xml:lang="ja">窓口</rdfs:label>
        <skos:definition xml:lang="es">Información relevante de contacto para el recurso catalogado. Se recomienda el uso de vCard.</skos:definition>
        <skos:definition xml:lang="it">Informazioni di contatto rilevanti per la risorsa catalogata. Si raccomanda l&apos;uso di vCard.</skos:definition>
        <skos:definition xml:lang="en">Relevant contact information for the catalogued resource. Use of vCard is recommended.</skos:definition>
        <skos:definition xml:lang="da">Relevante kontaktoplysninger for den katalogiserede ressource. Anvendelse af vCard anbefales.</skos:definition>
        <skos:definition xml:lang="cs">Relevantní kontaktní informace pro katalogizovaný zdroj. Doporučuje se použít slovník VCard.</skos:definition>
        <skos:definition xml:lang="fr">Relie un jeu de données à une information de contact utile en utilisant VCard.</skos:definition>
        <skos:definition xml:lang="el">Συνδέει ένα σύνολο δεδομένων με ένα σχετικό σημείο επικοινωνίας, μέσω VCard.</skos:definition>
        <skos:definition xml:lang="ar">تربط قائمة البيانات بعنوان اتصال موصف  باستخدام VCard</skos:definition>
        <skos:definition xml:lang="ja">データセットを、VCardを用いて提供されている適切な連絡先情報にリンクします。</skos:definition>
        <skos:editorialNote xml:lang="en">Status: English Definition text modified by DCAT revision team, Italian, Spanish and Czech translations provided, other translations pending.</skos:editorialNote>
    </owl:ObjectProperty>
    


    <!-- http://www.w3.org/ns/dcat#dataset -->


    <owl:ObjectProperty rdf:about="http://www.w3.org/ns/dcat#dataset">
        <rdfs:subPropertyOf rdf:resource="http://www.w3.org/ns/dcat#resource"/>
        <rdfs:domain rdf:resource="http://www.w3.org/ns/dcat#Catalog"/>
        <rdfs:range rdf:resource="http://www.w3.org/ns/dcat#Dataset"/>
        <rdfs:comment xml:lang="en">A dataset that is listed in the catalog.</rdfs:comment>
        <rdfs:comment xml:lang="da">En samling af data som er opført i kataloget.</rdfs:comment>
        <rdfs:comment xml:lang="cs">Kolekce dat, která je katalogizována v katalogu.</rdfs:comment>
        <rdfs:comment xml:lang="fr">Relie un catalogue à un jeu de données faisant partie de ce catalogue.</rdfs:comment>
        <rdfs:comment xml:lang="es">Un conjunto de datos que se lista en el catálogo.</rdfs:comment>
        <rdfs:comment xml:lang="it">Una raccolta di dati che è elencata nel catalogo.</rdfs:comment>
        <rdfs:comment xml:lang="el">Συνδέει έναν κατάλογο με ένα σύνολο δεδομένων το οποίο ανήκει στον εν λόγω κατάλογο.</rdfs:comment>
        <rdfs:comment xml:lang="ar">تربط الفهرس بقائمة بيانات ضمنه</rdfs:comment>
        <rdfs:comment xml:lang="ja">カタログの一部であるデータセット。</rdfs:comment>
        <rdfs:isDefinedBy rdf:resource="http://www.w3.org/TR/vocab-dcat/"/>
        <rdfs:label xml:lang="es">conjunto de datos</rdfs:label>
        <rdfs:label xml:lang="en">dataset</rdfs:label>
        <rdfs:label xml:lang="it">dataset</rdfs:label>
        <rdfs:label xml:lang="da">datasæt</rdfs:label>
        <rdfs:label xml:lang="cs">datová sada</rdfs:label>
        <rdfs:label xml:lang="fr">jeu de données</rdfs:label>
        <rdfs:label xml:lang="el">σύνολο δεδομένων</rdfs:label>
        <rdfs:label xml:lang="ar">قائمة بيانات</rdfs:label>
        <rdfs:label xml:lang="ja">データセット</rdfs:label>
        <skos:altLabel xml:lang="da">datasamling</skos:altLabel>
        <skos:altLabel xml:lang="da">har datasæt</skos:altLabel>
        <skos:altLabel xml:lang="en">has dataset</skos:altLabel>
        <skos:definition xml:lang="en">A dataset that is listed in the catalog.</skos:definition>
        <skos:definition xml:lang="da">En samling af data som er opført i kataloget.</skos:definition>
        <skos:definition xml:lang="cs">Kolekce dat, která je katalogizována v katalogu.</skos:definition>
        <skos:definition xml:lang="fr">Relie un catalogue à un jeu de données faisant partie de ce catalogue.</skos:definition>
        <skos:definition xml:lang="es">Un conjunto de datos que se lista en el catálogo.</skos:definition>
        <skos:definition xml:lang="it">Una raccolta di dati che è elencata nel catalogo.</skos:definition>
        <skos:definition xml:lang="el">Συνδέει έναν κατάλογο με ένα σύνολο δεδομένων το οποίο ανήκει στον εν λόγω κατάλογο.</skos:definition>
        <skos:definition xml:lang="ar">تربط الفهرس بقائمة بيانات ضمنه</skos:definition>
        <skos:definition xml:lang="ja">カタログの一部であるデータセット。</skos:definition>
        <skos:editorialNote xml:lang="en">Status: English Definition text modified by DCAT 3 revision team, translations pending.</skos:editorialNote>
    </owl:ObjectProperty>
    


    <!-- http://www.w3.org/ns/dcat#distribution -->


    <owl:ObjectProperty rdf:about="http://www.w3.org/ns/dcat#distribution">
        <rdfs:domain rdf:resource="http://www.w3.org/ns/dcat#Dataset"/>
        <rdfs:range rdf:resource="http://www.w3.org/ns/dcat#Distribution"/>
    </owl:ObjectProperty>
    


    <!-- http://www.w3.org/ns/dcat#downloadURL -->


    <owl:ObjectProperty rdf:about="http://www.w3.org/ns/dcat#downloadURL">
        <rdfs:domain rdf:resource="http://www.w3.org/ns/dcat#Distribution"/>
        <rdfs:range rdf:resource="http://www.w3.org/2000/01/rdf-schema#Resource"/>
        <rdfs:comment xml:lang="fr">Ceci est un lien direct à un fichier téléchargeable en un format donnée. Exple fichier CSV ou RDF. Le format est décrit par les propriétés de distribution dcterms:format et/ou dcat:mediaType.</rdfs:comment>
        <rdfs:comment xml:lang="es">La URL de un archivo descargable en el formato dato. Por ejemplo, archivo CSV o archivo RDF. El formato se describe con las propiedades de la distribución dcterms:format y/o dcat:mediaType.</rdfs:comment>
        <rdfs:comment xml:lang="it">Questo è un link diretto al file scaricabile in un dato formato. E.g. un file CSV o un file RDF. Il formato è descritto dal dcterms:format e/o dal dcat:mediaType della distribuzione.</rdfs:comment>
        <rdfs:comment xml:lang="en">The URL of the downloadable file in a given format. E.g. CSV file or RDF file. The format is indicated by the distribution&apos;s dcterms:format and/or dcat:mediaType.</rdfs:comment>
        <rdfs:comment xml:lang="cs">URL souboru ke stažení v daném formátu, například CSV nebo RDF soubor. Formát je popsán vlastností distribuce dcterms:format a/nebo dcat:mediaType.</rdfs:comment>
        <rdfs:comment xml:lang="da">URL til fil der kan downloades i et bestemt format. Fx en CSV-fil eller en RDF-fil. Formatet for distributionen angives ved hjælp af egenskaberne dcterms:format og/eller dcat:mediaType.</rdfs:comment>
        <rdfs:comment xml:lang="ja">dcat:downloadURLはdcat:accessURLの特定の形式です。しかし、DCATプロファイルが非ダウンロード・ロケーションに対してのみaccessURLを用いる場合には、より強い分離を課すことを望む可能性があるため、この含意を強化しないように、DCATは、dcat:downloadURLをdcat:accessURLのサブプロパティーであると定義しません。</rdfs:comment>
        <rdfs:comment xml:lang="el">Είναι ένας σύνδεσμος άμεσης μεταφόρτωσης ενός αρχείου σε μια δεδομένη μορφή. Π.χ. ένα αρχείο CSV ή RDF. Η μορφη αρχείου περιγράφεται από τις ιδιότητες dcterms:format ή/και dcat:mediaType της διανομής.</rdfs:comment>
        <rdfs:comment xml:lang="ar">رابط مباشر لملف يمكن تحميله. نوع الملف يتم توصيفه باستخدام الخاصية dcterms:format dcat:mediaType </rdfs:comment>
        <rdfs:isDefinedBy rdf:resource="http://www.w3.org/TR/vocab-dcat/"/>
        <rdfs:label xml:lang="es">URL de descarga</rdfs:label>
        <rdfs:label xml:lang="fr">URL de téléchargement</rdfs:label>
        <rdfs:label xml:lang="it">URL di scarico</rdfs:label>
        <rdfs:label xml:lang="cs">URL souboru ke stažení</rdfs:label>
        <rdfs:label xml:lang="el">URL μεταφόρτωσης</rdfs:label>
        <rdfs:label xml:lang="en">download URL</rdfs:label>
        <rdfs:label xml:lang="da">downloadURL</rdfs:label>
        <rdfs:label xml:lang="ar">رابط تحميل</rdfs:label>
        <rdfs:label xml:lang="ja">ダウンロードURL</rdfs:label>
        <skos:definition xml:lang="fr">Ceci est un lien direct à un fichier téléchargeable en un format donnée. Exple fichier CSV ou RDF. Le format est décrit par les propriétés de distribution dcterms:format et/ou dcat:mediaType.</skos:definition>
        <skos:definition xml:lang="es">La URL de un archivo descargable en el formato dato. Por ejemplo, archivo CSV o archivo RDF. El formato se describe con las propiedades de la distribución dcterms:format y/o dcat:mediaType.</skos:definition>
        <skos:definition xml:lang="it">Questo è un link diretto al file scaricabile in un dato formato. E.g. un file CSV o un file RDF. Il formato è descritto dal dcterms:format e/o dal dcat:mediaType della distribuzione.</skos:definition>
        <skos:definition xml:lang="en">The URL of the downloadable file in a given format. E.g. CSV file or RDF file. The format is indicated by the distribution&apos;s dcterms:format and/or dcat:mediaType.</skos:definition>
        <skos:definition xml:lang="cs">URL souboru ke stažení v daném formátu, například CSV nebo RDF soubor. Formát je popsán vlastností distribuce dcterms:format a/nebo dcat:mediaType.</skos:definition>
        <skos:definition xml:lang="da">URL til fil der kan downloades i et bestemt format. Fx en CSV-fil eller en RDF-fil. Formatet for distributionen angives ved hjælp af egenskaberne dcterms:format og/eller dcat:mediaType.</skos:definition>
        <skos:definition xml:lang="ja">dcat:downloadURLはdcat:accessURLの特定の形式です。しかし、DCATプロファイルが非ダウンロード・ロケーションに対してのみaccessURLを用いる場合には、より強い分離を課すことを望む可能性があるため、この含意を強化しないように、DCATは、dcat:downloadURLをdcat:accessURLのサブプロパティーであると定義しません。</skos:definition>
        <skos:definition xml:lang="el">Είναι ένας σύνδεσμος άμεσης μεταφόρτωσης ενός αρχείου σε μια δεδομένη μορφή. Π.χ. ένα αρχείο CSV ή RDF. Η μορφη αρχείου περιγράφεται από τις ιδιότητες dcterms:format ή/και dcat:mediaType της διανομής.</skos:definition>
        <skos:definition xml:lang="ar">رابط مباشر لملف يمكن تحميله. نوع الملف يتم توصيفه باستخدام الخاصية dcterms:format dcat:mediaType </skos:definition>
        <skos:editorialNote xml:lang="en">Status: English  Definition text modified by DCAT revision team, Italian, Spanish and Czech translation updated, other translations pending.</skos:editorialNote>
        <skos:editorialNote xml:lang="en">rdfs:label, rdfs:comment and/or skos:scopeNote have been modified. Non-english versions must be updated.</skos:editorialNote>
        <skos:scopeNote xml:lang="es">El valor es una URL.</skos:scopeNote>
        <skos:scopeNote xml:lang="fr">La valeur est une URL.</skos:scopeNote>
        <skos:scopeNote xml:lang="cs">dcat:downloadURL BY MĚLA být použita pro adresu, ze které je distribuce přímo přístupná, typicky skrze požadavek HTTP Get.</skos:scopeNote>
        <skos:scopeNote xml:lang="da">dcat:downloadURL BØR anvendes til angivelse af den adresse hvor distributionen er tilgængelig direkte, typisk gennem et HTTP Get request.</skos:scopeNote>
        <skos:scopeNote xml:lang="it">dcat:downloadURL DOVREBBE essere utilizzato per l&apos;indirizzo a cui questa distribuzione è disponibile direttamente, in genere attraverso una richiesta Get HTTP.</skos:scopeNote>
        <skos:scopeNote xml:lang="en">dcat:downloadURL SHOULD be used for the address at which this distribution is available directly, typically through a HTTP Get request.</skos:scopeNote>
        <skos:scopeNote xml:lang="el">Η τιμή είναι ένα URL.</skos:scopeNote>
    </owl:ObjectProperty>
    


    <!-- http://www.w3.org/ns/dcat#endpointDescription -->


    <owl:ObjectProperty rdf:about="http://www.w3.org/ns/dcat#endpointDescription">
        <rdfs:domain rdf:resource="http://www.w3.org/ns/dcat#DataService"/>
        <rdfs:comment xml:lang="en">A description of the service end-point, including its operations, parameters etc.</rdfs:comment>
        <rdfs:comment xml:lang="da">En beskrivelse af det pågældende tjenesteendpoint, inklusiv dets operationer, parametre etc.</rdfs:comment>
        <rdfs:comment xml:lang="cs">Popis přístupového bodu služby včetně operací, parametrů apod.</rdfs:comment>
        <rdfs:comment xml:lang="es">Una descripción del end-point del servicio, incluyendo sus operaciones, parámetros, etc.</rdfs:comment>
        <rdfs:comment xml:lang="it">Una descrizione dell&apos;endpoint del servizio, incluse le sue operazioni, parametri, ecc.</rdfs:comment>
        <rdfs:isDefinedBy rdf:resource="https://www.w3.org/TR/vocab-dcat-2/"/>
        <rdfs:label xml:lang="es">descripción del end-point del servicio</rdfs:label>
        <rdfs:label xml:lang="en">description of service end-point</rdfs:label>
        <rdfs:label xml:lang="it">descrizione dell&apos;endpoint del servizio</rdfs:label>
        <rdfs:label xml:lang="da">endpointbeskrivelse</rdfs:label>
        <rdfs:label xml:lang="cs">popis přístupového bodu služby</rdfs:label>
        <skos:changeNote xml:lang="en">New property in DCAT 2.</skos:changeNote>
        <skos:changeNote xml:lang="cs">Nová vlastnost přidaná ve verzi DCAT 2.</skos:changeNote>
        <skos:changeNote xml:lang="en">Nueva propiedad agregada en DCAT 2.</skos:changeNote>
        <skos:changeNote xml:lang="it">Nuova proprietà in DCAT 2.</skos:changeNote>
        <skos:changeNote xml:lang="da">Ny egenskab i DCAT 2.</skos:changeNote>
        <skos:definition xml:lang="en">A description of the service end-point, including its operations, parameters etc.</skos:definition>
        <skos:definition xml:lang="da">En beskrivelse af det pågældende tjenesteendpoint, inklusiv dets operationer, parametre etc.</skos:definition>
        <skos:definition xml:lang="cs">Popis přístupového bodu služby včetně operací, parametrů apod.</skos:definition>
        <skos:definition xml:lang="es">Una descripción del end-point del servicio, incluyendo sus operaciones, parámetros, etc..</skos:definition>
        <skos:definition xml:lang="it">Una descrizione dell&apos;endpoint del servizio, incluse le sue operazioni, parametri, ecc.</skos:definition>
        <skos:scopeNote xml:lang="en">An endpoint description may be expressed in a machine-readable form, such as an OpenAPI (Swagger) description, an OGC GetCapabilities response, a SPARQL Service Description, an OpenSearch or WSDL document, a Hydra API description, else in text or some other informal mode if a formal representation is not possible.</skos:scopeNote>
        <skos:scopeNote xml:lang="da">En beskrivelse af et endpoint kan udtrykkes i et maskinlæsbart format, såsom OpenAPI (Swagger)-beskrivelser, et OGC GetCapabilities svar, en SPARQL tjenestebeskrivelse, en OpenSearch- eller et WSDL-dokument, en Hydra-API-beskrivelse, eller i tekstformat eller i et andet uformelt format, hvis en formel repræsentation ikke er mulig.</skos:scopeNote>
        <skos:scopeNote xml:lang="da">Endpointbeskrivelsen giver specifikke oplysninger om den konkrete endpointinstans, mens dcterms:conformsTo anvendes til at indikere den overordnede standard eller specifikation som endpointet er i overensstemmelse med.</skos:scopeNote>
        <skos:scopeNote xml:lang="es">La descripción del endpoint brinda detalles específicos de la instancia del endpoint, mientras que dcterms:conformsTo se usa para indicar el estándar general o especificación que implementa el endpoint.</skos:scopeNote>
        <skos:scopeNote xml:lang="it">La descrizione dell&apos;endpoint fornisce dettagli specifici dell&apos;istanza dell&apos;endpoint reale, mentre dcterms:conformsTo viene utilizzato per indicare lo standard o le specifiche implementate dall&apos;endpoint.</skos:scopeNote>
        <skos:scopeNote xml:lang="cs">Popis přístupového bodu dává specifické detaily jeho konkrétní instance, zatímco dcterms:conformsTo indikuje obecný standard či specifikaci kterou přístupový bod implementuje.</skos:scopeNote>
        <skos:scopeNote xml:lang="cs">Popis přístupového bodu může být vyjádřen ve strojově čitelné formě, například jako popis OpenAPI (Swagger), odpověď služby OGC getCapabilities, pomocí slovníku SPARQL Service Description, jako OpenSearch či WSDL document, jako popis API dle slovníku Hydra, a nebo textově nebo jiným neformálním způsobem, pokud není možno použít formální reprezentaci.</skos:scopeNote>
        <skos:scopeNote xml:lang="en">The endpoint description gives specific details of the actual endpoint instance, while dcterms:conformsTo is used to indicate the general standard or specification that the endpoint implements.</skos:scopeNote>
        <skos:scopeNote xml:lang="es">Una descripción del endpoint del servicio puede expresarse en un formato que la máquina puede interpretar, tal como una descripción basada en OpenAPI (Swagger), una respuesta OGC GetCapabilities, una descripción de un servicio SPARQL, un documento OpenSearch o WSDL, una descripción con la Hydra API, o en texto u otro modo informal si la representación formal no es posible.</skos:scopeNote>
        <skos:scopeNote xml:lang="it">Una descrizione dell&apos;endpoint può essere espressa in un formato leggibile dalla macchina, come una descrizione OpenAPI (Swagger), una risposta GetCapabilities OGC, una descrizione del servizio SPARQL, un documento OpenSearch o WSDL, una descrizione API Hydra, o con del testo o qualche altra modalità informale se una rappresentazione formale non è possibile.</skos:scopeNote>
    </owl:ObjectProperty>
    


    <!-- http://www.w3.org/ns/dcat#endpointURL -->


    <owl:ObjectProperty rdf:about="http://www.w3.org/ns/dcat#endpointURL">
        <rdfs:domain rdf:resource="http://www.w3.org/ns/dcat#DataService"/>
        <rdfs:range rdf:resource="http://www.w3.org/2000/01/rdf-schema#Resource"/>
        <rdfs:comment xml:lang="cs">Kořenové umístění nebo hlavní přístupový bod služby (IRI přístupné přes Web).</rdfs:comment>
        <rdfs:comment xml:lang="it">La locazione principale o l&apos;endpoint primario del servizio (un IRI risolvibile via web).</rdfs:comment>
        <rdfs:comment xml:lang="es">La posición raíz o end-point principal del servicio (una IRI web).</rdfs:comment>
        <rdfs:comment xml:lang="da">Rodplaceringen eller det primære endpoint for en tjeneste (en web-resolverbar IRI).</rdfs:comment>
        <rdfs:comment xml:lang="en">The root location or primary endpoint of the service (a web-resolvable IRI).</rdfs:comment>
        <rdfs:isDefinedBy rdf:resource="https://www.w3.org/TR/vocab-dcat-2/"/>
        <rdfs:label xml:lang="es">end-point del servicio</rdfs:label>
        <rdfs:label xml:lang="it">end-point del servizio</rdfs:label>
        <rdfs:label xml:lang="cs">přístupový bod služby</rdfs:label>
        <rdfs:label xml:lang="en">service end-point</rdfs:label>
        <rdfs:label xml:lang="da">tjenesteendpoint</rdfs:label>
        <skos:changeNote xml:lang="en">New property in DCAT 2.</skos:changeNote>
        <skos:changeNote xml:lang="cs">Nová vlastnost přidaná ve verzi DCAT 2.</skos:changeNote>
        <skos:changeNote xml:lang="es">Nueva propiedad agregada en DCAT 2.</skos:changeNote>
        <skos:changeNote xml:lang="it">Nuova proprietà in DCAT 2.</skos:changeNote>
        <skos:definition xml:lang="cs">Kořenové umístění nebo hlavní přístupový bod služby (IRI přístupné přes Web).</skos:definition>
        <skos:definition xml:lang="it">La locazione principale o l&apos;endpoint primario del servizio (un IRI risolvibile via web).</skos:definition>
        <skos:definition xml:lang="es">La posición raíz o end-point principal del servicio (una IRI web).</skos:definition>
        <skos:definition xml:lang="da">Rodplaceringen eller det primære endpoint for en tjeneste (en web-resolverbar IRI).</skos:definition>
        <skos:definition xml:lang="en">The root location or primary endpoint of the service (a web-resolvable IRI).</skos:definition>
    </owl:ObjectProperty>
    


    <!-- http://www.w3.org/ns/dcat#first -->


    <owl:ObjectProperty rdf:about="http://www.w3.org/ns/dcat#first">
        <rdfs:subPropertyOf rdf:resource="http://www.w3.org/1999/xhtml/vocab#first"/>
        <rdfs:comment xml:lang="es">El primer recurso en una colección ordenada o serie de recursos, al que el recurso pertenece.</rdfs:comment>
        <rdfs:comment xml:lang="it">La prima risorsa in una collezione ordinata o in una serie di risorse, di cui la risorsa fa parte.</rdfs:comment>
        <rdfs:comment xml:lang="en">The first resource in an ordered collection or series of resources, to which the current resource belongs.</rdfs:comment>
        <rdfs:isDefinedBy rdf:resource="https://www.w3.org/TR/vocab-dcat-3/"/>
        <rdfs:label xml:lang="en">first</rdfs:label>
        <rdfs:label xml:lang="es">primero</rdfs:label>
        <rdfs:label xml:lang="it">primo</rdfs:label>
        <skos:changeNote xml:lang="en">New property added in DCAT 3.</skos:changeNote>
        <skos:changeNote xml:lang="cs">Nová vlastnost přidaná ve verzi DCAT 3.</skos:changeNote>
        <skos:changeNote xml:lang="es">Nueva propiedad agregada in DCAT 3.</skos:changeNote>
        <skos:changeNote xml:lang="it">Nuova proprietà aggiunta in DCAT 3.</skos:changeNote>
        <skos:changeNote xml:lang="da">Ny egenskab tilføjet i DCAT 3.</skos:changeNote>
        <skos:definition xml:lang="es">El primer recurso en una colección ordenada o serie de recursos, al que el recurso pertenece.</skos:definition>
        <skos:definition xml:lang="it">La prima risorsa in una collezione ordinata o in una serie di risorse, di cui la risorsa fa parte.</skos:definition>
        <skos:definition xml:lang="en">The first resource in an ordered collection or series of resources, to which the current resource belongs.</skos:definition>
        <skos:scopeNote xml:lang="es">En DCAT esta propiedad se usa para recursos que pertenecen a una dcat:DatasetSeries.</skos:scopeNote>
        <skos:scopeNote xml:lang="it">In DCAT questa proprietà è usata per risorse che fanno parte di una dcat:DatasetSeries.</skos:scopeNote>
        <skos:scopeNote xml:lang="en">In DCAT this property is used for resources belonging to a dcat:DatasetSeries.</skos:scopeNote>
    </owl:ObjectProperty>
    


    <!-- http://www.w3.org/ns/dcat#hadRole -->


    <owl:ObjectProperty rdf:about="http://www.w3.org/ns/dcat#hadRole">
        <rdfs:domain>
            <owl:Class>
                <owl:unionOf rdf:parseType="Collection">
                    <rdf:Description rdf:about="http://www.w3.org/ns/dcat#Relationship"/>
                    <rdf:Description rdf:about="http://www.w3.org/ns/prov#Attribution"/>
                </owl:unionOf>
            </owl:Class>
        </rdfs:domain>
        <rdfs:range rdf:resource="http://www.w3.org/ns/dcat#Role"/>
        <rdfs:comment xml:lang="da">Den funktion en entitet eller aktør har i forhold til en anden ressource.</rdfs:comment>
        <rdfs:comment xml:lang="cs">Funkce entity či agenta ve vztahu k jiné entitě či zdroji.</rdfs:comment>
        <rdfs:comment xml:lang="es">La función de una entidad o agente con respecto a otra entidad o recurso.</rdfs:comment>
        <rdfs:comment xml:lang="it">La funzione di un&apos;entità o un agente rispetto ad un&apos;altra entità o risorsa.</rdfs:comment>
        <rdfs:comment xml:lang="en">The function of an entity or agent with respect to another entity or resource.</rdfs:comment>
        <rdfs:isDefinedBy rdf:resource="https://www.w3.org/TR/vocab-dcat-2/"/>
        <rdfs:label xml:lang="it">haRuolo</rdfs:label>
        <rdfs:label xml:lang="en">hadRole</rdfs:label>
        <rdfs:label xml:lang="da">havde rolle</rdfs:label>
        <rdfs:label xml:lang="cs">sehraná role</rdfs:label>
        <rdfs:label xml:lang="it">tiene rol</rdfs:label>
        <skos:changeNote xml:lang="en">New property added in DCAT 2.</skos:changeNote>
        <skos:changeNote xml:lang="cs">Nová vlastnost přidaná ve verzi DCAT 2.</skos:changeNote>
        <skos:changeNote xml:lang="es">Nueva propiedad agregada en DCAT 2.</skos:changeNote>
        <skos:changeNote xml:lang="it">Nuova proprietà aggiunta in DCAT 2.</skos:changeNote>
        <skos:definition xml:lang="da">Den funktion en entitet eller aktør har i forhold til en anden ressource.</skos:definition>
        <skos:definition xml:lang="cs">Funkce entity či agenta ve vztahu k jiné entitě či zdroji.</skos:definition>
        <skos:definition xml:lang="es">La función de una entidad o agente con respecto a otra entidad o recurso.</skos:definition>
        <skos:definition xml:lang="it">La funzione di un&apos;entità o un agente rispetto ad un&apos;altra entità o risorsa.</skos:definition>
        <skos:definition xml:lang="en">The function of an entity or agent with respect to another entity or resource.</skos:definition>
        <skos:editorialNote xml:lang="es">Agregada en DCAT para complementar prov:hadRole (cuyo uso está limitado a roles en el contexto de una actividad, con dominio prov:Association.</skos:editorialNote>
        <skos:editorialNote xml:lang="it">Introdotta in DCAT per completare prov:hadRole (il cui uso è limitato ai ruoli nel contesto di un&apos;attività, con il dominio di prov:Association.</skos:editorialNote>
        <skos:editorialNote xml:lang="en">Introduced into DCAT to complement prov:hadRole (whose use is limited to roles in the context of an activity, with the domain of prov:Association.</skos:editorialNote>
        <skos:editorialNote xml:lang="da">Introduceret i DCAT for at supplere prov:hadRole (hvis anvendelse er begrænset til roller i forbindelse med en aktivitet med domænet prov:Association).</skos:editorialNote>
        <skos:editorialNote xml:lang="cs">Přidáno do DCAT pro doplnění vlastnosti prov:hadRole (jejíž užití je omezeno na role v kontextu aktivity, s definičním oborem prov:Association).</skos:editorialNote>
        <skos:scopeNote xml:lang="da">Kan vendes ved kvalificerede krediteringer til at angive en aktørs rolle i forhold en entitet. Det anbefales at værdierne styres som et kontrolleret udfaldsrum med aktørroller, såsom http://registry.it.csiro.au/def/isotc211/CI_RoleCode.</skos:scopeNote>
        <skos:scopeNote xml:lang="en">May be used in a qualified-attribution to specify the role of an Agent with respect to an Entity. It is recommended that the value be taken from a controlled vocabulary of agent roles, such as http://registry.it.csiro.au/def/isotc211/CI_RoleCode.</skos:scopeNote>
        <skos:scopeNote xml:lang="en">May be used in a qualified-relation to specify the role of an Entity with respect to another Entity.  It is recommended that the value be taken from a controlled vocabulary of entity roles such as: ISO 19115 DS_AssociationTypeCode http://registry.it.csiro.au/def/isotc211/DS_AssociationTypeCode; IANA Registry of Link Relations https://www.iana.org/assignments/link-relation; DataCite metadata schema; MARC relators https://id.loc.gov/vocabulary/relators.</skos:scopeNote>
        <skos:scopeNote xml:lang="cs">Může být použito v kvalifikovaném přiřazení pro specifikaci role Agenta ve vztahu k Entitě. Je doporučeno hodnotu vybrat z řízeného slovníku rolí agentů, jako například http://registry.it.csiro.au/def/isotc211/CI_RoleCode.</skos:scopeNote>
        <skos:scopeNote xml:lang="cs">Může být použito v kvalifikovaném vztahu pro specifikaci role Entity ve vztahu k jiné Entitě. Je doporučeno použít hodnotu z řízeného slovníku rolí entit, jako například ISO 19115 DS_AssociationTypeCode http://registry.it.csiro.au/def/isotc211/DS_AssociationTypeCode, IANA Registry of Link Relations https://www.iana.org/assignments/link-relation, DataCite metadata schema, MARC relators https://id.loc.gov/vocabulary/relators.</skos:scopeNote>
        <skos:scopeNote xml:lang="es">Puede usarse en una atribución cualificada para especificar el rol de un Agente con respecto a una Entidad. Se recomienda que el valor sea de un vocabulario controlado de roles de agentes, como por ejemplo http://registry.it.csiro.au/def/isotc211/CI_RoleCode.</skos:scopeNote>
        <skos:scopeNote xml:lang="es">Puede usarse en una atribución cualificada para especificar el rol de una Entidad con respecto a otra Entidad. Se recomienda que su valor se tome de un vocabulario controlado de roles de entidades como por ejemplo: ISO 19115 DS_AssociationTypeCode http://registry.it.csiro.au/def/isotc211/DS_AssociationTypeCode; IANA Registry of Link Relations https://www.iana.org/assignments/link-relation; esquema de metadatos de DataCite; MARC relators https://id.loc.gov/vocabulary/relators.</skos:scopeNote>
        <skos:scopeNote xml:lang="it">Può essere utilizzata in una relazione qualificata per specificare il ruolo di un&apos;entità rispetto a un&apos;altra entità. Si raccomanda che il valore sia preso da un vocabolario controllato di ruoli di entità come ISO 19115 DS_AssociationTypeCode http://registry.it.csiro.au/def/isotc211/DS_AssociationTypeCode, IANA Registry of Link Relations https://www.iana.org/assignments/link-relation, DataCite metadata schema, o MARC relators https://id.loc.gov/vocabulary/relators.</skos:scopeNote>
        <skos:scopeNote xml:lang="it">Può essere utilizzato in un&apos;attribuzione qualificata per specificare il ruolo di un agente rispetto a un&apos;entità. Si raccomanda che il valore sia preso da un vocabolario controllato di ruoli di agente, come ad esempio http://registry.it.csiro.au/def/isotc211/CI_RoleCode.</skos:scopeNote>
    </owl:ObjectProperty>
    


    <!-- http://www.w3.org/ns/dcat#hasCurrentVersion -->


    <owl:ObjectProperty rdf:about="http://www.w3.org/ns/dcat#hasCurrentVersion"/>
    


    <!-- http://www.w3.org/ns/dcat#hasVersion -->


    <owl:ObjectProperty rdf:about="http://www.w3.org/ns/dcat#hasVersion">
        <rdfs:subPropertyOf rdf:resource="http://purl.org/dc/terms/hasVersion"/>
        <rdfs:subPropertyOf rdf:resource="http://www.w3.org/ns/prov#generalizationOf"/>
        <rdfs:comment xml:lang="es">Este recurso tiene una versión específica.</rdfs:comment>
        <rdfs:comment xml:lang="it">Per questa risorsa esiste una risorsa più specifica e versionata.</rdfs:comment>
        <rdfs:comment xml:lang="en">This resource has a more specific, versioned resource [PAV].</rdfs:comment>
        <rdfs:isDefinedBy rdf:resource="https://www.w3.org/TR/vocab-dcat-3/"/>
        <rdfs:label xml:lang="it">ha versione</rdfs:label>
        <rdfs:label xml:lang="en">has version</rdfs:label>
        <rdfs:label xml:lang="es">tiene versión</rdfs:label>
        <skos:changeNote xml:lang="en">New property added in DCAT 3.</skos:changeNote>
        <skos:changeNote xml:lang="cs">Nová vlastnost přidaná ve verzi DCAT 3.</skos:changeNote>
        <skos:changeNote xml:lang="es">Nueva propiedad agregada in DCAT 3.</skos:changeNote>
        <skos:changeNote xml:lang="it">Nuova proprietà aggiunta in DCAT 3.</skos:changeNote>
        <skos:changeNote xml:lang="da">Ny egenskab tilføjet i DCAT 3.</skos:changeNote>
        <skos:definition xml:lang="es">Este recurso tiene una versión específica.</skos:definition>
        <skos:definition xml:lang="it">Per questa risorsa esiste una risorsa più specifica e versionata.</skos:definition>
        <skos:definition xml:lang="en">This resource has a more specific, versioned resource [PAV].</skos:definition>
        <skos:scopeNote xml:lang="es">Esta propiedad se utiliza para relacionar un recurso abstracto o no versionado de un recurso con varias versiones del recuros; por ejemplo, versiones intastáneas.</skos:scopeNote>
        <skos:scopeNote xml:lang="es">La noción de versión que se usa en esta propiedad está limitada a las versiones que resultan de revisiones de un recurso como parte de su ciclo de vida. Por lo tanto, su semántica es más específica que su super-propiedad dcterns:hasVersion, la cuál hace uso de la noción más amplia de versión, incluyendo ediciones y adaptaciones.</skos:scopeNote>
        <skos:scopeNote xml:lang="it">La nozione di versione usata da questa proprietà è limitata a versioni risultanti da revisioni a cui una risorsa è soggetta nel suo ciclo di vita. Quindi la sua semantica è più specifica di quella della sua super-proprietà dcterms:hasVersion, che utilizza una nozione di versione più ampia, e include, ad es., edizioni e adattamenti.</skos:scopeNote>
        <skos:scopeNote xml:lang="it">Questa proprietà è usata per correlare una risorsa non versionata o astratta a differenti risorse versionate, ad es., i relativi snapshot.</skos:scopeNote>
        <skos:scopeNote xml:lang="en">The notion of version used by this property is limited to versions resulting from revisions occurring to a resource as part of its life-cycle. Therefore, its semantics is more specific than its super-property dcterms:hasVersion, which makes use of a broader notion of version, including editions and adaptations.</skos:scopeNote>
        <skos:scopeNote xml:lang="en">This property is intended for relating a non-versioned or abstract resource to several versioned resources, e.g., snapshots [PAV].</skos:scopeNote>
    </owl:ObjectProperty>
    


    <!-- http://www.w3.org/ns/dcat#inCatalog -->


    <rdf:Description rdf:about="http://www.w3.org/ns/dcat#inCatalog">
        <owl:inverseOf rdf:resource="http://www.w3.org/ns/dcat#resource"/>
        <rdfs:isDefinedBy rdf:resource="https://www.w3.org/TR/vocab-dcat-3/"/>
        <skos:changeNote xml:lang="en">New property added in DCAT 3.</skos:changeNote>
        <skos:changeNote xml:lang="cs">Nová vlastnost přidaná ve verzi DCAT 3.</skos:changeNote>
        <skos:changeNote xml:lang="es">Nueva propiedad agregada en DCAT 3.</skos:changeNote>
        <skos:changeNote xml:lang="it">Nuova proprietà aggiunta in DCAT 3.</skos:changeNote>
        <skos:scopeNote xml:lang="es">Esta propiedad inversa PUEDE usarse sólo en combinación con su inversa, y NO PUEDE utilizarse en su reemplazo.</skos:scopeNote>
        <skos:scopeNote xml:lang="it">Questa proprietà PUÒ essere usata solo insieme alla sua inversa, e NON DEVE essere usata per sostituirla.</skos:scopeNote>
        <skos:scopeNote xml:lang="en">This property MAY be used only in addition to its inverse, and it MUST NOT be used to replace it.</skos:scopeNote>
    </rdf:Description>
    


    <!-- http://www.w3.org/ns/dcat#inSeries -->


    <owl:ObjectProperty rdf:about="http://www.w3.org/ns/dcat#inSeries">
        <rdfs:subPropertyOf rdf:resource="http://purl.org/dc/terms/isPartOf"/>
        <rdfs:comment xml:lang="en">A dataset series of which the dataset is part.</rdfs:comment>
        <rdfs:comment xml:lang="es">Una serie de conjuntos de datos del cuál un conjunto de datos es parte.</rdfs:comment>
        <rdfs:comment xml:lang="it">Una serie di dataset di cui questo dataset fa parte.</rdfs:comment>
        <rdfs:isDefinedBy rdf:resource="https://www.w3.org/TR/vocab-dcat-3/"/>
        <rdfs:label xml:lang="es">en serie</rdfs:label>
        <rdfs:label xml:lang="it">in serie</rdfs:label>
        <rdfs:label xml:lang="en">in series</rdfs:label>
        <skos:changeNote xml:lang="en">New property added in DCAT 3.</skos:changeNote>
        <skos:changeNote xml:lang="cs">Nová vlastnost přidaná ve verzi DCAT 3.</skos:changeNote>
        <skos:changeNote xml:lang="es">Nueva propiedad agregada in DCAT 3.</skos:changeNote>
        <skos:changeNote xml:lang="it">Nuova proprietà aggiunta in DCAT 3.</skos:changeNote>
        <skos:changeNote xml:lang="da">Ny egenskab tilføjet i DCAT 3.</skos:changeNote>
        <skos:definition xml:lang="en">A dataset series of which the dataset is part.</skos:definition>
        <skos:definition xml:lang="es">Una serie de conjuntos de datos del cuál un conjunto de datos es parte.</skos:definition>
        <skos:definition xml:lang="it">Una serie di dataset di cui questo dataset fa parte.</skos:definition>
    </owl:ObjectProperty>
    


    <!-- http://www.w3.org/ns/dcat#isDistributionOf -->


    <rdf:Description rdf:about="http://www.w3.org/ns/dcat#isDistributionOf">
        <owl:inverseOf rdf:resource="http://www.w3.org/ns/dcat#distribution"/>
        <rdfs:isDefinedBy rdf:resource="https://www.w3.org/TR/vocab-dcat-3/"/>
        <skos:changeNote xml:lang="en">New property added in DCAT 3.</skos:changeNote>
        <skos:changeNote xml:lang="cs">Nová vlastnost přidaná ve verzi DCAT 3.</skos:changeNote>
        <skos:changeNote xml:lang="es">Nueva propiedad agregada en DCAT 3.</skos:changeNote>
        <skos:changeNote xml:lang="it">Nuova proprietà aggiunta in DCAT 3.</skos:changeNote>
        <skos:scopeNote xml:lang="es">Esta propiedad inversa PUEDE usarse sólo en combinación con su inversa, y NO PUEDE utilizarse en su reemplazo.</skos:scopeNote>
        <skos:scopeNote xml:lang="it">Questa proprietà PUÒ essere usata solo insieme alla sua inversa, e NON DEVE essere usata per sostituirla.</skos:scopeNote>
        <skos:scopeNote xml:lang="en">This property MAY be used only in addition to its inverse, and it MUST NOT be used to replace it.</skos:scopeNote>
    </rdf:Description>
    


    <!-- http://www.w3.org/ns/dcat#isVersionOf -->


    <rdf:Description rdf:about="http://www.w3.org/ns/dcat#isVersionOf">
        <owl:inverseOf rdf:resource="http://www.w3.org/ns/dcat#hasVersion"/>
        <rdfs:isDefinedBy rdf:resource="https://www.w3.org/TR/vocab-dcat-3/"/>
        <skos:changeNote xml:lang="en">New property added in DCAT 3.</skos:changeNote>
        <skos:changeNote xml:lang="cs">Nová vlastnost přidaná ve verzi DCAT 3.</skos:changeNote>
        <skos:changeNote xml:lang="es">Nueva propiedad agregada en DCAT 3.</skos:changeNote>
        <skos:changeNote xml:lang="it">Nuova proprietà aggiunta in DCAT 3.</skos:changeNote>
        <skos:scopeNote xml:lang="es">Esta propiedad inversa PUEDE usarse sólo en combinación con su inversa, y NO PUEDE utilizarse en su reemplazo.</skos:scopeNote>
        <skos:scopeNote xml:lang="it">Questa proprietà PUÒ essere usata solo insieme alla sua inversa, e NON DEVE essere usata per sostituirla.</skos:scopeNote>
        <skos:scopeNote xml:lang="en">This property MAY be used only in addition to its inverse, and it MUST NOT be used to replace it.</skos:scopeNote>
    </rdf:Description>
    


    <!-- http://www.w3.org/ns/dcat#landingPage -->


    <owl:ObjectProperty rdf:about="http://www.w3.org/ns/dcat#landingPage">
        <rdfs:subPropertyOf rdf:resource="http://xmlns.com/foaf/0.1/page"/>
        <rdfs:range rdf:resource="http://xmlns.com/foaf/0.1/Document"/>
        <rdfs:comment xml:lang="en">A Web page that can be navigated to in a Web browser to gain access to the catalog, a dataset, its distributions and/or additional information.</rdfs:comment>
        <rdfs:comment xml:lang="da">En webside som der kan navigeres til i en webbrowser for at få adgang til kataloget, et datasæt, dets distributioner og/eller yderligere information.</rdfs:comment>
        <rdfs:comment xml:lang="it">Una pagina web che può essere navigata per ottenere l&apos;accesso al catalogo, ad un dataset, alle distribuzioni del dataset e/o ad informazioni addizionali.</rdfs:comment>
        <rdfs:comment xml:lang="es">Una página web que puede ser visitada en un explorador Web para tener acceso el catálogo, un conjunto de datos, sus distribuciones y/o información adicional.</rdfs:comment>
        <rdfs:comment xml:lang="fr">Une page Web accessible par un navigateur Web donnant accès au catalogue, un jeu de données, ses distributions et/ou des informations additionnelles.</rdfs:comment>
        <rdfs:comment xml:lang="cs">Webová stránka, na kterou lze pro získání přístupu ke katalogu, datové sadě, jejím distribucím a/nebo dalším informacím přistoupit webovým prohlížečem.</rdfs:comment>
        <rdfs:comment xml:lang="el">Μία ιστοσελίδα πλοηγίσιμη μέσω ενός φυλλομετρητή (Web browser) που δίνει πρόσβαση στο σύνολο δεδομένων, τις διανομές αυτού ή/και επιπρόσθετες πληροφορίες.</rdfs:comment>
        <rdfs:comment xml:lang="ar">صفحة وب يمكن من خلالها الوصول الى قائمة البيانات أو إلى معلومات إضافية متعلقة بها </rdfs:comment>
        <rdfs:comment xml:lang="ja">データセット、その配信および（または）追加情報にアクセスするためにウエブ・ブラウザでナビゲートできるウェブページ。</rdfs:comment>
        <rdfs:isDefinedBy rdf:resource="http://www.w3.org/TR/vocab-dcat/"/>
        <rdfs:label xml:lang="da">destinationsside</rdfs:label>
        <rdfs:label xml:lang="en">landing page</rdfs:label>
        <rdfs:label xml:lang="fr">page d&apos;atterrissage</rdfs:label>
        <rdfs:label xml:lang="it">pagina di destinazione</rdfs:label>
        <rdfs:label xml:lang="es">página de destino</rdfs:label>
        <rdfs:label xml:lang="cs">vstupní stránka</rdfs:label>
        <rdfs:label xml:lang="el">ιστοσελίδα αρχικής πρόσβασης</rdfs:label>
        <rdfs:label xml:lang="ar">صفحة وصول</rdfs:label>
        <rdfs:label xml:lang="ja">ランディング・ページ</rdfs:label>
        <skos:definition xml:lang="en">A Web page that can be navigated to in a Web browser to gain access to the catalog, a dataset, its distributions and/or additional information.</skos:definition>
        <skos:definition xml:lang="da">En webside som en webbrowser kan navigeres til for at få adgang til kataloget, et datasæt, dets distritbutioner og/eller yderligere information.</skos:definition>
        <skos:definition xml:lang="it">Una pagina web che può essere navigata per ottenere l&apos;accesso al catalogo, ad un dataset, alle distribuzioni del dataset e/o ad informazioni addizionali.</skos:definition>
        <skos:definition xml:lang="es">Una página web que puede ser visitada en un explorador Web para tener acceso el catálogo, un conjunto de datos, sus distribuciones y/o información adicional.</skos:definition>
        <skos:definition xml:lang="fr">Une page Web accessible par un navigateur Web donnant accès au catalogue, un jeu de données, ses distributions et/ou des informations additionnelles.</skos:definition>
        <skos:definition xml:lang="cs">Webová stránka, na kterou lze pro získání přístupu ke katalogu, datové sadě, jejím distribucím a/nebo dalším informacím přistoupit webovým prohlížečem.</skos:definition>
        <skos:definition xml:lang="el">Μία ιστοσελίδα πλοηγίσιμη μέσω ενός φυλλομετρητή (Web browser) που δίνει πρόσβαση στο σύνολο δεδομένων, τις διανομές αυτού ή/και επιπρόσθετες πληροφορίες.</skos:definition>
        <skos:definition xml:lang="ar">صفحة وب يمكن من خلالها الوصول الى قائمة البيانات أو إلى معلومات إضافية متعلقة بها </skos:definition>
        <skos:definition xml:lang="ja">データセット、その配信および（または）追加情報にアクセスするためにウエブ・ブラウザでナビゲートできるウェブページ。</skos:definition>
        <skos:scopeNote xml:lang="da">Hvis en eller flere distributioner kun er tilgængelige via en destinationsside (dvs. en URL til direkte download er ikke kendt), så bør destinationssidelinket gentages som adgangsadresse for en distribution.</skos:scopeNote>
        <skos:scopeNote xml:lang="en">If the distribution(s) are accessible only through a landing page (i.e. direct download URLs are not known), then the landing page link should be duplicated as accessURL on a distribution.</skos:scopeNote>
        <skos:scopeNote xml:lang="cs">Pokud je distribuce dostupná pouze přes vstupní stránku, t.j. přímý URL odkaz ke stažení není znám, URL přístupové stránky by mělo být duplikováno ve vlastnosti distribuce accessURL.</skos:scopeNote>
        <skos:scopeNote xml:lang="it">Se la distribuzione è accessibile solo attraverso una pagina di destinazione (cioè, un URL di download diretto non è noto), il link alla pagina di destinazione deve essere duplicato come accessURL sulla distribuzione.</skos:scopeNote>
        <skos:scopeNote xml:lang="es">Si la distribución es accesible solamente través de una página de aterrizaje (i.e., no se conoce una URL de descarga directa), entonces el enlance a la página de aterrizaje debe ser duplicado como accessURL sobre la distribución.</skos:scopeNote>
        <skos:scopeNote xml:lang="fr">Si la distribution est seulement accessible à travers une page d&apos;atterrissage (exple. pas de connaissance d&apos;URLS de téléchargement direct ), alors le lien de la page d&apos;atterrissage doit être dupliqué comme accessURL sur la distribution.</skos:scopeNote>
        <skos:scopeNote xml:lang="el">Αν η/οι διανομή/ές είναι προσβάσιμη/ες μόνο μέσω μίας ιστοσελίδας αρχικής πρόσβασης (δηλαδή αν δεν υπάρχουν γνωστές διευθύνσεις άμεσης μεταφόρτωσης), τότε ο σύνδεσμος της ιστοσελίδας αρχικής πρόσβασης πρέπει να αναπαραχθεί ως accessURL σε μία διανομή.</skos:scopeNote>
        <skos:scopeNote xml:lang="ja">ランディング・ページを通じてしか配信にアクセスできない場合（つまり、直接的なダウンロードURLが不明）には、配信におけるaccessURLとしてランディング・ページのリンクをコピーすべきです（SHOULD）。</skos:scopeNote>
    </owl:ObjectProperty>
    


    <!-- http://www.w3.org/ns/dcat#last -->


    <owl:ObjectProperty rdf:about="http://www.w3.org/ns/dcat#last"/>
    


    <!-- http://www.w3.org/ns/dcat#mediaType -->


    <owl:ObjectProperty rdf:about="http://www.w3.org/ns/dcat#mediaType">
        <rdfs:subPropertyOf rdf:resource="http://purl.org/dc/terms/format"/>
        <rdfs:domain rdf:resource="http://www.w3.org/ns/dcat#Distribution"/>
        <rdfs:range rdf:resource="http://purl.org/dc/terms/MediaType"/>
        <rdfs:comment xml:lang="fr">Cette propriété doit être utilisée quand c&apos;est définit le type de média de la distribution en IANA, sinon dcterms:format DOIT être utilisé avec différentes valeurs.</rdfs:comment>
        <rdfs:comment xml:lang="es">Esta propiedad debe ser usada cuando está definido el tipo de media de la distribución en IANA, de otra manera dcterms:format puede ser utilizado con diferentes valores</rdfs:comment>
        <rdfs:comment xml:lang="it">Il tipo di media della distribuzione come definito da IANA</rdfs:comment>
        <rdfs:comment xml:lang="da">Medietypen for distributionen som den er defineret af IANA.</rdfs:comment>
        <rdfs:comment xml:lang="en">The media type of the distribution as defined by IANA</rdfs:comment>
        <rdfs:comment xml:lang="cs">Typ média distribuce definovaný v IANA.</rdfs:comment>
        <rdfs:comment xml:lang="el">Η ιδιότητα αυτή ΘΑ ΠΡΕΠΕΙ να χρησιμοποιείται όταν ο τύπος μέσου μίας διανομής είναι ορισμένος στο IANA, αλλιώς η ιδιότητα dcterms:format ΔΥΝΑΤΑΙ να χρησιμοποιηθεί με διαφορετικές τιμές.</rdfs:comment>
        <rdfs:comment xml:lang="ar">يجب استخدام هذه الخاصية إذا كان نوع الملف معرف ضمن IANA</rdfs:comment>
        <rdfs:comment xml:lang="ja">このプロパティーは、配信のメディア・タイプがIANAで定義されているときに使用すべきで（SHOULD）、そうでない場合には、dcterms:formatを様々な値と共に使用できます（MAY）。</rdfs:comment>
        <rdfs:isDefinedBy rdf:resource="http://www.w3.org/TR/vocab-dcat/"/>
        <rdfs:label xml:lang="en">media type</rdfs:label>
        <rdfs:label xml:lang="da">medietype</rdfs:label>
        <rdfs:label xml:lang="es">tipo de media</rdfs:label>
        <rdfs:label xml:lang="it">tipo di media</rdfs:label>
        <rdfs:label xml:lang="cs">typ média</rdfs:label>
        <rdfs:label xml:lang="fr">type de média</rdfs:label>
        <rdfs:label xml:lang="el">τύπος μέσου</rdfs:label>
        <rdfs:label xml:lang="ar">نوع الميديا</rdfs:label>
        <rdfs:label xml:lang="ja">メディア・タイプ</rdfs:label>
        <skos:changeNote xml:lang="it">Il range di dcat:mediaType è stato ristretto  come parte della revisione di DCAT.</skos:changeNote>
        <skos:changeNote xml:lang="cs">Obor hodnot dcat:mediaType byl zúžen v této revizi DCAT.</skos:changeNote>
        <skos:changeNote xml:lang="en">The range of dcat:mediaType has been tightened as part of the revision of DCAT.</skos:changeNote>
        <skos:definition xml:lang="fr">Cette propriété doit être utilisée quand c&apos;est définit le type de média de la distribution en IANA, sinon dcterms:format DOIT être utilisé avec différentes valeurs.</skos:definition>
        <skos:definition xml:lang="es">Esta propiedad debe ser usada cuando está definido el tipo de media de la distribución en IANA, de otra manera dcterms:format puede ser utilizado con diferentes valores.</skos:definition>
        <skos:definition xml:lang="it">Il tipo di media della distribuzione come definito da IANA.</skos:definition>
        <skos:definition xml:lang="da">Medietypen for distributionen som den er defineret af IANA.</skos:definition>
        <skos:definition xml:lang="en">The media type of the distribution as defined by IANA.</skos:definition>
        <skos:definition xml:lang="cs">Typ média distribuce definovaný v IANA.</skos:definition>
        <skos:definition xml:lang="el">Η ιδιότητα αυτή ΘΑ ΠΡΕΠΕΙ να χρησιμοποιείται όταν ο τύπος μέσου μίας διανομής είναι ορισμένος στο IANA, αλλιώς η ιδιότητα dcterms:format ΔΥΝΑΤΑΙ να χρησιμοποιηθεί με διαφορετικές τιμές.</skos:definition>
        <skos:definition xml:lang="ar">يجب استخدام هذه الخاصية إذا كان نوع الملف معرف ضمن IANA</skos:definition>
        <skos:definition xml:lang="ja">このプロパティーは、配信のメディア・タイプがIANAで定義されているときに使用すべきで（SHOULD）、そうでない場合には、dcterms:formatを様々な値と共に使用できます（MAY）。</skos:definition>
        <skos:editorialNote xml:lang="en">Status: English Definition text modified by DCAT revision team, Italian and Czech translation provided, other translations pending. Note some inconsistency on def vs. usage.</skos:editorialNote>
        <skos:scopeNote xml:lang="da">Denne egenskab BØR anvendes hvis distributionens medietype optræder i &apos;IANA media types registry&apos; https://www.iana.org/assignments/media-types/, ellers KAN egenskaben dcterms:format anvendes med et andet udfaldsrum.</skos:scopeNote>
        <skos:scopeNote xml:lang="es">Esta propiedad DEBERÍA usarse cuando el &apos;media type&apos; de la distribución está definido en el registro IANA de &apos;media types&apos; https://www.iana.org/assignments/media-types/, de lo contrario, dcterms:format PUEDE usarse con distintos valores.</skos:scopeNote>
        <skos:scopeNote xml:lang="it">Questa proprietà DEVE essere usata quando il tipo di media della distribuzione è definito nel registro dei tipi di media IANA https://www.iana.org/assignments/media-types/, altrimenti dcterms:format PUO &apos;essere usato con differenti valori.</skos:scopeNote>
        <skos:scopeNote xml:lang="cs">Tato vlastnost BY MĚLA být použita, je-li typ média distribuce definován v registru IANA https://www.iana.org/assignments/media-types/. V ostatních případech MŮŽE být použita vlastnost dcterms:format s jinými hodnotami.</skos:scopeNote>
        <skos:scopeNote xml:lang="en">This property SHOULD be used when the media type of the distribution is defined in the IANA media types registry https://www.iana.org/assignments/media-types/, otherwise dcterms:format MAY be used with different values.</skos:scopeNote>
    </owl:ObjectProperty>
    


    <!-- http://www.w3.org/ns/dcat#next -->


    <rdf:Description rdf:about="http://www.w3.org/ns/dcat#next">
        <owl:inverseOf rdf:resource="http://www.w3.org/ns/dcat#prev"/>
        <rdfs:isDefinedBy rdf:resource="https://www.w3.org/TR/vocab-dcat-3/"/>
        <skos:changeNote xml:lang="en">New property added in DCAT 3.</skos:changeNote>
        <skos:changeNote xml:lang="cs">Nová vlastnost přidaná ve verzi DCAT 3.</skos:changeNote>
        <skos:changeNote xml:lang="es">Nueva propiedad agregada en DCAT 3.</skos:changeNote>
        <skos:changeNote xml:lang="it">Nuova proprietà aggiunta in DCAT 3.</skos:changeNote>
        <skos:scopeNote xml:lang="es">Esta propiedad inversa PUEDE usarse sólo en combinación con su inversa, y NO PUEDE utilizarse en su reemplazo.</skos:scopeNote>
        <skos:scopeNote xml:lang="it">Questa proprietà PUÒ essere usata solo insieme alla sua inversa, e NON DEVE essere usata per sostituirla.</skos:scopeNote>
        <skos:scopeNote xml:lang="en">This property MAY be used only in addition to its inverse, and it MUST NOT be used to replace it.</skos:scopeNote>
    </rdf:Description>
    


    <!-- http://www.w3.org/ns/dcat#nextVersion -->


    <rdf:Description rdf:about="http://www.w3.org/ns/dcat#nextVersion">
        <owl:inverseOf rdf:resource="http://www.w3.org/ns/dcat#previousVersion"/>
        <rdfs:isDefinedBy rdf:resource="https://www.w3.org/TR/vocab-dcat-3/"/>
        <skos:changeNote xml:lang="en">New property added in DCAT 3.</skos:changeNote>
        <skos:changeNote xml:lang="cs">Nová vlastnost přidaná ve verzi DCAT 3.</skos:changeNote>
        <skos:changeNote xml:lang="es">Nueva propiedad agregada en DCAT 3.</skos:changeNote>
        <skos:changeNote xml:lang="it">Nuova proprietà aggiunta in DCAT 3.</skos:changeNote>
        <skos:scopeNote xml:lang="es">Esta propiedad inversa PUEDE usarse sólo en combinación con su inversa, y NO PUEDE utilizarse en su reemplazo.</skos:scopeNote>
        <skos:scopeNote xml:lang="it">Questa proprietà PUÒ essere usata solo insieme alla sua inversa, e NON DEVE essere usata per sostituirla.</skos:scopeNote>
        <skos:scopeNote xml:lang="en">This property MAY be used only in addition to its inverse, and it MUST NOT be used to replace it.</skos:scopeNote>
    </rdf:Description>
    


    <!-- http://www.w3.org/ns/dcat#packageFormat -->


    <owl:ObjectProperty rdf:about="http://www.w3.org/ns/dcat#packageFormat">
        <rdfs:subPropertyOf rdf:resource="http://purl.org/dc/terms/format"/>
        <rdfs:domain rdf:resource="http://www.w3.org/ns/dcat#Distribution"/>
        <rdfs:range rdf:resource="http://purl.org/dc/terms/MediaType"/>
        <rdfs:comment xml:lang="cs">Balíčkový formát souboru, ve kterém je jeden či více souborů seskupeno dohromady, např. aby bylo možné stáhnout sadu souvisejících souborů naráz.</rdfs:comment>
        <rdfs:comment xml:lang="es">El formato del archivo en que se agrupan uno o más archivos de datos, e.g. para permitir que un conjunto de archivos relacionados se bajen juntos.</rdfs:comment>
        <rdfs:comment xml:lang="da">Format til pakning af data med henblik på distribution af en eller flere relaterede datafiler der samles til en enhed med henblik på samlet distribution. </rdfs:comment>
        <rdfs:comment xml:lang="it">Il formato di impacchettamento della distribuzione in cui uno o più file di dati sono raggruppati insieme, ad es. per abilitare un insieme di file correlati da scaricare insieme.</rdfs:comment>
        <rdfs:comment xml:lang="en">The package format of the distribution in which one or more data files are grouped together, e.g. to enable a set of related files to be downloaded together.</rdfs:comment>
        <rdfs:isDefinedBy rdf:resource="https://www.w3.org/TR/vocab-dcat-2/"/>
        <rdfs:label xml:lang="es">formato de empaquetado</rdfs:label>
        <rdfs:label xml:lang="it">formato di impacchettamento</rdfs:label>
        <rdfs:label xml:lang="cs">formát balíčku</rdfs:label>
        <rdfs:label xml:lang="en">packaging format</rdfs:label>
        <rdfs:label xml:lang="da">pakkeformat</rdfs:label>
        <skos:changeNote xml:lang="en">New property added in DCAT 2.</skos:changeNote>
        <skos:changeNote xml:lang="cs">Nová vlastnost přidaná ve verzi DCAT 2.</skos:changeNote>
        <skos:changeNote xml:lang="es">Nueva propiedad agregada en DCAT 2.</skos:changeNote>
        <skos:changeNote xml:lang="it">Nuova proprietà aggiunta in DCAT 2.</skos:changeNote>
        <skos:changeNote xml:lang="da">Ny egenskab tilføjet i DCAT 2.</skos:changeNote>
        <skos:definition xml:lang="cs">Balíčkový formát souboru, ve kterém je jeden či více souborů seskupeno dohromady, např. aby bylo možné stáhnout sadu souvisejících souborů naráz.</skos:definition>
        <skos:definition xml:lang="es">El formato del archivo en que se agrupan uno o más archivos de datos, e.g. para permitir que un conjunto de archivos relacionados se bajen juntos.</skos:definition>
        <skos:definition xml:lang="it">Il formato di impacchettamento della distribuzione in cui uno o più file di dati sono raggruppati insieme, ad es. per abilitare un insieme di file correlati da scaricare insieme.</skos:definition>
        <skos:definition xml:lang="en">The package format of the distribution in which one or more data files are grouped together, e.g. to enable a set of related files to be downloaded together.</skos:definition>
        <skos:scopeNote xml:lang="da">Denne egenskab kan anvendes hvis filerne i en distribution er pakket, fx i en TAR-fil, en Frictionless Data Package eller en Bagit-fil. Formatet BØR udtrykkes ved en medietype som defineret i &apos;IANA media types registry&apos;, hvis der optræder en relevant medietype dér: https://www.iana.org/assignments/media-types/.</skos:scopeNote>
        <skos:scopeNote xml:lang="es">Esta propiedad se debe usar cuando los archivos de la distribución están empaquetados, por ejemplo en un archivo TAR, Frictionless Data Package o Bagit. El formato DEBERÍA expresarse usando un &apos;media type&apos;, tales como los definidos en el registro IANA de &apos;media types&apos; https://www.iana.org/assignments/media-types/, si está disponibles.</skos:scopeNote>
        <skos:scopeNote xml:lang="it">Questa proprietà deve essere utilizzata quando i file nella distribuzione sono impacchettati, ad esempio in un file TAR, Frictionless Data Package o Bagit. Il formato DOVREBBE essere espresso utilizzando un tipo di supporto come definito dal registro dei tipi di media IANA https://www.iana.org/assignments/media-types/, se disponibili.</skos:scopeNote>
        <skos:scopeNote xml:lang="cs">Tato vlastnost se použije, když jsou soubory v distribuci zabaleny, např. v souboru TAR, v balíčku Frictionless Data Package nebo v souboru Bagit. Formát BY MĚL být vyjádřen pomocí typu média definovaného v registru IANA https://www.iana.org/assignments/media-types/, pokud existuje.</skos:scopeNote>
        <skos:scopeNote xml:lang="en">This property to be used when the files in the distribution are packaged, e.g. in a TAR file, a Frictionless Data Package or a Bagit file. The format SHOULD be expressed using a media type as defined by IANA media types registry https://www.iana.org/assignments/media-types/, if available.</skos:scopeNote>
    </owl:ObjectProperty>
    


    <!-- http://www.w3.org/ns/dcat#prev -->


    <owl:ObjectProperty rdf:about="http://www.w3.org/ns/dcat#prev">
        <rdfs:subPropertyOf rdf:resource="http://www.w3.org/1999/xhtml/vocab#prev"/>
        <rdfs:comment xml:lang="it">La risorsa precedente a quella attuale in una collezione ordinata o in una serie di risorse.</rdfs:comment>
        <rdfs:comment xml:lang="en">The previous resource (before the current one) in an ordered collection or series of resources.</rdfs:comment>
        <rdfs:isDefinedBy rdf:resource="https://www.w3.org/TR/vocab-dcat-3/"/>
        <rdfs:label xml:lang="it">precedente</rdfs:label>
        <rdfs:label xml:lang="es">previo</rdfs:label>
        <rdfs:label xml:lang="en">previous</rdfs:label>
        <skos:changeNote xml:lang="en">New property added in DCAT 3.</skos:changeNote>
        <skos:changeNote xml:lang="cs">Nová vlastnost přidaná ve verzi DCAT 3.</skos:changeNote>
        <skos:changeNote xml:lang="es">Nueva propiedad agregada in DCAT 3.</skos:changeNote>
        <skos:changeNote xml:lang="it">Nuova proprietà aggiunta in DCAT 3.</skos:changeNote>
        <skos:changeNote xml:lang="da">Ny egenskab tilføjet i DCAT 3.</skos:changeNote>
        <skos:definition xml:lang="it">La risorsa precedente a quella attuale in una collezione ordinata o in una serie di risorse.</skos:definition>
        <skos:definition xml:lang="en">The previous resource (before the current one) in an ordered collection or series of resources.</skos:definition>
        <skos:scopeNote xml:lang="es">En DCAT esta propiedad se usa para recursos que pertenecen a una dcat:DatasetSeries.</skos:scopeNote>
        <skos:scopeNote xml:lang="it">In DCAT questa proprietà è usata per risorse che fanno parte di una dcat:DatasetSeries.</skos:scopeNote>
        <skos:scopeNote xml:lang="en">In DCAT this property is used for resources belonging to a dcat:DatasetSeries.</skos:scopeNote>
        <skos:scopeNote xml:lang="en">It is important to note that this property is different from dcat:previousVersion, as it does not denote a previous version of the same resource, but a distinct resource immediately preceding the current one in an ordered collection of resources.</skos:scopeNote>
        <skos:scopeNote xml:lang="it">È importante notare che questa proprietà è diversa da dcat:previousVersion, dato che non indica una versione precedente della stessa risorsa, ma una risorsa distinta che precede immediatamente quella attuale in una collezione ordinata di risorse.</skos:scopeNote>
    </owl:ObjectProperty>
    


    <!-- http://www.w3.org/ns/dcat#previousVersion -->


    <owl:ObjectProperty rdf:about="http://www.w3.org/ns/dcat#previousVersion">
        <rdfs:subPropertyOf rdf:resource="http://www.w3.org/ns/prov#wasRevisionOf"/>
        <rdfs:comment xml:lang="it">La versione precedente di una risorsa.</rdfs:comment>
        <rdfs:comment xml:lang="en">The previous version of a resource in a lineage [PAV].</rdfs:comment>
        <rdfs:isDefinedBy rdf:resource="https://www.w3.org/TR/vocab-dcat-3/"/>
        <rdfs:label xml:lang="en">previous version</rdfs:label>
        <rdfs:label xml:lang="it">versione precedente</rdfs:label>
        <rdfs:label xml:lang="es">versión anterior</rdfs:label>
        <skos:changeNote xml:lang="en">New property added in DCAT 3.</skos:changeNote>
        <skos:changeNote xml:lang="cs">Nová vlastnost přidaná ve verzi DCAT 3.</skos:changeNote>
        <skos:changeNote xml:lang="es">Nueva propiedad agregada in DCAT 3.</skos:changeNote>
        <skos:changeNote xml:lang="it">Nuova proprietà aggiunta in DCAT 3.</skos:changeNote>
        <skos:changeNote xml:lang="da">Ny egenskab tilføjet i DCAT 3.</skos:changeNote>
        <skos:definition xml:lang="it">La versione precedente di una risorsa.</skos:definition>
        <skos:definition xml:lang="en">The previous version of a resource in a lineage [PAV].</skos:definition>
        <skos:scopeNote xml:lang="it">La nozione di versione usata da questa proprietà è limitata a versioni risultanti da revisioni a cui una risorsa è soggetta nel suo ciclo di vita. Uno dei casi tipici è la rappresentazione della storia delle versioni di un dataset, che sono state pubblicate nel corso del tempo.</skos:scopeNote>
        <skos:scopeNote xml:lang="it">Questa proprietà è usata per specificare una catena di versioni, costituita da snapshot di una risorsa.</skos:scopeNote>
        <skos:scopeNote xml:lang="en">The notion of version used by this property is limited to versions resulting from revisions occurring to a resource as part of its life-cycle. One of the typical cases here is representing the history of the versions of a dataset that have been released over time.</skos:scopeNote>
        <skos:scopeNote xml:lang="en">This property is meant to be used to specify a version chain, consisting of snapshots of a resource.</skos:scopeNote>
    </owl:ObjectProperty>
    


    <!-- http://www.w3.org/ns/dcat#qualifiedRelation -->


    <owl:ObjectProperty rdf:about="http://www.w3.org/ns/dcat#qualifiedRelation">
        <rdfs:domain rdf:resource="http://www.w3.org/ns/dcat#Resource"/>
        <rdfs:range rdf:resource="http://www.w3.org/ns/dcat#Relationship"/>
        <rdfs:comment xml:lang="es">Enlace a una descripción de la relación con otro recurso.</rdfs:comment>
        <rdfs:comment xml:lang="it">Link a una descrizione di una relazione con un&apos;altra risorsa.</rdfs:comment>
        <rdfs:comment xml:lang="en">Link to a description of a relationship with another resource.</rdfs:comment>
        <rdfs:comment xml:lang="cs">Odkaz na popis vztahu s jiným zdrojem.</rdfs:comment>
        <rdfs:comment xml:lang="da">Reference til en beskrivelse af en relation til en anden ressource.</rdfs:comment>
        <rdfs:isDefinedBy rdf:resource="https://www.w3.org/TR/vocab-dcat-2/"/>
        <rdfs:label xml:lang="da">Kvalificeret relation</rdfs:label>
        <rdfs:label xml:lang="cs">kvalifikovaný vztah</rdfs:label>
        <rdfs:label xml:lang="en">qualified relation</rdfs:label>
        <rdfs:label xml:lang="es">relación calificada</rdfs:label>
        <rdfs:label xml:lang="it">relazione qualificata</rdfs:label>
        <skos:changeNote xml:lang="en">New property added in DCAT 2.</skos:changeNote>
        <skos:changeNote xml:lang="cs">Nová vlastnost přidaná ve verzi DCAT 2.</skos:changeNote>
        <skos:changeNote xml:lang="it">Nuova proprietà aggiunta in DCAT 2.</skos:changeNote>
        <skos:changeNote xml:lang="da">Ny egenskab tilføjet i DCAT 2.</skos:changeNote>
        <skos:changeNote xml:lang="es">Propiedad nueva añadida en DCAT 2.</skos:changeNote>
        <skos:definition xml:lang="es">Enlace a una descripción de la relación con otro recurso.</skos:definition>
        <skos:definition xml:lang="it">Link a una descrizione di una relazione con un&apos;altra risorsa.</skos:definition>
        <skos:definition xml:lang="en">Link to a description of a relationship with another resource.</skos:definition>
        <skos:definition xml:lang="cs">Odkaz na popis vztahu s jiným zdrojem.</skos:definition>
        <skos:definition xml:lang="da">Reference til en beskrivelse af en relation til en anden ressource.</skos:definition>
        <skos:editorialNote xml:lang="it">Introdotta in DCAT per integrare le altre relazioni qualificate di PROV.</skos:editorialNote>
        <skos:editorialNote xml:lang="en">Introduced into DCAT to complement the other PROV qualified relations. </skos:editorialNote>
        <skos:editorialNote xml:lang="da">Introduceret i DCAT med henblik på at supplere de øvrige kvalificerede relationer fra PROV. </skos:editorialNote>
        <skos:editorialNote xml:lang="cs">Přidáno do DCAT k doplnění jiných kvalifikovaných vztahů ze slovníku PROV.</skos:editorialNote>
        <skos:editorialNote xml:lang="es">Se incluyó en DCAT para complementar las relaciones calificadas disponibles en PROV.</skos:editorialNote>
        <skos:scopeNote xml:lang="da">Anvendes til at referere til en anden ressource hvor relationens betydning er kendt men ikke matcher en af de standardiserede egenskaber fra Dublin Core (dcterms:hasPart, dcterms:isPartOf, dcterms:conformsTo, dcterms:isFormatOf, dcterms:hasFormat, dcterms:isVersionOf, dcterms:hasVersion, dcterms:replaces, dcterms:isReplacedBy, dcterms:references, dcterms:isReferencedBy, dcterms:requires, dcterms:isRequiredBy) eller PROV-O-egenskaber (prov:wasDerivedFrom, prov:wasInfluencedBy, prov:wasQuotedFrom, prov:wasRevisionOf, prov:hadPrimarySource, prov:alternateOf, prov:specializationOf).</skos:scopeNote>
        <skos:scopeNote xml:lang="cs">Použito pro odkazování na jiný zdroj, kde druh vztahu je znám, ale neodpovídá standardním vlastnostem ze slovníku Dublin Core (dcterms:hasPart, dcterms:isPartOf, dcterms:conformsTo, dcterms:isFormatOf, dcterms:hasFormat, dcterms:isVersionOf, dcterms:hasVersion, dcterms:replaces, dcterms:isReplacedBy, dcterms:references, dcterms:isReferencedBy, dcterms:requires, dcterms:isRequiredBy) či slovníku PROV-O (prov:wasDerivedFrom, prov:wasInfluencedBy, prov:wasQuotedFrom, prov:wasRevisionOf, prov:hadPrimarySource, prov:alternateOf, prov:specializationOf).</skos:scopeNote>
        <skos:scopeNote xml:lang="es">Se usa para asociar con otro recurso para el cuál la naturaleza de la relación es conocida pero no es ninguna de las propiedades que provee el estándar Dublin Core (dcterms:hasPart, dcterms:isPartOf, dcterms:conformsTo, dcterms:isFormatOf, dcterms:hasFormat, dcterms:isVersionOf, dcterms:hasVersion, dcterms:replaces, dcterms:isReplacedBy, dcterms:references, dcterms:isReferencedBy, dcterms:requires, dcterms:isRequiredBy) or PROV-O properties (prov:wasDerivedFrom, prov:wasInfluencedBy, prov:wasQuotedFrom, prov:wasRevisionOf, prov:hadPrimarySource, prov:alternateOf, prov:specializationOf).</skos:scopeNote>
        <skos:scopeNote xml:lang="en">Used to link to another resource where the nature of the relationship is known but does not match one of the standard Dublin Core properties (dcterms:hasPart, dcterms:isPartOf, dcterms:conformsTo, dcterms:isFormatOf, dcterms:hasFormat, dcterms:isVersionOf, dcterms:hasVersion, dcterms:replaces, dcterms:isReplacedBy, dcterms:references, dcterms:isReferencedBy, dcterms:requires, dcterms:isRequiredBy) or PROV-O properties (prov:wasDerivedFrom, prov:wasInfluencedBy, prov:wasQuotedFrom, prov:wasRevisionOf, prov:hadPrimarySource, prov:alternateOf, prov:specializationOf).</skos:scopeNote>
        <skos:scopeNote xml:lang="it">Viene utilizzato per associarsi a un&apos;altra risorsa nei casi per i quali la natura della relazione è nota ma non è alcuna delle proprietà fornite dallo standard Dublin Core (dcterms:hasPart, dcterms:isPartOf, dcterms:conformsTo, dcterms:isFormatOf, dcterms:hasFormat , dcterms:isVersionOf, dcterms:hasVersion, dcterms:replaces, dcterms:isReplacedBy, dcterms:references, dcterms:isReferencedBy, dcterms:require, dcterms:isRequiredBy) o dalle proprietà fornite da PROV-O (prov:wasDerivedFrom, prov:wasInfluencedBy, prov:wasQuotedFrom , prov:wasRevisionOf, prov:hadPrimarySource, prov:alternateOf, prov:specializationOf).</skos:scopeNote>
    </owl:ObjectProperty>
    


    <!-- http://www.w3.org/ns/dcat#record -->


    <owl:ObjectProperty rdf:about="http://www.w3.org/ns/dcat#record">
        <rdfs:domain rdf:resource="http://www.w3.org/ns/dcat#Catalog"/>
        <rdfs:range rdf:resource="http://www.w3.org/ns/dcat#CatalogRecord"/>
        <rdfs:comment xml:lang="en">A record describing the registration of a single dataset or data service that is part of the catalog.</rdfs:comment>
        <rdfs:comment xml:lang="es">Describe la registración de un conjunto de datos o un servicio de datos en el catálogo.</rdfs:comment>
        <rdfs:comment xml:lang="da">En post der beskriver registreringen af et enkelt datasæt eller en datatjeneste som er opført i kataloget.</rdfs:comment>
        <rdfs:comment xml:lang="cs">Propojuje katalog a jeho záznamy.</rdfs:comment>
        <rdfs:comment xml:lang="fr">Relie un catalogue à ses registres.</rdfs:comment>
        <rdfs:comment xml:lang="it">Un record che descrive la registrazione di un singolo set di dati o di un servizio dati che fa parte del catalogo.</rdfs:comment>
        <rdfs:comment xml:lang="cs">Záznam popisující registraci jedné datové sady či datové služby jakožto součásti katalogu.</rdfs:comment>
        <rdfs:comment xml:lang="el">Συνδέει έναν κατάλογο με τις καταγραφές του.</rdfs:comment>
        <rdfs:comment xml:lang="ar">تربط الفهرس بسجل ضمنه</rdfs:comment>
        <rdfs:comment xml:lang="ja">カタログの一部であるカタログ・レコード。</rdfs:comment>
        <rdfs:isDefinedBy rdf:resource="http://www.w3.org/TR/vocab-dcat/"/>
        <rdfs:label xml:lang="da">post</rdfs:label>
        <rdfs:label xml:lang="en">record</rdfs:label>
        <rdfs:label xml:lang="it">record</rdfs:label>
        <rdfs:label xml:lang="fr">registre</rdfs:label>
        <rdfs:label xml:lang="es">registro</rdfs:label>
        <rdfs:label xml:lang="cs">záznam</rdfs:label>
        <rdfs:label xml:lang="el">καταγραφή</rdfs:label>
        <rdfs:label xml:lang="ar">سجل</rdfs:label>
        <rdfs:label xml:lang="ja">カタログ・レコード</rdfs:label>
        <skos:altLabel xml:lang="da">har post</skos:altLabel>
        <skos:definition xml:lang="en">A record describing the registration of a single dataset or data service that is part of the catalog.</skos:definition>
        <skos:definition xml:lang="es">Describe la registración de un conjunto de datos o un servicio de datos en el catálogo.</skos:definition>
        <skos:definition xml:lang="da">En post der beskriver registreringen af et enkelt datasæt eller en datatjeneste som er opført i kataloget.</skos:definition>
        <skos:definition xml:lang="cs">Propojuje katalog a jeho záznamy.</skos:definition>
        <skos:definition xml:lang="fr">Relie un catalogue à ses registres.</skos:definition>
        <skos:definition xml:lang="it">Un record che descrive la registrazione di un singolo set di dati o di un servizio dati che fa parte del catalogo.</skos:definition>
        <skos:definition xml:lang="cs">Záznam popisující registraci jedné datové sady či datové služby jakožto součásti katalogu.</skos:definition>
        <skos:definition xml:lang="el">Συνδέει έναν κατάλογο με τις καταγραφές του.</skos:definition>
        <skos:definition xml:lang="ar">تربط الفهرس بسجل ضمنه</skos:definition>
        <skos:definition xml:lang="ja">カタログの一部であるカタログ・レコード。</skos:definition>
        <skos:editorialNote xml:lang="en">Status: English, Italian, Spanish and Czech Definitions modified by DCAT revision team, other translations pending.</skos:editorialNote>
    </owl:ObjectProperty>
    


    <!-- http://www.w3.org/ns/dcat#resource -->


    <owl:ObjectProperty rdf:about="http://www.w3.org/ns/dcat#resource">
        <rdfs:subPropertyOf rdf:resource="http://purl.org/dc/terms/hasPart"/>
        <rdfs:domain rdf:resource="http://www.w3.org/ns/dcat#Catalog"/>
        <rdfs:range rdf:resource="http://www.w3.org/ns/dcat#Resource"/>
        <rdfs:comment xml:lang="en">A resource that is listed in the catalog.</rdfs:comment>
        <rdfs:comment xml:lang="it">Una risorsa elencata nel catalogo.</rdfs:comment>
        <rdfs:isDefinedBy rdf:resource="https://www.w3.org/TR/vocab-dcat-3/"/>
        <rdfs:label xml:lang="en">resource</rdfs:label>
        <rdfs:label xml:lang="it">risorsa</rdfs:label>
        <skos:changeNote xml:lang="en">New property added in DCAT 3.</skos:changeNote>
        <skos:changeNote xml:lang="cs">Nová vlastnost přidaná ve verzi DCAT 3.</skos:changeNote>
        <skos:changeNote xml:lang="es">Nueva propiedad agregada en DCAT 3.</skos:changeNote>
        <skos:changeNote xml:lang="it">Nuova proprietà aggiunta in DCAT 3.</skos:changeNote>
        <skos:definition xml:lang="en">A resource that is listed in the catalog.</skos:definition>
        <skos:definition xml:lang="it">Una risorsa elencata nel catalogo.</skos:definition>
        <skos:editorialNote xml:lang="en">Status: English Definition text modified by DCAT 3 revision team, translations pending.</skos:editorialNote>
        <skos:scopeNote xml:lang="it">Questo è il predicate più generale per indicare l&apos;appartenenza di una risorsa a un catalogo. Si raccomanda l&apos;uso di una proprietà più specifica, quando disponibile.</skos:scopeNote>
        <skos:scopeNote xml:lang="en">See also:	Sub-properties of dcat:resource in particular dcat:dataset, dcat:catalog, dcat:service.</skos:scopeNote>
        <skos:scopeNote xml:lang="en">This is the most general predicate for membership of a catalog. Use of a more specific sub-property is recommended when available.</skos:scopeNote>
        <skos:scopeNote xml:lang="it">Vd. anche: Le sottoproprietà di dcat:resource, in particolare: dcat:dataset, dcat:catalog, dcat:service.</skos:scopeNote>
    </owl:ObjectProperty>
    


    <!-- http://www.w3.org/ns/dcat#seriesMember -->


    <rdf:Description rdf:about="http://www.w3.org/ns/dcat#seriesMember">
        <owl:inverseOf rdf:resource="http://www.w3.org/ns/dcat#inSeries"/>
        <rdfs:isDefinedBy rdf:resource="https://www.w3.org/TR/vocab-dcat-3/"/>
        <skos:changeNote xml:lang="en">New property added in DCAT 3.</skos:changeNote>
        <skos:changeNote xml:lang="cs">Nová vlastnost přidaná ve verzi DCAT 3.</skos:changeNote>
        <skos:changeNote xml:lang="es">Nueva propiedad agregada en DCAT 3.</skos:changeNote>
        <skos:changeNote xml:lang="it">Nuova proprietà aggiunta in DCAT 3.</skos:changeNote>
        <skos:scopeNote xml:lang="es">Esta propiedad inversa PUEDE usarse sólo en combinación con su inversa, y NO PUEDE utilizarse en su reemplazo.</skos:scopeNote>
        <skos:scopeNote xml:lang="it">Questa proprietà PUÒ essere usata solo insieme alla sua inversa, e NON DEVE essere usata per sostituirla.</skos:scopeNote>
        <skos:scopeNote xml:lang="en">This property MAY be used only in addition to its inverse, and it MUST NOT be used to replace it.</skos:scopeNote>
    </rdf:Description>
    


    <!-- http://www.w3.org/ns/dcat#servesDataset -->


    <owl:ObjectProperty rdf:about="http://www.w3.org/ns/dcat#servesDataset">
        <rdfs:domain rdf:resource="http://www.w3.org/ns/dcat#DataService"/>
        <rdfs:range rdf:resource="http://www.w3.org/ns/dcat#Dataset"/>
        <rdfs:comment xml:lang="en">A collection of data that this DataService can distribute.</rdfs:comment>
        <rdfs:comment xml:lang="da">En samling af data som denne datatjeneste kan distribuere.</rdfs:comment>
        <rdfs:comment xml:lang="cs">Kolekce dat, kterou je tato Datová služba schopna poskytnout.</rdfs:comment>
        <rdfs:comment xml:lang="es">Una colección de datos que este Servicio de Datos puede distribuir.</rdfs:comment>
        <rdfs:comment xml:lang="it">Una raccolta di dati che questo DataService può distribuire.</rdfs:comment>
        <rdfs:isDefinedBy rdf:resource="https://www.w3.org/TR/vocab-dcat-2/"/>
        <rdfs:label xml:lang="da">datatjeneste for datasæt</rdfs:label>
        <rdfs:label xml:lang="cs">poskytuje datovou sadu</rdfs:label>
        <rdfs:label xml:lang="es">provee conjunto de datos</rdfs:label>
        <rdfs:label xml:lang="it">serve set di dati</rdfs:label>
        <rdfs:label xml:lang="en">serves dataset</rdfs:label>
        <skos:altLabel xml:lang="da">distribuerer</skos:altLabel>
        <skos:altLabel xml:lang="da">ekspederer</skos:altLabel>
        <skos:altLabel xml:lang="da">udstiller</skos:altLabel>
        <skos:changeNote xml:lang="en">New property in DCAT 2.</skos:changeNote>
        <skos:changeNote xml:lang="cs">Nová vlastnost přidaná ve verzi DCAT 2.</skos:changeNote>
        <skos:changeNote xml:lang="es">Nueva propiedad agregada en DCAT 2.</skos:changeNote>
        <skos:changeNote xml:lang="it">Nuova proprietà in DCAT 2.</skos:changeNote>
        <skos:definition xml:lang="en">A collection of data that this DataService can distribute.</skos:definition>
        <skos:definition xml:lang="da">En samling af data som denne datatjeneste kan distribuere.</skos:definition>
        <skos:definition xml:lang="cs">Kolekce dat, kterou je tato Datová služba schopna poskytnout.</skos:definition>
        <skos:definition xml:lang="es">Una colección de datos que este Servicio de Datos puede distribuir.</skos:definition>
        <skos:definition xml:lang="it">Una raccolta di dati che questo DataService può distribuire.</skos:definition>
    </owl:ObjectProperty>
    


    <!-- http://www.w3.org/ns/dcat#service -->


    <owl:ObjectProperty rdf:about="http://www.w3.org/ns/dcat#service">
        <rdfs:subPropertyOf rdf:resource="http://www.w3.org/ns/dcat#resource"/>
        <rdfs:domain rdf:resource="http://www.w3.org/ns/dcat#Catalog"/>
        <rdfs:range rdf:resource="http://www.w3.org/ns/dcat#DataService"/>
        <rdfs:comment xml:lang="en">A service that is listed in the catalog.</rdfs:comment>
        <rdfs:comment xml:lang="da">Et websted eller et endpoint som er opført i kataloget.</rdfs:comment>
        <rdfs:comment xml:lang="cs">Umístění či přístupový bod registrovaný v katalogu.</rdfs:comment>
        <rdfs:comment xml:lang="es">Un sitio o &apos;endpoint&apos; que está listado en el catálogo.</rdfs:comment>
        <rdfs:comment xml:lang="it">Un sito o endpoint elencato nel catalogo.</rdfs:comment>
        <rdfs:isDefinedBy rdf:resource="https://www.w3.org/TR/vocab-dcat-2/"/>
        <rdfs:label xml:lang="da">datatjeneste</rdfs:label>
        <rdfs:label xml:lang="en">service</rdfs:label>
        <rdfs:label xml:lang="es">servicio</rdfs:label>
        <rdfs:label xml:lang="it">servizio</rdfs:label>
        <rdfs:label xml:lang="cs">služba</rdfs:label>
        <skos:altLabel xml:lang="da">har datatjeneste</skos:altLabel>
        <skos:altLabel xml:lang="en">has service</skos:altLabel>
        <skos:changeNote xml:lang="en">New property added in DCAT 2.</skos:changeNote>
        <skos:changeNote xml:lang="cs">Nová vlastnost přidaná ve verzi DCAT 2.</skos:changeNote>
        <skos:changeNote xml:lang="es">Nueva propiedad añadida en DCAT 2.</skos:changeNote>
        <skos:changeNote xml:lang="it">Nuova proprietà aggiunta in DCAT 2.</skos:changeNote>
        <skos:definition xml:lang="en">A service that is listed in the catalog.</skos:definition>
        <skos:definition xml:lang="da">Et websted eller et endpoint som er opført i kataloget.</skos:definition>
        <skos:definition xml:lang="cs">Umístění či přístupový bod registrovaný v katalogu.</skos:definition>
        <skos:definition xml:lang="es">Un sitio o &apos;endpoint&apos; que está listado en el catálogo.</skos:definition>
        <skos:definition xml:lang="it">Un sito o endpoint elencato nel catalogo.</skos:definition>
        <skos:editorialNote xml:lang="en">Status: English Definition text modified by DCAT 3 revision team, translations pending.</skos:editorialNote>
    </owl:ObjectProperty>
    


    <!-- http://www.w3.org/ns/dcat#theme -->


    <owl:ObjectProperty rdf:about="http://www.w3.org/ns/dcat#theme">
        <rdfs:subPropertyOf rdf:resource="http://purl.org/dc/terms/subject"/>
        <rdfs:comment xml:lang="en">A main category of the resource. A resource can have multiple themes.</rdfs:comment>
        <rdfs:comment xml:lang="da">Et centralt emne for ressourcen. En ressource kan have flere centrale emner.</rdfs:comment>
        <rdfs:comment xml:lang="cs">Hlavní téma zdroje. Zdroj může mít více témat.</rdfs:comment>
        <rdfs:comment xml:lang="it">La categoria principale della risorsa. Una risorsa può avere più temi.</rdfs:comment>
        <rdfs:comment xml:lang="es">La categoría principal del recurso. Un recurso puede tener varios temas.</rdfs:comment>
        <rdfs:comment xml:lang="fr">La catégorie principale de la ressource. Une ressource peut avoir plusieurs thèmes.</rdfs:comment>
        <rdfs:comment xml:lang="el">Η κύρια κατηγορία του συνόλου δεδομένων. Ένα σύνολο δεδομένων δύναται να έχει πολλαπλά θέματα.</rdfs:comment>
        <rdfs:comment xml:lang="ar">التصنيف الرئيسي لقائمة البيانات. قائمة البيانات يمكن أن تملك أكثر من تصنيف رئيسي واحد.</rdfs:comment>
        <rdfs:comment xml:lang="ja">データセットの主要カテゴリー。データセットは複数のテーマを持つことができます。</rdfs:comment>
        <rdfs:isDefinedBy rdf:resource="http://www.w3.org/TR/vocab-dcat/"/>
        <rdfs:label xml:lang="da">emne</rdfs:label>
        <rdfs:label xml:lang="es">tema</rdfs:label>
        <rdfs:label xml:lang="it">tema</rdfs:label>
        <rdfs:label xml:lang="en">theme</rdfs:label>
        <rdfs:label xml:lang="fr">thème</rdfs:label>
        <rdfs:label xml:lang="cs">téma</rdfs:label>
        <rdfs:label xml:lang="el">Θέμα</rdfs:label>
        <rdfs:label xml:lang="ar">التصنيف</rdfs:label>
        <rdfs:label xml:lang="ja">テーマ/カテゴリー</rdfs:label>
        <skos:altLabel xml:lang="da">tema</skos:altLabel>
        <skos:definition xml:lang="en">A main category of the resource. A resource can have multiple themes.</skos:definition>
        <skos:definition xml:lang="da">Et centralt emne for ressourcen. En ressource kan have flere centrale emner.</skos:definition>
        <skos:definition xml:lang="cs">Hlavní téma zdroje. Zdroj může mít více témat.</skos:definition>
        <skos:definition xml:lang="it">La categoria principale della risorsa. Una risorsa può avere più temi.</skos:definition>
        <skos:definition xml:lang="es">La categoría principal del recurso. Un recurso puede tener varios temas.</skos:definition>
        <skos:definition xml:lang="fr">La catégorie principale de la ressource. Une ressource peut avoir plusieurs thèmes.</skos:definition>
        <skos:definition xml:lang="el">Η κύρια κατηγορία του συνόλου δεδομένων. Ένα σύνολο δεδομένων δύναται να έχει πολλαπλά θέματα.</skos:definition>
        <skos:definition xml:lang="ar">التصنيف الرئيسي لقائمة البيانات. قائمة البيانات يمكن أن تملك أكثر من تصنيف رئيسي واحد.</skos:definition>
        <skos:definition xml:lang="ja">データセットの主要カテゴリー。データセットは複数のテーマを持つことができます。</skos:definition>
        <skos:editorialNote xml:lang="en">Status: English Definition text  modified by DCAT revision team, all except for Italian and Czech translations are pending. Scope note has changed and its translations should be updated</skos:editorialNote>
        <skos:scopeNote xml:lang="es">El conjunto de skos:Concepts utilizados para categorizar los recursos están organizados en un skos:ConceptScheme que describe todas las categorías y sus relaciones en el catálogo.</skos:scopeNote>
        <skos:scopeNote xml:lang="it">Il set di concetti skos usati per categorizzare le risorse sono organizzati in skos:ConceptScheme che descrive tutte le categorie e le loro relazioni nel catalogo.</skos:scopeNote>
        <skos:scopeNote xml:lang="cs">Sada instancí třídy skos:Concept použitá pro kategorizaci zdrojů je organizována do schématu konceptů skos:ConceptScheme, které popisuje všechny kategorie v katalogu a jejich vztahy.</skos:scopeNote>
        <skos:scopeNote xml:lang="da">Samlingen af begreber (skos:Concept) der anvendes til at emneinddele ressourcer organiseres i et begrebssystem (skos:ConceptScheme) som beskriver alle emnerne og deres relationer i kataloget.</skos:scopeNote>
        <skos:scopeNote xml:lang="en">The set of themes used to categorize the resources are organized in a skos:ConceptScheme, skos:Collection, owl:Ontology or similar, describing all the categories and their relations in the catalog.</skos:scopeNote>
        <skos:scopeNote xml:lang="fr">Un ensemble de skos:Concepts utilisés pour catégoriser les ressources sont organisés en un skos:ConceptScheme décrivant toutes les catégories et ses relations dans le catalogue.</skos:scopeNote>
        <skos:scopeNote xml:lang="el">Το σετ των skos:Concepts που χρησιμοποιείται για να κατηγοριοποιήσει τα σύνολα δεδομένων είναι οργανωμένο εντός ενός skos:ConceptScheme που περιγράφει όλες τις κατηγορίες και τις σχέσεις αυτών στον κατάλογο.</skos:scopeNote>
        <skos:scopeNote xml:lang="ja">データセットを分類するために用いられるskos:Conceptの集合は、カタログのすべてのカテゴリーとそれらの関係を記述しているskos:ConceptSchemeで組織化されます。</skos:scopeNote>
    </owl:ObjectProperty>
    


    <!-- http://www.w3.org/ns/dcat#themeTaxonomy -->


    <owl:ObjectProperty rdf:about="http://www.w3.org/ns/dcat#themeTaxonomy">
        <rdfs:domain rdf:resource="http://www.w3.org/ns/dcat#Catalog"/>
        <rdfs:range rdf:resource="http://www.w3.org/2000/01/rdf-schema#Resource"/>
        <schema:rangeIncludes rdf:resource="http://www.w3.org/2002/07/owl#Ontology"/>
        <schema:rangeIncludes rdf:resource="http://www.w3.org/2004/02/skos/core#Collection"/>
        <schema:rangeIncludes rdf:resource="http://www.w3.org/2004/02/skos/core#ConceptScheme"/>
        <rdfs:comment xml:lang="es">El sistema de organización del conocimiento utilizado para clasificar conjuntos de datos de catálogos.</rdfs:comment>
        <rdfs:comment xml:lang="it">Il sistema di organizzazione della conoscenza (KOS) usato per classificare i dataset del catalogo.</rdfs:comment>
        <rdfs:comment xml:lang="fr">Le systhème d&apos;ogranisation de connaissances utilisé pour classifier les jeux de données du catalogue.</rdfs:comment>
        <rdfs:comment xml:lang="cs">Systém organizace znalostí (KOS) použitý pro klasifikaci datových sad v katalogu.</rdfs:comment>
        <rdfs:comment xml:lang="en">The knowledge organization system (KOS) used to classify catalog&apos;s datasets.</rdfs:comment>
        <rdfs:comment xml:lang="da">Vidensorganiseringssystem (KOS) som anvendes til at klassificere datasæt i kataloget.</rdfs:comment>
        <rdfs:comment xml:lang="el">Το σύστημα οργάνωσης γνώσης που χρησιμοποιείται για την κατηγοριοποίηση των συνόλων δεδομένων του καταλόγου.</rdfs:comment>
        <rdfs:comment xml:lang="ar">لائحة التصنيفات المستخدمه لتصنيف قوائم البيانات ضمن الفهرس</rdfs:comment>
        <rdfs:comment xml:lang="ja">カタログのデータセットを分類するために用いられる知識組織化体系（KOS；knowledge organization system）。</rdfs:comment>
        <rdfs:isDefinedBy rdf:resource="http://www.w3.org/TR/vocab-dcat/"/>
        <rdfs:label xml:lang="da">emnetaksonomi</rdfs:label>
        <rdfs:label xml:lang="it">tassonomia dei temi</rdfs:label>
        <rdfs:label xml:lang="fr">taxonomie de thèmes</rdfs:label>
        <rdfs:label xml:lang="cs">taxonomie témat</rdfs:label>
        <rdfs:label xml:lang="es">taxonomía de temas</rdfs:label>
        <rdfs:label xml:lang="en">theme taxonomy</rdfs:label>
        <rdfs:label xml:lang="el">Ταξινομία θεματικών κατηγοριών.</rdfs:label>
        <rdfs:label xml:lang="ar">قائمة التصنيفات</rdfs:label>
        <rdfs:label xml:lang="ja">テーマ</rdfs:label>
        <skos:altLabel xml:lang="da">temataksonomi</skos:altLabel>
        <skos:definition xml:lang="es">El sistema de organización del conocimiento utilizado para clasificar conjuntos de datos de catálogos.</skos:definition>
        <skos:definition xml:lang="it">Il sistema di organizzazione della conoscenza (KOS) usato per classificare i dataset del catalogo.</skos:definition>
        <skos:definition xml:lang="fr">Le systhème d&apos;ogranisation de connaissances utilisé pour classifier les jeux de données du catalogue.</skos:definition>
        <skos:definition xml:lang="cs">Systém organizace znalostí (KOS) použitý pro klasifikaci datových sad v katalogu.</skos:definition>
        <skos:definition xml:lang="en">The knowledge organization system (KOS) used to classify catalog&apos;s datasets.</skos:definition>
        <skos:definition xml:lang="da">Vidensorganiseringssystem (KOS) som anvendes til at klassificere datasæt i kataloget.</skos:definition>
        <skos:definition xml:lang="el">Το σύστημα οργάνωσης γνώσης που χρησιμοποιείται για την κατηγοριοποίηση των συνόλων δεδομένων του καταλόγου.</skos:definition>
        <skos:definition xml:lang="ar">لائحة التصنيفات المستخدمه لتصنيف قوائم البيانات ضمن الفهرس</skos:definition>
        <skos:definition xml:lang="ja">カタログのデータセットを分類するために用いられる知識組織化体系（KOS；knowledge organization system）。</skos:definition>
        <skos:scopeNote xml:lang="da">Det anbefales at taksonomien organiseres i et skos:ConceptScheme, skos:Collection, owl:Ontology eller lignende, som giver mulighed for at ethvert medlem af taksonomien kan forsynes med en IRI og udgives som linked-data.</skos:scopeNote>
        <skos:scopeNote xml:lang="en">It is recommended that the taxonomy is organized in a skos:ConceptScheme, skos:Collection, owl:Ontology or similar, which allows each member to be denoted by an IRI and published as linked-data.</skos:scopeNote>
        <skos:scopeNote xml:lang="cs">Je doporučeno, aby byla taxonomie vyjádřena jako skos:ConceptScheme, skos:Collection, owl:Ontology nebo podobné, aby mohla být každá položka identifikována pomocí IRI a publikována jako propojená data.</skos:scopeNote>
        <skos:scopeNote xml:lang="es">Se recomienda que la taxonomía se organice como un skos:ConceptScheme, skos:Collection, owl:Ontology o similar, los cuáles permiten que cada miembro se denote con una IRI y se publique como datos enlazados.</skos:scopeNote>
        <skos:scopeNote xml:lang="it">Si raccomanda che la tassonomia sia organizzata in uno skos:ConceptScheme, skos:Collection, owl:Ontology o simili, che permette ad ogni membro di essere indicato da un IRI e pubblicato come linked-data.</skos:scopeNote>
    </owl:ObjectProperty>
    


    <!-- http://www.w3.org/ns/prov#wasDerivedFrom -->


    <owl:ObjectProperty rdf:about="http://www.w3.org/ns/prov#wasDerivedFrom"/>
    


    <!-- http://xmlns.com/foaf/0.1/homepage -->


    <owl:ObjectProperty rdf:about="http://xmlns.com/foaf/0.1/homepage"/>
    


    <!-- http://xmlns.com/foaf/0.1/primaryTopic -->


    <owl:ObjectProperty rdf:about="http://xmlns.com/foaf/0.1/primaryTopic">
        <rdfs:comment xml:lang="es">Este axioma se necesita de manera que Protege cargue DCAT 3 sin problemas.</rdfs:comment>
        <rdfs:comment xml:lang="en">This axiom needed so that Protege loads DCAT 3 without errors.</rdfs:comment>
    </owl:ObjectProperty>
    


    <!-- 
    ///////////////////////////////////////////////////////////////////////////////////////
    //
    // Data properties
    //
    ///////////////////////////////////////////////////////////////////////////////////////
     -->


    


    <!-- http://data.ign.fr/def/topo#artif -->


    <owl:DatatypeProperty rdf:about="http://data.ign.fr/def/topo#artif">
        <rdfs:domain rdf:resource="http://data.ign.fr/def/topo#CoursDEau"/>
        <rdfs:range rdf:resource="http://www.w3.org/2001/XMLSchema#boolean"/>
        <rdfs:comment xml:lang="en">Allows natural streams to be distinguished from artificial or artificialized streams.</rdfs:comment>
        <rdfs:comment xml:lang="fr">Permet de distinguer les cours d&apos;eau naturels des cours d&apos;eau artificiels ou artificialisés.</rdfs:comment>
        <rdfs:isDefinedBy rdf:resource="http://data.ign.fr/def/topo"/>
        <rdfs:label xml:lang="en">artificial</rdfs:label>
        <rdfs:label xml:lang="fr">artificiel</rdfs:label>
    </owl:DatatypeProperty>
    


    <!-- http://data.ign.fr/def/topo#codePostal -->


    <owl:DatatypeProperty rdf:about="http://data.ign.fr/def/topo#codePostal">
        <rdfs:domain rdf:resource="http://data.ign.fr/def/geofla#Commune"/>
        <rdfs:range rdf:resource="http://www.w3.org/2001/XMLSchema#integer"/>
        <rdfs:comment xml:lang="fr">Numéro de code postal.</rdfs:comment>
        <rdfs:comment xml:lang="en">Postal Code Number.</rdfs:comment>
        <rdfs:isDefinedBy rdf:resource="http://data.ign.fr/def/topo"/>
        <rdfs:label xml:lang="fr">code postal</rdfs:label>
        <rdfs:label xml:lang="en">postal code</rdfs:label>
    </owl:DatatypeProperty>
    


    <!-- http://data.ign.fr/def/topo#electrifie -->


    <owl:DatatypeProperty rdf:about="http://data.ign.fr/def/topo#electrifie">
        <rdfs:domain rdf:resource="http://data.ign.fr/def/topo#VoieFerree"/>
        <rdfs:range rdf:resource="http://www.w3.org/2001/XMLSchema#boolean"/>
        <rdfs:comment xml:lang="fr">Désigne le type d&apos;énergie servant à la propulsion des locomotives. Prends la valeur &apos;vrai&apos; s&apos;il s&apos;agit d&apos;une ligne électrifiée.</rdfs:comment>
        <rdfs:comment xml:lang="en">Refers to the type of energy used to propel locomotives. Take the value &apos;true&apos; if it is an electrified line.</rdfs:comment>
        <rdfs:isDefinedBy rdf:resource="http://data.ign.fr/def/topo"/>
        <rdfs:label xml:lang="en">electrified</rdfs:label>
        <rdfs:label xml:lang="fr">électrifié</rdfs:label>
    </owl:DatatypeProperty>
    


    <!-- http://data.ign.fr/def/topo#enConstruction -->


    <owl:DatatypeProperty rdf:about="http://data.ign.fr/def/topo#enConstruction">
        <rdfs:domain>
            <owl:Class>
                <owl:unionOf rdf:parseType="Collection">
                    <rdf:Description rdf:about="http://data.ign.fr/def/topo#Route"/>
                    <rdf:Description rdf:about="http://data.ign.fr/def/topo#VoieFerree"/>
                </owl:unionOf>
            </owl:Class>
        </rdfs:domain>
        <rdfs:range rdf:resource="http://www.w3.org/2001/XMLSchema#boolean"/>
        <rdfs:comment xml:lang="en">Indicates the state of an artificial topographic feature. Returns &apos;true&apos; if this entity is being built.</rdfs:comment>
        <rdfs:comment xml:lang="fr">Indique l&apos;état d&apos;une entité topographique artificielle. Renvoie &apos;vrai&apos; si cette entité est en cours de construction.</rdfs:comment>
        <rdfs:isDefinedBy rdf:resource="http://data.ign.fr/def/topo"/>
        <rdfs:label xml:lang="fr">en construction</rdfs:label>
        <rdfs:label xml:lang="en">under construction</rdfs:label>
    </owl:DatatypeProperty>
    


    <!-- http://data.ign.fr/def/topo#fictif -->


    <owl:DatatypeProperty rdf:about="http://data.ign.fr/def/topo#fictif">
        <rdfs:domain>
            <owl:Class>
                <owl:unionOf rdf:parseType="Collection">
                    <rdf:Description rdf:about="http://data.ign.fr/def/topo#CoursDEau"/>
                    <rdf:Description rdf:about="http://data.ign.fr/def/topo#Route"/>
                </owl:unionOf>
            </owl:Class>
        </rdfs:domain>
        <rdfs:range rdf:resource="http://www.w3.org/2001/XMLSchema#boolean"/>
        <rdfs:comment xml:lang="fr">La valeur &apos;oui&apos; indique que la géométrie du tronçon de réseau n&apos;est pas significative.</rdfs:comment>
        <rdfs:comment xml:lang="en">The value &apos;yes&apos; indicates that the geometry of the network section is not significant.</rdfs:comment>
        <rdfs:isDefinedBy rdf:resource="http://data.ign.fr/def/topo"/>
        <rdfs:label xml:lang="en">dummy</rdfs:label>
        <rdfs:label xml:lang="fr">fictif</rdfs:label>
    </owl:DatatypeProperty>
    


    <!-- http://data.ign.fr/def/topo#gestion -->


    <owl:DatatypeProperty rdf:about="http://data.ign.fr/def/topo#gestion">
        <rdfs:domain rdf:resource="http://data.ign.fr/def/topo#Route"/>
        <rdfs:range rdf:resource="http://www.w3.org/2001/XMLSchema#string"/>
        <rdfs:comment xml:lang="en">Defines the administrative manager of a route. All classified routes have a &apos;Manager&apos;.</rdfs:comment>
        <rdfs:comment xml:lang="fr">Définit le gestionnaire administratif d’une route. Toutes les routes classées possèdent un ‘Gestionnaire’.</rdfs:comment>
        <rdfs:isDefinedBy rdf:resource="http://data.ign.fr/def/topo"/>
        <rdfs:label xml:lang="fr">gestionnaire</rdfs:label>
        <rdfs:label xml:lang="en">manager</rdfs:label>
    </owl:DatatypeProperty>
    


    <!-- http://data.ign.fr/def/topo#hauteur -->


    <owl:DatatypeProperty rdf:about="http://data.ign.fr/def/topo#hauteur">
        <rdfs:domain rdf:resource="http://data.ign.fr/def/topo#Batiment"/>
        <rdfs:range rdf:resource="http://www.w3.org/2001/XMLSchema#integer"/>
        <rdfs:comment xml:lang="fr">Hauteur du bâtiment correspondant à la différence entre le Z le plus élevé du pourtour du bâtiment et un point situé au pied du bâtiment.</rdfs:comment>
        <rdfs:comment xml:lang="en">The height of the building corresponding to the difference between the highest Z around the building and a point at the foot of the building.</rdfs:comment>
        <rdfs:isDefinedBy rdf:resource="http://data.ign.fr/def/topo"/>
        <rdfs:label xml:lang="fr">hauteur</rdfs:label>
        <rdfs:label xml:lang="en">height</rdfs:label>
    </owl:DatatypeProperty>
    


    <!-- http://data.ign.fr/def/topo#importance -->


    <owl:DatatypeProperty rdf:about="http://data.ign.fr/def/topo#importance">
        <rdfs:domain rdf:resource="http://data.ign.fr/def/topo#EntiteTopographique"/>
        <rdfs:range>
            <rdfs:Datatype>
                <owl:oneOf>
                    <rdf:Description>
                        <rdf:type rdf:resource="http://www.w3.org/1999/02/22-rdf-syntax-ns#List"/>
                        <rdf:first>1</rdf:first>
                        <rdf:rest>
                            <rdf:Description>
                                <rdf:type rdf:resource="http://www.w3.org/1999/02/22-rdf-syntax-ns#List"/>
                                <rdf:first>2</rdf:first>
                                <rdf:rest>
                                    <rdf:Description>
                                        <rdf:type rdf:resource="http://www.w3.org/1999/02/22-rdf-syntax-ns#List"/>
                                        <rdf:first>3</rdf:first>
                                        <rdf:rest>
                                            <rdf:Description>
                                                <rdf:type rdf:resource="http://www.w3.org/1999/02/22-rdf-syntax-ns#List"/>
                                                <rdf:first>4</rdf:first>
                                                <rdf:rest>
                                                    <rdf:Description>
                                                        <rdf:type rdf:resource="http://www.w3.org/1999/02/22-rdf-syntax-ns#List"/>
                                                        <rdf:first>5</rdf:first>
                                                        <rdf:rest>
                                                            <rdf:Description>
                                                                <rdf:type rdf:resource="http://www.w3.org/1999/02/22-rdf-syntax-ns#List"/>
                                                                <rdf:first>6</rdf:first>
                                                                <rdf:rest>
                                                                    <rdf:Description>
                                                                        <rdf:type rdf:resource="http://www.w3.org/1999/02/22-rdf-syntax-ns#List"/>
                                                                        <rdf:first>7</rdf:first>
                                                                        <rdf:rest>
                                                                            <rdf:Description>
                                                                                <rdf:type rdf:resource="http://www.w3.org/1999/02/22-rdf-syntax-ns#List"/>
                                                                                <rdf:first>8</rdf:first>
                                                                                <rdf:rest>
                                                                                    <rdf:Description>
                                                                                        <rdf:type rdf:resource="http://www.w3.org/1999/02/22-rdf-syntax-ns#List"/>
                                                                                        <rdf:first>NC</rdf:first>
                                                                                        <rdf:rest>
                                                                                            <rdf:Description>
                                                                                                <rdf:type rdf:resource="http://www.w3.org/1999/02/22-rdf-syntax-ns#List"/>
                                                                                                <rdf:first>NR</rdf:first>
                                                                                                <rdf:rest rdf:resource="http://www.w3.org/1999/02/22-rdf-syntax-ns#nil"/>
                                                                                            </rdf:Description>
                                                                                        </rdf:rest>
                                                                                    </rdf:Description>
                                                                                </rdf:rest>
                                                                            </rdf:Description>
                                                                        </rdf:rest>
                                                                    </rdf:Description>
                                                                </rdf:rest>
                                                            </rdf:Description>
                                                        </rdf:rest>
                                                    </rdf:Description>
                                                </rdf:rest>
                                            </rdf:Description>
                                        </rdf:rest>
                                    </rdf:Description>
                                </rdf:rest>
                            </rdf:Description>
                        </rdf:rest>
                    </rdf:Description>
                </owl:oneOf>
            </rdfs:Datatype>
        </rdfs:range>
        <rdfs:comment xml:lang="fr">Importance du toponyme dans son environnement. Le toponyme de valeur 1 est plus important que le toponyme de valeur 2, lui-même plus important que le toponyme de valeur 3, etc.</rdfs:comment>
        <rdfs:comment xml:lang="en">Importance of the place name in its environment. The toponym of value 1 is more important than the toponym of value 2, itself more important than the toponym of value 3, etc.</rdfs:comment>
        <rdfs:isDefinedBy rdf:resource="http://data.ign.fr/def/topo"/>
        <rdfs:label xml:lang="en">importance</rdfs:label>
        <rdfs:label xml:lang="fr">importance</rdfs:label>
    </owl:DatatypeProperty>
    


    <!-- http://data.ign.fr/def/topo#itEurop -->


    <owl:DatatypeProperty rdf:about="http://data.ign.fr/def/topo#itEurop">
        <rdfs:domain rdf:resource="http://data.ign.fr/def/topo#Route"/>
        <rdfs:range rdf:resource="http://www.w3.org/2001/XMLSchema#string"/>
        <rdfs:comment xml:lang="en">European road number: a European road generally uses the motorway or national network (exceptionally departmental or unclassified).</rdfs:comment>
        <rdfs:comment xml:lang="fr">Numéro de route européenne : une route européenne emprunte en général le réseau autoroutier ou national (exceptionnellement départemental ou non classé).</rdfs:comment>
        <rdfs:isDefinedBy rdf:resource="http://data.ign.fr/def/topo"/>
        <rdfs:label xml:lang="en">european itinerary</rdfs:label>
        <rdfs:label xml:lang="fr">itinéraire européen</rdfs:label>
    </owl:DatatypeProperty>
    


    <!-- http://data.ign.fr/def/topo#itVert -->


    <owl:DatatypeProperty rdf:about="http://data.ign.fr/def/topo#itVert">
        <rdfs:domain rdf:resource="http://data.ign.fr/def/topo#Route"/>
        <rdfs:range rdf:resource="http://www.w3.org/2001/XMLSchema#boolean"/>
        <rdfs:comment xml:lang="en">Indicates whether or not a road segment belongs to the green network. The green network, made up of green poles and green links, covers the entire French territory. The green poles are made up of communes of more than 23,000 inhabitants in the province and 39,000 inhabitants in Ile-de-France, as well as certain poles of administrative, economic, tourist or industrial activities. We only remember the green transit network between green poles. The green network of drawdown, inside the cities, and the green network recommended to the trucks are not retained.</rdfs:comment>
        <rdfs:comment xml:lang="fr">Indique l’appartenance ou non d’un tronçon routier au réseau vert. Le réseau vert, composé de pôles verts et de liaisons vertes, couvre l’ensemble du territoire français. Les pôles verts sont composés de communes de plus de 23.000 habitants en province et de 39.000 habitants en Ile-de-France, ainsi que certains pôles d’activités administratifs, économiques, touristiques ou industriels. On retient seulement le réseau vert de transit entre pôles verts. Le réseau vert de rabattement, à l’intérieur des villes, et le réseau vert conseillé aux poids lourds ne sont pas retenus.</rdfs:comment>
        <rdfs:isDefinedBy rdf:resource="http://data.ign.fr/def/topo"/>
        <rdfs:label xml:lang="en">green itinerary</rdfs:label>
        <rdfs:label xml:lang="fr">itinéraire vert</rdfs:label>
    </owl:DatatypeProperty>
    


    <!-- http://data.ign.fr/def/topo#largeurChaussee -->


    <owl:DatatypeProperty rdf:about="http://data.ign.fr/def/topo#largeurChaussee">
        <rdfs:domain rdf:resource="http://data.ign.fr/def/topo#Route"/>
        <rdfs:range rdf:resource="http://www.w3.org/2001/XMLSchema#double"/>
        <rdfs:comment xml:lang="fr">Largeur de chaussée (d’accotement à accotement) exprimée en mètres.</rdfs:comment>
        <rdfs:comment xml:lang="en">Width of road (shoulder shoulders) expressed in meters.</rdfs:comment>
        <rdfs:isDefinedBy rdf:resource="http://data.ign.fr/def/topo"/>
        <rdfs:label xml:lang="en">carriageway width</rdfs:label>
        <rdfs:label xml:lang="fr">largeur de chaussée</rdfs:label>
    </owl:DatatypeProperty>
    


    <!-- http://data.ign.fr/def/topo#largeurVF -->


    <owl:DatatypeProperty rdf:about="http://data.ign.fr/def/topo#largeurVF">
        <rdfs:domain rdf:resource="http://data.ign.fr/def/topo#VoieFerree"/>
        <rdfs:range>
            <rdfs:Datatype>
                <owl:oneOf>
                    <rdf:Description>
                        <rdf:type rdf:resource="http://www.w3.org/1999/02/22-rdf-syntax-ns#List"/>
                        <rdf:first>large</rdf:first>
                        <rdf:rest>
                            <rdf:Description>
                                <rdf:type rdf:resource="http://www.w3.org/1999/02/22-rdf-syntax-ns#List"/>
                                <rdf:first>narrow</rdf:first>
                                <rdf:rest>
                                    <rdf:Description>
                                        <rdf:type rdf:resource="http://www.w3.org/1999/02/22-rdf-syntax-ns#List"/>
                                        <rdf:first>normal</rdf:first>
                                        <rdf:rest>
                                            <rdf:Description>
                                                <rdf:type rdf:resource="http://www.w3.org/1999/02/22-rdf-syntax-ns#List"/>
                                                <rdf:first>normale</rdf:first>
                                                <rdf:rest>
                                                    <rdf:Description>
                                                        <rdf:type rdf:resource="http://www.w3.org/1999/02/22-rdf-syntax-ns#List"/>
                                                        <rdf:first>étroite</rdf:first>
                                                        <rdf:rest rdf:resource="http://www.w3.org/1999/02/22-rdf-syntax-ns#nil"/>
                                                    </rdf:Description>
                                                </rdf:rest>
                                            </rdf:Description>
                                        </rdf:rest>
                                    </rdf:Description>
                                </rdf:rest>
                            </rdf:Description>
                        </rdf:rest>
                    </rdf:Description>
                </owl:oneOf>
            </rdfs:Datatype>
        </rdfs:range>
        <rdfs:comment xml:lang="fr">Attribut permettant de distinguer les voies ferrées de largeur standard (normale) pour la France (1,435 m), des voies ferrées plus larges ou plus étroites.</rdfs:comment>
        <rdfs:comment xml:lang="en">Attribute distinguishing between standard width (normal) railways for France (1.435 m), wider or narrower railways.</rdfs:comment>
        <rdfs:isDefinedBy rdf:resource="http://data.ign.fr/def/topo"/>
        <rdfs:label xml:lang="fr">largeur de la voie ferrée</rdfs:label>
        <rdfs:label xml:lang="en">railway track width</rdfs:label>
    </owl:DatatypeProperty>
    


    <!-- http://data.ign.fr/def/topo#militaire -->


    <owl:DatatypeProperty rdf:about="http://data.ign.fr/def/topo#militaire">
        <rdfs:domain>
            <owl:Class>
                <owl:unionOf rdf:parseType="Collection">
                    <rdf:Description rdf:about="http://data.ign.fr/def/topo#Cimetiere"/>
                    <owl:Restriction>
                        <owl:onProperty rdf:resource="http://data.ign.fr/def/topo#nature"/>
                        <owl:hasValue rdf:resource="http://data.ign.fr/id/codes/topo/typedezai/Aerodrome"/>
                    </owl:Restriction>
                </owl:unionOf>
            </owl:Class>
        </rdfs:domain>
        <rdfs:range rdf:resource="http://www.w3.org/2001/XMLSchema#boolean"/>
        <rdfs:comment xml:lang="fr">Attribut permettant de distinguer une entité topographique à vocation militaire ou simplement gérée par le ministère de la défense d&apos;une entité civile. La valeur « vrai » est également affectée aux cimetières militaires gérés par le Ministère des Anciens Combattants ou par des états étrangers.</rdfs:comment>
        <rdfs:comment xml:lang="en">Attribute to distinguish a topographic entity with a military purpose or simply managed by the Ministry of Defense of a civil entity. The true value is also assigned to military cemeteries operated by the Department of Veterans Affairs or foreign states.</rdfs:comment>
        <rdfs:isDefinedBy rdf:resource="http://data.ign.fr/def/topo"/>
        <rdfs:label xml:lang="fr">entité à vocation militaire</rdfs:label>
        <rdfs:label xml:lang="en">military feature</rdfs:label>
    </owl:DatatypeProperty>
    


    <!-- http://data.ign.fr/def/topo#miseEnService -->


    <owl:DatatypeProperty rdf:about="http://data.ign.fr/def/topo#miseEnService">
        <rdfs:domain rdf:resource="http://data.ign.fr/def/topo#Route"/>
        <rdfs:range rdf:resource="http://www.w3.org/2001/XMLSchema#string"/>
        <rdfs:comment xml:lang="en">Defines the planned date or effective date of bringing a section of road into service. This attribute is only filled for sections under construction, it is at &quot;NR&quot; in other cases. Sections with a date of commissioning are completely closed to vehicles before that date.</rdfs:comment>
        <rdfs:comment xml:lang="fr">Définit la date prévue ou la date effective de mise en service d’un tronçon de route. Cet attribut n&apos;est rempli que pour les tronçons en construction, il est à “NR“ dans les autres cas. Les tronçons qui possèdent une date de mise en service sont complètement fermés aux véhicules avant cette date.</rdfs:comment>
        <rdfs:isDefinedBy rdf:resource="http://data.ign.fr/def/topo"/>
        <rdfs:label xml:lang="fr">date de mise en service</rdfs:label>
        <rdfs:label xml:lang="en">in service date</rdfs:label>
    </owl:DatatypeProperty>
    


    <!-- http://data.ign.fr/def/topo#nbVoiesCirculation -->


    <owl:DatatypeProperty rdf:about="http://data.ign.fr/def/topo#nbVoiesCirculation">
        <rdfs:domain rdf:resource="http://data.ign.fr/def/topo#Route"/>
        <rdfs:range rdf:resource="http://www.w3.org/2001/XMLSchema#integer"/>
        <rdfs:comment xml:lang="fr">Nombre total de voies d’une route, d’une rue ou d’une chaussée de route à chaussées séparées.</rdfs:comment>
        <rdfs:comment xml:lang="en">Total number of lanes on a road, street or pavement with separate carriageways.</rdfs:comment>
        <rdfs:isDefinedBy rdf:resource="http://data.ign.fr/def/topo"/>
        <rdfs:label xml:lang="fr">nombre de voies de circulation</rdfs:label>
        <rdfs:label xml:lang="en">number of traffic lanes</rdfs:label>
    </owl:DatatypeProperty>
    


    <!-- http://data.ign.fr/def/topo#nbVoiesFerrees -->


    <owl:DatatypeProperty rdf:about="http://data.ign.fr/def/topo#nbVoiesFerrees">
        <rdfs:domain rdf:resource="http://data.ign.fr/def/topo#VoieFerree"/>
        <rdfs:range rdf:resource="http://www.w3.org/2001/XMLSchema#integer"/>
        <rdfs:comment xml:lang="fr">Nombre de voies constituant cette portion de ligne de chemin de fer. La valeur 0 indique que le nombre de voies est inconnu.</rdfs:comment>
        <rdfs:comment xml:lang="en">Number of lanes constituting this portion of a railway line. A value of 0 indicates that the number of channels is unknown.</rdfs:comment>
        <rdfs:isDefinedBy rdf:resource="http://data.ign.fr/def/topo"/>
        <rdfs:label xml:lang="fr">nombre de voies ferrées</rdfs:label>
        <rdfs:label xml:lang="en">number of tracks</rdfs:label>
    </owl:DatatypeProperty>
    


    <!-- http://data.ign.fr/def/topo#nomIti -->


    <owl:DatatypeProperty rdf:about="http://data.ign.fr/def/topo#nomIti">
        <rdfs:domain rdf:resource="http://data.ign.fr/def/topo#Route"/>
        <rdfs:range rdf:resource="http://www.w3.org/2001/XMLSchema#string"/>
        <rdfs:comment xml:lang="en">Define a named route.</rdfs:comment>
        <rdfs:comment xml:lang="fr">Définit un parcours routier nommé.</rdfs:comment>
        <rdfs:isDefinedBy rdf:resource="http://data.ign.fr/def/topo"/>
        <rdfs:label xml:lang="en">name of itinerary</rdfs:label>
        <rdfs:label xml:lang="fr">nom d&apos;itinéraire</rdfs:label>
    </owl:DatatypeProperty>
    


    <!-- http://data.ign.fr/def/topo#numero -->


    <owl:DatatypeProperty rdf:about="http://data.ign.fr/def/topo#numero">
        <rdfs:domain rdf:resource="http://data.ign.fr/def/topo#Route"/>
        <rdfs:range rdf:resource="http://www.w3.org/2001/XMLSchema#string"/>
        <rdfs:comment xml:lang="fr">Désigne le classement administratif d&apos;un tronçon routier.</rdfs:comment>
        <rdfs:comment xml:lang="en">Refers to the administrative classification of a road section.</rdfs:comment>
        <rdfs:isDefinedBy rdf:resource="http://data.ign.fr/def/topo"/>
        <rdfs:label xml:lang="en">number</rdfs:label>
        <rdfs:label xml:lang="fr">numéro</rdfs:label>
    </owl:DatatypeProperty>
    


    <!-- http://data.ign.fr/def/topo#numeroBorne -->


    <owl:DatatypeProperty rdf:about="http://data.ign.fr/def/topo#numeroBorne">
        <rdfs:domain rdf:resource="http://data.ign.fr/def/topo#BornePostale"/>
        <rdfs:range rdf:resource="http://www.w3.org/2001/XMLSchema#integer"/>
        <rdfs:comment xml:lang="fr">Numéro de borne postale.</rdfs:comment>
        <rdfs:comment xml:lang="en">Postal code number.</rdfs:comment>
        <rdfs:isDefinedBy rdf:resource="http://data.ign.fr/def/topo"/>
        <rdfs:label xml:lang="en">civic number</rdfs:label>
        <rdfs:label xml:lang="fr">numéro de borne postale</rdfs:label>
    </owl:DatatypeProperty>
    


    <!-- http://data.ign.fr/def/topo#posSol -->


    <owl:DatatypeProperty rdf:about="http://data.ign.fr/def/topo#posSol">
        <rdfs:domain rdf:resource="http://data.ign.fr/def/topo#Conduite"/>
        <rdfs:range rdf:resource="http://www.w3.org/2001/XMLSchema#integer"/>
        <rdfs:comment xml:lang="fr">Position par rapport au sol. Donne le niveau de l’objet par rapport à la surface du sol (valeur nulle pour un objet au sol, négative pour un objet situé au-dessous du niveau du sol et positive pour un objet en sursol).</rdfs:comment>
        <rdfs:comment xml:lang="en">Position relative to the ground. Gives the level of the object relative to the ground surface (zero value for a ground object, negative for an object below ground level and positive for an object on the ground).</rdfs:comment>
        <rdfs:isDefinedBy rdf:resource="http://data.ign.fr/def/topo"/>
        <rdfs:label xml:lang="en">position in relation to the ground</rdfs:label>
        <rdfs:label xml:lang="fr">position par rapport au sol</rdfs:label>
    </owl:DatatypeProperty>
    


    <!-- http://data.ign.fr/def/topo#precAlti -->


    <owl:DatatypeProperty rdf:about="http://data.ign.fr/def/topo#precAlti">
        <rdfs:domain rdf:resource="http://data.ign.fr/def/topo#EntiteTopographique"/>
        <rdfs:range rdf:resource="http://www.w3.org/2001/XMLSchema#double"/>
        <rdfs:comment xml:lang="en">Geometric altimetric accuracy.</rdfs:comment>
        <rdfs:comment xml:lang="fr">Précision géométrique altimétrique.</rdfs:comment>
        <rdfs:isDefinedBy rdf:resource="http://data.ign.fr/def/topo"/>
        <rdfs:label xml:lang="en">altimetric accuracy</rdfs:label>
        <rdfs:label xml:lang="fr">précision altimétrique</rdfs:label>
    </owl:DatatypeProperty>
    


    <!-- http://data.ign.fr/def/topo#precPlani -->


    <owl:DatatypeProperty rdf:about="http://data.ign.fr/def/topo#precPlani">
        <rdfs:domain rdf:resource="http://data.ign.fr/def/topo#EntiteTopographique"/>
        <rdfs:range rdf:resource="http://www.w3.org/2001/XMLSchema#double"/>
        <rdfs:comment xml:lang="en">Planimetric geometric precision.</rdfs:comment>
        <rdfs:comment xml:lang="fr">Précision géométrique planimétrique.</rdfs:comment>
        <rdfs:isDefinedBy rdf:resource="http://data.ign.fr/def/topo"/>
        <rdfs:label xml:lang="en">planimetric accuracy</rdfs:label>
        <rdfs:label xml:lang="fr">précision planimétrique</rdfs:label>
    </owl:DatatypeProperty>
    


    <!-- http://data.ign.fr/def/topo#regime -->


    <owl:DatatypeProperty rdf:about="http://data.ign.fr/def/topo#regime">
        <rdfs:domain rdf:resource="http://data.ign.fr/def/topo#CoursDEau"/>
        <rdfs:range>
            <rdfs:Datatype>
                <owl:oneOf>
                    <rdf:Description>
                        <rdf:type rdf:resource="http://www.w3.org/1999/02/22-rdf-syntax-ns#List"/>
                        <rdf:first>intermittent</rdf:first>
                        <rdf:rest>
                            <rdf:Description>
                                <rdf:type rdf:resource="http://www.w3.org/1999/02/22-rdf-syntax-ns#List"/>
                                <rdf:first>permanent</rdf:first>
                                <rdf:rest rdf:resource="http://www.w3.org/1999/02/22-rdf-syntax-ns#nil"/>
                            </rdf:Description>
                        </rdf:rest>
                    </rdf:Description>
                </owl:oneOf>
            </rdfs:Datatype>
        </rdfs:range>
        <rdfs:comment xml:lang="fr">Attribut permettant de caractériser un objet hydrographique en fonction du régime des eaux.</rdfs:comment>
        <rdfs:comment xml:lang="en">Attribute to characterize a hydrographic object according to the water regime.</rdfs:comment>
        <rdfs:isDefinedBy rdf:resource="http://data.ign.fr/def/topo"/>
        <rdfs:label xml:lang="fr">régime des eaux</rdfs:label>
        <rdfs:label xml:lang="en">water regime</rdfs:label>
    </owl:DatatypeProperty>
    


    <!-- http://data.ign.fr/def/topo#sens -->


    <owl:DatatypeProperty rdf:about="http://data.ign.fr/def/topo#sens">
        <rdfs:domain rdf:resource="http://data.ign.fr/def/topo#Route"/>
        <rdfs:range>
            <rdfs:Datatype>
                <owl:oneOf>
                    <rdf:Description>
                        <rdf:type rdf:resource="http://www.w3.org/1999/02/22-rdf-syntax-ns#List"/>
                        <rdf:first>NC</rdf:first>
                        <rdf:rest>
                            <rdf:Description>
                                <rdf:type rdf:resource="http://www.w3.org/1999/02/22-rdf-syntax-ns#List"/>
                                <rdf:first>NR</rdf:first>
                                <rdf:rest>
                                    <rdf:Description>
                                        <rdf:type rdf:resource="http://www.w3.org/1999/02/22-rdf-syntax-ns#List"/>
                                        <rdf:first>direct</rdf:first>
                                        <rdf:rest>
                                            <rdf:Description>
                                                <rdf:type rdf:resource="http://www.w3.org/1999/02/22-rdf-syntax-ns#List"/>
                                                <rdf:first>double</rdf:first>
                                                <rdf:rest>
                                                    <rdf:Description>
                                                        <rdf:type rdf:resource="http://www.w3.org/1999/02/22-rdf-syntax-ns#List"/>
                                                        <rdf:first>inverse</rdf:first>
                                                        <rdf:rest rdf:resource="http://www.w3.org/1999/02/22-rdf-syntax-ns#nil"/>
                                                    </rdf:Description>
                                                </rdf:rest>
                                            </rdf:Description>
                                        </rdf:rest>
                                    </rdf:Description>
                                </rdf:rest>
                            </rdf:Description>
                        </rdf:rest>
                    </rdf:Description>
                </owl:oneOf>
            </rdfs:Datatype>
        </rdfs:range>
        <rdfs:comment xml:lang="en">Permitted traffic direction for cars on tracks.</rdfs:comment>
        <rdfs:comment xml:lang="fr">Sens de circulation autorisée pour les automobiles sur les voies.</rdfs:comment>
        <rdfs:isDefinedBy rdf:resource="http://data.ign.fr/def/topo"/>
        <rdfs:label xml:lang="en">direction of traffic</rdfs:label>
        <rdfs:label xml:lang="fr">sens de circulation</rdfs:label>
    </owl:DatatypeProperty>
    


    <!-- http://data.ign.fr/def/topo#typAdres -->


    <owl:DatatypeProperty rdf:about="http://data.ign.fr/def/topo#typAdres">
        <rdfs:domain rdf:resource="http://data.ign.fr/def/topo#Route"/>
        <rdfs:range>
            <rdfs:Datatype>
                <owl:oneOf>
                    <rdf:Description>
                        <rdf:type rdf:resource="http://www.w3.org/1999/02/22-rdf-syntax-ns#List"/>
                        <rdf:first>NC</rdf:first>
                        <rdf:rest>
                            <rdf:Description>
                                <rdf:type rdf:resource="http://www.w3.org/1999/02/22-rdf-syntax-ns#List"/>
                                <rdf:first>NR</rdf:first>
                                <rdf:rest>
                                    <rdf:Description>
                                        <rdf:type rdf:resource="http://www.w3.org/1999/02/22-rdf-syntax-ns#List"/>
                                        <rdf:first>autre</rdf:first>
                                        <rdf:rest>
                                            <rdf:Description>
                                                <rdf:type rdf:resource="http://www.w3.org/1999/02/22-rdf-syntax-ns#List"/>
                                                <rdf:first>classique</rdf:first>
                                                <rdf:rest>
                                                    <rdf:Description>
                                                        <rdf:type rdf:resource="http://www.w3.org/1999/02/22-rdf-syntax-ns#List"/>
                                                        <rdf:first>linéaire</rdf:first>
                                                        <rdf:rest>
                                                            <rdf:Description>
                                                                <rdf:type rdf:resource="http://www.w3.org/1999/02/22-rdf-syntax-ns#List"/>
                                                                <rdf:first>métrique</rdf:first>
                                                                <rdf:rest rdf:resource="http://www.w3.org/1999/02/22-rdf-syntax-ns#nil"/>
                                                            </rdf:Description>
                                                        </rdf:rest>
                                                    </rdf:Description>
                                                </rdf:rest>
                                            </rdf:Description>
                                        </rdf:rest>
                                    </rdf:Description>
                                </rdf:rest>
                            </rdf:Description>
                        </rdf:rest>
                    </rdf:Description>
                </owl:oneOf>
            </rdfs:Datatype>
        </rdfs:range>
        <rdfs:comment xml:lang="en">Provides information on the type of addressing of the section.</rdfs:comment>
        <rdfs:comment xml:lang="fr">Renseigne sur le type d’adressage du tronçon.</rdfs:comment>
        <rdfs:isDefinedBy rdf:resource="http://data.ign.fr/def/topo"/>
        <rdfs:label xml:lang="fr">type d’adressage</rdfs:label>
        <rdfs:label xml:lang="en">type of addressing</rdfs:label>
    </owl:DatatypeProperty>
    


    <!-- http://data.ign.fr/def/topo#typeDePiste -->


    <owl:DatatypeProperty rdf:about="http://data.ign.fr/def/topo#typeDePiste">
        <rdfs:domain rdf:resource="http://data.ign.fr/def/topo#PisteAerodrome"/>
        <rdfs:range>
            <rdfs:Datatype>
                <owl:oneOf>
                    <rdf:Description>
                        <rdf:type rdf:resource="http://www.w3.org/1999/02/22-rdf-syntax-ns#List"/>
                        <rdf:first>Piste aménagée sur de l&apos;herbe</rdf:first>
                        <rdf:rest>
                            <rdf:Description>
                                <rdf:type rdf:resource="http://www.w3.org/1999/02/22-rdf-syntax-ns#List"/>
                                <rdf:first>Piste aménagée sur une surface dure</rdf:first>
                                <rdf:rest>
                                    <rdf:Description>
                                        <rdf:type rdf:resource="http://www.w3.org/1999/02/22-rdf-syntax-ns#List"/>
                                        <rdf:first>Track arranged on grass</rdf:first>
                                        <rdf:rest>
                                            <rdf:Description>
                                                <rdf:type rdf:resource="http://www.w3.org/1999/02/22-rdf-syntax-ns#List"/>
                                                <rdf:first>Track laid out on a hard surface</rdf:first>
                                                <rdf:rest rdf:resource="http://www.w3.org/1999/02/22-rdf-syntax-ns#nil"/>
                                            </rdf:Description>
                                        </rdf:rest>
                                    </rdf:Description>
                                </rdf:rest>
                            </rdf:Description>
                        </rdf:rest>
                    </rdf:Description>
                </owl:oneOf>
            </rdfs:Datatype>
        </rdfs:range>
        <rdfs:comment xml:lang="fr">Attribut permettant de distinguer différentes natures d&apos;aérodrome.</rdfs:comment>
        <rdfs:comment xml:lang="en">Attribute to distinguish different types of aerodrome.</rdfs:comment>
        <rdfs:isDefinedBy rdf:resource="http://data.ign.fr/def/topo"/>
        <rdfs:label xml:lang="fr">type de piste</rdfs:label>
        <rdfs:label xml:lang="en">type of taxiway</rdfs:label>
    </owl:DatatypeProperty>
    


    <!-- http://data.ign.fr/def/topo#voltage -->


    <owl:DatatypeProperty rdf:about="http://data.ign.fr/def/topo#voltage">
        <rdfs:domain rdf:resource="http://data.ign.fr/def/topo#LigneElectrique"/>
        <rdfs:range>
            <rdfs:Datatype>
                <owl:oneOf>
                    <rdf:Description>
                        <rdf:type rdf:resource="http://www.w3.org/1999/02/22-rdf-syntax-ns#List"/>
                        <rdf:first>150</rdf:first>
                        <rdf:rest>
                            <rdf:Description>
                                <rdf:type rdf:resource="http://www.w3.org/1999/02/22-rdf-syntax-ns#List"/>
                                <rdf:first>225</rdf:first>
                                <rdf:rest>
                                    <rdf:Description>
                                        <rdf:type rdf:resource="http://www.w3.org/1999/02/22-rdf-syntax-ns#List"/>
                                        <rdf:first>400</rdf:first>
                                        <rdf:rest>
                                            <rdf:Description>
                                                <rdf:type rdf:resource="http://www.w3.org/1999/02/22-rdf-syntax-ns#List"/>
                                                <rdf:first>63</rdf:first>
                                                <rdf:rest>
                                                    <rdf:Description>
                                                        <rdf:type rdf:resource="http://www.w3.org/1999/02/22-rdf-syntax-ns#List"/>
                                                        <rdf:first>90</rdf:first>
                                                        <rdf:rest>
                                                            <rdf:Description>
                                                                <rdf:type rdf:resource="http://www.w3.org/1999/02/22-rdf-syntax-ns#List"/>
                                                                <rdf:first>NR</rdf:first>
                                                                <rdf:rest rdf:resource="http://www.w3.org/1999/02/22-rdf-syntax-ns#nil"/>
                                                            </rdf:Description>
                                                        </rdf:rest>
                                                    </rdf:Description>
                                                </rdf:rest>
                                            </rdf:Description>
                                        </rdf:rest>
                                    </rdf:Description>
                                </rdf:rest>
                            </rdf:Description>
                        </rdf:rest>
                    </rdf:Description>
                </owl:oneOf>
            </rdfs:Datatype>
        </rdfs:range>
        <rdfs:comment xml:lang="fr">Tension de construction de la ligne électrique en kV (kilo Volts).</rdfs:comment>
        <rdfs:comment xml:lang="en">Voltage of construction of the electric line in kV (kilo volts).</rdfs:comment>
        <rdfs:isDefinedBy rdf:resource="http://data.ign.fr/def/topo"/>
        <rdfs:label xml:lang="en">voltage</rdfs:label>
        <rdfs:label xml:lang="fr">voltage</rdfs:label>
    </owl:DatatypeProperty>
    


    <!-- http://data.ign.fr/def/topo#zFin -->


    <owl:DatatypeProperty rdf:about="http://data.ign.fr/def/topo#zFin">
        <rdfs:domain>
            <owl:Class>
                <owl:intersectionOf rdf:parseType="Collection">
                    <rdf:Description rdf:about="http://data.ign.fr/def/topo#EntiteTopographique"/>
                    <owl:Restriction>
                        <owl:onProperty rdf:resource="http://data.ign.fr/def/geometrie#geometry"/>
                        <owl:someValuesFrom rdf:resource="http://data.ign.fr/def/geometrie#Curve"/>
                    </owl:Restriction>
                </owl:intersectionOf>
            </owl:Class>
        </rdfs:domain>
        <rdfs:range rdf:resource="http://www.w3.org/2001/XMLSchema#double"/>
        <rdfs:comment xml:lang="fr">Altitude du sommet final d&apos;une portion d&apos;élément linéaire d&apos;un réseau.</rdfs:comment>
        <rdfs:comment xml:lang="en">Altitude of the final peak of a linear element portion of a network.</rdfs:comment>
        <rdfs:isDefinedBy rdf:resource="http://data.ign.fr/def/topo"/>
        <rdfs:label xml:lang="en">final z</rdfs:label>
        <rdfs:label xml:lang="fr">z final</rdfs:label>
    </owl:DatatypeProperty>
    


    <!-- http://data.ign.fr/def/topo#zIni -->


    <owl:DatatypeProperty rdf:about="http://data.ign.fr/def/topo#zIni">
        <rdfs:domain>
            <owl:Class>
                <owl:intersectionOf rdf:parseType="Collection">
                    <rdf:Description rdf:about="http://data.ign.fr/def/topo#EntiteTopographique"/>
                    <owl:Restriction>
                        <owl:onProperty rdf:resource="http://data.ign.fr/def/geometrie#geometry"/>
                        <owl:someValuesFrom rdf:resource="http://data.ign.fr/def/geometrie#Curve"/>
                    </owl:Restriction>
                </owl:intersectionOf>
            </owl:Class>
        </rdfs:domain>
        <rdfs:range rdf:resource="http://www.w3.org/2001/XMLSchema#double"/>
        <rdfs:comment xml:lang="fr">Altitude du sommet initial d&apos;une portion d&apos;élément linéaire d&apos;un réseau.</rdfs:comment>
        <rdfs:comment xml:lang="en">Altitude of the initial vertex of a linear element portion of a network.</rdfs:comment>
        <rdfs:isDefinedBy rdf:resource="http://data.ign.fr/def/topo"/>
        <rdfs:label xml:lang="en">initial z</rdfs:label>
        <rdfs:label xml:lang="fr">z initial</rdfs:label>
    </owl:DatatypeProperty>
    


    <!-- http://data.ign.fr/def/topo#zMax -->


    <owl:DatatypeProperty rdf:about="http://data.ign.fr/def/topo#zMax">
        <rdfs:domain rdf:resource="http://data.ign.fr/def/topo#EntiteTopographique"/>
        <rdfs:range rdf:resource="http://www.w3.org/2001/XMLSchema#double"/>
        <rdfs:comment xml:lang="fr">Altitude maximale d’un objet linéaire ou surfacique. Cette information est issue de la saisie photogrammétrique et concerne des objets dont les points initiaux et finaux ne sont pas caractéristiques de l’altitude de l’objet (objets surfaciques, objets linéaires isolés). Pour des objets surfaciques comme les bâtiments ou les réservoirs, il s’agit de l’altitude maximum du pourtour tel qu’il est défini en planimétrie (généralement l’altitude aux gouttières) et non de l’altitude maximum absolue (voir schéma ci-dessus). Dans le cas d’un bâtiment obtenu après intégration du bâti issu du cadastre, Z_MAX correspond à une altitude toit médiane calculée, en prenant en compte les altitudes des contours des bâtiments directement contigus s’ils existent. Dans ce cas Z_MAX et Z_MIN prennent la même valeur. L’attribut peut prendre une valeur conventionnelle (9999) lorsque la géométrie de l’objet n’est pas issue d’une saisie photogrammétrique (ex. objets numérisés sur la carte en service). </rdfs:comment>
        <rdfs:comment xml:lang="en">Maximum altitude of a linear or polygon object. This information comes from the photogrammetric input and concerns objects whose initial and final points are not characteristic of the altitude of the object (surface objects, isolated linear objects). For areal objects such as buildings or reservoirs, this is the maximum altitude of the circumference as it is defined in planimetry (usually the altitude at the gutters) and not the absolute maximum altitude (see diagram below). -above). In the case of a building obtained after integration of the frame from the cadastre, Z_MAX corresponds to a computed median roof altitude, taking into account the altitudes of the outlines of buildings directly adjacent if they exist. In this case Z_MAX and Z_MIN take the same value. The attribute can take a conventional value (9999) when the geometry of the object is not the result of a photogrammetric capture (eg objects scanned on the map in use).</rdfs:comment>
        <rdfs:isDefinedBy rdf:resource="http://data.ign.fr/def/topo"/>
        <rdfs:label xml:lang="en">max z</rdfs:label>
        <rdfs:label xml:lang="fr">z max</rdfs:label>
    </owl:DatatypeProperty>
    


    <!-- http://data.ign.fr/def/topo#zMin -->


    <owl:DatatypeProperty rdf:about="http://data.ign.fr/def/topo#zMin">
        <rdfs:domain rdf:resource="http://data.ign.fr/def/topo#EntiteTopographique"/>
        <rdfs:range rdf:resource="http://www.w3.org/2001/XMLSchema#double"/>
        <rdfs:comment xml:lang="fr">Altitude minimale d’un objet linéaire ou surfacique. Cette information est issue de la saisie photogrammétrique et concerne des objets dont les points initiaux et finaux ne sont pas caractéristiques de l’altitude de l’objet (objets surfaciques, objets linéaires isolés). Pour des objets surfaciques comme les bâtiments ou les réservoirs, il s’agit de l’altitude minimum du pourtour tel qu’il est défini en planimétrie (généralement l’altitude aux gouttières) et non de l’altitude minimum absolue. Dans le cas d’un bâtiment obtenu après intégration du bâti issu du cadastre, Z_MIN correspond à une altitude toit médiane calculée, en prenant en compte les altitudes des contours des bâtiments directement contigus s’ils existent. Dans ce cas Z_MAX et Z_MIN prennent la même valeur. L’attribut peut prendre une valeur conventionnelle (9999) lorsque la géométrie de l’objet n’est pas issue d’une saisie photogrammétrique (ex. objets numérisés sur la carte en service).</rdfs:comment>
        <rdfs:comment xml:lang="en">Minimum altitude of a linear or polygon object. This information comes from the photogrammetric input and concerns objects whose initial and final points are not characteristic of the altitude of the object (surface objects, isolated linear objects). For areal objects such as buildings or reservoirs, this is the minimum altitude of the perimeter as defined in planimetry (usually the elevation at the gutters) and not the absolute minimum altitude. In the case of a building obtained after integration of the frame from the cadastre, Z_MIN corresponds to a computed median roof altitude, taking into account the altitudes of the outlines of buildings directly contiguous if they exist. In this case Z_MAX and Z_MIN take the same value. The attribute can take a conventional value (9999) when the geometry of the object is not the result of a photogrammetric capture (eg objects scanned on the map in use).</rdfs:comment>
        <rdfs:isDefinedBy rdf:resource="http://data.ign.fr/def/topo"/>
        <rdfs:label xml:lang="en">min z</rdfs:label>
        <rdfs:label xml:lang="fr">z min</rdfs:label>
    </owl:DatatypeProperty>
    


    <!-- http://data.ign.fr/def/topo#zMoyen -->


    <owl:DatatypeProperty rdf:about="http://data.ign.fr/def/topo#zMoyen">
        <rdfs:domain rdf:resource="http://data.ign.fr/def/topo#EntiteTopographique"/>
        <rdfs:range rdf:resource="http://www.w3.org/2001/XMLSchema#double"/>
        <rdfs:comment xml:lang="fr">Altitude moyenne des points composants la géométrie de l’objet telle qu’il a été saisi à l’origine lorsqu’il est issu d’une saisie photogrammétrique. L’attribut peut prendre une valeur conventionnelle (9999) lorsque la géométrie de l’objet n’est pas issue d’une saisie photogrammétrique (ex. objets numérisés sur la carte en service).</rdfs:comment>
        <rdfs:comment xml:lang="en">Average altitude of the points that make up the geometry of the object as it was originally entered when it came from a photogrammetric capture. The attribute can take a conventional value (9999) when the geometry of the object is not the result of a photogrammetric capture (eg objects scanned on the map in use).</rdfs:comment>
        <rdfs:isDefinedBy rdf:resource="http://data.ign.fr/def/topo"/>
        <rdfs:label xml:lang="en">average z</rdfs:label>
        <rdfs:label xml:lang="fr">z moyen</rdfs:label>
    </owl:DatatypeProperty>
    


    <!-- http://purl.org/dc/terms/alternative -->


    <rdf:Description rdf:about="http://purl.org/dc/terms/alternative">
        <rdfs:subPropertyOf rdf:resource="http://purl.org/dc/terms/title"/>
        <rdfs:range rdf:resource="http://www.w3.org/2000/01/rdf-schema#Literal"/>
    </rdf:Description>
    


    <!-- http://purl.org/dc/terms/available -->


    <rdf:Description rdf:about="http://purl.org/dc/terms/available">
        <rdfs:subPropertyOf rdf:resource="http://purl.org/dc/terms/date"/>
        <rdfs:range rdf:resource="http://www.w3.org/2000/01/rdf-schema#Literal"/>
    </rdf:Description>
    


    <!-- http://purl.org/dc/terms/bibliographicCitation -->


    <rdf:Description rdf:about="http://purl.org/dc/terms/bibliographicCitation">
        <rdfs:subPropertyOf rdf:resource="http://purl.org/dc/terms/identifier"/>
        <rdfs:range rdf:resource="http://www.w3.org/2000/01/rdf-schema#Literal"/>
    </rdf:Description>
    


    <!-- http://purl.org/dc/terms/created -->


    <rdf:Description rdf:about="http://purl.org/dc/terms/created">
        <rdfs:subPropertyOf rdf:resource="http://purl.org/dc/terms/date"/>
        <rdfs:range rdf:resource="http://www.w3.org/2000/01/rdf-schema#Literal"/>
    </rdf:Description>
    


    <!-- http://purl.org/dc/terms/date -->


    <rdf:Description rdf:about="http://purl.org/dc/terms/date">
        <rdfs:range rdf:resource="http://www.w3.org/2000/01/rdf-schema#Literal"/>
    </rdf:Description>
    


    <!-- http://purl.org/dc/terms/dateAccepted -->


    <rdf:Description rdf:about="http://purl.org/dc/terms/dateAccepted">
        <rdfs:subPropertyOf rdf:resource="http://purl.org/dc/terms/date"/>
        <rdfs:range rdf:resource="http://www.w3.org/2000/01/rdf-schema#Literal"/>
    </rdf:Description>
    


    <!-- http://purl.org/dc/terms/dateCopyrighted -->


    <rdf:Description rdf:about="http://purl.org/dc/terms/dateCopyrighted">
        <rdfs:subPropertyOf rdf:resource="http://purl.org/dc/terms/date"/>
        <rdfs:range rdf:resource="http://www.w3.org/2000/01/rdf-schema#Literal"/>
    </rdf:Description>
    


    <!-- http://purl.org/dc/terms/dateSubmitted -->


    <rdf:Description rdf:about="http://purl.org/dc/terms/dateSubmitted">
        <rdfs:subPropertyOf rdf:resource="http://purl.org/dc/terms/date"/>
        <rdfs:range rdf:resource="http://www.w3.org/2000/01/rdf-schema#Literal"/>
    </rdf:Description>
    


    <!-- http://purl.org/dc/terms/identifier -->


    <rdf:Description rdf:about="http://purl.org/dc/terms/identifier">
        <rdfs:range rdf:resource="http://www.w3.org/2000/01/rdf-schema#Literal"/>
    </rdf:Description>
    


    <!-- http://purl.org/dc/terms/issued -->


    <rdf:Description rdf:about="http://purl.org/dc/terms/issued">
        <rdfs:subPropertyOf rdf:resource="http://purl.org/dc/terms/date"/>
        <rdfs:range rdf:resource="http://www.w3.org/2000/01/rdf-schema#Literal"/>
    </rdf:Description>
    


    <!-- http://purl.org/dc/terms/modified -->


    <rdf:Description rdf:about="http://purl.org/dc/terms/modified">
        <rdfs:subPropertyOf rdf:resource="http://purl.org/dc/terms/date"/>
        <rdfs:range rdf:resource="http://www.w3.org/2000/01/rdf-schema#Literal"/>
    </rdf:Description>
    


    <!-- http://purl.org/dc/terms/title -->


    <rdf:Description rdf:about="http://purl.org/dc/terms/title">
        <rdfs:range rdf:resource="http://www.w3.org/2000/01/rdf-schema#Literal"/>
    </rdf:Description>
    


    <!-- http://purl.org/dc/terms/valid -->


    <rdf:Description rdf:about="http://purl.org/dc/terms/valid">
        <rdfs:subPropertyOf rdf:resource="http://purl.org/dc/terms/date"/>
        <rdfs:range rdf:resource="http://www.w3.org/2000/01/rdf-schema#Literal"/>
    </rdf:Description>
    


    <!-- http://www.w3.org/2004/02/skos/core#notation -->


    <owl:DatatypeProperty rdf:about="http://www.w3.org/2004/02/skos/core#notation">
        <rdfs:isDefinedBy rdf:resource="http://www.w3.org/2004/02/skos/core"/>
        <rdfs:label xml:lang="en">notation</rdfs:label>
        <skos:definition xml:lang="en">A notation, also known as classification code, is a string of characters such as &quot;T58.5&quot; or &quot;303.4833&quot; used to uniquely identify a concept within the scope of a given concept scheme.</skos:definition>
        <skos:scopeNote xml:lang="en">By convention, skos:notation is used with a typed literal in the object position of the triple.</skos:scopeNote>
    </owl:DatatypeProperty>
    


    <!-- http://www.w3.org/ns/dcat#bbox -->


    <owl:DatatypeProperty rdf:about="http://www.w3.org/ns/dcat#bbox">
        <rdfs:domain rdf:resource="http://purl.org/dc/terms/Location"/>
        <rdfs:range rdf:resource="http://www.w3.org/2000/01/rdf-schema#Literal"/>
        <rdfs:comment xml:lang="da">Den geografiske omskrevne firkant af en ressource.</rdfs:comment>
        <rdfs:comment xml:lang="es">El cuadro delimitador geográfico para un recurso.</rdfs:comment>
        <rdfs:comment xml:lang="it">Il riquadro di delimitazione geografica di una risorsa.</rdfs:comment>
        <rdfs:comment xml:lang="cs">Ohraničení geografické oblasti zdroje.</rdfs:comment>
        <rdfs:comment xml:lang="en">The geographic bounding box of a spatial thing [SDW-BP].</rdfs:comment>
        <rdfs:isDefinedBy rdf:resource="https://www.w3.org/TR/vocab-dcat-2/"/>
        <rdfs:label xml:lang="da">bounding box</rdfs:label>
        <rdfs:label xml:lang="en">bounding box</rdfs:label>
        <rdfs:label xml:lang="es">cuadro delimitador</rdfs:label>
        <rdfs:label xml:lang="cs">ohraničení oblasti</rdfs:label>
        <rdfs:label xml:lang="it">quadro di delimitazione</rdfs:label>
        <skos:changeNote xml:lang="en">New property added in DCAT 2.</skos:changeNote>
        <skos:changeNote xml:lang="cs">Nová vlastnost přidaná ve verzi DCAT 2.</skos:changeNote>
        <skos:changeNote xml:lang="it">Nuova proprietà aggiunta in DCAT 2.</skos:changeNote>
        <skos:changeNote xml:lang="da">Ny egenskab tilføjet i DCAT 2.</skos:changeNote>
        <skos:changeNote xml:lang="es">Propiedad nueva agregada en DCAT 2.</skos:changeNote>
        <skos:definition xml:lang="da">Den geografiske omskrevne firkant af en ressource.</skos:definition>
        <skos:definition xml:lang="es">El cuadro delimitador geográfico para un recurso.</skos:definition>
        <skos:definition xml:lang="it">Il riquadro di delimitazione geografica di una risorsa.</skos:definition>
        <skos:definition xml:lang="cs">Ohraničení geografické oblasti zdroje.</skos:definition>
        <skos:definition xml:lang="en">The geographic bounding box of a spatial thing [SDW-BP].</skos:definition>
        <skos:editorialNote xml:lang="en">English language definitions and comments updated in this revision in line with ED. Multilingual text unevenly updated.</skos:editorialNote>
        <skos:scopeNote xml:lang="es">El rango de esta propiedad es intencionalmente genérico con el propósito de permitir distintas codificaciones geométricas. Por ejemplo, la geometría puede ser codificada como WKT (geosparql:wktLiteral [GeoSPARQL]) o [GML] (geosparql:asGML [GeoSPARQL]).</skos:scopeNote>
        <skos:scopeNote xml:lang="it">Il range di questa proprietà (rdfs:Literal) è volutamente generica, con lo scopo di consentire diverse codifiche geometriche letterali. Ad esempio, la geometria potrebbe essere codificata con un letterale WKT (geosparql:wktLiteral [GeoSPARQL]) o [GML] (geosparql:asGML [GeoSPARQL]).</skos:scopeNote>
        <skos:scopeNote xml:lang="cs">Obor hodnot této vlastnosti je úmyslně obecný, aby umožnil různé kódování geometrií. Geometrie by kupříkladu mohla být kódována jako WKT (geosparql:wktLiteral [GeoSPARQL]) či [GML] (geosparql:asGML [GeoSPARQL]).</skos:scopeNote>
        <skos:scopeNote xml:lang="da">Rækkevidden for denne egenskab er bevidst generisk defineret med det formål at tillade forskellige kodninger af geometrier. Geometrien kan eksempelvis repræsenteres som WKT (geosparql:asWKT [GeoSPARQL]) eller [GML] (geosparql:asGML [GeoSPARQL]).</skos:scopeNote>
        <skos:scopeNote xml:lang="en">The range of this property (rdfs:Literal) is intentionally generic, with the purpose of allowing different geometry literal encodings. E.g., the geometry could be encoded as a WKT literal (geosparql:wktLiteral [GeoSPARQL]).</skos:scopeNote>
    </owl:DatatypeProperty>
    


    <!-- http://www.w3.org/ns/dcat#byteSize -->


    <owl:DatatypeProperty rdf:about="http://www.w3.org/ns/dcat#byteSize">
        <rdfs:domain rdf:resource="http://www.w3.org/ns/dcat#Distribution"/>
        <rdfs:range rdf:resource="http://www.w3.org/2000/01/rdf-schema#Literal"/>
        <rdfs:comment xml:lang="es">El tamaño de una distribución en bytes.</rdfs:comment>
        <rdfs:comment xml:lang="it">La dimensione di una distribuzione in byte.</rdfs:comment>
        <rdfs:comment xml:lang="fr">La taille de la distribution en octects</rdfs:comment>
        <rdfs:comment xml:lang="da">Størrelsen af en distributionen angivet i bytes.</rdfs:comment>
        <rdfs:comment xml:lang="en">The size of a distribution in bytes.</rdfs:comment>
        <rdfs:comment xml:lang="cs">Velikost distribuce v bajtech.</rdfs:comment>
        <rdfs:comment xml:lang="el">Το μέγεθος μιας διανομής σε bytes.</rdfs:comment>
        <rdfs:comment xml:lang="ar">الحجم بالبايتات </rdfs:comment>
        <rdfs:comment xml:lang="ja">バイトによる配信のサイズ。</rdfs:comment>
        <rdfs:isDefinedBy rdf:resource="http://www.w3.org/TR/vocab-dcat/"/>
        <rdfs:label xml:lang="en">byte size</rdfs:label>
        <rdfs:label xml:lang="da">bytestørrelse</rdfs:label>
        <rdfs:label xml:lang="it">dimensione in byte</rdfs:label>
        <rdfs:label xml:lang="fr">taille en octects</rdfs:label>
        <rdfs:label xml:lang="es">tamaño en bytes</rdfs:label>
        <rdfs:label xml:lang="cs">velikost v bajtech</rdfs:label>
        <rdfs:label xml:lang="el">μέγεθος σε bytes</rdfs:label>
        <rdfs:label xml:lang="ar">الحجم بالبايت</rdfs:label>
        <rdfs:label xml:lang="ja">バイト・サイズ</rdfs:label>
        <skos:definition xml:lang="es">El tamaño de una distribución en bytes.</skos:definition>
        <skos:definition xml:lang="it">La dimensione di una distribuzione in byte.</skos:definition>
        <skos:definition xml:lang="fr">La taille de la distribution en octects.</skos:definition>
        <skos:definition xml:lang="da">Størrelsen af en distribution angivet i bytes.</skos:definition>
        <skos:definition xml:lang="en">The size of a distribution in bytes.</skos:definition>
        <skos:definition xml:lang="cs">Velikost distribuce v bajtech.</skos:definition>
        <skos:definition xml:lang="el">Το μέγεθος μιας διανομής σε bytes.</skos:definition>
        <skos:definition xml:lang="ar">الحجم بالبايتات </skos:definition>
        <skos:definition xml:lang="ja">バイトによる配信のサイズ。</skos:definition>
        <skos:scopeNote xml:lang="da">Bytestørrelsen kan approximeres hvis den præcise størrelse ikke er kendt. Værdien af dcat:byteSize bør angives som xsd:decimal.</skos:scopeNote>
        <skos:scopeNote xml:lang="es">El tamaño en bytes puede ser aproximado cuando se desconoce el tamaño exacto. El valor literal de dcat:byteSize debe tener tipo &apos;xsd:decimal&apos;.</skos:scopeNote>
        <skos:scopeNote xml:lang="it">La dimensione in byte può essere approssimata quando non si conosce la dimensione precisa. Il valore di dcat:byteSize dovrebbe essere espresso come un xsd:decimal.</skos:scopeNote>
        <skos:scopeNote xml:lang="fr">La taille en octects peut être approximative lorsque l&apos;on ignore la taille réelle. La valeur littérale de dcat:byteSize doit être de type xsd:decimal.</skos:scopeNote>
        <skos:scopeNote xml:lang="en">The size in bytes can be approximated when the precise size is not known. The literal value of dcat:byteSize should by typed as xsd:decimal.</skos:scopeNote>
        <skos:scopeNote xml:lang="cs">Velikost v bajtech může být přibližná, pokud její přesná hodnota není známa. Literál s hodnotou dcat:byteSize by měl mít datový typ xsd:decimal.</skos:scopeNote>
        <skos:scopeNote xml:lang="el">Το μέγεθος σε bytes μπορεί να προσεγγιστεί όταν η ακριβής τιμή δεν είναι γνωστή. Η τιμή της dcat:byteSize θα πρέπει να δίνεται με τύπο δεδομένων xsd:decimal.</skos:scopeNote>
        <skos:scopeNote xml:lang="ar">الحجم يمكن أن يكون تقريبي إذا كان الحجم الدقيق غير معروف</skos:scopeNote>
        <skos:scopeNote xml:lang="ja">正確なサイズが不明である場合、サイズは、バイトによる近似値を示すことができます。</skos:scopeNote>
    </owl:DatatypeProperty>
    


    <!-- http://www.w3.org/ns/dcat#centroid -->


    <owl:DatatypeProperty rdf:about="http://www.w3.org/ns/dcat#centroid">
        <rdfs:domain rdf:resource="http://purl.org/dc/terms/Location"/>
        <rdfs:range rdf:resource="http://www.w3.org/2000/01/rdf-schema#Literal"/>
        <rdfs:comment xml:lang="da">Det geometrisk tyngdepunkt (centroid) for en ressource.</rdfs:comment>
        <rdfs:comment xml:lang="es">El centro geográfico (centroide) de un recurso.</rdfs:comment>
        <rdfs:comment xml:lang="cs">Geografický střed (centroid) zdroje.</rdfs:comment>
        <rdfs:comment xml:lang="it">Il centro geografico (centroide) di una risorsa.</rdfs:comment>
        <rdfs:comment xml:lang="en">The geographic center (centroid) of a spatial thing [SDW-BP].</rdfs:comment>
        <rdfs:isDefinedBy rdf:resource="https://www.w3.org/TR/vocab-dcat-2/"/>
        <rdfs:label xml:lang="cs">centroid</rdfs:label>
        <rdfs:label xml:lang="en">centroid</rdfs:label>
        <rdfs:label xml:lang="es">centroide</rdfs:label>
        <rdfs:label xml:lang="it">centroide</rdfs:label>
        <rdfs:label xml:lang="da">geometrisk tyngdepunkt</rdfs:label>
        <skos:altLabel xml:lang="da">centroide</skos:altLabel>
        <skos:changeNote xml:lang="en">New property added in DCAT 2.</skos:changeNote>
        <skos:changeNote xml:lang="cs">Nová vlastnost přidaná ve verzi DCAT 2.</skos:changeNote>
        <skos:changeNote xml:lang="es">Nueva propiedad agregada en DCAT 2.</skos:changeNote>
        <skos:changeNote xml:lang="it">Nuova proprietà aggiunta in DCAT 2.</skos:changeNote>
        <skos:changeNote xml:lang="da">Ny egenskab tilføjet i DCAT 2.</skos:changeNote>
        <skos:definition xml:lang="da">Det geometrisk tyngdepunkt (centroid) for en ressource.</skos:definition>
        <skos:definition xml:lang="es">El centro geográfico (centroide) de un recurso.</skos:definition>
        <skos:definition xml:lang="cs">Geografický střed (centroid) zdroje.</skos:definition>
        <skos:definition xml:lang="it">Il centro geografico (centroide) di una risorsa.</skos:definition>
        <skos:definition xml:lang="en">The geographic center (centroid) of a spatial thing [SDW-BP].</skos:definition>
        <skos:editorialNote xml:lang="en">English language definitions and comments updated in this revision in line with ED. Multilingual text unevenly updated.</skos:editorialNote>
        <skos:scopeNote xml:lang="es">El rango de esta propiedad es intencionalmente genérico con el objetivo de permitir distintas codificaciones geométricas. Por ejemplo, la geometría puede codificarse como WKT (geosparql:wktLiteral [GeoSPARQL]) o [GML] (geosparql:asGML [GeoSPARQL]).</skos:scopeNote>
        <skos:scopeNote xml:lang="it">Il range di questa proprietà (rdfs:Literal) è volutamente generica, con lo scopo di consentire diverse codifiche geometriche letterali. Ad esempio, la geometria potrebbe essere codificata con un letterale WKT (geosparql:wktLiteral [GeoSPARQL]) o [GML] (geosparql:asGML [GeoSPARQL]).</skos:scopeNote>
        <skos:scopeNote xml:lang="cs">Obor hodnot této vlastnosti je úmyslně obecný, aby umožnil různé kódování geometrií. Geometrie by kupříkladu mohla být kódována jako WKT (geosparql:wktLiteral [GeoSPARQL]) či [GML] (geosparql:asGML [GeoSPARQL]).</skos:scopeNote>
        <skos:scopeNote xml:lang="da">Rækkevidden for denne egenskab er bevidst generisk definere med det formål at tillade forskellige geokodninger. Geometrien kan eksempelvis repræsenteres som WKT (geosparql:asWKT [GeoSPARQL]) eller [GML] (geosparql:asGML [GeoSPARQL]).</skos:scopeNote>
        <skos:scopeNote xml:lang="en">The range of this property (rdfs:Literal) is intentionally generic, with the purpose of allowing different geometry literal encodings. E.g., the geometry could be encoded as a WKT literal (geosparql:wktLiteral [GeoSPARQL]).</skos:scopeNote>
    </owl:DatatypeProperty>
    


    <!-- http://www.w3.org/ns/dcat#endDate -->


    <owl:DatatypeProperty rdf:about="http://www.w3.org/ns/dcat#endDate">
        <rdfs:domain rdf:resource="http://purl.org/dc/terms/PeriodOfTime"/>
        <rdfs:range rdf:resource="http://www.w3.org/2000/01/rdf-schema#Literal"/>
        <rdfs:comment xml:lang="es">El fin del período.</rdfs:comment>
        <rdfs:comment xml:lang="cs">Konec doby trvání.</rdfs:comment>
        <rdfs:comment xml:lang="it">La fine del periodo.</rdfs:comment>
        <rdfs:comment xml:lang="da">Slutningen på perioden.</rdfs:comment>
        <rdfs:comment xml:lang="en">The end of the period.</rdfs:comment>
        <rdfs:isDefinedBy rdf:resource="https://www.w3.org/TR/vocab-dcat-2/"/>
        <rdfs:label xml:lang="it">data di fine</rdfs:label>
        <rdfs:label xml:lang="cs">datum konce</rdfs:label>
        <rdfs:label xml:lang="en">end date</rdfs:label>
        <rdfs:label xml:lang="es">fecha final</rdfs:label>
        <rdfs:label xml:lang="da">slutdato</rdfs:label>
        <skos:altLabel xml:lang="da">sluttidspunkt</skos:altLabel>
        <skos:changeNote xml:lang="en">New property added in DCAT 2.</skos:changeNote>
        <skos:changeNote xml:lang="cs">Nová vlastnost přidaná ve verzi DCAT 2.</skos:changeNote>
        <skos:changeNote xml:lang="es">Nueva propiedad agregada en DCAT 2.</skos:changeNote>
        <skos:changeNote xml:lang="it">Nuova proprietà aggiunta in DCAT 2.</skos:changeNote>
        <skos:changeNote xml:lang="da">Ny egenskab i DCAT 2.</skos:changeNote>
        <skos:definition xml:lang="es">El fin del período.</skos:definition>
        <skos:definition xml:lang="cs">Konec doby trvání.</skos:definition>
        <skos:definition xml:lang="it">La fine del periodo.</skos:definition>
        <skos:definition xml:lang="da">Slutningen på perioden.</skos:definition>
        <skos:definition xml:lang="en">The end of the period.</skos:definition>
        <skos:scopeNote xml:lang="es">El rango de esta propiedad es intencionalmente genérico con el propósito de permitir distintos niveles de precisión temporal para especificar el fin del período. Por ejemplo, puede expresarse como una fecha (xsd:date), una fecha y un tiempo (xsd:dateTime), o un año (xsd:gYear).</skos:scopeNote>
        <skos:scopeNote xml:lang="it">La range di questa proprietà è volutamente generico, con lo scopo di consentire diversi livelli di precisione temporale per specificare la fine di un periodo. Ad esempio, può essere espresso con una data (xsd:date), una data e un&apos;ora (xsd:dateTime), o un anno (xsd:gYear).</skos:scopeNote>
        <skos:scopeNote xml:lang="cs">Obor hodnot této vlastnosti je úmyslně obecný, aby umožnil různé úrovně časového rozlišení pro specifikaci konce doby trvání. Ten může být kupříkladu vyjádřen datumem (xsd:date), datumem a časem (xsd:dateTime) či rokem (xsd:gYear).</skos:scopeNote>
        <skos:scopeNote xml:lang="da">Rækkeviden for denne egenskab er bevidst generisk defineret med det formål at tillade forskellige niveauer af tidslig præcision ifm. angivelse af slutdatoen for en periode. Den kan eksempelvis udtrykkes som en dato (xsd:date), en dato og et tidspunkt (xsd:dateTime), eller et årstal (xsd:gYear).</skos:scopeNote>
        <skos:scopeNote xml:lang="en">The range of this property is intentionally generic, with the purpose of allowing different level of temporal precision for specifying the end of a period. E.g., it can be expressed with a date (xsd:date), a date and time (xsd:dateTime), or a year (xsd:gYear).</skos:scopeNote>
    </owl:DatatypeProperty>
    


    <!-- http://www.w3.org/ns/dcat#keyword -->


    <owl:DatatypeProperty rdf:about="http://www.w3.org/ns/dcat#keyword">
        <rdfs:range rdf:resource="http://www.w3.org/2000/01/rdf-schema#Literal"/>
        <rdfs:comment xml:lang="en">A keyword or tag describing a resource.</rdfs:comment>
        <rdfs:comment xml:lang="da">Et nøgleord eller tag til beskrivelse af en ressource.</rdfs:comment>
        <rdfs:comment xml:lang="cs">Klíčové slovo nebo značka popisující zdroj.</rdfs:comment>
        <rdfs:comment xml:lang="fr">Un mot-clé ou étiquette décrivant une ressource.</rdfs:comment>
        <rdfs:comment xml:lang="es">Una palabra clave o etiqueta que describe un recurso.</rdfs:comment>
        <rdfs:comment xml:lang="it">Una parola chiave o un&apos;etichetta per descrivere la risorsa.</rdfs:comment>
        <rdfs:comment xml:lang="el">Μία λέξη-κλειδί ή μία ετικέτα που περιγράφει το σύνολο δεδομένων.</rdfs:comment>
        <rdfs:comment xml:lang="ar">كلمة  مفتاحيه توصف قائمة البيانات</rdfs:comment>
        <rdfs:comment xml:lang="ja">データセットを記述しているキーワードまたはタグ。</rdfs:comment>
        <rdfs:isDefinedBy rdf:resource="http://www.w3.org/TR/vocab-dcat/"/>
        <rdfs:label xml:lang="en">keyword</rdfs:label>
        <rdfs:label xml:lang="cs">klíčové slovo</rdfs:label>
        <rdfs:label xml:lang="fr">mot-clés </rdfs:label>
        <rdfs:label xml:lang="da">nøgleord</rdfs:label>
        <rdfs:label xml:lang="es">palabra clave</rdfs:label>
        <rdfs:label xml:lang="it">parola chiave</rdfs:label>
        <rdfs:label xml:lang="el">λέξη-κλειδί</rdfs:label>
        <rdfs:label xml:lang="ar">كلمة  مفتاحية </rdfs:label>
        <rdfs:label xml:lang="ja">キーワード/タグ</rdfs:label>
        <skos:definition xml:lang="en">A keyword or tag describing a resource.</skos:definition>
        <skos:definition xml:lang="da">Et nøgleord eller tag til beskrivelse af en ressource.</skos:definition>
        <skos:definition xml:lang="cs">Klíčové slovo nebo značka popisující zdroj.</skos:definition>
        <skos:definition xml:lang="fr">Un mot-clé ou étiquette décrivant une ressource.</skos:definition>
        <skos:definition xml:lang="es">Una palabra clave o etiqueta que describe un recurso.</skos:definition>
        <skos:definition xml:lang="it">Una parola chiave o un&apos;etichetta per descrivere la risorsa.</skos:definition>
        <skos:definition xml:lang="el">Μία λέξη-κλειδί ή μία ετικέτα που περιγράφει το σύνολο δεδομένων.</skos:definition>
        <skos:definition xml:lang="ar">كلمة  مفتاحيه توصف قائمة البيانات</skos:definition>
        <skos:definition xml:lang="ja">データセットを記述しているキーワードまたはタグ。</skos:definition>
    </owl:DatatypeProperty>
    


    <!-- http://www.w3.org/ns/dcat#spatialResolutionInMeters -->


    <owl:DatatypeProperty rdf:about="http://www.w3.org/ns/dcat#spatialResolutionInMeters">
        <rdfs:range rdf:resource="http://www.w3.org/2001/XMLSchema#decimal"/>
        <rdfs:comment xml:lang="da">mindste geografiske afstand som kan erkendes i et datasæt, målt i meter.</rdfs:comment>
        <rdfs:comment xml:lang="en-us">minimum spatial separation resolvable in a dataset, measured in meters.</rdfs:comment>
        <rdfs:comment xml:lang="en-gb">minimum spatial separation resolvable in a dataset, measured in metres.</rdfs:comment>
        <rdfs:comment xml:lang="cs">minimální prostorový rozestup rozeznatelný v datové sadě, měřeno v metrech.</rdfs:comment>
        <rdfs:comment xml:lang="es">mínima separacíon espacial disponible en un conjunto de datos, medida en metros.</rdfs:comment>
        <rdfs:comment xml:lang="it">separazione spaziale minima risolvibile in un set di dati, misurata in metri.</rdfs:comment>
        <rdfs:isDefinedBy rdf:resource="https://www.w3.org/TR/vocab-dcat-2/"/>
        <rdfs:label xml:lang="da">geografisk opløsning (meter)</rdfs:label>
        <rdfs:label xml:lang="cs">prostorové rozlišení (metry)</rdfs:label>
        <rdfs:label xml:lang="es">resolución espacial (metros)</rdfs:label>
        <rdfs:label xml:lang="it">risoluzione spaziale (metri)</rdfs:label>
        <rdfs:label xml:lang="en-us">spatial resolution (meters)</rdfs:label>
        <rdfs:label xml:lang="en-gb">spatial resolution (metres)</rdfs:label>
        <skos:changeNote xml:lang="en">New property added in DCAT 2.</skos:changeNote>
        <skos:changeNote xml:lang="cs">Nová vlastnost přidaná ve verzi DCAT 2.</skos:changeNote>
        <skos:changeNote xml:lang="es">Nueva propiedad añadida en DCAT 2.</skos:changeNote>
        <skos:changeNote xml:lang="it">Nuova proprietà aggiunta in DCAT 2.</skos:changeNote>
        <skos:changeNote xml:lang="da">Ny genskab tilføjet i DCAT 2.</skos:changeNote>
        <skos:definition xml:lang="da">mindste geografiske afstand som kan resolveres i et datasæt, målt i meter.</skos:definition>
        <skos:definition xml:lang="en-us">minimum spatial separation resolvable in a dataset, measured in meters.</skos:definition>
        <skos:definition xml:lang="en-gb">minimum spatial separation resolvable in a dataset, measured in metres.</skos:definition>
        <skos:definition xml:lang="cs">minimální prostorový rozestup rozeznatelný v datové sadě, měřeno v metrech.</skos:definition>
        <skos:definition xml:lang="es">mínima separacíon espacial disponible en un conjunto de datos, medida en metros.</skos:definition>
        <skos:definition xml:lang="it">separazione spaziale minima risolvibile in un set di dati, misurata in metri.</skos:definition>
        <skos:editorialNote xml:lang="da">Kan optræde i forbindelse med beskrivelse af datasættet eller datasætditributionen, så der er ikke angivet et domæne for egenskaben.</skos:editorialNote>
        <skos:editorialNote xml:lang="en">Might appear in the description of a Dataset or a Distribution, so no domain is specified.</skos:editorialNote>
        <skos:editorialNote xml:lang="cs">Může se vyskytnout v popisu Datové sady nebo Distribuce, takže nebyl specifikován definiční obor.</skos:editorialNote>
        <skos:scopeNote xml:lang="da">Alternative geografiske opløsninger kan leveres som forskellige datasætdistributioner.</skos:scopeNote>
        <skos:scopeNote xml:lang="en">Alternative spatial resolutions might be provided as different dataset distributions.</skos:scopeNote>
        <skos:scopeNote xml:lang="es">Distintas distribuciones de un conjunto de datos pueden tener resoluciones espaciales diferentes.</skos:scopeNote>
        <skos:scopeNote xml:lang="da">Hvis datasættet udgøres af et billede eller et grid, så bør dette svare til afstanden mellem elementerne. For andre typer af spatiale datasæt, vil denne egenskab typisk indikere den mindste afstand mellem elementerne i datasættet.</skos:scopeNote>
        <skos:scopeNote xml:lang="en">If the dataset is an image or grid this should correspond to the spacing of items. For other kinds of spatial dataset, this property will usually indicate the smallest distance between items in the dataset.</skos:scopeNote>
        <skos:scopeNote xml:lang="cs">Pokud je datová sada obraz či mřížka, měla by tato vlastnost odpovídat rozestupu položek. Pro ostatní druhy prostorových datových sad bude tato vlastnost obvykle indikovat nejmenší vzdálenost mezi položkami této datové sady.</skos:scopeNote>
        <skos:scopeNote xml:lang="it">Risoluzioni spaziali alternative possono essere fornite come diverse distribuzioni di set di dati.</skos:scopeNote>
        <skos:scopeNote xml:lang="cs">Různá prostorová rozlišení mohou být poskytována jako různé distribuce datové sady.</skos:scopeNote>
        <skos:scopeNote xml:lang="it">Se il set di dati è un&apos;immagine o una griglia, questo dovrebbe corrispondere alla spaziatura degli elementi. Per altri tipi di set di dati spaziali, questa proprietà di solito indica la distanza minima tra gli elementi nel set di dati.</skos:scopeNote>
        <skos:scopeNote xml:lang="es">Si el conjunto de datos es una imágen o grilla, esta propiedad corresponde al espaciado de los elementos. Para otro tipo de conjunto de datos espaciales, esta propieda usualmente indica la menor distancia entre los elementos de dichos datos.</skos:scopeNote>
    </owl:DatatypeProperty>
    


    <!-- http://www.w3.org/ns/dcat#startDate -->


    <owl:DatatypeProperty rdf:about="http://www.w3.org/ns/dcat#startDate">
        <rdfs:domain rdf:resource="http://purl.org/dc/terms/PeriodOfTime"/>
        <rdfs:range rdf:resource="http://www.w3.org/2000/01/rdf-schema#Literal"/>
        <rdfs:isDefinedBy rdf:resource="https://www.w3.org/TR/vocab-dcat-2/"/>
        <rdfs:label xml:lang="it">data di inizio</rdfs:label>
        <rdfs:label xml:lang="cs">datum začátku</rdfs:label>
        <rdfs:label xml:lang="en">start date</rdfs:label>
        <rdfs:label xml:lang="da">startdato</rdfs:label>
        <skos:altLabel xml:lang="da">starttidspunkt</skos:altLabel>
        <skos:changeNote xml:lang="en">New property added in DCAT 2.</skos:changeNote>
        <skos:changeNote xml:lang="cs">Nová vlastnost přidaná ve verzi DCAT 2.</skos:changeNote>
        <skos:changeNote xml:lang="es">Nueva propiedad agregada en DCAT 2.</skos:changeNote>
        <skos:changeNote xml:lang="it">Nuova proprietà aggiunta in DCAT 2.</skos:changeNote>
        <skos:changeNote xml:lang="da">Ny egenskab tilføjet i DCAT 2.</skos:changeNote>
        <skos:definition xml:lang="es">El comienzo del período</skos:definition>
        <skos:definition xml:lang="it">L&apos;inizio del periodo</skos:definition>
        <skos:definition xml:lang="da">Start på perioden.</skos:definition>
        <skos:definition xml:lang="en">The start of the period</skos:definition>
        <skos:definition xml:lang="cs">Začátek doby trvání</skos:definition>
        <skos:scopeNote xml:lang="es">El rango de esta propiedad es intencionalmente genérico con el propósito de permitir distintos niveles de precisión temporal para especificar el comienzo de un período. Por ejemplo, puede expresarse como una fecha (xsd:date), una fecha y un tiempo (xsd:dateTime), o un año (xsd:gYear).</skos:scopeNote>
        <skos:scopeNote xml:lang="it">Il range di questa proprietà è volutamente generico, con lo scopo di consentire diversi livelli di precisione temporale per specificare l&apos;inizio di un periodo. Ad esempio, può essere espresso con una data (xsd:date), una data e un&apos;ora (xsd:dateTime), o un anno (xsd:gYear).</skos:scopeNote>
        <skos:scopeNote xml:lang="cs">Obor hodnot této vlastnosti je úmyslně obecný, aby umožnil různé úrovně časového rozlišení pro specifikaci začátku doby trvání. Ten může být kupříkladu vyjádřen datumem (xsd:date), datumem a časem (xsd:dateTime) či rokem (xsd:gYear).</skos:scopeNote>
        <skos:scopeNote xml:lang="da">Rækkeviden for denne egenskab er bevidst generisk defineret med det formål at tillade forskellige niveauer af tidslig præcision ifm. angivelse af startdatoen for en periode. Den kan eksempelvis udtrykkes som en dato (xsd:date), en dato og et tidspunkt (xsd:dateTime), eller et årstal (xsd:gYear).</skos:scopeNote>
        <skos:scopeNote xml:lang="en">The range of this property is intentionally generic, with the purpose of allowing different level of temporal precision for specifying the start of a period. E.g., it can be expressed with a date (xsd:date), a date and time (xsd:dateTime), or a year (xsd:gYear).</skos:scopeNote>
    </owl:DatatypeProperty>
    


    <!-- http://www.w3.org/ns/dcat#temporalResolution -->


    <owl:DatatypeProperty rdf:about="http://www.w3.org/ns/dcat#temporalResolution">
        <rdfs:range rdf:resource="http://www.w3.org/2001/XMLSchema#duration"/>
        <rdfs:comment xml:lang="da">mindste tidsperiode der kan resolveres i datasættet.</rdfs:comment>
        <rdfs:comment xml:lang="en">minimum time period resolvable in a dataset.</rdfs:comment>
        <rdfs:comment xml:lang="cs">minimální doba trvání rozlišitelná v datové sadě.</rdfs:comment>
        <rdfs:comment xml:lang="it">periodo di tempo minimo risolvibile in un set di dati.</rdfs:comment>
        <rdfs:comment xml:lang="es">período de tiempo mínimo en el conjunto de datos.</rdfs:comment>
        <rdfs:isDefinedBy rdf:resource="https://www.w3.org/TR/vocab-dcat-2/"/>
        <rdfs:label xml:lang="es">resolución temporal</rdfs:label>
        <rdfs:label xml:lang="it">risoluzione temporale</rdfs:label>
        <rdfs:label xml:lang="en">temporal resolution</rdfs:label>
        <rdfs:label xml:lang="da">tidslig opløsning</rdfs:label>
        <rdfs:label xml:lang="cs">časové rozlišení</rdfs:label>
        <skos:changeNote xml:lang="en">New property added in DCAT 2.</skos:changeNote>
        <skos:changeNote xml:lang="cs">Nová vlastnost přidaná ve verzi DCAT 2.</skos:changeNote>
        <skos:changeNote xml:lang="es">Nueva propiedad añadida en DCAT 2.</skos:changeNote>
        <skos:changeNote xml:lang="it">Nuova proprietà aggiunta in DCAT 2.</skos:changeNote>
        <skos:definition xml:lang="da">mindste tidsperiode der kan resolveres i datasættet.</skos:definition>
        <skos:definition xml:lang="en">minimum time period resolvable in a dataset.</skos:definition>
        <skos:definition xml:lang="cs">minimální doba trvání rozlišitelná v datové sadě.</skos:definition>
        <skos:definition xml:lang="it">periodo di tempo minimo risolvibile in un set di dati.</skos:definition>
        <skos:definition xml:lang="es">período de tiempo mínimo en el conjunto de datos.</skos:definition>
        <skos:editorialNote xml:lang="da">Kan optræde i forbindelse med beskrivelse af datasættet eller datasætditributionen, så der er ikke angivet et domæne for egenskaben.</skos:editorialNote>
        <skos:editorialNote xml:lang="en">Might appear in the description of a Dataset or a Distribution, so no domain is specified.</skos:editorialNote>
        <skos:editorialNote xml:lang="cs">Může se vyskytnout v popisu Datové sady nebo Distribuce, takže nebyl specifikován definiční obor.</skos:editorialNote>
        <skos:scopeNote xml:lang="en">Alternative temporal resolutions might be provided as different dataset distributions.</skos:scopeNote>
        <skos:scopeNote xml:lang="da">Alternative tidslige opløsninger kan leveres som forskellige datasætdistributioner.</skos:scopeNote>
        <skos:scopeNote xml:lang="es">Distintas distribuciones del conjunto de datos pueden tener resoluciones temporales diferentes.</skos:scopeNote>
        <skos:scopeNote xml:lang="da">Hvis datasættet er en tidsserie, så bør denne egenskab svare til afstanden mellem elementerne i tidsserien. For andre typer af datasæt indikerer denne egenskab den mindste tidsforskel mellem elementer i datasættet.</skos:scopeNote>
        <skos:scopeNote xml:lang="en">If the dataset is a time-series this should correspond to the spacing of items in the series. For other kinds of dataset, this property will usually indicate the smallest time difference between items in the dataset.</skos:scopeNote>
        <skos:scopeNote xml:lang="cs">Pokud je datová sada časovou řadou, měla by tato vlastnost odpovídat rozestupu položek v řadě. Pro ostatní druhy datových sad bude tato vlastnost obvykle indikovat nejmenší časovou vzdálenost mezi položkami této datové sady.</skos:scopeNote>
        <skos:scopeNote xml:lang="it">Risoluzioni temporali alternative potrebbero essere fornite come diverse distribuzioni di set di dati.</skos:scopeNote>
        <skos:scopeNote xml:lang="cs">Různá časová rozlišení mohou být poskytována jako různé distribuce datové sady.</skos:scopeNote>
        <skos:scopeNote xml:lang="it">Se il set di dati è una serie temporale, questo dovrebbe corrispondere alla spaziatura degli elementi della serie. Per altri tipi di set di dati, questa proprietà di solito indica la più piccola differenza di tempo tra gli elementi nel set di dati.</skos:scopeNote>
        <skos:scopeNote xml:lang="es">Si el conjunto de datos es una serie temporal, debe corresponder al espaciado de los elementos de la serie. Para otro tipo de conjuntos de datos, esta propiedad indicará usualmente la menor diferencia de tiempo entre elementos en el dataset.</skos:scopeNote>
    </owl:DatatypeProperty>
    


    <!-- http://www.w3.org/ns/dcat#version -->


    <owl:DatatypeProperty rdf:about="http://www.w3.org/ns/dcat#version">
        <rdfs:comment xml:lang="es">El indicador de versión (nombre o identificador) del recurso.</rdfs:comment>
        <rdfs:comment xml:lang="it">L&apos;indicatore di versione (un nome o un identificatore) di una risorsa.</rdfs:comment>
        <rdfs:comment xml:lang="en">The version indicator (name or identifier) of a resource.</rdfs:comment>
        <rdfs:isDefinedBy rdf:resource="https://www.w3.org/TR/vocab-dcat-3/"/>
        <rdfs:label xml:lang="en">version</rdfs:label>
        <rdfs:label xml:lang="it">versione</rdfs:label>
        <rdfs:label xml:lang="es">versión</rdfs:label>
        <skos:changeNote xml:lang="en">New property added in DCAT 3.</skos:changeNote>
        <skos:changeNote xml:lang="cs">Nová vlastnost přidaná ve verzi DCAT 3.</skos:changeNote>
        <skos:changeNote xml:lang="es">Nueva propiedad agregada in DCAT 3.</skos:changeNote>
        <skos:changeNote xml:lang="it">Nuova proprietà aggiunta in DCAT 3.</skos:changeNote>
        <skos:changeNote xml:lang="da">Ny egenskab tilføjet i DCAT 3.</skos:changeNote>
        <skos:definition xml:lang="es">El indicador de versión (nombre o identificador) del recurso.</skos:definition>
        <skos:definition xml:lang="it">L&apos;indicatore di versione (un nome o un identificatore) di una risorsa</skos:definition>
        <skos:definition xml:lang="en">The version indicator (name or identifier) of a resource.</skos:definition>
        <skos:scopeNote xml:lang="en">DCAT does not prescribe how a version name / identifier should be specified, and refers for guidance to [DWBP]&apos;s Best Practice 7: Provide a version indicator.</skos:scopeNote>
        <skos:scopeNote xml:lang="es">DCAT no prescribe cómo especificar el nombre or identificador de una versión, y como guía sugiere leer las práctica 7 en [DWBP] sobre cómo proveer un indicador de versión</skos:scopeNote>
        <skos:scopeNote xml:lang="it">DCAT non prescrive come un nome o identificatore di versione dovrebbe essere specificato, e fa riferimento alle linee guida indicate in [DWBP] Best Practice 7: Provide a version indicator.</skos:scopeNote>
    </owl:DatatypeProperty>
    


    <!-- 
    ///////////////////////////////////////////////////////////////////////////////////////
    //
    // Classes
    //
    ///////////////////////////////////////////////////////////////////////////////////////
     -->


    


    <!-- http://data.ign.fr/def/geofla#Commune -->


    <owl:Class rdf:about="http://data.ign.fr/def/geofla#Commune">
        <rdfs:isDefinedBy rdf:resource="http://data.ign.fr/def/geofla#"/>
        <rdfs:label xml:lang="en">Commune</rdfs:label>
        <rdfs:label xml:lang="fr">Commune</rdfs:label>
    </owl:Class>
    


    <!-- http://data.ign.fr/def/geometrie#Curve -->


    <owl:Class rdf:about="http://data.ign.fr/def/geometrie#Curve"/>
    


    <!-- http://data.ign.fr/def/topo#AireDePeage -->


    <owl:Class rdf:about="http://data.ign.fr/def/topo#AireDePeage">
        <rdfs:subClassOf rdf:resource="http://data.ign.fr/def/topo#ElementReseauRoutier"/>
        <rdfs:comment xml:lang="fr">Emprise de la chaussée d&apos;une aire de péage.</rdfs:comment>
        <rdfs:comment xml:lang="en">Roadway of a toll area.</rdfs:comment>
        <rdfs:isDefinedBy rdf:resource="http://data.ign.fr/def/topo"/>
        <rdfs:label xml:lang="fr">Aire de péage</rdfs:label>
        <rdfs:label xml:lang="en">Toll-gate area</rdfs:label>
    </owl:Class>
    


    <!-- http://data.ign.fr/def/topo#AireDeTriage -->


    <owl:Class rdf:about="http://data.ign.fr/def/topo#AireDeTriage">
        <rdfs:subClassOf rdf:resource="http://data.ign.fr/def/topo#ElementReseauFerroviaire"/>
        <rdfs:comment xml:lang="en">Area encompassing all sections of tracks, sidings, switches for sorting cars and the composition of trains. Sorting area, beam of tracks.</rdfs:comment>
        <rdfs:comment xml:lang="fr">Surface qui englobe l’ensemble des tronçons de voies, voies de garage, aiguillages permettant le tri des wagons et la composition des trains. Aire de triage, faisceau de voies.</rdfs:comment>
        <rdfs:isDefinedBy rdf:resource="http://data.ign.fr/def/topo"/>
        <rdfs:label xml:lang="fr">Aire de triage</rdfs:label>
        <rdfs:label xml:lang="en">Marshalling yard</rdfs:label>
    </owl:Class>
    


    <!-- http://data.ign.fr/def/topo#Bassin -->


    <owl:Class rdf:about="http://data.ign.fr/def/topo#Bassin">
        <rdfs:subClassOf rdf:resource="http://data.ign.fr/def/topo#EntiteHydrographiqueTerrestre"/>
        <rdfs:comment xml:lang="fr">Construction non couverte destinée à recevoir de l&apos;eau temporairement ou de manière permanente.</rdfs:comment>
        <rdfs:comment xml:lang="en">Uncovered construction intended to receive water temporarily or permanently.</rdfs:comment>
        <rdfs:isDefinedBy rdf:resource="http://data.ign.fr/def/topo"/>
        <rdfs:label xml:lang="en">Basin</rdfs:label>
        <rdfs:label xml:lang="fr">Bassin</rdfs:label>
    </owl:Class>
    


    <!-- http://data.ign.fr/def/topo#Bati -->


    <owl:Class rdf:about="http://data.ign.fr/def/topo#Bati">
        <rdfs:subClassOf rdf:resource="http://data.ign.fr/def/topo#EntiteTopographique"/>
        <rdfs:comment xml:lang="en">Buildings (undifferentiated, industrial and remarkable) and other constructions.</rdfs:comment>
        <rdfs:comment xml:lang="fr">Bâtiments (indifférenciés, industriels et remarquables) et autres constructions.</rdfs:comment>
        <rdfs:isDefinedBy rdf:resource="http://data.ign.fr/def/topo"/>
        <rdfs:label xml:lang="en">Buildings and structures</rdfs:label>
        <rdfs:label xml:lang="fr">Bâti</rdfs:label>
    </owl:Class>
    


    <!-- http://data.ign.fr/def/topo#Batiment -->


    <owl:Class rdf:about="http://data.ign.fr/def/topo#Batiment">
        <rdfs:subClassOf rdf:resource="http://data.ign.fr/def/topo#Bati"/>
        <rdfs:comment xml:lang="fr">Construction d&apos;une certaine importance destinée à abriter des personnes, des choses ou des animaux.</rdfs:comment>
        <rdfs:comment xml:lang="en">Construction of a certain importance intended to shelter people, things or animals.</rdfs:comment>
        <rdfs:isDefinedBy rdf:resource="http://data.ign.fr/def/topo"/>
        <rdfs:label xml:lang="en">Building</rdfs:label>
        <rdfs:label xml:lang="fr">Bâtiment</rdfs:label>
    </owl:Class>
    


    <!-- http://data.ign.fr/def/topo#BornePostale -->


    <owl:Class rdf:about="http://data.ign.fr/def/topo#BornePostale">
        <rdfs:subClassOf rdf:resource="http://data.ign.fr/def/topo#ElementReseauRoutier"/>
        <rdfs:comment xml:lang="fr">Borne postale située à l&apos;extrémité d&apos;un tronçon de route.</rdfs:comment>
        <rdfs:comment xml:lang="en">Postal terminal located at the end of a stretch of road.</rdfs:comment>
        <rdfs:isDefinedBy rdf:resource="http://data.ign.fr/def/topo"/>
        <rdfs:label xml:lang="fr">Borne postale</rdfs:label>
        <rdfs:label xml:lang="en">Civic number marker</rdfs:label>
    </owl:Class>
    


    <!-- http://data.ign.fr/def/topo#CanalisationDEau -->


    <owl:Class rdf:about="http://data.ign.fr/def/topo#CanalisationDEau">
        <rdfs:subClassOf rdf:resource="http://data.ign.fr/def/topo#EntiteHydrographiqueTerrestre"/>
        <rdfs:comment xml:lang="en">Aerial water pipeline.</rdfs:comment>
        <rdfs:comment xml:lang="fr">Canalisation d&apos;eau aérienne.</rdfs:comment>
        <rdfs:isDefinedBy rdf:resource="http://data.ign.fr/def/topo"/>
        <rdfs:label xml:lang="fr">Canalisation d&apos;eau</rdfs:label>
        <rdfs:label xml:lang="en">Water pipe</rdfs:label>
    </owl:Class>
    


    <!-- http://data.ign.fr/def/topo#Cimetiere -->


    <owl:Class rdf:about="http://data.ign.fr/def/topo#Cimetiere">
        <rdfs:subClassOf rdf:resource="http://data.ign.fr/def/topo#Bati"/>
        <rdfs:comment xml:lang="fr">Lieu où l’on enterre les morts.</rdfs:comment>
        <rdfs:comment xml:lang="en">Place where we bury the dead.</rdfs:comment>
        <rdfs:isDefinedBy rdf:resource="http://data.ign.fr/def/topo"/>
        <rdfs:label xml:lang="en">Cemetery</rdfs:label>
        <rdfs:label xml:lang="fr">Cimetière</rdfs:label>
    </owl:Class>
    


    <!-- http://data.ign.fr/def/topo#Conduite -->


    <owl:Class rdf:about="http://data.ign.fr/def/topo#Conduite">
        <rdfs:subClassOf rdf:resource="http://data.ign.fr/def/topo#InfrastructureTransportEnergie"/>
        <rdfs:comment xml:lang="fr">Conduite (autre que canalisation d’eau) ou tapis roulant utilisés pour le transport de matière première (gaz, hydrocarbure, minerai, etc.) ou canalisation de nature inconnue.</rdfs:comment>
        <rdfs:comment xml:lang="en">Driving (other than water piping) or treadmill used for the transportation of raw material (gas, hydrocarbon, ore, etc.) or pipeline of unknown nature.</rdfs:comment>
        <rdfs:isDefinedBy rdf:resource="http://data.ign.fr/def/topo"/>
        <rdfs:label xml:lang="fr">Conduite</rdfs:label>
        <rdfs:label xml:lang="en">Pipeline</rdfs:label>
    </owl:Class>
    


    <!-- http://data.ign.fr/def/topo#Construction -->


    <owl:Class rdf:about="http://data.ign.fr/def/topo#Construction">
        <rdfs:subClassOf rdf:resource="http://data.ign.fr/def/topo#Bati"/>
        <rdfs:comment xml:lang="en">Civil engineering works.</rdfs:comment>
        <rdfs:comment xml:lang="fr">Ouvrage de génie civil.</rdfs:comment>
        <rdfs:isDefinedBy rdf:resource="http://data.ign.fr/def/topo"/>
        <rdfs:label xml:lang="fr">Construction</rdfs:label>
        <rdfs:label xml:lang="en">Structure</rdfs:label>
    </owl:Class>
    


    <!-- http://data.ign.fr/def/topo#CoursDEau -->


    <owl:Class rdf:about="http://data.ign.fr/def/topo#CoursDEau">
        <rdfs:subClassOf rdf:resource="http://data.ign.fr/def/topo#EntiteHydrographiqueTerrestre"/>
        <rdfs:comment xml:lang="fr">Portion de cours d&apos;eau, réel ou fictif, permanent ou temporaire, naturel ou artificiel, homogène pour l&apos;ensemble des attributs qui la concernent, et qui n&apos;inclut pas de confluent.</rdfs:comment>
        <rdfs:comment xml:lang="en">Portion of watercourses, real or fictitious, permanent or temporary, natural or artificial, homogeneous for all the attributes which concern it, and which does not include a confluence.</rdfs:comment>
        <rdfs:isDefinedBy rdf:resource="http://data.ign.fr/def/topo"/>
        <rdfs:label xml:lang="fr">Cours d&apos;eau</rdfs:label>
        <rdfs:label xml:lang="en">Watercourse</rdfs:label>
    </owl:Class>
    


    <!-- http://data.ign.fr/def/topo#ElementDuRelief -->


    <owl:Class rdf:about="http://data.ign.fr/def/topo#ElementDuRelief">
        <rdfs:subClassOf rdf:resource="http://data.ign.fr/def/topo#EntiteTopographique"/>
        <rdfs:comment xml:lang="fr">Entité topographique correspondant à une rupture de pente artificielle, ou à un élément remarquable du relief nommé.</rdfs:comment>
        <rdfs:comment xml:lang="en">Topographic entity corresponding to an artificial slope break, or to a remarkable element of the named relief.</rdfs:comment>
        <rdfs:isDefinedBy rdf:resource="http://data.ign.fr/def/topo"/>
        <rdfs:label xml:lang="en">Relief feature</rdfs:label>
        <rdfs:label xml:lang="fr">Élément du relief</rdfs:label>
    </owl:Class>
    


    <!-- http://data.ign.fr/def/topo#ElementReseauFerroviaire -->


    <owl:Class rdf:about="http://data.ign.fr/def/topo#ElementReseauFerroviaire">
        <rdfs:subClassOf rdf:resource="http://data.ign.fr/def/topo#EntiteTopographique"/>
        <rdfs:comment xml:lang="en">Elements of the rail transportation system: railways and marshalling yards.</rdfs:comment>
        <rdfs:comment xml:lang="fr">Éléments du réseau de transport ferroviaire: voies ferrées et aires de triage.</rdfs:comment>
        <rdfs:isDefinedBy rdf:resource="http://data.ign.fr/def/topo"/>
        <rdfs:label xml:lang="en">Transport by rail feature</rdfs:label>
        <rdfs:label xml:lang="fr">Élément du réseau ferroviaire</rdfs:label>
    </owl:Class>
    


    <!-- http://data.ign.fr/def/topo#ElementReseauRoutier -->


    <owl:Class rdf:about="http://data.ign.fr/def/topo#ElementReseauRoutier">
        <rdfs:subClassOf rdf:resource="http://data.ign.fr/def/topo#EntiteTopographique"/>
        <rdfs:comment xml:lang="en">Elements of the road transport network: paved and unpaved roads, &apos;addressed&apos; network, and a selection of roads and trails.</rdfs:comment>
        <rdfs:comment xml:lang="fr">Éléments du réseau de transport routier: voies de communication revêtues et non revêtues, réseau &apos;adressé&apos;, et une sélection des chemins et sentiers.</rdfs:comment>
        <rdfs:isDefinedBy rdf:resource="http://data.ign.fr/def/topo"/>
        <rdfs:label xml:lang="en">Road transport feature</rdfs:label>
        <rdfs:label xml:lang="fr">Élément du réseau routier</rdfs:label>
    </owl:Class>
    


    <!-- http://data.ign.fr/def/topo#EntiteHydrographiqueTerrestre -->


    <owl:Class rdf:about="http://data.ign.fr/def/topo#EntiteHydrographiqueTerrestre">
        <rdfs:subClassOf rdf:resource="http://data.ign.fr/def/topo#EntiteTopographique"/>
        <rdfs:comment xml:lang="fr">Entité topographique relative au réseau hydrographique terrestre, à la production ou au stockage d&apos;eau.</rdfs:comment>
        <rdfs:comment xml:lang="en">Topographic entity relating to the terrestrial hydrographic network, the production or the storage of water.</rdfs:comment>
        <rdfs:isDefinedBy rdf:resource="http://data.ign.fr/def/topo"/>
        <rdfs:label xml:lang="fr">Entité hydrographique terrestre</rdfs:label>
        <rdfs:label xml:lang="en">Inland hydrographic feature</rdfs:label>
    </owl:Class>
    


    <!-- http://data.ign.fr/def/topo#EntiteTopographique -->


    <owl:Class rdf:about="http://data.ign.fr/def/topo#EntiteTopographique">
        <owl:equivalentClass rdf:resource="http://www.geonames.org/ontology#Feature"/>
        <rdfs:comment xml:lang="en">A real world phenomenon that is associated with a location on earth</rdfs:comment>
        <rdfs:comment xml:lang="fr">Un phénomène du monde réel qui est associé à une localisation sur la terre</rdfs:comment>
        <rdfs:isDefinedBy rdf:resource="http://data.ign.fr/def/topo"/>
        <rdfs:label xml:lang="fr">Entité topographique</rdfs:label>
        <rdfs:label xml:lang="en">Topographic entity</rdfs:label>
    </owl:Class>
    


    <!-- http://data.ign.fr/def/topo#InfrastructureTransportEnergie -->


    <owl:Class rdf:about="http://data.ign.fr/def/topo#InfrastructureTransportEnergie">
        <rdfs:subClassOf rdf:resource="http://data.ign.fr/def/topo#EntiteTopographique"/>
        <rdfs:comment xml:lang="en">Elements of the electricity transmission network at high and very high voltage, and pipes used for the transport of raw material.</rdfs:comment>
        <rdfs:comment xml:lang="fr">Éléments du réseau de transport d&apos;électricité à une haute et très haute tension, et conduites utilisées pour le transport de matière première.</rdfs:comment>
        <rdfs:isDefinedBy rdf:resource="http://data.ign.fr/def/topo"/>
        <rdfs:label xml:lang="en">Energy transport infrastructure</rdfs:label>
        <rdfs:label xml:lang="fr">Infrastructure de transport d&apos;énergie</rdfs:label>
    </owl:Class>
    


    <!-- http://data.ign.fr/def/topo#Laisse -->


    <owl:Class rdf:about="http://data.ign.fr/def/topo#Laisse">
        <rdfs:subClassOf rdf:resource="http://data.ign.fr/def/topo#EntiteHydrographiqueTerrestre"/>
        <rdfs:comment xml:lang="fr">Limite supérieure ou inférieure de l&apos;estran.</rdfs:comment>
        <rdfs:comment xml:lang="en">Upper or lower limit of the foreshore.</rdfs:comment>
        <rdfs:isDefinedBy rdf:resource="http://data.ign.fr/def/topo"/>
        <rdfs:label xml:lang="fr">Laisse</rdfs:label>
        <rdfs:label xml:lang="en">Tide line</rdfs:label>
    </owl:Class>
    


    <!-- http://data.ign.fr/def/topo#LigneElectrique -->


    <owl:Class rdf:about="http://data.ign.fr/def/topo#LigneElectrique">
        <rdfs:subClassOf rdf:resource="http://data.ign.fr/def/topo#InfrastructureTransportEnergie"/>
        <rdfs:comment xml:lang="fr">Portion de ligne électrique homogène pour l&apos;ensemble des attributs qui la concernent.</rdfs:comment>
        <rdfs:comment xml:lang="en">Portion of homogeneous electrical line for all the attributes that concern it.</rdfs:comment>
        <rdfs:isDefinedBy rdf:resource="http://data.ign.fr/def/topo"/>
        <rdfs:label xml:lang="en">Electricity transmission line</rdfs:label>
        <rdfs:label xml:lang="fr">Ligne électrique</rdfs:label>
    </owl:Class>
    


    <!-- http://data.ign.fr/def/topo#LigneTransportCable -->


    <owl:Class rdf:about="http://data.ign.fr/def/topo#LigneTransportCable">
        <rdfs:subClassOf rdf:resource="http://data.ign.fr/def/topo#EntiteTopographique"/>
        <rdfs:comment xml:lang="en">Means of transport consisting of one or more carrying cables.</rdfs:comment>
        <rdfs:comment xml:lang="fr">Moyen de transport constitué d&apos;un ou de plusieurs câbles porteurs.</rdfs:comment>
        <rdfs:isDefinedBy rdf:resource="http://data.ign.fr/def/topo"/>
        <rdfs:label xml:lang="en">Cableway transport line</rdfs:label>
        <rdfs:label xml:lang="fr">Ligne de transport par câble</rdfs:label>
    </owl:Class>
    


    <!-- http://data.ign.fr/def/topo#Parking -->


    <owl:Class rdf:about="http://data.ign.fr/def/topo#Parking">
        <rdfs:subClassOf rdf:resource="http://data.ign.fr/def/topo#ElementReseauRoutier"/>
        <rdfs:comment xml:lang="en">Area developed for the parking of automobiles. Parking uncovered, public or private, parking area of about half a hectare and more.</rdfs:comment>
        <rdfs:comment xml:lang="fr">Zone aménagée pour le parcage des automobiles. Parking non couvert, public ou privé, aire de stationnement d’environ un demi hectare et plus.</rdfs:comment>
        <rdfs:isDefinedBy rdf:resource="http://data.ign.fr/def/topo"/>
        <rdfs:label xml:lang="en">Car park</rdfs:label>
        <rdfs:label xml:lang="fr">Parking</rdfs:label>
    </owl:Class>
    


    <!-- http://data.ign.fr/def/topo#PisteAerodrome -->


    <owl:Class rdf:about="http://data.ign.fr/def/topo#PisteAerodrome">
        <rdfs:subClassOf rdf:resource="http://data.ign.fr/def/topo#Bati"/>
        <rdfs:comment xml:lang="fr">Aire située sur un aérodrome, aménagée afin de servir au roulement des aéronefs, au décollage et à l’atterrissage, en dur ou en herbe.</rdfs:comment>
        <rdfs:comment xml:lang="en">Area located on an aerodrome, designed for use in aircraft rolling, take-off and landing, hard or grass.</rdfs:comment>
        <rdfs:isDefinedBy rdf:resource="http://data.ign.fr/def/topo"/>
        <rdfs:label xml:lang="fr">Piste d&apos;aérodrome</rdfs:label>
        <rdfs:label xml:lang="en">Taxiway</rdfs:label>
    </owl:Class>
    


    <!-- http://data.ign.fr/def/topo#Place -->


    <owl:Class rdf:about="http://data.ign.fr/def/topo#Place">
        <rdfs:subClassOf rdf:resource="http://data.ign.fr/def/topo#ElementReseauRoutier"/>
        <rdfs:comment xml:lang="en">Place or crossroads covered with wide width.</rdfs:comment>
        <rdfs:comment xml:lang="fr">Place ou carrefour revêtu de grande largeur.</rdfs:comment>
        <rdfs:isDefinedBy rdf:resource="http://data.ign.fr/def/topo"/>
        <rdfs:label xml:lang="fr">Place</rdfs:label>
        <rdfs:label xml:lang="en">Square</rdfs:label>
    </owl:Class>
    


    <!-- http://data.ign.fr/def/topo#PointDEau -->


    <owl:Class rdf:about="http://data.ign.fr/def/topo#PointDEau">
        <rdfs:subClassOf rdf:resource="http://data.ign.fr/def/topo#EntiteHydrographiqueTerrestre"/>
        <rdfs:comment xml:lang="en">Source (captured or not), point of water production (pumping, drilling, well, ...) or small water storage point (cistern, waterer, laundry, basin).</rdfs:comment>
        <rdfs:comment xml:lang="fr">Source (captée ou non), point de production d’eau (pompage, forage, puits,...) ou point de stockage d’eau de petite dimension (citerne, abreuvoir, lavoir, bassin).</rdfs:comment>
        <rdfs:isDefinedBy rdf:resource="http://data.ign.fr/def/topo"/>
        <rdfs:label xml:lang="fr">Point d&apos;eau</rdfs:label>
        <rdfs:label xml:lang="en">Waterhole</rdfs:label>
    </owl:Class>
    


    <!-- http://data.ign.fr/def/topo#PosteTransformation -->


    <owl:Class rdf:about="http://data.ign.fr/def/topo#PosteTransformation">
        <rdfs:subClassOf rdf:resource="http://data.ign.fr/def/topo#InfrastructureTransportEnergie"/>
        <rdfs:comment xml:lang="fr">Enceinte à l&apos;intérieur de laquelle le courant transporté par une ligne électrique est transformé.</rdfs:comment>
        <rdfs:comment xml:lang="en">Enclosure inside which the current carried by a power line is transformed.</rdfs:comment>
        <rdfs:isDefinedBy rdf:resource="http://data.ign.fr/def/topo"/>
        <rdfs:label xml:lang="fr">Poste de transformation</rdfs:label>
        <rdfs:label xml:lang="en">Transformation sub-station</rdfs:label>
    </owl:Class>
    


    <!-- http://data.ign.fr/def/topo#Pylone -->


    <owl:Class rdf:about="http://data.ign.fr/def/topo#Pylone">
        <rdfs:subClassOf rdf:resource="http://data.ign.fr/def/topo#InfrastructureTransportEnergie"/>
        <rdfs:comment xml:lang="en">Electric line support. Pylon, portico.</rdfs:comment>
        <rdfs:comment xml:lang="fr">Support de ligne électrique. Pylône, portique.</rdfs:comment>
        <rdfs:isDefinedBy rdf:resource="http://data.ign.fr/def/topo"/>
        <rdfs:label xml:lang="en">Pylon</rdfs:label>
        <rdfs:label xml:lang="fr">Pylône</rdfs:label>
    </owl:Class>
    


    <!-- http://data.ign.fr/def/topo#Reservoir -->


    <owl:Class rdf:about="http://data.ign.fr/def/topo#Reservoir">
        <rdfs:subClassOf rdf:resource="http://data.ign.fr/def/topo#Bati"/>
        <rdfs:comment xml:lang="fr">Réservoir (eau, matières industrielles,...) de plus de 10m de diamètre.</rdfs:comment>
        <rdfs:comment xml:lang="en">Tank (water, industrial materials, ...) more than 10m in diameter.</rdfs:comment>
        <rdfs:isDefinedBy rdf:resource="http://data.ign.fr/def/topo"/>
        <rdfs:label xml:lang="fr">Réservoir</rdfs:label>
        <rdfs:label xml:lang="en">Tank</rdfs:label>
    </owl:Class>
    


    <!-- http://data.ign.fr/def/topo#Route -->


    <owl:Class rdf:about="http://data.ign.fr/def/topo#Route">
        <rdfs:subClassOf rdf:resource="http://data.ign.fr/def/topo#ElementReseauRoutier"/>
        <rdfs:subClassOf>
            <owl:Restriction>
                <owl:onProperty rdf:resource="http://purl.org/dc/terms/isPartOf"/>
                <owl:someValuesFrom rdf:resource="http://data.ign.fr/def/topo#Voie"/>
            </owl:Restriction>
        </rdfs:subClassOf>
        <rdfs:comment xml:lang="fr">Portion de voie de communication destinée aux automobiles, aux piétons, aux cycles ou aux animaux, homogène pour l&apos;ensemble des attributs et des relations qui la concerne. Le tronçon de route peut être revêtu ou non revêtu (pas de revêtement de surface ou revêtement de surface fortement dégradé).</rdfs:comment>
        <rdfs:comment xml:lang="en">Portion of communication channel intended for automobiles, pedestrians, cycles or animals, homogeneous for all the attributes and relations that concern it. The road section may be coated or uncoated (no surface coating or highly degraded surface coating).</rdfs:comment>
        <rdfs:isDefinedBy rdf:resource="http://data.ign.fr/def/topo"/>
        <rdfs:label xml:lang="en">Road</rdfs:label>
        <rdfs:label xml:lang="fr">Route</rdfs:label>
    </owl:Class>
    


    <!-- http://data.ign.fr/def/topo#SurfaceDEau -->


    <owl:Class rdf:about="http://data.ign.fr/def/topo#SurfaceDEau">
        <rdfs:subClassOf rdf:resource="http://data.ign.fr/def/topo#EntiteHydrographiqueTerrestre"/>
        <rdfs:comment xml:lang="en">Non-marine water surface: wide channel, pond, wide river, lake, pond, wide river.</rdfs:comment>
        <rdfs:comment xml:lang="fr">Surface d&apos;eau non marine : large canal, étang, large fleuve, lac, mare, large rivière.</rdfs:comment>
        <rdfs:isDefinedBy rdf:resource="http://data.ign.fr/def/topo"/>
        <rdfs:label xml:lang="fr">Surface d&apos;eau</rdfs:label>
        <rdfs:label xml:lang="en">Water surface</rdfs:label>
    </owl:Class>
    


    <!-- http://data.ign.fr/def/topo#TerrainDeSport -->


    <owl:Class rdf:about="http://data.ign.fr/def/topo#TerrainDeSport">
        <rdfs:subClassOf rdf:resource="http://data.ign.fr/def/topo#Bati"/>
        <rdfs:comment xml:lang="en">Outdoor sports equipment.</rdfs:comment>
        <rdfs:comment xml:lang="fr">Équipement sportif de plein air.</rdfs:comment>
        <rdfs:isDefinedBy rdf:resource="http://data.ign.fr/def/topo"/>
        <rdfs:label xml:lang="en">Sports ground</rdfs:label>
        <rdfs:label xml:lang="fr">Terrain de sport</rdfs:label>
    </owl:Class>
    


    <!-- http://data.ign.fr/def/topo#TypeDeBatiment -->


    <owl:Class rdf:about="http://data.ign.fr/def/topo#TypeDeBatiment">
        <rdfs:subClassOf rdf:resource="http://www.w3.org/2004/02/skos/core#Concept"/>
        <rdfs:comment xml:lang="en">Includes all instances designating building types.</rdfs:comment>
        <rdfs:comment xml:lang="fr">Regroupe l&apos;ensemble des instances désignant des types de bâtiments.</rdfs:comment>
        <rdfs:isDefinedBy rdf:resource="http://data.ign.fr/def/topo"/>
        <rdfs:label xml:lang="fr">Type de bâtiment</rdfs:label>
        <rdfs:label xml:lang="en">Type of building </rdfs:label>
    </owl:Class>
    


    <!-- http://data.ign.fr/def/topo#TypeDeConstruction -->


    <owl:Class rdf:about="http://data.ign.fr/def/topo#TypeDeConstruction">
        <rdfs:subClassOf rdf:resource="http://www.w3.org/2004/02/skos/core#Concept"/>
        <rdfs:comment xml:lang="en">Group together all the instances designating types of constructions.</rdfs:comment>
        <rdfs:comment xml:lang="fr">Regroupe l&apos;ensemble des instances désignant des types de constructions.</rdfs:comment>
        <rdfs:isDefinedBy rdf:resource="http://data.ign.fr/def/topo"/>
        <rdfs:label xml:lang="fr">Type de construction</rdfs:label>
        <rdfs:label xml:lang="en">Type of structure</rdfs:label>
    </owl:Class>
    


    <!-- http://data.ign.fr/def/topo#TypeDeFranchissement -->


    <owl:Class rdf:about="http://data.ign.fr/def/topo#TypeDeFranchissement">
        <rdfs:subClassOf rdf:resource="http://www.w3.org/2004/02/skos/core#Concept"/>
        <rdfs:comment xml:lang="en">Includes all instances designating types of crossing structures.</rdfs:comment>
        <rdfs:comment xml:lang="fr">Regroupe l&apos;ensemble des instances désignant des types d&apos;ouvrages de franchissement.</rdfs:comment>
        <rdfs:isDefinedBy rdf:resource="http://data.ign.fr/def/topo"/>
        <rdfs:label xml:lang="fr">Type de franchissement</rdfs:label>
        <rdfs:label xml:lang="en">Type of crossing</rdfs:label>
    </owl:Class>
    


    <!-- http://data.ign.fr/def/topo#TypeDeLaisse -->


    <owl:Class rdf:about="http://data.ign.fr/def/topo#TypeDeLaisse">
        <rdfs:subClassOf rdf:resource="http://www.w3.org/2004/02/skos/core#Concept"/>
        <rdfs:comment xml:lang="en">Group together all instances designating leash types.</rdfs:comment>
        <rdfs:comment xml:lang="fr">Regroupe l&apos;ensemble des instances désignant des types de laisses.</rdfs:comment>
        <rdfs:isDefinedBy rdf:resource="http://data.ign.fr/def/topo"/>
        <rdfs:label xml:lang="fr">Type de laisse</rdfs:label>
        <rdfs:label xml:lang="en">Type of tide line</rdfs:label>
    </owl:Class>
    


    <!-- http://data.ign.fr/def/topo#TypeDePointDEau -->


    <owl:Class rdf:about="http://data.ign.fr/def/topo#TypeDePointDEau">
        <rdfs:subClassOf rdf:resource="http://www.w3.org/2004/02/skos/core#Concept"/>
        <rdfs:comment xml:lang="en">Gathers all the instances designating types of water points.</rdfs:comment>
        <rdfs:comment xml:lang="fr">Regroupe l&apos;ensemble des instances désignant des types de points d&apos;eau.</rdfs:comment>
        <rdfs:isDefinedBy rdf:resource="http://data.ign.fr/def/topo"/>
        <rdfs:label xml:lang="fr">Type de point d&apos;eau</rdfs:label>
        <rdfs:label xml:lang="en">Type of waterhole</rdfs:label>
    </owl:Class>
    


    <!-- http://data.ign.fr/def/topo#TypeDeRelief -->


    <owl:Class rdf:about="http://data.ign.fr/def/topo#TypeDeRelief">
        <rdfs:subClassOf rdf:resource="http://www.w3.org/2004/02/skos/core#Concept"/>
        <rdfs:comment xml:lang="en">Gathers all the instances designating types of reliefs.</rdfs:comment>
        <rdfs:comment xml:lang="fr">Regroupe l&apos;ensemble des instances désignant des types de reliefs.</rdfs:comment>
        <rdfs:isDefinedBy rdf:resource="http://data.ign.fr/def/topo"/>
        <rdfs:label xml:lang="fr">Type d&apos;élément du relief</rdfs:label>
        <rdfs:label xml:lang="en">Type of relief feature</rdfs:label>
    </owl:Class>
    


    <!-- http://data.ign.fr/def/topo#TypeDeReservoir -->


    <owl:Class rdf:about="http://data.ign.fr/def/topo#TypeDeReservoir">
        <rdfs:subClassOf rdf:resource="http://www.w3.org/2004/02/skos/core#Concept"/>
        <rdfs:comment xml:lang="en">Group together all instances designating types of tanks.</rdfs:comment>
        <rdfs:comment xml:lang="fr">Regroupe l&apos;ensemble des instances désignant des types de réservoirs.</rdfs:comment>
        <rdfs:isDefinedBy rdf:resource="http://data.ign.fr/def/topo"/>
        <rdfs:label xml:lang="fr">Type de réservoir</rdfs:label>
        <rdfs:label xml:lang="en">Type of tank</rdfs:label>
    </owl:Class>
    


    <!-- http://data.ign.fr/def/topo#TypeDeRoute -->


    <owl:Class rdf:about="http://data.ign.fr/def/topo#TypeDeRoute">
        <rdfs:subClassOf rdf:resource="http://www.w3.org/2004/02/skos/core#Concept"/>
        <rdfs:comment xml:lang="en">Group together all instances designating types of routes.</rdfs:comment>
        <rdfs:comment xml:lang="fr">Regroupe l&apos;ensemble des instances désignant des types de routes.</rdfs:comment>
        <rdfs:isDefinedBy rdf:resource="http://data.ign.fr/def/topo"/>
        <rdfs:label xml:lang="fr">Type de route</rdfs:label>
        <rdfs:label xml:lang="en">Type of road</rdfs:label>
    </owl:Class>
    


    <!-- http://data.ign.fr/def/topo#TypeDeTerrainDeSport -->


    <owl:Class rdf:about="http://data.ign.fr/def/topo#TypeDeTerrainDeSport">
        <rdfs:subClassOf rdf:resource="http://www.w3.org/2004/02/skos/core#Concept"/>
        <rdfs:comment xml:lang="en">Includes all instances designating types of sports fields.</rdfs:comment>
        <rdfs:comment xml:lang="fr">Regroupe l&apos;ensemble des instances désignant des types de terrains de sports.</rdfs:comment>
        <rdfs:isDefinedBy rdf:resource="http://data.ign.fr/def/topo"/>
        <rdfs:label xml:lang="fr">Type de terrain de sport</rdfs:label>
        <rdfs:label xml:lang="en">Type of sports ground </rdfs:label>
    </owl:Class>
    


    <!-- http://data.ign.fr/def/topo#TypeDeTransportCable -->


    <owl:Class rdf:about="http://data.ign.fr/def/topo#TypeDeTransportCable">
        <rdfs:subClassOf rdf:resource="http://www.w3.org/2004/02/skos/core#Concept"/>
        <rdfs:comment xml:lang="en">Consists of all instances designating types of cable transport infrastructure.</rdfs:comment>
        <rdfs:comment xml:lang="fr">Regroupe l&apos;ensemble des instances désignant des types d&apos;infrastructures de transport par câble.</rdfs:comment>
        <rdfs:isDefinedBy rdf:resource="http://data.ign.fr/def/topo"/>
        <rdfs:label xml:lang="fr">Type de ligne de transport par câble</rdfs:label>
        <rdfs:label xml:lang="en">Type of cableway transport line</rdfs:label>
    </owl:Class>
    


    <!-- http://data.ign.fr/def/topo#TypeDeVegetation -->


    <owl:Class rdf:about="http://data.ign.fr/def/topo#TypeDeVegetation">
        <rdfs:subClassOf rdf:resource="http://www.w3.org/2004/02/skos/core#Concept"/>
        <rdfs:comment xml:lang="en">Includes all instances designating tree vegetation types.</rdfs:comment>
        <rdfs:comment xml:lang="fr">Regroupe l&apos;ensemble des instances désignant des types de végétation arborée.</rdfs:comment>
        <rdfs:isDefinedBy rdf:resource="http://data.ign.fr/def/topo"/>
        <rdfs:label xml:lang="fr">Type de végétation</rdfs:label>
        <rdfs:label xml:lang="en">Type of vegetation </rdfs:label>
    </owl:Class>
    


    <!-- http://data.ign.fr/def/topo#TypeDeVoieFerree -->


    <owl:Class rdf:about="http://data.ign.fr/def/topo#TypeDeVoieFerree">
        <rdfs:subClassOf rdf:resource="http://www.w3.org/2004/02/skos/core#Concept"/>
        <rdfs:comment xml:lang="en">Includes all instances designating railway types.</rdfs:comment>
        <rdfs:comment xml:lang="fr">Regroupe l&apos;ensemble des instances désignant des types de voies ferrées.</rdfs:comment>
        <rdfs:isDefinedBy rdf:resource="http://data.ign.fr/def/topo"/>
        <rdfs:label xml:lang="fr">Type de voie ferrée</rdfs:label>
        <rdfs:label xml:lang="en">Type of railway track</rdfs:label>
    </owl:Class>
    


    <!-- http://data.ign.fr/def/topo#TypeDeZAI -->


    <owl:Class rdf:about="http://data.ign.fr/def/topo#TypeDeZAI">
        <rdfs:subClassOf rdf:resource="http://www.w3.org/2004/02/skos/core#Concept"/>
        <rdfs:comment xml:lang="en">Includes all instances designating types of activity and interest areas.</rdfs:comment>
        <rdfs:comment xml:lang="fr">Regroupe l&apos;ensemble des instances désignant des types de zones d&apos;activités et d&apos;intérêt.</rdfs:comment>
        <rdfs:isDefinedBy rdf:resource="http://data.ign.fr/def/topo"/>
        <rdfs:label xml:lang="fr">Type de ZAI</rdfs:label>
        <rdfs:label xml:lang="en">Type of Area Of Interest (AOI)</rdfs:label>
    </owl:Class>
    


    <!-- http://data.ign.fr/def/topo#Voie -->


    <owl:Class rdf:about="http://data.ign.fr/def/topo#Voie">
        <rdfs:subClassOf rdf:resource="http://data.ign.fr/def/topo#ElementReseauRoutier"/>
        <rdfs:comment xml:lang="en">A lane is a set of road sections associated with the same name. A path is identified by name in a given commune. The channel name is the one used for addressing.</rdfs:comment>
        <rdfs:comment xml:lang="fr">Une voie est un ensemble de tronçons de route associés à un même nom. Une voie est identifiée par son nom dans une commune donnée. Le nom de voie est celui qui sert à l’adressage.</rdfs:comment>
        <rdfs:isDefinedBy rdf:resource="http://data.ign.fr/def/topo"/>
        <rdfs:label xml:lang="en">Named street</rdfs:label>
        <rdfs:label xml:lang="fr">Voie nommée</rdfs:label>
    </owl:Class>
    


    <!-- http://data.ign.fr/def/topo#VoieFerree -->


    <owl:Class rdf:about="http://data.ign.fr/def/topo#VoieFerree">
        <rdfs:subClassOf rdf:resource="http://data.ign.fr/def/topo#ElementReseauFerroviaire"/>
        <rdfs:comment xml:lang="fr">Portion de voie ferrée homogène pour l&apos;ensemble des attributs qui la concernent. Dans le cas d’une ligne composée de deux à quatre voies parallèles, l’ensemble des voies est modélisé par un seul objet.</rdfs:comment>
        <rdfs:comment xml:lang="en">Portion of homogeneous railway for all the attributes that concern it. In the case of a line composed of two to four parallel tracks, the set of channels is modeled by a single object.</rdfs:comment>
        <rdfs:isDefinedBy rdf:resource="http://data.ign.fr/def/topo"/>
        <rdfs:label xml:lang="en">Railway track</rdfs:label>
        <rdfs:label xml:lang="fr">Voie ferrée</rdfs:label>
    </owl:Class>
    


    <!-- http://data.ign.fr/def/topo#ZoneActiviteInteret -->


    <owl:Class rdf:about="http://data.ign.fr/def/topo#ZoneActiviteInteret">
        <rdfs:subClassOf rdf:resource="http://data.ign.fr/def/topo#EntiteTopographique"/>
        <rdfs:comment xml:lang="en">Building or site with a specific vocation or character (administrative, religious, sports, industrial, etc.).</rdfs:comment>
        <rdfs:comment xml:lang="fr">Bâtiment ou site ayant une vocation ou un caractère particuliers (administratif, religieux, sportif, industriel, etc.).</rdfs:comment>
        <rdfs:isDefinedBy rdf:resource="http://data.ign.fr/def/topo"/>
        <rdfs:label xml:lang="en">Working area or area of interest</rdfs:label>
        <rdfs:label xml:lang="fr">Zone d&apos;activité ou d&apos;intérêt</rdfs:label>
    </owl:Class>
    


    <!-- http://data.ign.fr/def/topo#ZoneDeVegetation -->


    <owl:Class rdf:about="http://data.ign.fr/def/topo#ZoneDeVegetation">
        <rdfs:subClassOf rdf:resource="http://data.ign.fr/def/topo#EntiteTopographique"/>
        <rdfs:comment xml:lang="fr">Espace végétal naturel ou non différencié selon le couvert forestier.</rdfs:comment>
        <rdfs:comment xml:lang="en">Natural space of vegetation or undifferentiated according to the forest cover.</rdfs:comment>
        <rdfs:isDefinedBy rdf:resource="http://data.ign.fr/def/topo"/>
        <rdfs:label xml:lang="en">Vegetation area</rdfs:label>
        <rdfs:label xml:lang="fr">Zone de végétation</rdfs:label>
    </owl:Class>
    


    <!-- http://purl.org/dc/terms/Agent -->


    <owl:Class rdf:about="http://purl.org/dc/terms/Agent"/>
    


    <!-- http://purl.org/dc/terms/AgentClass -->


    <owl:Class rdf:about="http://purl.org/dc/terms/AgentClass">
        <rdfs:subClassOf rdf:resource="http://www.w3.org/2000/01/rdf-schema#Class"/>
    </owl:Class>
    


    <!-- http://purl.org/dc/terms/BibliographicResource -->


    <owl:Class rdf:about="http://purl.org/dc/terms/BibliographicResource"/>
    


    <!-- http://purl.org/dc/terms/FileFormat -->


    <owl:Class rdf:about="http://purl.org/dc/terms/FileFormat">
        <rdfs:subClassOf rdf:resource="http://purl.org/dc/terms/MediaType"/>
    </owl:Class>
    


    <!-- http://purl.org/dc/terms/Frequency -->


    <owl:Class rdf:about="http://purl.org/dc/terms/Frequency"/>
    


    <!-- http://purl.org/dc/terms/Jurisdiction -->


    <owl:Class rdf:about="http://purl.org/dc/terms/Jurisdiction">
        <rdfs:subClassOf rdf:resource="http://purl.org/dc/terms/LocationPeriodOrJurisdiction"/>
    </owl:Class>
    


    <!-- http://purl.org/dc/terms/LicenseDocument -->


    <owl:Class rdf:about="http://purl.org/dc/terms/LicenseDocument">
        <rdfs:subClassOf rdf:resource="http://purl.org/dc/terms/RightsStatement"/>
    </owl:Class>
    


    <!-- http://purl.org/dc/terms/LinguisticSystem -->


    <owl:Class rdf:about="http://purl.org/dc/terms/LinguisticSystem"/>
    


    <!-- http://purl.org/dc/terms/Location -->


    <owl:Class rdf:about="http://purl.org/dc/terms/Location">
        <rdfs:subClassOf rdf:resource="http://purl.org/dc/terms/LocationPeriodOrJurisdiction"/>
    </owl:Class>
    


    <!-- http://purl.org/dc/terms/LocationPeriodOrJurisdiction -->


    <owl:Class rdf:about="http://purl.org/dc/terms/LocationPeriodOrJurisdiction"/>
    


    <!-- http://purl.org/dc/terms/MediaType -->


    <owl:Class rdf:about="http://purl.org/dc/terms/MediaType">
        <rdfs:subClassOf rdf:resource="http://purl.org/dc/terms/MediaTypeOrExtent"/>
    </owl:Class>
    


    <!-- http://purl.org/dc/terms/MediaTypeOrExtent -->


    <owl:Class rdf:about="http://purl.org/dc/terms/MediaTypeOrExtent"/>
    


    <!-- http://purl.org/dc/terms/MethodOfAccrual -->


    <owl:Class rdf:about="http://purl.org/dc/terms/MethodOfAccrual"/>
    


    <!-- http://purl.org/dc/terms/MethodOfInstruction -->


    <owl:Class rdf:about="http://purl.org/dc/terms/MethodOfInstruction"/>
    


    <!-- http://purl.org/dc/terms/PeriodOfTime -->


    <owl:Class rdf:about="http://purl.org/dc/terms/PeriodOfTime">
        <rdfs:subClassOf rdf:resource="http://purl.org/dc/terms/LocationPeriodOrJurisdiction"/>
    </owl:Class>
    


    <!-- http://purl.org/dc/terms/PhysicalMedium -->


    <owl:Class rdf:about="http://purl.org/dc/terms/PhysicalMedium">
        <rdfs:subClassOf rdf:resource="http://purl.org/dc/terms/MediaType"/>
    </owl:Class>
    


    <!-- http://purl.org/dc/terms/PhysicalResource -->


    <owl:Class rdf:about="http://purl.org/dc/terms/PhysicalResource"/>
    


    <!-- http://purl.org/dc/terms/Policy -->


    <owl:Class rdf:about="http://purl.org/dc/terms/Policy"/>
    


    <!-- http://purl.org/dc/terms/ProvenanceStatement -->


    <owl:Class rdf:about="http://purl.org/dc/terms/ProvenanceStatement"/>
    


    <!-- http://purl.org/dc/terms/RightsStatement -->


    <owl:Class rdf:about="http://purl.org/dc/terms/RightsStatement"/>
    


    <!-- http://purl.org/dc/terms/SizeOrDuration -->


    <owl:Class rdf:about="http://purl.org/dc/terms/SizeOrDuration">
        <rdfs:subClassOf rdf:resource="http://purl.org/dc/terms/MediaTypeOrExtent"/>
    </owl:Class>
    


    <!-- http://purl.org/dc/terms/Standard -->


    <owl:Class rdf:about="http://purl.org/dc/terms/Standard"/>
    


    <!-- http://purl.org/vocommons/voaf#Vocabulary -->


    <owl:Class rdf:about="http://purl.org/vocommons/voaf#Vocabulary"/>
    


    <!-- http://www.geonames.org/ontology#Feature -->


    <owl:Class rdf:about="http://www.geonames.org/ontology#Feature"/>
    


    <!-- http://www.semanticweb.org/bbucher/ontologies/2025/9/geodata#Collection -->


    <owl:Class rdf:about="http://www.semanticweb.org/bbucher/ontologies/2025/9/geodata#Collection">
        <rdfs:comment>Collection of items that supports the usage of geodata for a pedagogic or learning purpose, in relationship with given concepts</rdfs:comment>
    </owl:Class>
    


    <!-- http://www.semanticweb.org/bbucher/ontologies/2025/9/geodata#CollectionItem -->


    <owl:Class rdf:about="http://www.semanticweb.org/bbucher/ontologies/2025/9/geodata#CollectionItem">
        <rdfs:comment>A collection item is composed of different pieces of data, usually selections from bigger datasets, associated with a proposed visualisation, and narratives that connect the visual items to the concepts of the collection. It has a spatial and temporal extent.</rdfs:comment>
    </owl:Class>
    


    <!-- http://www.semanticweb.org/bbucher/ontologies/2025/9/geodata#Geodata_process -->


    <owl:Class rdf:about="http://www.semanticweb.org/bbucher/ontologies/2025/9/geodata#Geodata_process">
        <rdfs:subClassOf rdf:resource="http://www.w3.org/ns/dcat#Resource"/>
        <rdfs:comment>Process to derive data, that may combine data services but not necessarily</rdfs:comment>
    </owl:Class>
    


    <!-- http://www.semanticweb.org/bbucher/ontologies/2025/9/geodata#Geodataset -->


    <owl:Class rdf:about="http://www.semanticweb.org/bbucher/ontologies/2025/9/geodata#Geodataset">
        <rdfs:subClassOf rdf:resource="http://www.w3.org/ns/dcat#Dataset"/>
    </owl:Class>
    


    <!-- http://www.semanticweb.org/bbucher/ontologies/2025/9/geodata#Geodataset_series -->


    <owl:Class rdf:about="http://www.semanticweb.org/bbucher/ontologies/2025/9/geodata#Geodataset_series">
        <rdfs:subClassOf rdf:resource="http://www.w3.org/ns/dcat#DatasetSeries"/>
    </owl:Class>
    


    <!-- http://www.semanticweb.org/bbucher/ontologies/2025/9/geodata#Representation -->


    <owl:Class rdf:about="http://www.semanticweb.org/bbucher/ontologies/2025/9/geodata#Representation">
        <rdfs:comment>Cette classe décrit la représentation d&apos;un concept dans un jeu de données, dans un schéma de données, dans une collection. Elle permet de faire le lien entre des données et des concepts. C&apos;est une classe plutôt qu&apos;une propriété pour permettre de plus facilement lui ajouter des propriétés qui précisent le mode de représentation, par exemple si un jeu ReseauDeMobilité comporte des instances de réseaux de mobilité ou alors représente globalement un réseau de mobilité.</rdfs:comment>
    </owl:Class>
    


    <!-- http://www.w3.org/2004/02/skos/core#Collection -->


    <owl:Class rdf:about="http://www.w3.org/2004/02/skos/core#Collection">
        <owl:disjointWith rdf:resource="http://www.w3.org/2004/02/skos/core#Concept"/>
        <owl:disjointWith rdf:resource="http://www.w3.org/2004/02/skos/core#ConceptScheme"/>
        <rdfs:isDefinedBy rdf:resource="http://www.w3.org/2004/02/skos/core"/>
        <rdfs:label xml:lang="en">Collection</rdfs:label>
        <skos:definition xml:lang="en">A meaningful collection of concepts.</skos:definition>
        <skos:scopeNote xml:lang="en">Labelled collections can be used where you would like a set of concepts to be displayed under a &apos;node label&apos; in the hierarchy.</skos:scopeNote>
    </owl:Class>
    


    <!-- http://www.w3.org/2004/02/skos/core#Concept -->


    <owl:Class rdf:about="http://www.w3.org/2004/02/skos/core#Concept">
        <owl:disjointWith rdf:resource="http://www.w3.org/2004/02/skos/core#ConceptScheme"/>
        <rdfs:isDefinedBy rdf:resource="http://www.w3.org/2004/02/skos/core"/>
        <rdfs:label xml:lang="en">Concept</rdfs:label>
        <skos:definition xml:lang="en">An idea or notion; a unit of thought.</skos:definition>
    </owl:Class>
    


    <!-- http://www.w3.org/2004/02/skos/core#ConceptScheme -->


    <owl:Class rdf:about="http://www.w3.org/2004/02/skos/core#ConceptScheme">
        <rdfs:isDefinedBy rdf:resource="http://www.w3.org/2004/02/skos/core"/>
        <rdfs:label xml:lang="en">Concept Scheme</rdfs:label>
        <skos:definition xml:lang="en">A set of concepts, optionally including statements about semantic relationships between those concepts.</skos:definition>
        <skos:example xml:lang="en">Thesauri, classification schemes, subject heading lists, taxonomies, &apos;folksonomies&apos;, and other types of controlled vocabulary are all examples of concept schemes. Concept schemes are also embedded in glossaries and terminologies.</skos:example>
        <skos:scopeNote xml:lang="en">A concept scheme may be defined to include concepts from different sources.</skos:scopeNote>
    </owl:Class>
    


    <!-- http://www.w3.org/2004/02/skos/core#OrderedCollection -->


    <owl:Class rdf:about="http://www.w3.org/2004/02/skos/core#OrderedCollection">
        <rdfs:subClassOf rdf:resource="http://www.w3.org/2004/02/skos/core#Collection"/>
        <rdfs:isDefinedBy rdf:resource="http://www.w3.org/2004/02/skos/core"/>
        <rdfs:label xml:lang="en">Ordered Collection</rdfs:label>
        <skos:definition xml:lang="en">An ordered collection of concepts, where both the grouping and the ordering are meaningful.</skos:definition>
        <skos:scopeNote xml:lang="en">Ordered collections can be used where you would like a set of concepts to be displayed in a specific order, and optionally under a &apos;node label&apos;.</skos:scopeNote>
    </owl:Class>
    


    <!-- http://www.w3.org/2006/time#Instant -->


    <owl:Class rdf:about="http://www.w3.org/2006/time#Instant"/>
    


    <!-- http://www.w3.org/2006/time#Interval -->


    <owl:Class rdf:about="http://www.w3.org/2006/time#Interval"/>
    


    <!-- http://www.w3.org/ns/dcat#Catalog -->


    <owl:Class rdf:about="http://www.w3.org/ns/dcat#Catalog">
        <rdfs:subClassOf rdf:resource="http://www.w3.org/ns/dcat#Dataset"/>
        <rdfs:comment xml:lang="en">A curated collection of metadata about resources (e.g., datasets and data services in the context of a data catalog).</rdfs:comment>
        <rdfs:comment xml:lang="da">En udvalgt og arrangeret samling af metadata om ressourcer (fx datasæt og datatjenester i kontekst af et datakatalog). </rdfs:comment>
        <rdfs:comment xml:lang="es">Una colección curada de metadatos sobre recursos (por ejemplo, conjuntos de datos y servicios de datos en el contexto de un catálogo de datos).</rdfs:comment>
        <rdfs:comment xml:lang="it">Una raccolta curata di metadati sulle risorse (ad es. sui dataset e relativi servizi nel contesto di cataloghi di dati).</rdfs:comment>
        <rdfs:comment xml:lang="fr">Une collection élaborée de métadonnées sur les jeux de données</rdfs:comment>
        <rdfs:comment xml:lang="cs">Řízená kolekce metadat o datových sadách a datových službách</rdfs:comment>
        <rdfs:comment xml:lang="el">Μια επιμελημένη συλλογή μεταδεδομένων περί συνόλων δεδομένων</rdfs:comment>
        <rdfs:comment xml:lang="ar">مجموعة من توصيفات قوائم البيانات</rdfs:comment>
        <rdfs:comment xml:lang="ja">データ・カタログは、データセットに関するキュレートされたメタデータの集合です。</rdfs:comment>
        <rdfs:isDefinedBy rdf:resource="http://www.w3.org/TR/vocab-dcat/"/>
        <rdfs:label xml:lang="en">Catalog</rdfs:label>
        <rdfs:label xml:lang="it">Catalogo</rdfs:label>
        <rdfs:label xml:lang="fr">Catalogue</rdfs:label>
        <rdfs:label xml:lang="es">Catálogo</rdfs:label>
        <rdfs:label xml:lang="cs">Katalog</rdfs:label>
        <rdfs:label xml:lang="da">Katalog</rdfs:label>
        <rdfs:label xml:lang="el">Κατάλογος</rdfs:label>
        <rdfs:label xml:lang="ar">فهرس قوائم البيانات</rdfs:label>
        <rdfs:label xml:lang="ja">カタログ</rdfs:label>
        <skos:definition xml:lang="en">A curated collection of metadata about resources.</skos:definition>
        <skos:definition xml:lang="da">En samling af metadata om ressourcer.</skos:definition>
        <skos:definition xml:lang="es">Una colección curada de metadatos sobre recursos.</skos:definition>
        <skos:definition xml:lang="it">Una raccolta curata di metadati sulle risorse.</skos:definition>
        <skos:definition xml:lang="fr">Une collection élaborée de métadonnées sur les jeux de données.</skos:definition>
        <skos:definition xml:lang="cs">Řízená kolekce metadat o datových sadách a datových službách.</skos:definition>
        <skos:definition xml:lang="el">Μια επιμελημένη συλλογή μεταδεδομένων περί συνόλων δεδομένων.</skos:definition>
        <skos:definition xml:lang="ar">مجموعة من توصيفات قوائم البيانات</skos:definition>
        <skos:definition xml:lang="ja">データ・カタログは、データセットに関するキュレートされたメタデータの集合です。</skos:definition>
        <skos:editorialNote xml:lang="en">Multilingual text not completelly updated. Translations for skos:scopeNote and definitions to doublecheck.</skos:editorialNote>
        <skos:scopeNote xml:lang="en">A web-based data catalog is typically represented as a single instance of this class.</skos:scopeNote>
        <skos:scopeNote xml:lang="en">Datasets and data services are examples of resources in the context of a data catalog.</skos:scopeNote>
        <skos:scopeNote xml:lang="da">Et webbaseret datakatalog repræsenteres typisk ved en enkelt instans af denne klasse.</skos:scopeNote>
        <skos:scopeNote xml:lang="it">Normalmente, un catalogo di dati nel web viene rappresentato come una singola istanza di questa classe.</skos:scopeNote>
        <skos:scopeNote xml:lang="es">Normalmente, un catálogo de datos disponible en la web se representa como una única instancia de esta clase.</skos:scopeNote>
        <skos:scopeNote xml:lang="cs">Webový datový katalog je typicky reprezentován jako jedna instance této třídy.</skos:scopeNote>
        <skos:scopeNote xml:lang="el">Συνήθως, ένας κατάλογος δεδομένων στον Παγκόσμιο Ιστό αναπαρίσταται ως ένα στιγμιότυπο αυτής της κλάσης.</skos:scopeNote>
        <skos:scopeNote xml:lang="ja">通常、ウェブ・ベースのデータ・カタログは、このクラスの1つのインスタンスとして表わされます。</skos:scopeNote>
    </owl:Class>
    


    <!-- http://www.w3.org/ns/dcat#CatalogRecord -->


    <owl:Class rdf:about="http://www.w3.org/ns/dcat#CatalogRecord">
        <rdfs:subClassOf>
            <owl:Restriction>
                <owl:onProperty rdf:resource="http://xmlns.com/foaf/0.1/primaryTopic"/>
                <owl:allValuesFrom rdf:resource="http://www.w3.org/ns/dcat#Resource"/>
            </owl:Restriction>
        </rdfs:subClassOf>
        <rdfs:subClassOf>
            <owl:Restriction>
                <owl:onProperty rdf:resource="http://xmlns.com/foaf/0.1/primaryTopic"/>
                <owl:cardinality rdf:datatype="http://www.w3.org/2001/XMLSchema#nonNegativeInteger">1</owl:cardinality>
            </owl:Restriction>
        </rdfs:subClassOf>
        <rdfs:comment xml:lang="ja">1つのデータセットを記述したデータ・カタログ内のレコード。</rdfs:comment>
        <rdfs:comment xml:lang="en">A record in a data catalog, describing the registration of a single dataset or data service.</rdfs:comment>
        <rdfs:comment xml:lang="da">En post i et datakatalog der beskriver registreringen af et enkelt datasæt eller en datatjeneste.</rdfs:comment>
        <rdfs:comment xml:lang="it">Un record in un catalogo di dati che descrive un singolo dataset o servizio di dati.</rdfs:comment>
        <rdfs:comment xml:lang="fr">Un registre du catalogue ou une entrée du catalogue, décrivant un seul jeu de données.</rdfs:comment>
        <rdfs:comment xml:lang="es">Un registro en un catálogo de datos que describe un solo conjunto de datos o un servicio de datos.</rdfs:comment>
        <rdfs:comment xml:lang="cs">Záznam v datovém katalogu popisující jednu datovou sadu či datovou službu.</rdfs:comment>
        <rdfs:comment xml:lang="el">Μία καταγραφή ενός καταλόγου, η οποία περιγράφει ένα συγκεκριμένο σύνολο δεδομένων.</rdfs:comment>
        <rdfs:isDefinedBy rdf:resource="http://www.w3.org/TR/vocab-dcat/"/>
        <rdfs:label xml:lang="en">Catalog Record</rdfs:label>
        <rdfs:label xml:lang="cs">Katalogizační záznam</rdfs:label>
        <rdfs:label xml:lang="da">Katalogpost</rdfs:label>
        <rdfs:label xml:lang="it">Record di catalogo</rdfs:label>
        <rdfs:label xml:lang="fr">Registre du catalogue</rdfs:label>
        <rdfs:label xml:lang="es">Registro del catálogo</rdfs:label>
        <rdfs:label xml:lang="el">Καταγραφή καταλόγου</rdfs:label>
        <rdfs:label xml:lang="ar">سجل</rdfs:label>
        <rdfs:label xml:lang="ja">カタログ・レコード</rdfs:label>
        <skos:definition xml:lang="ja">1つのデータセットを記述したデータ・カタログ内のレコード。</skos:definition>
        <skos:definition xml:lang="en">A record in a data catalog, describing the registration of a single dataset or data service.</skos:definition>
        <skos:definition xml:lang="da">En post i et datakatalog der beskriver registreringen af et enkelt datasæt eller en datatjeneste.</skos:definition>
        <skos:definition xml:lang="it">Un record in un catalogo di dati che descrive un singolo dataset o servizio di dati.</skos:definition>
        <skos:definition xml:lang="fr">Un registre du catalogue ou une entrée du catalogue, décrivant un seul jeu de données.</skos:definition>
        <skos:definition xml:lang="es">Un registro en un catálogo de datos que describe un solo conjunto de datos o un servicio de datos.</skos:definition>
        <skos:definition xml:lang="cs">Záznam v datovém katalogu popisující jednu datovou sadu či datovou službu.</skos:definition>
        <skos:definition xml:lang="el">Μία καταγραφή ενός καταλόγου, η οποία περιγράφει ένα συγκεκριμένο σύνολο δεδομένων.</skos:definition>
        <skos:editorialNote xml:lang="en">English definition updated in this revision. Multilingual text not yet updated except the Spanish one and the Czech one and Italian one.</skos:editorialNote>
        <skos:scopeNote xml:lang="fr">C&apos;est une classe facultative et tous les catalogues ne l&apos;utiliseront pas. Cette classe existe pour les catalogues	ayant une distinction entre les métadonnées sur le jeu de données et les métadonnées sur une entrée du jeu de données dans le catalogue.</skos:scopeNote>
        <skos:scopeNote xml:lang="da">Denne klasse er valgfri og ikke alle kataloger vil anvende denne klasse. Den kan anvendes i de kataloger hvor der skelnes mellem metadata om datasættet eller datatjenesten og metadata om selve posten til registreringen af datasættet eller datatjenesten i kataloget. Udgivelsesdatoen for datasættet afspejler for eksempel den dato hvor informationerne oprindeligt blev gjort tilgængelige af udgiveren, hvorimod udgivelsesdatoen for katalogposten er den dato hvor datasættet blev føjet til kataloget. I de tilfælde hvor de to datoer er forskellige eller hvor blot sidstnævnte er kendt, bør udgivelsesdatoen kun angives for katalogposten. Bemærk at W3Cs PROV ontologi gør til muligt at tilføje yderligere proveniensoplysninger eksempelvis om processen eller aktøren involveret i en given ændring af datasættet.</skos:scopeNote>
        <skos:scopeNote xml:lang="es">Esta clase es opcional y no todos los catálogos la utilizarán. Esta clase existe para catálogos que hacen una distinción entre los metadatos acerca de un conjunto de datos o un servicio de datos y los metadatos acerca de una entrada en ese conjunto de datos en el catálogo. Por ejemplo, la propiedad sobre la fecha de la publicación de los datos refleja la fecha en que la información fue originalmente publicada, mientras que la fecha de publicación del registro del catálogo es la fecha en que los datos se agregaron al mismo. En caso en que ambas fechas fueran diferentes, o en que sólo la fecha de publicación del registro del catálogo estuviera disponible, sólo debe especificarse en el registro del catálogo. Tengan en cuenta que la ontología PROV de W3C permite describir otra información sobre la proveniencia de los datos, como por ejemplo detalles del proceso y de los agentes involucrados en algún cambio específico a los datos.</skos:scopeNote>
        <skos:scopeNote xml:lang="it">Questa classe è opzionale e non tutti i cataloghi la utilizzeranno. Esiste per cataloghi in cui si opera una distinzione tra i metadati relativi al dataset ed i metadati relativi alla gestione del dataset nel catalogo. Ad esempio, la  proprietà per indicare la data di pubblicazione del dataset rifletterà la data in cui l&apos;informazione è stata originariamente messa a disposizione dalla casa editrice, mentre la data di pubblicazione per il record nel catalogo rifletterà la data in cui il dataset è stato aggiunto al catalogo. Nei casi dove solo quest&apos;ultima sia nota, si utilizzerà esclusivamente la data di  pubblicazione relativa al record del catalogo. Si noti che l&apos;Ontologia W3C PROV permette di descrivere ulteriori informazioni sulla provenienza, quali i dettagli del processo, la procedura e l&apos;agente coinvolto in una particolare modifica di un dataset.</skos:scopeNote>
        <skos:scopeNote xml:lang="cs">Tato třída je volitelná a ne všechny katalogy ji využijí. Existuje pro katalogy, ve kterých se rozlišují metadata datové sady či datové služby a metadata o záznamu o datové sadě či datové službě v katalogu. Například datum publikace datové sady odráží datum, kdy byla datová sada původně zveřejněna poskytovatelem dat, zatímco datum publikace katalogizačního záznamu je datum zanesení datové sady do katalogu. V případech kdy se obě data liší, nebo je známo jen to druhé, by mělo být specifikováno jen datum publikace katalogizačního záznamu. Všimněte si, že ontologie W3C PROV umožňuje popsat další informace o původu jako například podrobnosti o procesu konkrétní změny datové sady a jeho účastnících.</skos:scopeNote>
        <skos:scopeNote xml:lang="en">This class is optional and not all catalogs will use it. It exists for catalogs where a distinction is made between metadata about a dataset or data service and metadata about the entry for the dataset or data service in the catalog. For example, the publication date property of the dataset reflects the date when the information was originally made available by the publishing agency, while the publication date of the catalog record is the date when the dataset was added to the catalog. In cases where both dates differ, or where only the latter is known, the publication date should only be specified for the catalog record. Notice that the W3C PROV Ontology allows describing further provenance information such as the details of the process and the agent involved in a particular change to a dataset.</skos:scopeNote>
        <skos:scopeNote xml:lang="el">Αυτή η κλάση είναι προαιρετική και δεν χρησιμοποιείται από όλους τους καταλόγους. Υπάρχει για τις περιπτώσεις καταλόγων όπου γίνεται διαχωρισμός μεταξύ των μεταδεδομένων για το σύνολο των δεδομένων και των μεταδεδομένων για την καταγραφή του συνόλου δεδομένων εντός του καταλόγου. Για παράδειγμα, η ιδιότητα της ημερομηνίας δημοσίευσης του συνόλου δεδομένων δείχνει την ημερομηνία κατά την οποία οι πληροφορίες έγιναν διαθέσιμες από τον φορέα δημοσίευσης, ενώ η ημερομηνία δημοσίευσης της καταγραφής του καταλόγου δείχνει την ημερομηνία που το σύνολο δεδομένων προστέθηκε στον κατάλογο. Σε περιπτώσεις που οι δύο ημερομηνίες διαφέρουν, ή που μόνο η τελευταία είναι γνωστή, η ημερομηνία δημοσίευσης θα πρέπει να δίνεται για την καταγραφή του καταλόγου. Να σημειωθεί πως η οντολογία W3C PROV επιτρέπει την περιγραφή επιπλέον πληροφοριών ιστορικού όπως λεπτομέρειες για τη διαδικασία και τον δράστη που εμπλέκονται σε μία συγκεκριμένη αλλαγή εντός του συνόλου δεδομένων.</skos:scopeNote>
        <skos:scopeNote xml:lang="ja">このクラスはオプションで、すべてのカタログがそれを用いるとは限りません。これは、データセットに関するメタデータとカタログ内のデータセットのエントリーに関するメタデータとで区別が行われるカタログのために存在しています。例えば、データセットの公開日プロパティーは、公開機関が情報を最初に利用可能とした日付を示しますが、カタログ・レコードの公開日は、データセットがカタログに追加された日付です。両方の日付が異っていたり、後者だけが分かっている場合は、カタログ・レコードに対してのみ公開日を指定すべきです。W3CのPROVオントロジー[prov-o]を用いれば、データセットに対する特定の変更に関連するプロセスやエージェントの詳細などの、さらに詳しい来歴情報の記述が可能となることに注意してください。</skos:scopeNote>
    </owl:Class>
    


    <!-- http://www.w3.org/ns/dcat#DataService -->


    <owl:Class rdf:about="http://www.w3.org/ns/dcat#DataService">
        <rdfs:subClassOf rdf:resource="http://purl.org/dc/dcmitype/Service"/>
        <rdfs:subClassOf rdf:resource="http://www.w3.org/ns/dcat#Resource"/>
        <rdfs:comment xml:lang="en">A site or end-point providing operations related to the discovery of, access to, or processing functions on, data or related resources.</rdfs:comment>
        <rdfs:comment xml:lang="da">Et websted eller endpoint der udstiller operationer relateret til opdagelse af, adgang til eller behandlende funktioner på data eller relaterede ressourcer.</rdfs:comment>
        <rdfs:comment xml:lang="cs">Umístění či přístupový bod poskytující operace související s hledáním, přistupem k, či výkonem funkcí na datech či souvisejících zdrojích.</rdfs:comment>
        <rdfs:comment xml:lang="es">Un sitio o end-point que provee operaciones relacionadas a funciones de descubrimiento, acceso, o procesamiento de datos o recursos relacionados.</rdfs:comment>
        <rdfs:comment xml:lang="it">Un sito o end-point che fornisce operazioni relative alla scoperta, all&apos;accesso o all&apos;elaborazione di funzioni su dati o risorse correlate.</rdfs:comment>
        <rdfs:label xml:lang="en">Data service</rdfs:label>
        <rdfs:label xml:lang="da">Datatjeneste</rdfs:label>
        <rdfs:label xml:lang="es">Servicio de datos</rdfs:label>
        <rdfs:label xml:lang="it">Servizio di dati</rdfs:label>
        <skos:altLabel xml:lang="da">Dataservice</skos:altLabel>
        <skos:changeNote xml:lang="en">New class added in DCAT 2.</skos:changeNote>
        <skos:changeNote xml:lang="cs">Nová třída přidaná ve verzi DCAT 2.</skos:changeNote>
        <skos:changeNote xml:lang="es">Nueva clase añadida en DCAT 2.</skos:changeNote>
        <skos:changeNote xml:lang="it">Nuova classe aggiunta in DCAT 2.</skos:changeNote>
        <skos:changeNote xml:lang="da">Ny klasse tilføjet i DCAT 2.</skos:changeNote>
        <skos:definition xml:lang="en">A site or end-point providing operations related to the discovery of, access to, or processing functions on, data or related resources.</skos:definition>
        <skos:definition xml:lang="da">Et site eller endpoint der udstiller operationer relateret til opdagelse af, adgang til eller behandlende funktioner på data eller relaterede ressourcer.</skos:definition>
        <skos:definition xml:lang="cs">Umístění či přístupový bod poskytující operace související s hledáním, přistupem k, či výkonem funkcí na datech či souvisejících zdrojích.</skos:definition>
        <skos:definition xml:lang="es">Un sitio o end-point que provee operaciones relacionadas a funciones de descubrimiento, acceso, o procesamiento de datos o recursos relacionados.</skos:definition>
        <skos:definition xml:lang="it">Un sito o end-point che fornisce operazioni relative alla scoperta, all&apos;accesso o all&apos;elaborazione di funzioni su dati o risorse correlate.</skos:definition>
        <skos:scopeNote xml:lang="da">Datatjenestetypen kan indikeres ved hjælp af egenskaben dcterms:type. Værdien kan tages fra kontrollerede udfaldsrum såsom INSPIRE spatial data service vocabulary.</skos:scopeNote>
        <skos:scopeNote xml:lang="cs">Druh služby může být indikován vlastností dcterms:type. Její hodnota může být z řízeného slovníku, kterým je například slovník typů prostorových datových služeb INSPIRE.</skos:scopeNote>
        <skos:scopeNote xml:lang="es">El tipo de servicio puede indicarse usando la propiedad dcterms:type. Su valor puede provenir de un vocabulario controlado, como por ejemplo el vocabulario de servicios de datos espaciales de INSPIRE.</skos:scopeNote>
        <skos:scopeNote xml:lang="da">Hvis en dcat:DataService er bundet til en eller flere specifikke datasæt kan dette indikeres ved hjælp af egenskaben dcat:servesDataset. </skos:scopeNote>
        <skos:scopeNote xml:lang="en">If a dcat:DataService is bound to one or more specified Datasets, they are indicated by the dcat:servesDataset property.</skos:scopeNote>
        <skos:scopeNote xml:lang="it">Il tipo di servizio può essere indicato usando la proprietà dcterms:type. Il suo valore può essere preso da un vocabolario controllato come il vocabolario dei tipi di servizi per dati spaziali di INSPIRE.</skos:scopeNote>
        <skos:scopeNote xml:lang="cs">Pokud je dcat:DataService navázána na jednu či více Datových sad, jsou tyto indikovány vlstností dcat:servesDataset.</skos:scopeNote>
        <skos:scopeNote xml:lang="it">Se un dcat:DataService è associato a uno o più Dataset specificati, questi sono indicati dalla proprietà dcat:serveDataset.</skos:scopeNote>
        <skos:scopeNote xml:lang="es">Si un dcat:DataService está asociado con uno o más conjuntos de datos especificados, dichos conjuntos de datos pueden indicarse con la propiedad dcat:servesDataset.</skos:scopeNote>
        <skos:scopeNote xml:lang="en">The kind of service can be indicated using the dcterms:type property. Its value may be taken from a controlled vocabulary such as the INSPIRE spatial data service type vocabulary.</skos:scopeNote>
    </owl:Class>
    


    <!-- http://www.w3.org/ns/dcat#Dataset -->


    <owl:Class rdf:about="http://www.w3.org/ns/dcat#Dataset">
        <rdfs:subClassOf rdf:resource="http://www.w3.org/ns/dcat#Resource"/>
        <rdfs:comment xml:lang="ja">1つのエージェントによって公開またはキュレートされ、1つ以上の形式でアクセスまたはダウンロードできるデータの集合。</rdfs:comment>
        <rdfs:comment xml:lang="en">A collection of data, published or curated by a single source, and available for access or download in one or more representations.</rdfs:comment>
        <rdfs:comment xml:lang="da">En samling af data, udgivet eller udvalgt og arrangeret af en enkelt kilde og som er til råde for adgang til eller download af i en eller flere repræsentationer.</rdfs:comment>
        <rdfs:comment xml:lang="cs">Kolekce dat poskytovaná či řízená jedním zdrojem, která je k dispozici pro přístup či stažení v jednom či více formátech.</rdfs:comment>
        <rdfs:comment xml:lang="it">Raccolta di dati, pubblicati o curati da un&apos;unica fonte, disponibili per l&apos;accesso o il download in uno o più formati.</rdfs:comment>
        <rdfs:comment xml:lang="es">Una colección de datos, publicados o conservados por una única fuente, y disponibles para ser accedidos o descargados en uno o más formatos.</rdfs:comment>
        <rdfs:comment xml:lang="fr">Une collection de données, publiée ou élaborée par une seule source, et disponible pour accès ou téléchargement dans un ou plusieurs formats.</rdfs:comment>
        <rdfs:comment xml:lang="el">Μία συλλογή από δεδομένα, δημοσιευμένη ή επιμελημένη από μία και μόνο πηγή, διαθέσιμη δε προς πρόσβαση ή μεταφόρτωση σε μία ή περισσότερες μορφές.</rdfs:comment>
        <rdfs:comment xml:lang="ar">قائمة بيانات منشورة أو مجموعة من قبل مصدر ما و متاح الوصول إليها أو تحميلها</rdfs:comment>
        <rdfs:isDefinedBy rdf:resource="http://www.w3.org/TR/vocab-dcat/"/>
        <rdfs:label xml:lang="es">Conjunto de datos</rdfs:label>
        <rdfs:label xml:lang="en">Dataset</rdfs:label>
        <rdfs:label xml:lang="it">Dataset</rdfs:label>
        <rdfs:label xml:lang="da">Datasæt</rdfs:label>
        <rdfs:label xml:lang="cs">Datová sada</rdfs:label>
        <rdfs:label xml:lang="fr">Jeu de données</rdfs:label>
        <rdfs:label xml:lang="el">Σύνολο Δεδομένων</rdfs:label>
        <rdfs:label xml:lang="ar">قائمة بيانات</rdfs:label>
        <rdfs:label xml:lang="ja">データセット</rdfs:label>
        <skos:altLabel xml:lang="da">Datasamling</skos:altLabel>
        <skos:changeNote xml:lang="cs">2018-02 - odstraněno tvrzení o podtřídě dctype:Dataset, jelikož rozsah dcat:Dataset zahrnuje několik dalších typů ze slovníku dctype.</skos:changeNote>
        <skos:changeNote xml:lang="es">2018-02 - se eliminó el axioma de subclase con dctype:Dataset porque el alcance de dcat:Dataset incluye muchos otros tipos del vocabulario dctype.</skos:changeNote>
        <skos:changeNote xml:lang="it">2018-02 - sottoclasse di dctype:Dataset rimosso perché l&apos;ambito di dcat:Dataset include diversi altri tipi dal vocabolario dctype.</skos:changeNote>
        <skos:changeNote xml:lang="en">2018-02 - subclass of dctype:Dataset removed because scope of dcat:Dataset includes several other types from the dctype vocabulary.</skos:changeNote>
        <skos:changeNote xml:lang="da">2018-02 - subklasse af dctype:Dataset fjernet da scope af dcat:Dataset omfatter flere forskellige typer fra dctype-vokabularet.</skos:changeNote>
        <skos:definition xml:lang="ja">1つのエージェントによって公開またはキュレートされ、1つ以上の形式でアクセスまたはダウンロードできるデータの集合。</skos:definition>
        <skos:definition xml:lang="en">A collection of data, published or curated by a single source, and available for access or download in one or more representations.</skos:definition>
        <skos:definition xml:lang="da">En samling a data, udgivet eller udvalgt og arrangeret af en enkelt kilde og som der er adgang til i en eller flere repræsentationer.</skos:definition>
        <skos:definition xml:lang="cs">Kolekce dat poskytovaná či řízená jedním zdrojem, která je k dispozici pro přístup či stažení v jednom či více formátech.</skos:definition>
        <skos:definition xml:lang="it">Raccolta di dati, pubblicati o curati da un&apos;unica fonte, disponibili per l&apos;accesso o il download in uno o più formati.</skos:definition>
        <skos:definition xml:lang="es">Una colección de datos, publicados o conservados por una única fuente, y disponibles para ser accedidos o descargados en uno o más formatos.</skos:definition>
        <skos:definition xml:lang="fr">Une collection de données, publiée ou élaborée par une seule source, et disponible pour accès ou téléchargement dans un ou plusieurs formats.</skos:definition>
        <skos:definition xml:lang="el">Μία συλλογή από δεδομένα, δημοσιευμένη ή επιμελημένη από μία και μόνο πηγή, διαθέσιμη δε προς πρόσβαση ή μεταφόρτωση σε μία ή περισσότερες μορφές.</skos:definition>
        <skos:definition xml:lang="ar">قائمة بيانات منشورة أو مجموعة من قبل مصدر ما و متاح الوصول إليها أو تحميلها</skos:definition>
        <skos:editorialNote xml:lang="en">2020-03-16 A new scopenote added and need to be translated</skos:editorialNote>
        <skos:scopeNote xml:lang="fr">Cette classe représente le jeu de données publié par le fournisseur de données. Dans les cas où une distinction est nécessaire entre le jeu de donénes et son entrée dans le catalogue, la classe registre de données peut être utilisée pour ce dernier.</skos:scopeNote>
        <skos:scopeNote xml:lang="da">Denne klasse beskriver det konceptuelle datasæt. En eller flere repræsentationer kan være tilgængelige med forskellige skematiske opsætninger, formater eller serialiseringer.</skos:scopeNote>
        <skos:scopeNote xml:lang="da">Denne klasse repræsenterer det konkrete datasæt som det udgives af datasætleverandøren. I de tilfælde hvor det er nødvendigt at skelne mellem det konkrete datasæt og dets registrering i kataloget (fordi metadata såsom ændringsdato og vedligeholder er forskellige), så kan klassen katalogpost anvendes. </skos:scopeNote>
        <skos:scopeNote xml:lang="es">Esta clase representa el conjunto de datos publicados. En los casos donde es necesario distinguir entre el conjunto de datos y su entrada en el catálogo de datos, se debe utilizar la clase &apos;registro del catálogo&apos;.</skos:scopeNote>
        <skos:scopeNote xml:lang="it">Questa classe descrive il dataset dal punto di vista concettuale. Possono essere disponibili una o più rappresentazioni, con diversi layout e formati schematici o serializzazioni.</skos:scopeNote>
        <skos:scopeNote xml:lang="it">Questa classe rappresenta il dataset come pubblicato dall’editore. Nel caso in cui sia necessario operare  una distinzione fra i metadati originali del dataset e il record dei metadati ad esso associato nel catalogo (ad esempio, per distinguere la data di modifica del dataset da quella del dataset nel catalogo) si può impiegare la classe catalog record.</skos:scopeNote>
        <skos:scopeNote xml:lang="cs">Tato třída reprezentuje datovou sadu tak, jak je publikována poskytovatelem dat. V případě potřeby rozlišení datové sady a jejího katalogizačního záznamu (jelikož metadata jako datum modifikace se mohou lišit) pro něj může být použita třída &quot;katalogizační záznam&quot;.</skos:scopeNote>
        <skos:scopeNote xml:lang="en">The notion of dataset in DCAT is broad and inclusive, with the intention of accommodating resource types arising from all communities. Data comes in many forms including numbers, text, pixels, imagery, sound and other multi-media, and potentially other types, any of which might be collected into a dataset.</skos:scopeNote>
        <skos:scopeNote xml:lang="en">This class describes the conceptual dataset. One or more representations might be available, with differing schematic layouts and formats or serializations.</skos:scopeNote>
        <skos:scopeNote xml:lang="en">This class represents the actual dataset as published by the dataset provider. In cases where a distinction between the actual dataset and its entry in the catalog is necessary (because metadata such as modification date and maintainer might differ), the catalog record class can be used for the latter.</skos:scopeNote>
        <skos:scopeNote xml:lang="el">Η κλάση αυτή αναπαριστά το σύνολο δεδομένων αυτό καθ&apos;εαυτό, όπως έχει δημοσιευθεί από τον εκδότη. Σε περιπτώσεις όπου είναι απαραίτητος ο διαχωρισμός μεταξύ του συνόλου δεδομένων και της καταγραφής αυτού στον κατάλογο (γιατί μεταδεδομένα όπως η ημερομηνία αλλαγής και ο συντηρητής μπορεί να διαφέρουν) η κλάση της καταγραφής καταλόγου μπορεί να χρησιμοποιηθεί για το τελευταίο.</skos:scopeNote>
        <skos:scopeNote xml:lang="ja">このクラスは、データセットの公開者が公開する実際のデータセットを表わします。カタログ内の実際のデータセットとそのエントリーとの区別が必要な場合（修正日と維持者などのメタデータが異なるかもしれないので）は、後者にcatalog recordというクラスを使用できます。</skos:scopeNote>
    </owl:Class>
    


    <!-- http://www.w3.org/ns/dcat#DatasetSeries -->


    <owl:Class rdf:about="http://www.w3.org/ns/dcat#DatasetSeries">
        <rdfs:subClassOf rdf:resource="http://www.w3.org/ns/dcat#Dataset"/>
        <rdfs:comment xml:lang="en">A collection of datasets that are published separately, but share some characteristics that group them.</rdfs:comment>
        <rdfs:comment xml:lang="es">Una colección de conjuntos de datos publicados por separado, pero que comparten características que los agrupan.</rdfs:comment>
        <rdfs:comment xml:lang="it">Una collezione di dataset che sono pubblicati separatamente, ma che condividono caratteristiche che li rendono parte di uno stesso gruppo.</rdfs:comment>
        <rdfs:isDefinedBy rdf:resource="https://www.w3.org/TR/vocab-dcat-3/"/>
        <rdfs:label xml:lang="en">Dataset series</rdfs:label>
        <rdfs:label xml:lang="es">Serie de conjuntos de datos</rdfs:label>
        <rdfs:label xml:lang="it">Serie di dataset</rdfs:label>
        <skos:changeNote xml:lang="en">New class added in DCAT 3.</skos:changeNote>
        <skos:changeNote xml:lang="cs">Nová třída přidaná ve verzi DCAT 3</skos:changeNote>
        <skos:changeNote xml:lang="es">Nueva clase agregada en DCAT 3.</skos:changeNote>
        <skos:changeNote xml:lang="it">Nuova classe aggiunta in DCAT 3</skos:changeNote>
        <skos:changeNote xml:lang="da">Ny klasse tilføjet i DCAT 3</skos:changeNote>
        <skos:definition xml:lang="en">A collection of datasets that are published separately, but share some common characteristics that groups them.</skos:definition>
        <skos:definition xml:lang="es">Una colección de conjuntos de datos publicados por separado, pero que comparten características comunes que los agrupan.</skos:definition>
        <skos:definition xml:lang="it">Una collezione di dataset che sono pubblicati separatamente, ma che condividono caratteristiche che li rendono parte di uno stesso gruppo.</skos:definition>
        <skos:editorialNote xml:lang="en">2022-05-08 Added to ttl file with annotations in English, Spanish and Italian, except notes that are in other languages too.</skos:editorialNote>
        <skos:scopeNote xml:lang="es">Algunos escenarios comunes para series de conjuntos de datos son: series temporales compuestas de subconjuntos de datos publicados periódicamente; series de mapas compuestos de elementos del mismo tipo o tema pero con distintas huellas espaciales.</skos:scopeNote>
        <skos:scopeNote xml:lang="en">Common scenarios for dataset series include: time series composed of periodically released subsets; map-series composed of items of the same type or theme but with differing spatial footprints.</skos:scopeNote>
        <skos:scopeNote xml:lang="en">Dataset series can be also soft-typed via property dcterms:type as in the approach used in [GeoDCAT-AP], and adopted in [DCAT-AP-IT] and [GeoDCAT-AP-IT]).</skos:scopeNote>
        <skos:scopeNote xml:lang="it">Le serie di dati possono anche essere denotate come tali usando la proprietà dcterms:type, secondo l&apos;approccio usato in [GeoDCAT-AP], e adottato in [DCAT-AP-IT] e [GeoDCAT-AP-IT]).</skos:scopeNote>
        <skos:scopeNote xml:lang="it">Scenari tipici per l&apos;uso di serie di dataset: serie temporali costituite di dataset pubblicati regolarmente; serie di mappe costituite da elementi dello stesso tipo o tematica ma relative a differenti aree geografiche.</skos:scopeNote>
        <skos:scopeNote xml:lang="es">También puede asignarse un tipo a las series de datos usando la propiedad dcterms:type como se hace en [GeoDCAT-AP], y adoptado en [DCAT-AP-IT] y [GeoDCAT-AP-IT]).</skos:scopeNote>
    </owl:Class>
    


    <!-- http://www.w3.org/ns/dcat#Distribution -->


    <owl:Class rdf:about="http://www.w3.org/ns/dcat#Distribution">
        <rdfs:comment xml:lang="en">A specific representation of a dataset. A dataset might be available in multiple serializations that may differ in various ways, including natural language, media-type or format, schematic organization, temporal and spatial resolution, level of detail or profiles (which might specify any or all of the above).</rdfs:comment>
        <rdfs:comment xml:lang="da">En specifik repræsentation af et datasæt. Et datasæt kan være tilgængelig i mange serialiseringer der kan variere på forskellige vis, herunder sprog, medietype eller format, systemorganisering, tidslig- og geografisk opløsning, detaljeringsniveau eller profiler (der kan specificere en eller flere af ovenstående).</rdfs:comment>
        <rdfs:comment xml:lang="cs">Konkrétní reprezentace datové sady. Datová sada může být dostupná v různých serializacích, které se mohou navzájem lišit různými způsoby, mimo jiné přirozeným jazykem, media-typem či formátem, schematickou organizací, časovým a prostorovým rozlišením, úrovní detailu či profily (které mohou specifikovat některé či všechny tyto rozdíly).</rdfs:comment>
        <rdfs:comment xml:lang="it">Rappresenta una forma disponibile e specifica del dataset. Ciascun dataset può essere disponibile in forme differenti, che possono rappresentare formati diversi o diversi punti di accesso per un dataset. Esempi di distribuzioni sono un file CSV scaricabile, una API o un RSS feed.</rdfs:comment>
        <rdfs:comment xml:lang="fr">Représente une forme spécifique d&apos;un jeu de données. Caque jeu de données peut être disponible sous différentes formes, celles-ci pouvant représenter différents formats du jeu de données ou différents endpoint. Des exemples de distribution sont des fichirs CSV, des API ou des flux RSS.</rdfs:comment>
        <rdfs:comment xml:lang="es">Una representación específica de los datos. Cada conjunto de datos puede estar disponible en formas diferentes, las cuáles pueden variar en distintas formas, incluyendo el idioma, &apos;media-type&apos; o formato, organización esquemática, resolución temporal y espacial, nivel de detalle o perfiles (que pueden especificar cualquiera o todas las diferencias anteriores).</rdfs:comment>
        <rdfs:comment xml:lang="el">Αναπαριστά μία συγκεκριμένη διαθέσιμη μορφή ενός συνόλου δεδομένων. Κάθε σύνολο δεδομενων μπορεί να είναι διαθέσιμο σε διαφορετικές μορφές, οι μορφές αυτές μπορεί να αναπαριστούν διαφορετικές μορφές αρχείων ή διαφορετικά σημεία διάθεσης. Παραδείγματα διανομών συμπεριλαμβάνουν ένα μεταφορτώσιμο αρχείο μορφής CSV, ένα API ή ένα RSS feed.</rdfs:comment>
        <rdfs:comment xml:lang="ar">شكل محدد لقائمة البيانات يمكن الوصول إليه. قائمة بيانات ما يمكن أن تكون متاحه باشكال و أنواع متعددة.  ملف يمكن تحميله أو واجهة برمجية يمكن من خلالها الوصول إلى البيانات هي أمثلة على ذلك.</rdfs:comment>
        <rdfs:comment xml:lang="ja">データセットの特定の利用可能な形式を表わします。各データセットは、異なる形式で利用できることがあり、これらの形式は、データセットの異なる形式や、異なるエンドポイントを表わす可能性があります。配信の例には、ダウンロード可能なCSVファイル、API、RSSフィードが含まれます。</rdfs:comment>
        <rdfs:isDefinedBy rdf:resource="http://www.w3.org/TR/vocab-dcat/"/>
        <rdfs:label xml:lang="cs">Distribuce</rdfs:label>
        <rdfs:label xml:lang="es">Distribución</rdfs:label>
        <rdfs:label xml:lang="da">Distribution</rdfs:label>
        <rdfs:label xml:lang="en">Distribution</rdfs:label>
        <rdfs:label xml:lang="fr">Distribution</rdfs:label>
        <rdfs:label xml:lang="it">Distribuzione</rdfs:label>
        <rdfs:label xml:lang="el">Διανομή</rdfs:label>
        <rdfs:label xml:lang="ar">التوزيع</rdfs:label>
        <rdfs:label xml:lang="ja">配信</rdfs:label>
        <skos:altLabel xml:lang="da">Datadistribution</skos:altLabel>
        <skos:altLabel xml:lang="da">Datamanifestation</skos:altLabel>
        <skos:altLabel xml:lang="da">Datarepræsentation</skos:altLabel>
        <skos:altLabel xml:lang="da">Dataudstilling</skos:altLabel>
        <skos:definition xml:lang="en">A specific representation of a dataset. A dataset might be available in multiple serializations that may differ in various ways, including natural language, media-type or format, schematic organization, temporal and spatial resolution, level of detail or profiles (which might specify any or all of the above).</skos:definition>
        <skos:definition xml:lang="da">En specifik repræsentation af et datasæt. Et datasæt kan være tilgængelig i mange serialiseringer der kan variere på forskellige vis, herunder sprog, medietype eller format, systemorganisering, tidslig- og geografisk opløsning, detaljeringsniveau eller profiler (der kan specificere en eller flere af ovenstående).</skos:definition>
        <skos:definition xml:lang="cs">Konkrétní reprezentace datové sady. Datová sada může být dostupná v různých serializacích, které se mohou navzájem lišit různými způsoby, mimo jiné přirozeným jazykem, media-typem či formátem, schematickou organizací, časovým a prostorovým rozlišením, úrovní detailu či profily (které mohou specifikovat některé či všechny tyto rozdíly).</skos:definition>
        <skos:definition xml:lang="it">Rappresenta una forma disponibile e specifica del dataset. Ciascun dataset può essere disponibile in forme differenti, che possono rappresentare formati diversi o diversi punti di accesso per un dataset. Esempi di distribuzioni sono un file CSV scaricabile, una API o un RSS feed.</skos:definition>
        <skos:definition xml:lang="fr">Représente une forme spécifique d&apos;un jeu de données. Caque jeu de données peut être disponible sous différentes formes, celles-ci pouvant représenter différents formats du jeu de données ou différents endpoint. Des exemples de distribution sont des fichirs CSV, des API ou des flux RSS.</skos:definition>
        <skos:definition xml:lang="es">Una representación específica de los datos. Cada conjunto de datos puede estar disponible en formas diferentes, las cuáles pueden variar en distintas formas, incluyendo el idioma, &apos;media-type&apos; o formato, organización esquemática, resolución temporal y espacial, nivel de detalle o perfiles (que pueden especificar cualquiera o todas las diferencias anteriores).</skos:definition>
        <skos:definition xml:lang="el">Αναπαριστά μία συγκεκριμένη διαθέσιμη μορφή ενός συνόλου δεδομένων. Κάθε σύνολο δεδομενων μπορεί να είναι διαθέσιμο σε διαφορετικές μορφές, οι μορφές αυτές μπορεί να αναπαριστούν διαφορετικές μορφές αρχείων ή διαφορετικά σημεία διάθεσης. Παραδείγματα διανομών συμπεριλαμβάνουν ένα μεταφορτώσιμο αρχείο μορφής CSV, ένα API ή ένα RSS feed.</skos:definition>
        <skos:definition xml:lang="ar">شكل محدد لقائمة البيانات يمكن الوصول إليه. قائمة بيانات ما يمكن أن تكون متاحه باشكال و أنواع متعددة.  ملف يمكن تحميله أو واجهة برمجية يمكن من خلالها الوصول إلى البيانات هي أمثلة على ذلك.</skos:definition>
        <skos:definition xml:lang="ja">データセットの特定の利用可能な形式を表わします。各データセットは、異なる形式で利用できることがあり、これらの形式は、データセットの異なる形式や、異なるエンドポイントを表わす可能性があります。配信の例には、ダウンロード可能なCSVファイル、API、RSSフィードが含まれます。</skos:definition>
        <skos:scopeNote xml:lang="fr">Ceci représente une disponibilité générale du jeu de données, et implique qu&apos;il n&apos;existe pas d&apos;information sur la méthode d&apos;accès réelle des données, par exple, si c&apos;est un lien de téléchargement direct ou à travers une page Web.</skos:scopeNote>
        <skos:scopeNote xml:lang="da">Denne klasse repræsenterer datasættets overordnede tilgængelighed og giver ikke oplysninger om hvilken metode der kan anvendes til at få adgang til data, dvs. om adgang til datasættet realiseres ved direkte download, API eller via et websted. Anvendelsen af egenskaben dcat:downloadURL indikerer at distributionen kan downloades direkte.</skos:scopeNote>
        <skos:scopeNote xml:lang="es">Esta clase representa una disponibilidad general de un conjunto de datos, e implica que no existe información acerca del método de acceso real a los datos, i.e., si es un enlace de descarga directa o a través de una página Web.</skos:scopeNote>
        <skos:scopeNote xml:lang="it">Questa classe rappresenta una disponibilità generale di un dataset e non implica alcuna informazione sul metodo di accesso effettivo ai dati, ad esempio se si tratta di un accesso a download diretto, API, o attraverso una pagina Web. L&apos;utilizzo della proprietà dcat:downloadURL indica distribuzioni direttamente scaricabili.</skos:scopeNote>
        <skos:scopeNote xml:lang="en">This represents a general availability of a dataset it implies no information about the actual access method of the data, i.e. whether by direct download, API, or through a Web page. The use of dcat:downloadURL property indicates directly downloadable distributions.</skos:scopeNote>
        <skos:scopeNote xml:lang="cs">Toto popisuje obecnou dostupnost datové sady. Neimplikuje žádnou informaci o skutečné metodě přístupu k datům, tj. zda jsou přímo ke stažení, skrze API či přes webovou stránku. Použití vlastnosti dcat:downloadURL indikuje přímo stažitelné distribuce.</skos:scopeNote>
        <skos:scopeNote xml:lang="el">Αυτό αναπαριστά μία γενική διαθεσιμότητα ενός συνόλου δεδομένων και δεν υπονοεί τίποτα περί του πραγματικού τρόπου πρόσβασης στα δεδομένα, αν είναι άμεσα μεταφορτώσιμα, μέσω API ή μέσω μίας ιστοσελίδας. Η χρήση της ιδιότητας dcat:downloadURL δείχνει μόνο άμεσα μεταφορτώσιμες διανομές.</skos:scopeNote>
        <skos:scopeNote xml:lang="ja">これは、データセットの一般的な利用可能性を表わし、データの実際のアクセス方式に関する情報（つまり、直接ダウンロードなのか、APIなのか、ウェブページを介したものなのか）を意味しません。dcat:downloadURLプロパティーの使用は、直接ダウンロード可能な配信を意味します。</skos:scopeNote>
    </owl:Class>
    


    <!-- http://www.w3.org/ns/dcat#Relationship -->


    <owl:Class rdf:about="http://www.w3.org/ns/dcat#Relationship">
        <rdfs:comment xml:lang="en">An association class for attaching additional information to a relationship between DCAT Resources.</rdfs:comment>
        <rdfs:comment xml:lang="cs">Asociační třída pro připojení dodatečných informací ke vztahu mezi zdroji DCAT.</rdfs:comment>
        <rdfs:comment xml:lang="da">En associationsklasse til brug for tilknytning af yderligere information til en relation mellem DCAT-ressourcer.</rdfs:comment>
        <rdfs:comment xml:lang="es">Una clase de asociación para adjuntar información adicional a una relación entre recursos DCAT.</rdfs:comment>
        <rdfs:comment xml:lang="it">Una classe di associazione per il collegamento di informazioni aggiuntive a una relazione tra le risorse DCAT.</rdfs:comment>
        <rdfs:isDefinedBy rdf:resource="https://www.w3.org/TR/vocab-dcat-2/"/>
        <rdfs:label xml:lang="es">Relación</rdfs:label>
        <rdfs:label xml:lang="da">Relation</rdfs:label>
        <rdfs:label xml:lang="en">Relationship</rdfs:label>
        <rdfs:label xml:lang="it">Relazione</rdfs:label>
        <rdfs:label xml:lang="cs">Vztah</rdfs:label>
        <skos:changeNote xml:lang="en">New class added in DCAT 2</skos:changeNote>
        <skos:changeNote xml:lang="cs">Nová třída přidaná ve verzi DCAT 2</skos:changeNote>
        <skos:changeNote xml:lang="es">Nueva clase añadida en DCAT 2</skos:changeNote>
        <skos:changeNote xml:lang="it">Nuova classe aggiunta in DCAT 2</skos:changeNote>
        <skos:changeNote xml:lang="da">Ny klasse i DCAT 2</skos:changeNote>
        <skos:definition xml:lang="en">An association class for attaching additional information to a relationship between DCAT Resources.</skos:definition>
        <skos:definition xml:lang="cs">Asociační třída pro připojení dodatečných informací ke vztahu mezi zdroji DCAT.</skos:definition>
        <skos:definition xml:lang="da">En associationsklasse til brug for tilknytning af yderligere information til en relation mellem DCAT-ressourcer.</skos:definition>
        <skos:definition xml:lang="es">Una clase de asociación para adjuntar información adicional a una relación entre recursos DCAT.</skos:definition>
        <skos:definition xml:lang="it">Una classe di associazione per il collegamento di informazioni aggiuntive a una relazione tra le risorse DCAT.</skos:definition>
        <skos:scopeNote xml:lang="da">Anvendes til at karakterisere en relation mellem datasæt, og potentielt andre ressourcer, hvor relationen er kendt men ikke tilstrækkeligt beskrevet af de standardiserede egenskaber i Dublin Core (dcterms:hasPart, dcterms:isPartOf, dcterms:conformsTo, dcterms:isFormatOf, dcterms:hasFormat, dcterms:isVersionOf, dcterms:hasVersion, dcterms:replaces, dcterms:isReplacedBy, dcterms:references, dcterms:isReferencedBy, dcterms:requires, dcterms:isRequiredBy) eller PROV-O-egenskaber (prov:wasDerivedFrom, prov:wasInfluencedBy, prov:wasQuotedFrom, prov:wasRevisionOf, prov:hadPrimarySource, prov:alternateOf, prov:specializationOf).</skos:scopeNote>
        <skos:scopeNote xml:lang="cs">Používá se pro charakterizaci vztahu mezi datovými sadami a případně i jinými zdroji, kde druh vztahu je sice znám, ale není přiměřeně charakterizován standardními vlastnostmi slovníku Dublin Core (dcterms:hasPart, dcterms:isPartOf, dcterms:conformsTo, dcterms:isFormatOf, dcterms:hasFormat, dcterms:isVersionOf, dcterms:hasVersion, dcterms:replaces, dcterms:isReplacedBy, dcterms:references, dcterms:isReferencedBy, dcterms:requires, dcterms:isRequiredBy) či vlastnostmi slovníku PROV-O (prov:wasDerivedFrom, prov:wasInfluencedBy, prov:wasQuotedFrom, prov:wasRevisionOf, prov:hadPrimarySource, prov:alternateOf, prov:specializationOf).</skos:scopeNote>
        <skos:scopeNote xml:lang="es">Se usa para caracterizar la relación entre conjuntos de datos, y potencialmente otros recursos, donde la naturaleza de la relación se conoce pero no está caracterizada adecuadamente con propiedades del estándar &apos;Dublin Core&apos; (dcterms:hasPart, dcterms:isPartOf, dcterms:conformsTo, dcterms:isFormatOf, dcterms:hasFormat, dcterms:isVersionOf, dcterms:hasVersion, dcterms:replaces, dcterms:isReplacedBy, dcterms:references, dcterms:isReferencedBy, dcterms:requires, dcterms:isRequiredBy) or PROV-O properties (prov:wasDerivedFrom, prov:wasInfluencedBy, prov:wasQuotedFrom, prov:wasRevisionOf, prov:hadPrimarySource, prov:alternateOf, prov:specializationOf).</skos:scopeNote>
        <skos:scopeNote xml:lang="en">Use to characterize a relationship between datasets, and potentially other resources, where the nature of the relationship is known but is not adequately characterized by the standard Dublin Core properties (dcterms:hasPart, dcterms:isPartOf, dcterms:conformsTo, dcterms:isFormatOf, dcterms:hasFormat, dcterms:isVersionOf, dcterms:hasVersion, dcterms:replaces, dcterms:isReplacedBy, dcterms:references, dcterms:isReferencedBy, dcterms:requires, dcterms:isRequiredBy) or PROV-O properties (prov:wasDerivedFrom, prov:wasInfluencedBy, prov:wasQuotedFrom, prov:wasRevisionOf, prov:hadPrimarySource, prov:alternateOf, prov:specializationOf).</skos:scopeNote>
        <skos:scopeNote xml:lang="it">Viene utilizzato per caratterizzare la relazione tra insiemi di dati, e potenzialmente altri tipi di risorse, nei casi in cui la natura della relazione è nota ma non adeguatamente caratterizzata dalle proprietà dello standard &apos;Dublin Core&apos; (dcterms:hasPart, dcterms:isPartOf, dcterms:conformsTo, dcterms:isFormatOf, dcterms:hasFormat, dcterms:isVersionOf, dcterms:hasVersion, dcterms:replaces, dcterms:isReplacedBy, dcterms:references, dcterms:isReferencedBy, dcterms:require, dcterms:isRequiredBy) o dalle propietà fornite da PROV-O  (prov:wasDerivedFrom, prov:wasInfluencedBy, prov:wasQuotedFrom, prov:wasRevisionOf, prov: hadPrimarySource, prov:alternateOf, prov:specializationOf).</skos:scopeNote>
    </owl:Class>
    


    <!-- http://www.w3.org/ns/dcat#Resource -->


    <owl:Class rdf:about="http://www.w3.org/ns/dcat#Resource">
        <rdfs:comment xml:lang="es">Recurso publicado o curado por un agente único.</rdfs:comment>
        <rdfs:comment xml:lang="en">Resource published or curated by a single agent.</rdfs:comment>
        <rdfs:comment xml:lang="da">Ressource udgivet eller udvalgt og arrangeret af en enkelt aktør.</rdfs:comment>
        <rdfs:comment xml:lang="it">Risorsa pubblicata o curata da un singolo agente.</rdfs:comment>
        <rdfs:comment xml:lang="cs">Zdroj publikovaný či řízený jediným činitelem.</rdfs:comment>
        <rdfs:isDefinedBy rdf:resource="https://www.w3.org/TR/vocab-dcat-2/"/>
        <rdfs:label xml:lang="en">Catalogued resource</rdfs:label>
        <rdfs:label xml:lang="da">Katalogiseret ressource</rdfs:label>
        <rdfs:label xml:lang="cs">Katalogizovaný zdroj</rdfs:label>
        <rdfs:label xml:lang="es">Recurso catalogado</rdfs:label>
        <rdfs:label xml:lang="it">Risorsa catalogata</rdfs:label>
        <skos:changeNote xml:lang="en">New class added in DCAT 2</skos:changeNote>
        <skos:changeNote xml:lang="cs">Nová třída přidaná ve verzi DCAT 2</skos:changeNote>
        <skos:changeNote xml:lang="es">Nueva clase agregada en DCAT 2</skos:changeNote>
        <skos:changeNote xml:lang="it">Nuova classe aggiunta in DCAT 2</skos:changeNote>
        <skos:changeNote xml:lang="da">Ny klasse i DCAT 2</skos:changeNote>
        <skos:definition xml:lang="es">Recurso publicado o curado por un agente único.</skos:definition>
        <skos:definition xml:lang="en">Resource published or curated by a single agent.</skos:definition>
        <skos:definition xml:lang="da">Ressource udgivet eller udvalgt og arrangeret af en enkelt aktør.</skos:definition>
        <skos:definition xml:lang="it">Risorsa pubblicata o curata da un singolo agente.</skos:definition>
        <skos:definition xml:lang="cs">Zdroj publikovaný či řízený jediným činitelem.</skos:definition>
        <skos:editorialNote xml:lang="en">2020-08-23 Scopenote updated  and needs to be translated</skos:editorialNote>
        <skos:scopeNote xml:lang="da">Klassen for alle katalogiserede ressourcer, den overordnede klasse for dcat:Dataset, dcat:DataService, dcat:Catalog og enhvert medlem af et dcat:Catalog. Denne klasse bærer egenskaber der gælder alle katalogiserede ressourcer, herunder dataset og datatjenester. Det anbefales kraftigt at mere specifikke subklasser oprettes. Når der beskrives ressourcer der ikke er dcat:Dataset eller dcat:DataService, anbefales det at oprette passende subklasser af dcat:Resource eller at dcat:Resource anvendes sammen med egenskaben dcterms:type til opmærkning med en specifik typeangivelse.</skos:scopeNote>
        <skos:scopeNote xml:lang="es">La clase de todos los recursos catalogados, la superclase de dcat:Dataset, dcat:DataService, dcat:Catalog y cualquier otro miembro de un dcat:Catalog. Esta clase tiene propiedades comunes a todos los recursos catalogados, incluyendo conjuntos de datos y servicios de datos. Se recomienda fuertemente que se use una clase más específica. Cuando se describe un recurso que no es un dcat:Dataset o dcat:DataService, se recomienda crear una sub-clase apropiada de dcat:Resource, o usar dcat:Resource con la propiedad dcterms:type to indicar el tipo específico.</skos:scopeNote>
        <skos:scopeNote xml:lang="it">La classe di tutte le risorse catalogate, la Superclasse di dcat:Dataset, dcat:DataService, dcat:Catalog e qualsiasi altro membro di dcat:Catalog. Questa classe porta proprietà comuni a tutte le risorse catalogate, inclusi set di dati e servizi dati. Si raccomanda vivamente di utilizzare una sottoclasse più specifica. Quando si descrive una risorsa che non è un dcat:Dataset o dcat:DataService, si raccomanda di creare una sottoclasse di dcat:Resource appropriata, o utilizzare dcat:Resource con la proprietà dcterms:type per indicare il tipo specifico.</skos:scopeNote>
        <skos:scopeNote xml:lang="en">The class of all catalogued resources, the Superclass of dcat:Dataset, dcat:DataService, dcat:Catalog and any other member of a dcat:Catalog. This class carries properties common to all catalogued resources, including datasets and data services. The instances of this class SHOULD be included in a catalog. The instances of this class SHOULD be included in a catalog. It is strongly recommended to use a more specific sub-class. When describing a resource which is not a dcat:Dataset or dcat:DataService, it is recommended to create a suitable sub-class of dcat:Resource, or use dcat:Resource with the dcterms:type property to indicate the specific type.</skos:scopeNote>
        <skos:scopeNote xml:lang="cs">Třída všech katalogizovaných zdrojů, nadtřída dcat:Dataset, dcat:DataService, dcat:Catalog a všech ostatních členů dcat:Catalog. Tato třída nese vlastnosti společné všem katalogizovaným zdrojům včetně datových sad a datových služeb. Je silně doporučeno používat specifičtější podtřídy, pokud je to možné. Při popisu zdroje, který není ani dcat:Dataset, ani dcat:DataService se doporučuje vytvořit odpovídající podtřídu dcat:Resrouce a nebo použít dcat:Resource s vlastností dcterms:type pro určení konkrétního typu.</skos:scopeNote>
        <skos:scopeNote xml:lang="da">dcat:Resource er et udvidelsespunkt der tillader oprettelsen af enhver type af kataloger. Yderligere subklasser kan defineres i en DCAT-profil eller i en applikation til kataloger med andre typer af ressourcer.</skos:scopeNote>
        <skos:scopeNote xml:lang="es">dcat:Resource es un punto de extensión que permite la definición de cualquier tipo de catálogo. Se pueden definir subclases adicionales en perfil de DCAT o una aplicación para catálogos de otro tipo de recursos.</skos:scopeNote>
        <skos:scopeNote xml:lang="en">dcat:Resource is an extension point that enables the definition of any kind of catalog. Additional subclasses may be defined in a DCAT profile or application for catalogs of other kinds of resources.</skos:scopeNote>
        <skos:scopeNote xml:lang="cs">dcat:Resource je bod pro rozšíření umožňující definici různých druhů katalogů. Další podtřídy lze definovat v profilech DCAT či aplikacích pro katalogy zdrojů jiných druhů.</skos:scopeNote>
        <skos:scopeNote xml:lang="it">dcat:Resource è un punto di estensione che consente la definizione di qualsiasi tipo di catalogo. Sottoclassi aggiuntive possono essere definite in un profilo DCAT o in un&apos;applicazione per cataloghi di altri tipi di risorse.</skos:scopeNote>
    </owl:Class>
    


    <!-- http://www.w3.org/ns/dcat#Role -->


    <owl:Class rdf:about="http://www.w3.org/ns/dcat#Role">
        <rdfs:subClassOf rdf:resource="http://www.w3.org/2004/02/skos/core#Concept"/>
        <rdfs:comment xml:lang="en">A role is the function of a resource or agent with respect to another resource, in the context of resource attribution or resource relationships.</rdfs:comment>
        <rdfs:comment xml:lang="da">En rolle er den funktion en ressource eller aktør har i forhold til en anden ressource, i forbindelse med ressourcekreditering eller ressourcerelationer.</rdfs:comment>
        <rdfs:comment xml:lang="cs">Role je funkce zdroje či agenta ve vztahu k jinému zdroji, v kontextu přiřazení zdrojů či vztahů mezi zdroji.</rdfs:comment>
        <rdfs:comment xml:lang="es">Un rol es la función de un recurso o agente con respecto a otro recuros, en el contexto de atribución del recurso o de las relaciones entre recursos.</rdfs:comment>
        <rdfs:comment xml:lang="it">Un ruolo è la funzione di una risorsa o di un agente rispetto ad un&apos;altra risorsa, nel contesto dell&apos;attribuzione delle risorse o delle relazioni tra risorse.</rdfs:comment>
        <rdfs:isDefinedBy rdf:resource="https://www.w3.org/TR/vocab-dcat-2/"/>
        <rdfs:label xml:lang="es">Rol</rdfs:label>
        <rdfs:label xml:lang="cs">Role</rdfs:label>
        <rdfs:label xml:lang="en">Role</rdfs:label>
        <rdfs:label xml:lang="da">Rolle</rdfs:label>
        <rdfs:label xml:lang="it">Ruolo</rdfs:label>
        <rdfs:seeAlso rdf:resource="http://www.w3.org/ns/dcat#hadRole"/>
        <skos:changeNote xml:lang="en">New class added in DCAT 2</skos:changeNote>
        <skos:changeNote xml:lang="cs">Nová třída přidaná ve verzi DCAT 2</skos:changeNote>
        <skos:changeNote xml:lang="es">Nueva clase agregada en DCAT 2</skos:changeNote>
        <skos:changeNote xml:lang="it">Nuova classe aggiunta in DCAT 2</skos:changeNote>
        <skos:changeNote xml:lang="da">Ny klasse tilføjet i DCAT 2</skos:changeNote>
        <skos:definition xml:lang="en">A role is the function of a resource or agent with respect to another resource, in the context of resource attribution or resource relationships.</skos:definition>
        <skos:definition xml:lang="da">En rolle er den funktion en ressource eller aktør har i forhold til en anden ressource, i forbindelse med ressourcekreditering eller ressourcerelationer.</skos:definition>
        <skos:definition xml:lang="cs">Role je funkce zdroje či agenta ve vztahu k jinému zdroji, v kontextu přiřazení zdrojů či vztahů mezi zdroji.</skos:definition>
        <skos:definition xml:lang="es">Un rol es la función de un recurso o agente con respecto a otro recuros, en el contexto de atribución del recurso o de las relaciones entre recursos.</skos:definition>
        <skos:definition xml:lang="it">Un ruolo è la funzione di una risorsa o di un agente rispetto ad un&apos;altra risorsa, nel contesto dell&apos;attribuzione delle risorse o delle relazioni tra risorse.</skos:definition>
        <skos:editorialNote xml:lang="es">Incluída en DCAT para complementar prov:Role (cuyo uso está limitado a roles en el contexto de una actividad, ya que es el rango es prov:hadRole).</skos:editorialNote>
        <skos:editorialNote xml:lang="it">Introdotta in DCAT per completare prov:Role (il cui uso è limitato ai ruoli nel contesto di un&apos;attività, in conseguenza alla definizione del codominio di prov:hadRole).</skos:editorialNote>
        <skos:editorialNote xml:lang="en">Introduced into DCAT to complement prov:Role (whose use is limited to roles in the context of an activity, as the range of prov:hadRole).</skos:editorialNote>
        <skos:editorialNote xml:lang="da">Introduceret i DCAT for at supplere prov:Role (hvis anvendelse er begrænset til roller i forbindelse med en aktivitet, som er rækkevidde for prov:hadRole).</skos:editorialNote>
        <skos:editorialNote xml:lang="cs">Přidáno do DCAT pro doplnění třídy prov:Role (jejíž užití je omezeno na role v kontextu aktivit, jakožto obor hodnot vlastnosti prov:hadRole).</skos:editorialNote>
        <skos:scopeNote xml:lang="da">Anvendes i forbindelse med kvalificerede krediteringer til at angive aktørens rolle i forhold til en entitet. Det anbefales at værdierne styres som et kontrolleret udfaldsrum med aktørroller, såsom http://registry.it.csiro.au/def/isotc211/CI_RoleCode.</skos:scopeNote>
        <skos:scopeNote xml:lang="da">Anvendes i forbindelse med kvalificerede relationer til at specificere en entitets rolle i forhold til en anden entitet. Det anbefales at værdierne styres med et kontrolleret udfaldsrum for for entitetsroller såsom: ISO 19115 DS_AssociationTypeCode http://registry.it.csiro.au/def/isotc211/DS_AssociationTypeCode; IANA Registry of Link Relations https://www.iana.org/assignments/link-relation;  DataCite metadata schema;  MARC relators https://id.loc.gov/vocabulary/relators.</skos:scopeNote>
        <skos:scopeNote xml:lang="cs">Použito v kvalifikovaném přiřazení pro specifikaci role Agenta ve vztahu k Entitě. Je doporučeno množinu hodnot spravovat jako řízený slovník rolí agentů, jako například http://registry.it.csiro.au/def/isotc211/CI_RoleCode.</skos:scopeNote>
        <skos:scopeNote xml:lang="cs">Použito v kvalifikovaném vztahu pro specifikaci role Entity ve vztahu k jiné Entitě. Je doporučeno množinu hodnot spravovat jako řízený slovník rolí entit, jako například ISO 19115 DS_AssociationTypeCode http://registry.it.csiro.au/def/isotc211/DS_AssociationTypeCode, IANA Registry of Link Relations https://www.iana.org/assignments/link-relation, DataCite metadata schema, či MARC relators https://id.loc.gov/vocabulary/relators.</skos:scopeNote>
        <skos:scopeNote xml:lang="es">Se usa en una atribución cualificada para especificar el rol de un Agente con respecto a una Entidad. Se recomienda que los valores se administren como un vocabulario controlado de roles de agente, como por ejemplo http://registry.it.csiro.au/def/isotc211/CI_RoleCode.</skos:scopeNote>
        <skos:scopeNote xml:lang="es">Se usa en una relación cualificada para especificar el rol de una Entidad con respecto a otra Entidad. Se recomienda que los valores se administren como los valores de un vocabulario controlado de roles de entidad como por ejemplo: ISO 19115 DS_AssociationTypeCode http://registry.it.csiro.au/def/isotc211/DS_AssociationTypeCode; IANA Registry of Link Relations https://www.iana.org/assignments/link-relation; el esquema de metadatos de DataCite; MARC relators https://id.loc.gov/vocabulary/relators.</skos:scopeNote>
        <skos:scopeNote xml:lang="en">Used in a qualified-attribution to specify the role of an Agent with respect to an Entity. It is recommended that the values be managed as a controlled vocabulary of agent roles, such as http://registry.it.csiro.au/def/isotc211/CI_RoleCode.</skos:scopeNote>
        <skos:scopeNote xml:lang="en">Used in a qualified-relation to specify the role of an Entity with respect to another Entity. It is recommended that the values be managed as a controlled vocabulary of entity roles such as: ISO 19115 DS_AssociationTypeCode http://registry.it.csiro.au/def/isotc211/DS_AssociationTypeCode; IANA Registry of Link Relations https://www.iana.org/assignments/link-relation;  DataCite metadata schema;  MARC relators https://id.loc.gov/vocabulary/relators.</skos:scopeNote>
        <skos:scopeNote xml:lang="it">Utilizzato in un&apos;attribuzione qualificata per specificare il ruolo di un agente rispetto a un&apos;entità. Si consiglia di attribuire i valori considerando un vocabolario controllato dei ruoli dell&apos;agente, ad esempio http://registry.it.csiro.au/def/isotc211/CI_RoleCode.</skos:scopeNote>
        <skos:scopeNote xml:lang="it">Utilizzato in una relazione qualificata per specificare il ruolo di un&apos;entità rispetto a un&apos;altra entità. Si raccomanda che il valore sia preso da un vocabolario controllato di ruoli di entità come ISO 19115 DS_AssociationTypeCode http://registry.it.csiro.au/def/isotc211/DS_AssociationTypeCode, IANA Registry of Link Relations https://www.iana.org/assignments/link-relation, DataCite metadata schema, o MARC relators https://id.loc.gov/vocabulary/relators.</skos:scopeNote>
    </owl:Class>
    


    <!-- http://www.w3.org/ns/org#Membership -->


    <owl:Class rdf:about="http://www.w3.org/ns/org#Membership"/>
    


    <!-- http://www.w3.org/ns/org#Role -->


    <owl:Class rdf:about="http://www.w3.org/ns/org#Role"/>
    


    <!-- http://www.w3.org/ns/prov#Entity -->


    <owl:Class rdf:about="http://www.w3.org/ns/prov#Entity"/>
    


    <!-- http://xmlns.com/foaf/0.1/Organization -->


    <owl:Class rdf:about="http://xmlns.com/foaf/0.1/Organization"/>
    


    <!-- http://xmlns.com/foaf/0.1/Person -->


    <owl:Class rdf:about="http://xmlns.com/foaf/0.1/Person"/>
    


    <!-- 
    ///////////////////////////////////////////////////////////////////////////////////////
    //
    // Individuals
    //
    ///////////////////////////////////////////////////////////////////////////////////////
     -->


    


    <!-- http://data.ign.fr/def/topo# -->


    <owl:NamedIndividual rdf:about="http://data.ign.fr/def/topo#">
        <rdf:type rdf:resource="http://purl.org/vocommons/voaf#Vocabulary"/>
    </owl:NamedIndividual>
    


    <!-- http://data.ign.fr/id/codes/topo/typedebatiment/Aerogare -->


    <owl:NamedIndividual rdf:about="http://data.ign.fr/id/codes/topo/typedebatiment/Aerogare">
        <rdf:type rdf:resource="http://data.ign.fr/def/topo#TypeDeBatiment"/>
        <rdf:type rdf:resource="http://www.w3.org/2004/02/skos/core#Concept"/>
        <skos:inScheme rdf:resource="http://data.ign.fr/id/codes/topo/typedebatiment/liste"/>
        <skos:definition xml:lang="fr">Ensemble des bâtiments d&apos;un aéroport réservés aux voyageurs et aux marchandises.</skos:definition>
        <skos:definition xml:lang="en">Set of airport buildings reserved for travelers and goods.</skos:definition>
        <skos:prefLabel xml:lang="en">air terminal</skos:prefLabel>
        <skos:prefLabel xml:lang="fr">aérogare</skos:prefLabel>
    </owl:NamedIndividual>
    


    <!-- http://data.ign.fr/id/codes/topo/typedebatiment/ArcDeTriomphe -->


    <owl:NamedIndividual rdf:about="http://data.ign.fr/id/codes/topo/typedebatiment/ArcDeTriomphe">
        <rdf:type rdf:resource="http://data.ign.fr/def/topo#TypeDeBatiment"/>
        <rdf:type rdf:resource="http://www.w3.org/2004/02/skos/core#Concept"/>
        <skos:inScheme rdf:resource="http://data.ign.fr/id/codes/topo/typedebatiment/liste"/>
        <skos:definition xml:lang="en">Monumental portico: triumphal arch, city gate.</skos:definition>
        <skos:definition xml:lang="fr">Portique monumental : arc de triomphe, porte de ville.</skos:definition>
        <skos:prefLabel xml:lang="fr">arc de triomphe</skos:prefLabel>
        <skos:prefLabel xml:lang="en">triumphal arch</skos:prefLabel>
    </owl:NamedIndividual>
    


    <!-- http://data.ign.fr/id/codes/topo/typedebatiment/Arene -->


    <owl:NamedIndividual rdf:about="http://data.ign.fr/id/codes/topo/typedebatiment/Arene">
        <rdf:type rdf:resource="http://data.ign.fr/def/topo#TypeDeBatiment"/>
        <rdf:type rdf:resource="http://www.w3.org/2004/02/skos/core#Concept"/>
        <skos:inScheme rdf:resource="http://data.ign.fr/id/codes/topo/typedebatiment/liste"/>
        <skos:altLabel xml:lang="en">roman theater</skos:altLabel>
        <skos:altLabel xml:lang="fr">théâtre antique</skos:altLabel>
        <skos:definition xml:lang="en">Large tiered building, partly or totally round or elliptical in shape: amphitheater, arena, antique theater, outdoor theater.</skos:definition>
        <skos:definition xml:lang="fr">Vaste édifice à gradins, de forme en partie ou totalement ronde ou elliptique : amphithéâtre, arène, théâtre antique, théâtre de plein air.</skos:definition>
        <skos:prefLabel xml:lang="en">arena</skos:prefLabel>
        <skos:prefLabel xml:lang="fr">arène</skos:prefLabel>
    </owl:NamedIndividual>
    


    <!-- http://data.ign.fr/id/codes/topo/typedebatiment/BatimentAgricole -->


    <owl:NamedIndividual rdf:about="http://data.ign.fr/id/codes/topo/typedebatiment/BatimentAgricole">
        <rdf:type rdf:resource="http://data.ign.fr/def/topo#TypeDeBatiment"/>
        <rdf:type rdf:resource="http://www.w3.org/2004/02/skos/core#Concept"/>
        <skos:inScheme rdf:resource="http://data.ign.fr/id/codes/topo/typedebatiment/liste"/>
        <skos:definition xml:lang="en">Building reserved for agricultural activities: industrial breeding building, agricultural shed (large), flour mill.</skos:definition>
        <skos:definition xml:lang="fr">Bâtiment réservé à des activités agricoles : bâtiment d&apos;élevage industriel, hangar agricole (grand), minoterie.</skos:definition>
        <skos:prefLabel xml:lang="fr">bâtiment agricole</skos:prefLabel>
        <skos:prefLabel xml:lang="en">farm building</skos:prefLabel>
    </owl:NamedIndividual>
    


    <!-- http://data.ign.fr/id/codes/topo/typedebatiment/BatimentCommercial -->


    <owl:NamedIndividual rdf:about="http://data.ign.fr/id/codes/topo/typedebatiment/BatimentCommercial">
        <rdf:type rdf:resource="http://data.ign.fr/def/topo#TypeDeBatiment"/>
        <rdf:type rdf:resource="http://data.ign.fr/def/topo#TypeDeZAI"/>
        <rdf:type rdf:resource="http://www.w3.org/2004/02/skos/core#Concept"/>
        <skos:inScheme rdf:resource="http://data.ign.fr/id/codes/topo/typedebatiment/liste"/>
        <skos:inScheme rdf:resource="http://data.ign.fr/id/codes/topo/typedezai/liste"/>
        <skos:broader rdf:resource="http://data.ign.fr/id/codes/topo/typedezai/PAIIndustrielCommercial"/>
        <skos:definition xml:lang="en">Building or area of large area reserved for commercial activities: shopping center, hypermarket, store (large, isolated), fairground (building), commercial area.</skos:definition>
        <skos:definition xml:lang="fr">Bâtiment ou zone de grande surface réservé à des activités commerciales : centre commercial, hypermarché, magasin (grand, isolé), parc des expositions (bâtiment), zone à caractère commercial.</skos:definition>
        <skos:prefLabel xml:lang="fr">bâtiment ou zone à caractère commercial</skos:prefLabel>
        <skos:prefLabel xml:lang="en">commercial building or area</skos:prefLabel>
    </owl:NamedIndividual>
    


    <!-- http://data.ign.fr/id/codes/topo/typedebatiment/BatimentIndustriel -->


    <owl:NamedIndividual rdf:about="http://data.ign.fr/id/codes/topo/typedebatiment/BatimentIndustriel">
        <rdf:type rdf:resource="http://data.ign.fr/def/topo#TypeDeBatiment"/>
        <rdf:type rdf:resource="http://data.ign.fr/def/topo#TypeDeZAI"/>
        <rdf:type rdf:resource="http://www.w3.org/2004/02/skos/core#Concept"/>
        <skos:inScheme rdf:resource="http://data.ign.fr/id/codes/topo/typedebatiment/liste"/>
        <skos:inScheme rdf:resource="http://data.ign.fr/id/codes/topo/typedezai/liste"/>
        <skos:broader rdf:resource="http://data.ign.fr/id/codes/topo/typedezai/PAIIndustrielCommercial"/>
        <skos:definition xml:lang="en">Building or area reserved for industrial activities not specifically distinguished: research center, depot, cooperative (winemaking, cereal &apos;), mushroom, poultry farming, stud farm, slaughterhouse, refuse center, workshop (large), station platform awning) , toll canopy, industrial building (large), power station (building), technical construction, warehouse, industrial shed (big), sawmill, factory.</skos:definition>
        <skos:definition xml:lang="fr">Bâtiment ou zone réservé à des activités industrielles non distingué de façon spécifique : centre de recherche, dépôt, coopérative (vinicole, céréaliè&apos;), champignonniè, élevage avicole, haras, abattoir, déchèterie, atelier (grand), auvent de quai de gare), auvent de péage, bâtiment industriel (grand), centrale électrique (bâtiment), construction technique, entrepôt, hangar industriel (grand), scierie, usine.</skos:definition>
        <skos:prefLabel xml:lang="fr">bâtiment ou zone à caractère industriel</skos:prefLabel>
        <skos:prefLabel xml:lang="en">industrial building or area</skos:prefLabel>
    </owl:NamedIndividual>
    


    <!-- http://data.ign.fr/id/codes/topo/typedebatiment/BatimentReligieux -->


    <owl:NamedIndividual rdf:about="http://data.ign.fr/id/codes/topo/typedebatiment/BatimentReligieux">
        <rdf:type rdf:resource="http://data.ign.fr/def/topo#TypeDeBatiment"/>
        <rdf:type rdf:resource="http://www.w3.org/2004/02/skos/core#Concept"/>
        <skos:inScheme rdf:resource="http://data.ign.fr/id/codes/topo/typedebatiment/liste"/>
        <skos:definition xml:lang="en">Building reserved for the exercise of a religious cult, other than a chapel or a church: mosque, synagogue, temple.</skos:definition>
        <skos:definition xml:lang="fr">Bâtiment réservé à l’exercice d’un culte religieux, autre qu’une chapelle ou qu’une église : mosquée, synagogue, temple.</skos:definition>
        <skos:prefLabel xml:lang="fr">bâtiment religieux</skos:prefLabel>
        <skos:prefLabel xml:lang="en">religious building</skos:prefLabel>
    </owl:NamedIndividual>
    


    <!-- http://data.ign.fr/id/codes/topo/typedebatiment/BatimentSportif -->


    <owl:NamedIndividual rdf:about="http://data.ign.fr/id/codes/topo/typedebatiment/BatimentSportif">
        <rdf:type rdf:resource="http://data.ign.fr/def/topo#TypeDeBatiment"/>
        <rdf:type rdf:resource="http://www.w3.org/2004/02/skos/core#Concept"/>
        <skos:inScheme rdf:resource="http://data.ign.fr/id/codes/topo/typedebatiment/liste"/>
        <skos:definition xml:lang="fr">Bâtiment réservé à la pratique sportive : gymnase, piscine couverte, salle de sport, tennis couvert.</skos:definition>
        <skos:definition xml:lang="en">Sports building: gym, indoor pool, gym, indoor tennis.</skos:definition>
        <skos:prefLabel xml:lang="fr">bâtiment sportif</skos:prefLabel>
        <skos:prefLabel xml:lang="en">sports building</skos:prefLabel>
    </owl:NamedIndividual>
    


    <!-- http://data.ign.fr/id/codes/topo/typedebatiment/Chapelle -->


    <owl:NamedIndividual rdf:about="http://data.ign.fr/id/codes/topo/typedebatiment/Chapelle">
        <rdf:type rdf:resource="http://data.ign.fr/def/topo#TypeDeBatiment"/>
        <rdf:type rdf:resource="http://www.w3.org/2004/02/skos/core#Concept"/>
        <skos:inScheme rdf:resource="http://data.ign.fr/id/codes/topo/typedebatiment/liste"/>
        <skos:definition xml:lang="fr">Petit édifice religieux catholique de forme caractéristique.</skos:definition>
        <skos:definition xml:lang="en">Small Catholic religious building of characteristic form.</skos:definition>
        <skos:prefLabel xml:lang="en">chapel</skos:prefLabel>
        <skos:prefLabel xml:lang="fr">chapelle</skos:prefLabel>
    </owl:NamedIndividual>
    


    <!-- http://data.ign.fr/id/codes/topo/typedebatiment/Chateau -->


    <owl:NamedIndividual rdf:about="http://data.ign.fr/id/codes/topo/typedebatiment/Chateau">
        <rdf:type rdf:resource="http://data.ign.fr/def/topo#TypeDeBatiment"/>
        <rdf:type rdf:resource="http://data.ign.fr/def/topo#TypeDeZAI"/>
        <rdf:type rdf:resource="http://www.w3.org/2004/02/skos/core#Concept"/>
        <skos:inScheme rdf:resource="http://data.ign.fr/id/codes/topo/typedebatiment/liste"/>
        <skos:inScheme rdf:resource="http://data.ign.fr/id/codes/topo/typedezai/liste"/>
        <skos:broader rdf:resource="http://data.ign.fr/id/codes/topo/typedezai/PAIZoneHabitation"/>
        <skos:definition xml:lang="en">Habitation or former feudal, royal or seigniorial dwelling: castle, castle, citadel, tower. The locality, still named, may not be inhabited or be inhabited but is not totally in ruins.</skos:definition>
        <skos:definition xml:lang="fr">Habitation ou ancienne habitation féodale, royale ou seigneuriale: château, château fort, citadelle, tour. Le lieu-dit, toujours nommé, peut ne pas être habité ou ne plus être habité mais n&apos;est pas totalement en ruines.</skos:definition>
        <skos:prefLabel xml:lang="en">castle</skos:prefLabel>
        <skos:prefLabel xml:lang="fr">château</skos:prefLabel>
    </owl:NamedIndividual>
    


    <!-- http://data.ign.fr/id/codes/topo/typedebatiment/ConstructionLegere -->


    <owl:NamedIndividual rdf:about="http://data.ign.fr/id/codes/topo/typedebatiment/ConstructionLegere">
        <rdf:type rdf:resource="http://data.ign.fr/def/topo#TypeDeBatiment"/>
        <rdf:type rdf:resource="http://www.w3.org/2004/02/skos/core#Concept"/>
        <skos:inScheme rdf:resource="http://data.ign.fr/id/codes/topo/typedebatiment/liste"/>
        <skos:definition xml:lang="en">Light structure not attached to the ground through foundations (cabins, garden sheds ...) or any building open on at least one side (yards, awnings, stands).</skos:definition>
        <skos:definition xml:lang="fr">Structure légère non attachée au sol par l’intermédiaire de fondations (cabanes, abris de jardins…) ou bâtiment quelconque ouvert sur au moins un côté (préaux, auvents, tribunes).</skos:definition>
        <skos:prefLabel xml:lang="fr">construction légère</skos:prefLabel>
        <skos:prefLabel xml:lang="en">light construction</skos:prefLabel>
    </owl:NamedIndividual>
    


    <!-- http://data.ign.fr/id/codes/topo/typedebatiment/Eglise -->


    <owl:NamedIndividual rdf:about="http://data.ign.fr/id/codes/topo/typedebatiment/Eglise">
        <rdf:type rdf:resource="http://data.ign.fr/def/topo#TypeDeBatiment"/>
        <rdf:type rdf:resource="http://www.w3.org/2004/02/skos/core#Concept"/>
        <skos:inScheme rdf:resource="http://data.ign.fr/id/codes/topo/typedebatiment/liste"/>
        <skos:definition xml:lang="en">Characteristic Catholic religious building: basilica, cathedral, church.</skos:definition>
        <skos:definition xml:lang="fr">Édifice religieux catholique de forme caractéristique : basilique, cathédrale, église.</skos:definition>
        <skos:prefLabel xml:lang="en">church</skos:prefLabel>
        <skos:prefLabel xml:lang="fr">église</skos:prefLabel>
    </owl:NamedIndividual>
    


    <!-- http://data.ign.fr/id/codes/topo/typedebatiment/Fort -->


    <owl:NamedIndividual rdf:about="http://data.ign.fr/id/codes/topo/typedebatiment/Fort">
        <rdf:type rdf:resource="http://data.ign.fr/def/topo#TypeDeBatiment"/>
        <rdf:type rdf:resource="http://www.w3.org/2004/02/skos/core#Concept"/>
        <skos:inScheme rdf:resource="http://data.ign.fr/id/codes/topo/typedebatiment/liste"/>
        <skos:altLabel xml:lang="fr">blockhaus</skos:altLabel>
        <skos:altLabel xml:lang="en">blockhouse</skos:altLabel>
        <skos:altLabel xml:lang="en">casemate</skos:altLabel>
        <skos:altLabel xml:lang="fr">casemate</skos:altLabel>
        <skos:definition xml:lang="en">Military work: blockhouse, casemate, fort, fortified work.</skos:definition>
        <skos:definition xml:lang="fr">Ouvrage militaire : blockhaus, casemate, fort, ouvrage fortifié.</skos:definition>
        <skos:prefLabel xml:lang="en">fort</skos:prefLabel>
        <skos:prefLabel xml:lang="fr">fort</skos:prefLabel>
    </owl:NamedIndividual>
    


    <!-- http://data.ign.fr/id/codes/topo/typedebatiment/Gare -->


    <owl:NamedIndividual rdf:about="http://data.ign.fr/id/codes/topo/typedebatiment/Gare">
        <rdf:type rdf:resource="http://data.ign.fr/def/topo#TypeDeBatiment"/>
        <rdf:type rdf:resource="http://www.w3.org/2004/02/skos/core#Concept"/>
        <skos:inScheme rdf:resource="http://data.ign.fr/id/codes/topo/typedebatiment/liste"/>
        <skos:definition xml:lang="en">Building used for boarding and disembarking passengers by train.</skos:definition>
        <skos:definition xml:lang="fr">Bâtiment servant à l&apos;embarquement et au débarquement des voyageurs en train.</skos:definition>
        <skos:prefLabel xml:lang="fr">gare</skos:prefLabel>
        <skos:prefLabel xml:lang="en">station</skos:prefLabel>
    </owl:NamedIndividual>
    


    <!-- http://data.ign.fr/id/codes/topo/typedebatiment/Mairie -->


    <owl:NamedIndividual rdf:about="http://data.ign.fr/id/codes/topo/typedebatiment/Mairie">
        <rdf:type rdf:resource="http://data.ign.fr/def/topo#TypeDeBatiment"/>
        <rdf:type rdf:resource="http://www.w3.org/2004/02/skos/core#Concept"/>
        <skos:inScheme rdf:resource="http://data.ign.fr/id/codes/topo/typedebatiment/liste"/>
        <skos:inScheme rdf:resource="http://data.ign.fr/id/codes/topo/typedezai/liste"/>
        <skos:altLabel xml:lang="en">city hall</skos:altLabel>
        <skos:altLabel xml:lang="fr">hôtel de ville</skos:altLabel>
        <skos:broader rdf:resource="http://data.ign.fr/id/codes/topo/typedezai/PAIAdministratifOuMilitaire"/>
        <skos:definition xml:lang="en">Building where are the services of the municipal administration, also called city hall.</skos:definition>
        <skos:definition xml:lang="fr">Édifice où se trouvent les services de l&apos;administration municipale, appelé aussi hôtel de ville.</skos:definition>
        <skos:prefLabel xml:lang="fr">mairie</skos:prefLabel>
        <skos:prefLabel xml:lang="en">town-hall</skos:prefLabel>
    </owl:NamedIndividual>
    


    <!-- http://data.ign.fr/id/codes/topo/typedebatiment/Monument -->


    <owl:NamedIndividual rdf:about="http://data.ign.fr/id/codes/topo/typedebatiment/Monument">
        <rdf:type rdf:resource="http://data.ign.fr/def/topo#TypeDeBatiment"/>
        <rdf:type rdf:resource="http://www.w3.org/2004/02/skos/core#Concept"/>
        <skos:inScheme rdf:resource="http://data.ign.fr/id/codes/topo/typedebatiment/liste"/>
        <skos:inScheme rdf:resource="http://data.ign.fr/id/codes/topo/typedezai/liste"/>
        <skos:broader rdf:resource="http://data.ign.fr/id/codes/topo/typedezai/PAICultureLoisirs"/>
        <skos:definition xml:lang="en">Any memorial without particular religious character: monument, statue, stele. The triumphal arches are excluded.</skos:definition>
        <skos:definition xml:lang="fr">Monument commémoratif quelconque, sans caractère religieux particulier : monument, statue, stèle. Les arcs de triomphe sont exclus.</skos:definition>
        <skos:prefLabel xml:lang="en">monument</skos:prefLabel>
        <skos:prefLabel xml:lang="fr">monument</skos:prefLabel>
    </owl:NamedIndividual>
    


    <!-- http://data.ign.fr/id/codes/topo/typedebatiment/Peage -->


    <owl:NamedIndividual rdf:about="http://data.ign.fr/id/codes/topo/typedebatiment/Peage">
        <rdf:type rdf:resource="http://data.ign.fr/def/topo#TypeDeBatiment"/>
        <rdf:type rdf:resource="http://www.w3.org/2004/02/skos/core#Concept"/>
        <skos:inScheme rdf:resource="http://data.ign.fr/id/codes/topo/typedebatiment/liste"/>
        <skos:definition xml:lang="en">Building where are collected the rights of use.</skos:definition>
        <skos:definition xml:lang="fr">Bâtiment où sont perçus les droits d‘usage.</skos:definition>
        <skos:prefLabel xml:lang="fr">péage</skos:prefLabel>
        <skos:prefLabel xml:lang="en">toll</skos:prefLabel>
        <skos:relatedMatch rdf:resource="http://data.ign.fr/id/codes/topo/typedezai/Peage"/>
    </owl:NamedIndividual>
    


    <!-- http://data.ign.fr/id/codes/topo/typedebatiment/Prefecture -->


    <owl:NamedIndividual rdf:about="http://data.ign.fr/id/codes/topo/typedebatiment/Prefecture">
        <rdf:type rdf:resource="http://data.ign.fr/def/topo#TypeDeBatiment"/>
        <rdf:type rdf:resource="http://www.w3.org/2004/02/skos/core#Concept"/>
        <skos:inScheme rdf:resource="http://data.ign.fr/id/codes/topo/typedebatiment/liste"/>
        <skos:inScheme rdf:resource="http://data.ign.fr/id/codes/topo/typedezai/liste"/>
        <skos:broader rdf:resource="http://data.ign.fr/id/codes/topo/typedezai/PAIAdministratifOuMilitaire"/>
        <skos:definition xml:lang="en">Building where prefectural services are installed.</skos:definition>
        <skos:definition xml:lang="fr">Bâtiment où sont installés les services préfectoraux.</skos:definition>
        <skos:prefLabel xml:lang="en">prefecture</skos:prefLabel>
        <skos:prefLabel xml:lang="fr">préfecture</skos:prefLabel>
    </owl:NamedIndividual>
    


    <!-- http://data.ign.fr/id/codes/topo/typedebatiment/Serre -->


    <owl:NamedIndividual rdf:about="http://data.ign.fr/id/codes/topo/typedebatiment/Serre">
        <rdf:type rdf:resource="http://data.ign.fr/def/topo#TypeDeBatiment"/>
        <rdf:type rdf:resource="http://www.w3.org/2004/02/skos/core#Concept"/>
        <skos:inScheme rdf:resource="http://data.ign.fr/id/codes/topo/typedebatiment/liste"/>
        <skos:definition xml:lang="fr">Abri clos à parois translucides destiné à protéger les végétaux du froid : jardinerie, serre.</skos:definition>
        <skos:definition xml:lang="en">Closed shelter with translucent walls intended to protect plants from the cold: gardening, greenhouse.</skos:definition>
        <skos:prefLabel xml:lang="en">glass-house</skos:prefLabel>
        <skos:prefLabel xml:lang="fr">serre</skos:prefLabel>
    </owl:NamedIndividual>
    


    <!-- http://data.ign.fr/id/codes/topo/typedebatiment/Silo -->


    <owl:NamedIndividual rdf:about="http://data.ign.fr/id/codes/topo/typedebatiment/Silo">
        <rdf:type rdf:resource="http://data.ign.fr/def/topo#TypeDeBatiment"/>
        <rdf:type rdf:resource="http://www.w3.org/2004/02/skos/core#Concept"/>
        <skos:inScheme rdf:resource="http://data.ign.fr/id/codes/topo/typedebatiment/liste"/>
        <skos:definition xml:lang="fr">Réservoir, qui chargé par le haut se vide par le bas, et qui sert de dépôt, de magasin, etc. Le silo est exclusivement destiné aux produits agricoles : cuve à vin, silo.</skos:definition>
        <skos:definition xml:lang="en">Tank, which is loaded from the top empties from the bottom, and which serves as a depot, store, etc. The silo is exclusively for agricultural products: wine tank, silo.</skos:definition>
        <skos:prefLabel xml:lang="en">silo</skos:prefLabel>
        <skos:prefLabel xml:lang="fr">silo</skos:prefLabel>
    </owl:NamedIndividual>
    


    <!-- http://data.ign.fr/id/codes/topo/typedebatiment/SousPrefecture -->


    <owl:NamedIndividual rdf:about="http://data.ign.fr/id/codes/topo/typedebatiment/SousPrefecture">
        <rdf:type rdf:resource="http://data.ign.fr/def/topo#TypeDeBatiment"/>
        <rdf:type rdf:resource="http://www.w3.org/2004/02/skos/core#Concept"/>
        <skos:inScheme rdf:resource="http://data.ign.fr/id/codes/topo/typedebatiment/liste"/>
        <skos:inScheme rdf:resource="http://data.ign.fr/id/codes/topo/typedezai/liste"/>
        <skos:broader rdf:resource="http://data.ign.fr/id/codes/topo/typedezai/PAIAdministratifOuMilitaire"/>
        <skos:definition xml:lang="en">Building where are the offices of the sub-prefect: chief town of district.</skos:definition>
        <skos:definition xml:lang="fr">Bâtiment où sont les bureaux du sous-préfet: chef-lieu d’arrondissement.</skos:definition>
        <skos:prefLabel xml:lang="fr">sous-préfecture</skos:prefLabel>
        <skos:prefLabel xml:lang="en">subprefecture</skos:prefLabel>
    </owl:NamedIndividual>
    


    <!-- http://data.ign.fr/id/codes/topo/typedebatiment/Tour -->


    <owl:NamedIndividual rdf:about="http://data.ign.fr/id/codes/topo/typedebatiment/Tour">
        <rdf:type rdf:resource="http://data.ign.fr/def/topo#TypeDeBatiment"/>
        <rdf:type rdf:resource="http://www.w3.org/2004/02/skos/core#Concept"/>
        <skos:inScheme rdf:resource="http://data.ign.fr/id/codes/topo/typedebatiment/liste"/>
        <skos:altLabel xml:lang="en">donjon</skos:altLabel>
        <skos:altLabel xml:lang="fr">donjon</skos:altLabel>
        <skos:altLabel xml:lang="en">mill</skos:altLabel>
        <skos:altLabel xml:lang="fr">moulin</skos:altLabel>
        <skos:definition xml:lang="fr">Bâtiment remarquable dans le paysage par sa forme élevée : donjon, moulin à vent, tour, tour de contrôle.</skos:definition>
        <skos:definition xml:lang="en">Remarkable building in the landscape by its high form: dungeon, windmill, tower, control tower.</skos:definition>
        <skos:prefLabel xml:lang="fr">tour</skos:prefLabel>
        <skos:prefLabel xml:lang="en">tower</skos:prefLabel>
    </owl:NamedIndividual>
    


    <!-- http://data.ign.fr/id/codes/topo/typedebatiment/Tribune -->


    <owl:NamedIndividual rdf:about="http://data.ign.fr/id/codes/topo/typedebatiment/Tribune">
        <rdf:type rdf:resource="http://data.ign.fr/def/topo#TypeDeBatiment"/>
        <rdf:type rdf:resource="http://www.w3.org/2004/02/skos/core#Concept"/>
        <skos:inScheme rdf:resource="http://data.ign.fr/id/codes/topo/typedebatiment/liste"/>
        <skos:definition xml:lang="fr">Tribune de terrain de sport (stade, hippodrome, vélodrome,…).</skos:definition>
        <skos:definition xml:lang="en">Tribune of sports ground (stadium, racecourse, velodrome, ...).</skos:definition>
        <skos:prefLabel xml:lang="en">stand</skos:prefLabel>
        <skos:prefLabel xml:lang="fr">tribune</skos:prefLabel>
    </owl:NamedIndividual>
    


    <!-- http://data.ign.fr/id/codes/topo/typedebatiment/liste -->


    <owl:NamedIndividual rdf:about="http://data.ign.fr/id/codes/topo/typedebatiment/liste">
        <rdf:type rdf:resource="http://www.w3.org/2004/02/skos/core#ConceptScheme"/>
        <rdfs:comment xml:lang="en">List of different types of buildings, represented as a hierarchy of SKOS concepts.</rdfs:comment>
        <rdfs:comment xml:lang="fr">Liste des différents types de bâtiments, représentés comme une hiérarchie de concepts SKOS.</rdfs:comment>
        <rdfs:label xml:lang="fr">Type de bâtiment</rdfs:label>
        <rdfs:label xml:lang="en">Type of building</rdfs:label>
    </owl:NamedIndividual>
    


    <!-- http://data.ign.fr/id/codes/topo/typedeconstruction/Antenne -->


    <owl:NamedIndividual rdf:about="http://data.ign.fr/id/codes/topo/typedeconstruction/Antenne">
        <rdf:type rdf:resource="http://data.ign.fr/def/topo#TypeDeConstruction"/>
        <rdf:type rdf:resource="http://www.w3.org/2004/02/skos/core#Concept"/>
        <skos:inScheme rdf:resource="http://data.ign.fr/id/codes/topo/typedeconstruction/liste"/>
        <skos:definition xml:lang="fr">Construction destinée à la réception ou à l&apos;émission d&apos;ondes électromagnétiques : antenne, pylône de télécommunication.</skos:definition>
        <skos:definition xml:lang="en">Construction intended for receiving or emitting electromagnetic waves: antenna, telecommunication tower.</skos:definition>
        <skos:prefLabel xml:lang="en">antenna</skos:prefLabel>
        <skos:prefLabel xml:lang="fr">antenne</skos:prefLabel>
    </owl:NamedIndividual>
    


    <!-- http://data.ign.fr/id/codes/topo/typedeconstruction/Barrage -->


    <owl:NamedIndividual rdf:about="http://data.ign.fr/id/codes/topo/typedeconstruction/Barrage">
        <rdf:type rdf:resource="http://data.ign.fr/def/topo#TypeDeConstruction"/>
        <rdf:type rdf:resource="http://data.ign.fr/def/topo#TypeDeFranchissement"/>
        <rdf:type rdf:resource="http://www.w3.org/2004/02/skos/core#Concept"/>
        <skos:inScheme rdf:resource="http://data.ign.fr/id/codes/topo/typedeconstruction/liste"/>
        <skos:inScheme rdf:resource="http://data.ign.fr/id/codes/topo/typedefranchissement/liste"/>
        <skos:broadMatch rdf:resource="http://data.ign.fr/id/codes/topo/typedezai/Barrage"/>
        <skos:definition xml:lang="fr">Ouvrage établi en travers du lit d’un cours d’eau et créant une dénivellation du plan d’eau entre l’amont et l’aval : barrage, vanne.</skos:definition>
        <skos:definition xml:lang="en">Work established across the bed of a river and creating a difference in level of water between upstream and downstream: dam, valve.</skos:definition>
        <skos:prefLabel xml:lang="fr">barrage</skos:prefLabel>
        <skos:prefLabel xml:lang="en">dam</skos:prefLabel>
    </owl:NamedIndividual>
    


    <!-- http://data.ign.fr/id/codes/topo/typedeconstruction/Cheminee -->


    <owl:NamedIndividual rdf:about="http://data.ign.fr/id/codes/topo/typedeconstruction/Cheminee">
        <rdf:type rdf:resource="http://data.ign.fr/def/topo#TypeDeConstruction"/>
        <rdf:type rdf:resource="http://www.w3.org/2004/02/skos/core#Concept"/>
        <skos:inScheme rdf:resource="http://data.ign.fr/id/codes/topo/typedeconstruction/liste"/>
        <skos:definition xml:lang="fr">Construction destinée à l&apos;émission de fumées ou de gaz.</skos:definition>
        <skos:definition xml:lang="en">Construction intended for the emission of fumes or gas.</skos:definition>
        <skos:prefLabel xml:lang="fr">cheminée</skos:prefLabel>
        <skos:prefLabel xml:lang="en">chimney</skos:prefLabel>
    </owl:NamedIndividual>
    


    <!-- http://data.ign.fr/id/codes/topo/typedeconstruction/DalleDeProtection -->


    <owl:NamedIndividual rdf:about="http://data.ign.fr/id/codes/topo/typedeconstruction/DalleDeProtection">
        <rdf:type rdf:resource="http://data.ign.fr/def/topo#TypeDeConstruction"/>
        <rdf:type rdf:resource="http://www.w3.org/2004/02/skos/core#Concept"/>
        <skos:inScheme rdf:resource="http://data.ign.fr/id/codes/topo/typedeconstruction/liste"/>
        <skos:definition xml:lang="fr">Dalle (ou auvent) horizontale protégeant une voie de communication des chutes de pierres, des coulées de neige, ou protégeant le voisinage du bruit.</skos:definition>
        <skos:definition xml:lang="en">Horizontal slab (or awning) protecting a communication path from falling rocks, snowflows, or protecting the neighborhood from noise.</skos:definition>
        <skos:prefLabel xml:lang="fr">dalle de protection</skos:prefLabel>
        <skos:prefLabel xml:lang="en">protective wall</skos:prefLabel>
    </owl:NamedIndividual>
    


    <!-- http://data.ign.fr/id/codes/topo/typedeconstruction/Ecluse -->


    <owl:NamedIndividual rdf:about="http://data.ign.fr/id/codes/topo/typedeconstruction/Ecluse">
        <rdf:type rdf:resource="http://data.ign.fr/def/topo#TypeDeConstruction"/>
        <rdf:type rdf:resource="http://www.w3.org/2004/02/skos/core#Concept"/>
        <skos:inScheme rdf:resource="http://data.ign.fr/id/codes/topo/typedeconstruction/liste"/>
        <skos:broadMatch rdf:resource="http://data.ign.fr/id/codes/topo/typedezai/Barrage"/>
        <skos:definition xml:lang="en">Hydraulic structure consisting essentially of doors equipped with valves to retain or release water as needed: boat lift, dry dock, lock, refit.</skos:definition>
        <skos:definition xml:lang="fr">Ouvrage hydraulique formé essentiellement de portes munies de vannes destiné à retenir ou à lâcher l’eau selon les besoins : ascenseur à bateaux, cale sèche, écluse, radoub.</skos:definition>
        <skos:prefLabel xml:lang="en">lock</skos:prefLabel>
        <skos:prefLabel xml:lang="fr">écluse</skos:prefLabel>
    </owl:NamedIndividual>
    


    <!-- http://data.ign.fr/id/codes/topo/typedeconstruction/Eolienne -->


    <owl:NamedIndividual rdf:about="http://data.ign.fr/id/codes/topo/typedeconstruction/Eolienne">
        <rdf:type rdf:resource="http://data.ign.fr/def/topo#TypeDeConstruction"/>
        <rdf:type rdf:resource="http://www.w3.org/2004/02/skos/core#Concept"/>
        <skos:inScheme rdf:resource="http://data.ign.fr/id/codes/topo/typedeconstruction/liste"/>
        <skos:definition xml:lang="en">A wind turbine is a device that uses wind energy to produce mechanical energy or electricity.</skos:definition>
        <skos:definition xml:lang="fr">Une éolienne est un dispositif permettant d&apos;utiliser l&apos;énergie éolienne pour produire de l&apos;énergie mécanique ou bien de l&apos;électricité.</skos:definition>
        <skos:prefLabel xml:lang="en">wind pump</skos:prefLabel>
        <skos:prefLabel xml:lang="fr">éolienne</skos:prefLabel>
    </owl:NamedIndividual>
    


    <!-- http://data.ign.fr/id/codes/topo/typedeconstruction/EscalierMonumental -->


    <owl:NamedIndividual rdf:about="http://data.ign.fr/id/codes/topo/typedeconstruction/EscalierMonumental">
        <rdf:type rdf:resource="http://data.ign.fr/def/topo#TypeDeConstruction"/>
        <rdf:type rdf:resource="http://www.w3.org/2004/02/skos/core#Concept"/>
        <skos:inScheme rdf:resource="http://data.ign.fr/id/codes/topo/typedeconstruction/liste"/>
        <skos:definition xml:lang="fr">Escalier monumental.</skos:definition>
        <skos:definition xml:lang="en">Monumental staircase.</skos:definition>
        <skos:prefLabel xml:lang="fr">escalier monumental</skos:prefLabel>
        <skos:prefLabel xml:lang="en">monumental stairs</skos:prefLabel>
    </owl:NamedIndividual>
    


    <!-- http://data.ign.fr/id/codes/topo/typedeconstruction/MurAntiBruit -->


    <owl:NamedIndividual rdf:about="http://data.ign.fr/id/codes/topo/typedeconstruction/MurAntiBruit">
        <rdf:type rdf:resource="http://data.ign.fr/def/topo#TypeDeConstruction"/>
        <rdf:type rdf:resource="http://www.w3.org/2004/02/skos/core#Concept"/>
        <skos:inScheme rdf:resource="http://data.ign.fr/id/codes/topo/typedeconstruction/liste"/>
        <skos:definition xml:lang="fr">Mur destiné à protéger les riverains d’une voie de communication du bruit qu’elle engendre.</skos:definition>
        <skos:definition xml:lang="en">Wall intended to protect residents of a communication channel from the noise it generates.</skos:definition>
        <skos:prefLabel xml:lang="fr">mur anti-bruit</skos:prefLabel>
        <skos:prefLabel xml:lang="en">sound attenuation barrier</skos:prefLabel>
    </owl:NamedIndividual>
    


    <!-- http://data.ign.fr/id/codes/topo/typedeconstruction/Phare -->


    <owl:NamedIndividual rdf:about="http://data.ign.fr/id/codes/topo/typedeconstruction/Phare">
        <rdf:type rdf:resource="http://data.ign.fr/def/topo#TypeDeConstruction"/>
        <rdf:type rdf:resource="http://www.w3.org/2004/02/skos/core#Concept"/>
        <skos:inScheme rdf:resource="http://data.ign.fr/id/codes/topo/typedeconstruction/liste"/>
        <skos:definition xml:lang="en">High tower carrying at the top a more or less powerful focus intended to guide the ships during the night.</skos:definition>
        <skos:definition xml:lang="fr">Tour élevée portant au sommet un foyer plus ou moins puissant destiné à guider les navires pendant la nuit.</skos:definition>
        <skos:prefLabel xml:lang="en">lighthouse</skos:prefLabel>
        <skos:prefLabel xml:lang="fr">phare</skos:prefLabel>
    </owl:NamedIndividual>
    


    <!-- http://data.ign.fr/id/codes/topo/typedeconstruction/Quai -->


    <owl:NamedIndividual rdf:about="http://data.ign.fr/id/codes/topo/typedeconstruction/Quai">
        <rdf:type rdf:resource="http://data.ign.fr/def/topo#TypeDeConstruction"/>
        <rdf:type rdf:resource="http://www.w3.org/2004/02/skos/core#Concept"/>
        <skos:inScheme rdf:resource="http://data.ign.fr/id/codes/topo/typedeconstruction/liste"/>
        <skos:definition xml:lang="fr">Muraille en maçonnerie ou enrochement, élevée le long d’un cours d’eau pour retenir les berges, pour empêcher les débordements. Rivage d’un port aménagé pour l’accostage des bateaux. Ouvrage en maçonnerie s’opposant à l’écoulement des eaux marines ou fluviales.</skos:definition>
        <skos:definition xml:lang="en">Wall in masonry or rip rap, raised along a stream to retain the banks, to prevent overflows. Shoreline of a harbor arranged for the docking of the boats. Masonry structure opposing the flow of marine or fluvial waters.</skos:definition>
        <skos:prefLabel xml:lang="fr">quai</skos:prefLabel>
        <skos:prefLabel xml:lang="en">wharf</skos:prefLabel>
    </owl:NamedIndividual>
    


    <!-- http://data.ign.fr/id/codes/topo/typedeconstruction/Ruines -->


    <owl:NamedIndividual rdf:about="http://data.ign.fr/id/codes/topo/typedeconstruction/Ruines">
        <rdf:type rdf:resource="http://data.ign.fr/def/topo#TypeDeConstruction"/>
        <rdf:type rdf:resource="http://www.w3.org/2004/02/skos/core#Concept"/>
        <skos:inScheme rdf:resource="http://data.ign.fr/id/codes/topo/typedeconstruction/liste"/>
        <skos:inScheme rdf:resource="http://data.ign.fr/id/codes/topo/typedezai/liste"/>
        <skos:broader rdf:resource="http://data.ign.fr/id/codes/topo/typedezai/PAIZoneHabitation"/>
        <skos:definition xml:lang="en">Building or construction in ruins.</skos:definition>
        <skos:definition xml:lang="fr">Bâtiment ou construction en ruines.</skos:definition>
        <skos:prefLabel xml:lang="fr">ruines</skos:prefLabel>
        <skos:prefLabel xml:lang="en">ruins</skos:prefLabel>
    </owl:NamedIndividual>
    


    <!-- http://data.ign.fr/id/codes/topo/typedeconstruction/Torchere -->


    <owl:NamedIndividual rdf:about="http://data.ign.fr/id/codes/topo/typedeconstruction/Torchere">
        <rdf:type rdf:resource="http://data.ign.fr/def/topo#TypeDeConstruction"/>
        <rdf:type rdf:resource="http://www.w3.org/2004/02/skos/core#Concept"/>
        <skos:inScheme rdf:resource="http://data.ign.fr/id/codes/topo/typedeconstruction/liste"/>
        <skos:definition xml:lang="fr">Canalisation verticale par laquelle s&apos;échappent et brûlent les résidus gazeux d&apos;une raffinerie.</skos:definition>
        <skos:definition xml:lang="en">Vertical pipe through which escape and burn the gaseous residues of a refinery.</skos:definition>
        <skos:prefLabel xml:lang="en">flare tower</skos:prefLabel>
        <skos:prefLabel xml:lang="fr">torchère</skos:prefLabel>
    </owl:NamedIndividual>
    


    <!-- http://data.ign.fr/id/codes/topo/typedeconstruction/Transformateur -->


    <owl:NamedIndividual rdf:about="http://data.ign.fr/id/codes/topo/typedeconstruction/Transformateur">
        <rdf:type rdf:resource="http://data.ign.fr/def/topo#TypeDeConstruction"/>
        <rdf:type rdf:resource="http://www.w3.org/2004/02/skos/core#Concept"/>
        <skos:inScheme rdf:resource="http://data.ign.fr/id/codes/topo/typedeconstruction/liste"/>
        <skos:definition xml:lang="fr">Bâtiment technique dont la fonction est de transformer un système de courants variables en un ou plusieurs autres systèmes de courants variables de même fréquence, mais d’intensité ou de tension généralement différentes.</skos:definition>
        <skos:definition xml:lang="en">Technical building whose function is to transform a system of variable currents into one or more other systems of variable currents of the same frequency, but of generally different intensity or voltage.</skos:definition>
        <skos:prefLabel xml:lang="fr">transformateur</skos:prefLabel>
        <skos:prefLabel xml:lang="en">transformer</skos:prefLabel>
    </owl:NamedIndividual>
    


    <!-- http://data.ign.fr/id/codes/topo/typedeconstruction/liste -->


    <owl:NamedIndividual rdf:about="http://data.ign.fr/id/codes/topo/typedeconstruction/liste">
        <rdf:type rdf:resource="http://www.w3.org/2004/02/skos/core#ConceptScheme"/>
        <rdfs:comment xml:lang="en">List of different types of constructions, represented as a hierarchy of SKOS concepts.</rdfs:comment>
        <rdfs:comment xml:lang="fr">Liste des différents types de constructions, représentés comme une hiérarchie de concepts SKOS.</rdfs:comment>
        <rdfs:label xml:lang="fr">Type de construction</rdfs:label>
        <rdfs:label xml:lang="en">Type of structure</rdfs:label>
    </owl:NamedIndividual>
    


    <!-- http://data.ign.fr/id/codes/topo/typedefranchissement/Cascade -->


    <owl:NamedIndividual rdf:about="http://data.ign.fr/id/codes/topo/typedefranchissement/Cascade">
        <rdf:type rdf:resource="http://data.ign.fr/def/topo#TypeDeFranchissement"/>
        <rdf:type rdf:resource="http://data.ign.fr/def/topo#TypeDeZAI"/>
        <rdf:type rdf:resource="http://www.w3.org/2004/02/skos/core#Concept"/>
        <skos:inScheme rdf:resource="http://data.ign.fr/id/codes/topo/typedefranchissement/liste"/>
        <skos:inScheme rdf:resource="http://data.ign.fr/id/codes/topo/typedezai/liste"/>
        <skos:broader rdf:resource="http://data.ign.fr/id/codes/topo/typedezai/PAIHydrographie"/>
        <skos:definition xml:lang="fr">Chute d’eau, cascade.</skos:definition>
        <skos:definition xml:lang="en">Waterfall</skos:definition>
        <skos:prefLabel xml:lang="fr">cascade</skos:prefLabel>
        <skos:prefLabel xml:lang="en">waterfall</skos:prefLabel>
    </owl:NamedIndividual>
    


    <!-- http://data.ign.fr/id/codes/topo/typedefranchissement/Ecluse -->


    <owl:NamedIndividual rdf:about="http://data.ign.fr/id/codes/topo/typedefranchissement/Ecluse">
        <rdf:type rdf:resource="http://data.ign.fr/def/topo#TypeDeFranchissement"/>
        <rdf:type rdf:resource="http://www.w3.org/2004/02/skos/core#Concept"/>
        <skos:inScheme rdf:resource="http://data.ign.fr/id/codes/topo/typedefranchissement/liste"/>
        <skos:definition xml:lang="en">Hydraulic structure consisting essentially of doors equipped with valves to retain or release water as needed: Boat lift, lock.</skos:definition>
        <skos:definition xml:lang="fr">Ouvrage hydraulique formé essentiellement de portes munies de vannes destiné à retenir ou à lâcher l’eau selon les besoins : Ascenseur à bateaux, écluse.</skos:definition>
        <skos:prefLabel xml:lang="en">lock</skos:prefLabel>
        <skos:prefLabel xml:lang="fr">écluse</skos:prefLabel>
    </owl:NamedIndividual>
    


    <!-- http://data.ign.fr/id/codes/topo/typedefranchissement/Gue -->


    <owl:NamedIndividual rdf:about="http://data.ign.fr/id/codes/topo/typedefranchissement/Gue">
        <rdf:type rdf:resource="http://data.ign.fr/def/topo#TypeDeFranchissement"/>
        <rdf:type rdf:resource="http://www.w3.org/2004/02/skos/core#Concept"/>
        <skos:inScheme rdf:resource="http://data.ign.fr/id/codes/topo/typedefranchissement/liste"/>
        <skos:definition xml:lang="en">Passage natural or arranged allowing vehicles to work a watercourse without the use of a bridge or a boat.</skos:definition>
        <skos:definition xml:lang="fr">Passage naturel ou aménagé permettant aux véhicules de travaerser un cours d&apos;eau sans le recours d&apos;un pont ou d&apos;un bateau.</skos:definition>
        <skos:prefLabel xml:lang="en">ford</skos:prefLabel>
        <skos:prefLabel xml:lang="fr">gué</skos:prefLabel>
    </owl:NamedIndividual>
    


    <!-- http://data.ign.fr/id/codes/topo/typedefranchissement/Pont -->


    <owl:NamedIndividual rdf:about="http://data.ign.fr/id/codes/topo/typedefranchissement/Pont">
        <rdf:type rdf:resource="http://data.ign.fr/def/topo#TypeDeFranchissement"/>
        <rdf:type rdf:resource="http://www.w3.org/2004/02/skos/core#Concept"/>
        <skos:inScheme rdf:resource="http://data.ign.fr/id/codes/topo/typedeconstruction/liste"/>
        <skos:inScheme rdf:resource="http://data.ign.fr/id/codes/topo/typedefranchissement/liste"/>
        <skos:inScheme rdf:resource="http://data.ign.fr/id/codes/topo/typedezai/liste"/>
        <skos:broader rdf:resource="http://data.ign.fr/id/codes/topo/typedezai/PAITransport"/>
        <skos:definition xml:lang="en">A work of art likely to span one or more elements of the road, rail or hydrographic network or allowing the crossing of a valley: bridge, footbridge, isolated bridge, moving bridge. Portion of the network located above the ground level.</skos:definition>
        <skos:definition xml:lang="fr">Ouvrage d’art susceptible d’enjamber un ou plusieurs éléments du réseau routier, ferré ou hydrographique ou permettant le franchissement d&apos;une vallée : pont, passerelle, pont isolé, pont mobile. Portion du réseau située au dessus du niveau du sol.</skos:definition>
        <skos:prefLabel xml:lang="en">bridge</skos:prefLabel>
        <skos:prefLabel xml:lang="fr">pont</skos:prefLabel>
    </owl:NamedIndividual>
    


    <!-- http://data.ign.fr/id/codes/topo/typedefranchissement/PontCanal -->


    <owl:NamedIndividual rdf:about="http://data.ign.fr/id/codes/topo/typedefranchissement/PontCanal">
        <rdf:type rdf:resource="http://data.ign.fr/def/topo#TypeDeFranchissement"/>
        <rdf:type rdf:resource="http://www.w3.org/2004/02/skos/core#Concept"/>
        <skos:inScheme rdf:resource="http://data.ign.fr/id/codes/topo/typedefranchissement/liste"/>
        <skos:definition xml:lang="en">Section of artificial watercourses passing over a bridge.</skos:definition>
        <skos:definition xml:lang="fr">Tronçon de cours d’eau artificiel passant sur un pont.</skos:definition>
        <skos:prefLabel xml:lang="en">canal aqueduct</skos:prefLabel>
        <skos:prefLabel xml:lang="fr">pont-canal</skos:prefLabel>
    </owl:NamedIndividual>
    


    <!-- http://data.ign.fr/id/codes/topo/typedefranchissement/Tunnel -->


    <owl:NamedIndividual rdf:about="http://data.ign.fr/id/codes/topo/typedefranchissement/Tunnel">
        <rdf:type rdf:resource="http://data.ign.fr/def/topo#TypeDeFranchissement"/>
        <rdf:type rdf:resource="http://www.w3.org/2004/02/skos/core#Concept"/>
        <skos:inScheme rdf:resource="http://data.ign.fr/id/codes/topo/typedefranchissement/liste"/>
        <skos:inScheme rdf:resource="http://data.ign.fr/id/codes/topo/typedezai/liste"/>
        <skos:broader rdf:resource="http://data.ign.fr/id/codes/topo/typedezai/PAITransport"/>
        <skos:definition xml:lang="fr">Portion souterraine du réseau.</skos:definition>
        <skos:definition xml:lang="en">Underground portion of the network.</skos:definition>
        <skos:prefLabel xml:lang="en">tunnel</skos:prefLabel>
        <skos:prefLabel xml:lang="fr">tunnel</skos:prefLabel>
    </owl:NamedIndividual>
    


    <!-- http://data.ign.fr/id/codes/topo/typedefranchissement/liste -->


    <owl:NamedIndividual rdf:about="http://data.ign.fr/id/codes/topo/typedefranchissement/liste">
        <rdf:type rdf:resource="http://www.w3.org/2004/02/skos/core#ConceptScheme"/>
        <rdfs:comment xml:lang="en">List of the different types of obstacle or infrastructure dedicated to obstacle clearance, represented as a hierarchy of SKOS concepts.</rdfs:comment>
        <rdfs:comment xml:lang="fr">Liste des différents types d&apos;obstacles ou d&apos;infrastructures dédiées au franchissement d&apos;obstacles, représentés comme une hiérarchie de concepts SKOS.</rdfs:comment>
        <rdfs:label xml:lang="fr">Type de franchissement</rdfs:label>
        <rdfs:label xml:lang="en">Type of crossing</rdfs:label>
    </owl:NamedIndividual>
    


    <!-- http://data.ign.fr/id/codes/topo/typedelaisse/BassesMers -->


    <owl:NamedIndividual rdf:about="http://data.ign.fr/id/codes/topo/typedelaisse/BassesMers">
        <rdf:type rdf:resource="http://data.ign.fr/def/topo#TypeDeLaisse"/>
        <rdf:type rdf:resource="http://www.w3.org/2004/02/skos/core#Concept"/>
        <skos:inScheme rdf:resource="http://data.ign.fr/id/codes/topo/typedelaisse/liste"/>
        <skos:definition xml:lang="fr">Limite inférieure de l&apos;estran. Elle sépare la zone littorale découvrante de la zone toujours envahie par la mer.</skos:definition>
        <skos:definition xml:lang="en">Lower limit of the foreshore. It separates the discovering littoral zone from the zone always invaded by the sea.</skos:definition>
        <skos:prefLabel xml:lang="fr">laisse des plus basses mers</skos:prefLabel>
        <skos:prefLabel xml:lang="en">low-tide line</skos:prefLabel>
    </owl:NamedIndividual>
    


    <!-- http://data.ign.fr/id/codes/topo/typedelaisse/HautesMers -->


    <owl:NamedIndividual rdf:about="http://data.ign.fr/id/codes/topo/typedelaisse/HautesMers">
        <rdf:type rdf:resource="http://data.ign.fr/def/topo#TypeDeLaisse"/>
        <rdf:type rdf:resource="http://www.w3.org/2004/02/skos/core#Concept"/>
        <skos:inScheme rdf:resource="http://data.ign.fr/id/codes/topo/typedelaisse/liste"/>
        <skos:definition xml:lang="fr">Limite supérieure de l&apos;estran. Elle sépare la zone littorale découvrante de la zone jamais envahie par la mer.</skos:definition>
        <skos:definition xml:lang="en">Upper limit of the foreshore. It separates the discovering littoral zone from the zone never invaded by the sea.</skos:definition>
        <skos:prefLabel xml:lang="en">high-tide line</skos:prefLabel>
        <skos:prefLabel xml:lang="fr">laisse des plus hautes mers</skos:prefLabel>
    </owl:NamedIndividual>
    


    <!-- http://data.ign.fr/id/codes/topo/typedelaisse/liste -->


    <owl:NamedIndividual rdf:about="http://data.ign.fr/id/codes/topo/typedelaisse/liste">
        <rdf:type rdf:resource="http://www.w3.org/2004/02/skos/core#ConceptScheme"/>
        <rdfs:comment xml:lang="en">List of different types of leashes, represented as a hierarchy of SKOS concepts.</rdfs:comment>
        <rdfs:comment xml:lang="fr">Liste des différents types de laisses, représentés comme une hiérarchie de concepts SKOS.</rdfs:comment>
        <rdfs:label xml:lang="fr">Type de laisse</rdfs:label>
        <rdfs:label xml:lang="en">Type of tide line</rdfs:label>
    </owl:NamedIndividual>
    


    <!-- http://data.ign.fr/id/codes/topo/typedepointdeau/Citerne -->


    <owl:NamedIndividual rdf:about="http://data.ign.fr/id/codes/topo/typedepointdeau/Citerne">
        <rdf:type rdf:resource="http://data.ign.fr/def/topo#TypeDePointDEau"/>
        <rdf:type rdf:resource="http://www.w3.org/2004/02/skos/core#Concept"/>
        <skos:inScheme rdf:resource="http://data.ign.fr/id/codes/topo/typedepointdeau/liste"/>
        <skos:definition xml:lang="fr">Réservoir où l&apos;on recueille et conserve les eaux de pluie.</skos:definition>
        <skos:definition xml:lang="en">Tank where rainwater is collected and stored.</skos:definition>
        <skos:prefLabel xml:lang="en">cistern</skos:prefLabel>
        <skos:prefLabel xml:lang="fr">citerne</skos:prefLabel>
    </owl:NamedIndividual>
    


    <!-- http://data.ign.fr/id/codes/topo/typedepointdeau/Fontaine -->


    <owl:NamedIndividual rdf:about="http://data.ign.fr/id/codes/topo/typedepointdeau/Fontaine">
        <rdf:type rdf:resource="http://data.ign.fr/def/topo#TypeDePointDEau"/>
        <rdf:type rdf:resource="http://www.w3.org/2004/02/skos/core#Concept"/>
        <skos:inScheme rdf:resource="http://data.ign.fr/id/codes/topo/typedepointdeau/liste"/>
        <skos:definition xml:lang="fr">Construction comportant une alimentation en eau et généralement un bassin.</skos:definition>
        <skos:definition xml:lang="en">Construction comprising a water supply and generally a pond.</skos:definition>
        <skos:prefLabel xml:lang="fr">fontaine</skos:prefLabel>
        <skos:prefLabel xml:lang="en">fountain</skos:prefLabel>
    </owl:NamedIndividual>
    


    <!-- http://data.ign.fr/id/codes/topo/typedepointdeau/Source -->


    <owl:NamedIndividual rdf:about="http://data.ign.fr/id/codes/topo/typedepointdeau/Source">
        <rdf:type rdf:resource="http://data.ign.fr/def/topo#TypeDePointDEau"/>
        <rdf:type rdf:resource="http://www.w3.org/2004/02/skos/core#Concept"/>
        <skos:inScheme rdf:resource="http://data.ign.fr/id/codes/topo/typedepointdeau/liste"/>
        <skos:definition xml:lang="fr">Point d&apos;émergence à la surface du sol de l&apos;eau emmagasinée à l&apos;intérieur. Exsurgence, résurgence, source.</skos:definition>
        <skos:definition xml:lang="en">Point of emergence on the soil surface of the water stored inside. Exsurgence, resurgence, source.</skos:definition>
        <skos:prefLabel xml:lang="fr">source</skos:prefLabel>
        <skos:prefLabel xml:lang="en">spring</skos:prefLabel>
    </owl:NamedIndividual>
    


    <!-- http://data.ign.fr/id/codes/topo/typedepointdeau/SourceCaptee -->


    <owl:NamedIndividual rdf:about="http://data.ign.fr/id/codes/topo/typedepointdeau/SourceCaptee">
        <rdf:type rdf:resource="http://data.ign.fr/def/topo#TypeDePointDEau"/>
        <rdf:type rdf:resource="http://www.w3.org/2004/02/skos/core#Concept"/>
        <skos:inScheme rdf:resource="http://data.ign.fr/id/codes/topo/typedepointdeau/liste"/>
        <skos:definition xml:lang="en">Collection installation of a source.</skos:definition>
        <skos:definition xml:lang="fr">Installation de captage d’une source.</skos:definition>
        <skos:prefLabel xml:lang="fr">source captée</skos:prefLabel>
        <skos:prefLabel xml:lang="en">water catchment</skos:prefLabel>
    </owl:NamedIndividual>
    


    <!-- http://data.ign.fr/id/codes/topo/typedepointdeau/StationDePompage -->


    <owl:NamedIndividual rdf:about="http://data.ign.fr/id/codes/topo/typedepointdeau/StationDePompage">
        <rdf:type rdf:resource="http://data.ign.fr/def/topo#TypeDePointDEau"/>
        <rdf:type rdf:resource="http://data.ign.fr/def/topo#TypeDeZAI"/>
        <rdf:type rdf:resource="http://www.w3.org/2004/02/skos/core#Concept"/>
        <skos:inScheme rdf:resource="http://data.ign.fr/id/codes/topo/typedepointdeau/liste"/>
        <skos:inScheme rdf:resource="http://data.ign.fr/id/codes/topo/typedezai/liste"/>
        <skos:broader rdf:resource="http://data.ign.fr/id/codes/topo/typedezai/PAIGestionEaux"/>
        <skos:definition xml:lang="fr">Installation comprenant une pompe destinée à pomper l&apos;eau du sous-sol, d&apos;une rivière, ou à monter de l&apos;eau dans un réservoir ou un château d&apos;eau.</skos:definition>
        <skos:definition xml:lang="en">Installation comprising a pump for pumping water from the basement, a river, or to raise water in a tank or a water tower.</skos:definition>
        <skos:prefLabel xml:lang="en">pumping station</skos:prefLabel>
        <skos:prefLabel xml:lang="fr">station de pompage</skos:prefLabel>
    </owl:NamedIndividual>
    


    <!-- http://data.ign.fr/id/codes/topo/typedepointdeau/liste -->


    <owl:NamedIndividual rdf:about="http://data.ign.fr/id/codes/topo/typedepointdeau/liste">
        <rdf:type rdf:resource="http://www.w3.org/2004/02/skos/core#ConceptScheme"/>
        <rdfs:comment xml:lang="en">List of different types of water points, represented as a hierarchy of SKOS concepts.</rdfs:comment>
        <rdfs:comment xml:lang="fr">Liste des différents types de points d&apos;eau, représentés comme une hiérarchie de concepts SKOS.</rdfs:comment>
        <rdfs:label xml:lang="fr">Type de point d&apos;eau</rdfs:label>
        <rdfs:label xml:lang="en">Type of waterhole</rdfs:label>
    </owl:NamedIndividual>
    


    <!-- http://data.ign.fr/id/codes/topo/typederelief/Cap -->


    <owl:NamedIndividual rdf:about="http://data.ign.fr/id/codes/topo/typederelief/Cap">
        <rdf:type rdf:resource="http://data.ign.fr/def/topo#TypeDeRelief"/>
        <rdf:type rdf:resource="http://www.w3.org/2004/02/skos/core#Concept"/>
        <skos:inScheme rdf:resource="http://data.ign.fr/id/codes/topo/typederelief/liste"/>
        <skos:inScheme rdf:resource="http://data.ign.fr/id/codes/topo/typedezai/liste"/>
        <skos:broader rdf:resource="http://data.ign.fr/id/codes/topo/typedezai/PAIOrographie"/>
        <skos:definition xml:lang="en">Predominance in the outline of a coast: cape, point, promontory.</skos:definition>
        <skos:definition xml:lang="fr">Prédominance dans le contour d&apos;une côte : cap, pointe, promontoire.</skos:definition>
        <skos:prefLabel xml:lang="fr">cap</skos:prefLabel>
        <skos:prefLabel xml:lang="en">cape</skos:prefLabel>
    </owl:NamedIndividual>
    


    <!-- http://data.ign.fr/id/codes/topo/typederelief/Carriere -->


    <owl:NamedIndividual rdf:about="http://data.ign.fr/id/codes/topo/typederelief/Carriere">
        <rdf:type rdf:resource="http://data.ign.fr/def/topo#TypeDeRelief"/>
        <rdf:type rdf:resource="http://www.w3.org/2004/02/skos/core#Concept"/>
        <skos:inScheme rdf:resource="http://data.ign.fr/id/codes/topo/typederelief/liste"/>
        <skos:inScheme rdf:resource="http://data.ign.fr/id/codes/topo/typedezai/liste"/>
        <skos:broader rdf:resource="http://data.ign.fr/id/codes/topo/typedezai/PAIIndustrielCommercial"/>
        <skos:definition xml:lang="fr">Lieu d&apos;où l&apos;on extrait à ciel ouvert des matériaux de construction (pierre, roche) : carrière, sablière, ballastière, gravière. Grand talus marquant le front et la structure principale d’une carrière : gravière (talus), mine à ciel ouvert (talus), talus de carrière.</skos:definition>
        <skos:definition xml:lang="en">Place from where we extract construction materials (stone, rock): quarry, sandpit, ballast tank, gravel pit. Large embankment marking the front and main structure of a quarry: gravel pit (embankment), open pit mine (slope), quarry slope.</skos:definition>
        <skos:prefLabel xml:lang="fr">carrière</skos:prefLabel>
        <skos:prefLabel xml:lang="en">quarry</skos:prefLabel>
    </owl:NamedIndividual>
    


    <!-- http://data.ign.fr/id/codes/topo/typederelief/Cirque -->


    <owl:NamedIndividual rdf:about="http://data.ign.fr/id/codes/topo/typederelief/Cirque">
        <rdf:type rdf:resource="http://data.ign.fr/def/topo#TypeDeRelief"/>
        <rdf:type rdf:resource="http://www.w3.org/2004/02/skos/core#Concept"/>
        <skos:inScheme rdf:resource="http://data.ign.fr/id/codes/topo/typederelief/liste"/>
        <skos:inScheme rdf:resource="http://data.ign.fr/id/codes/topo/typedezai/liste"/>
        <skos:broader rdf:resource="http://data.ign.fr/id/codes/topo/typedezai/PAIOrographie"/>
        <skos:definition xml:lang="fr">Dépression semi-circulaire, à bords raides.</skos:definition>
        <skos:definition xml:lang="en">Semi-circular depression, with steep edges.</skos:definition>
        <skos:prefLabel xml:lang="en">cirque</skos:prefLabel>
        <skos:prefLabel xml:lang="fr">cirque</skos:prefLabel>
    </owl:NamedIndividual>
    


    <!-- http://data.ign.fr/id/codes/topo/typederelief/Col -->


    <owl:NamedIndividual rdf:about="http://data.ign.fr/id/codes/topo/typederelief/Col">
        <rdf:type rdf:resource="http://data.ign.fr/def/topo#TypeDeRelief"/>
        <rdf:type rdf:resource="http://www.w3.org/2004/02/skos/core#Concept"/>
        <skos:inScheme rdf:resource="http://data.ign.fr/id/codes/topo/typederelief/liste"/>
        <skos:inScheme rdf:resource="http://data.ign.fr/id/codes/topo/typedezai/liste"/>
        <skos:broader rdf:resource="http://data.ign.fr/id/codes/topo/typedezai/PAIOrographie"/>
        <skos:definition xml:lang="fr">Point de passage imposé par la configuration du relief : col, passage.</skos:definition>
        <skos:definition xml:lang="en">Point of passage imposed by the relief configuration: pass, passage.</skos:definition>
        <skos:prefLabel xml:lang="fr">col</skos:prefLabel>
        <skos:prefLabel xml:lang="en">mountain pass</skos:prefLabel>
    </owl:NamedIndividual>
    


    <!-- http://data.ign.fr/id/codes/topo/typederelief/Crete -->


    <owl:NamedIndividual rdf:about="http://data.ign.fr/id/codes/topo/typederelief/Crete">
        <rdf:type rdf:resource="http://data.ign.fr/def/topo#TypeDeRelief"/>
        <rdf:type rdf:resource="http://www.w3.org/2004/02/skos/core#Concept"/>
        <skos:inScheme rdf:resource="http://data.ign.fr/id/codes/topo/typederelief/liste"/>
        <skos:inScheme rdf:resource="http://data.ign.fr/id/codes/topo/typedezai/liste"/>
        <skos:broader rdf:resource="http://data.ign.fr/id/codes/topo/typedezai/PAIOrographie"/>
        <skos:definition xml:lang="fr">Ligne de partage des eaux : crête, arête, ligne de faîte.</skos:definition>
        <skos:definition xml:lang="en">Watershed: crest, ridge, ridge line.</skos:definition>
        <skos:prefLabel xml:lang="en">crest</skos:prefLabel>
        <skos:prefLabel xml:lang="fr">crête</skos:prefLabel>
    </owl:NamedIndividual>
    


    <!-- http://data.ign.fr/id/codes/topo/typederelief/Depression -->


    <owl:NamedIndividual rdf:about="http://data.ign.fr/id/codes/topo/typederelief/Depression">
        <rdf:type rdf:resource="http://data.ign.fr/def/topo#TypeDeRelief"/>
        <rdf:type rdf:resource="http://www.w3.org/2004/02/skos/core#Concept"/>
        <skos:inScheme rdf:resource="http://data.ign.fr/id/codes/topo/typederelief/liste"/>
        <skos:inScheme rdf:resource="http://data.ign.fr/id/codes/topo/typedezai/liste"/>
        <skos:broader rdf:resource="http://data.ign.fr/id/codes/topo/typedezai/PAIOrographie"/>
        <skos:definition xml:lang="fr">Dépression naturelle du sol : cuvette, bassin fermé, dépression, doline.</skos:definition>
        <skos:definition xml:lang="en">Natural soil depression: basin, closed basin, depression, sinkhole.</skos:definition>
        <skos:prefLabel xml:lang="en">depression</skos:prefLabel>
        <skos:prefLabel xml:lang="fr">dépression</skos:prefLabel>
    </owl:NamedIndividual>
    


    <!-- http://data.ign.fr/id/codes/topo/typederelief/Dune -->


    <owl:NamedIndividual rdf:about="http://data.ign.fr/id/codes/topo/typederelief/Dune">
        <rdf:type rdf:resource="http://data.ign.fr/def/topo#TypeDeRelief"/>
        <rdf:type rdf:resource="http://www.w3.org/2004/02/skos/core#Concept"/>
        <skos:inScheme rdf:resource="http://data.ign.fr/id/codes/topo/typederelief/liste"/>
        <skos:inScheme rdf:resource="http://data.ign.fr/id/codes/topo/typedezai/liste"/>
        <skos:broader rdf:resource="http://data.ign.fr/id/codes/topo/typedezai/PAIOrographie"/>
        <skos:definition xml:lang="fr">Monticule de sable sur les bords de la mer.</skos:definition>
        <skos:definition xml:lang="en">Sand mound on the shores of the sea.</skos:definition>
        <skos:prefLabel xml:lang="en">dune</skos:prefLabel>
        <skos:prefLabel xml:lang="fr">dune</skos:prefLabel>
    </owl:NamedIndividual>
    


    <!-- http://data.ign.fr/id/codes/topo/typederelief/Escarpement -->


    <owl:NamedIndividual rdf:about="http://data.ign.fr/id/codes/topo/typederelief/Escarpement">
        <rdf:type rdf:resource="http://data.ign.fr/def/topo#TypeDeRelief"/>
        <rdf:type rdf:resource="http://www.w3.org/2004/02/skos/core#Concept"/>
        <skos:inScheme rdf:resource="http://data.ign.fr/id/codes/topo/typederelief/liste"/>
        <skos:inScheme rdf:resource="http://data.ign.fr/id/codes/topo/typedezai/liste"/>
        <skos:broader rdf:resource="http://data.ign.fr/id/codes/topo/typedezai/PAIOrographie"/>
        <skos:definition xml:lang="fr">Escarpement du relief : barre rocheuse, escarpement rocheux, face abrupte, falaise.</skos:definition>
        <skos:definition xml:lang="en">Relief of the relief: rocky ledge, rocky escarpment, abrupt face, cliff.</skos:definition>
        <skos:prefLabel xml:lang="fr">escarpement</skos:prefLabel>
        <skos:prefLabel xml:lang="en">escarpment</skos:prefLabel>
    </owl:NamedIndividual>
    


    <!-- http://data.ign.fr/id/codes/topo/typederelief/Gorge -->


    <owl:NamedIndividual rdf:about="http://data.ign.fr/id/codes/topo/typederelief/Gorge">
        <rdf:type rdf:resource="http://data.ign.fr/def/topo#TypeDeRelief"/>
        <rdf:type rdf:resource="http://www.w3.org/2004/02/skos/core#Concept"/>
        <skos:inScheme rdf:resource="http://data.ign.fr/id/codes/topo/typederelief/liste"/>
        <skos:inScheme rdf:resource="http://data.ign.fr/id/codes/topo/typedezai/liste"/>
        <skos:broader rdf:resource="http://data.ign.fr/id/codes/topo/typedezai/PAIOrographie"/>
        <skos:definition xml:lang="en">Valley narrow and concealed: canyon, cluse, parade, gorge.</skos:definition>
        <skos:definition xml:lang="fr">Vallée étroite et encaissée : canyon, cluse, défilé, gorge.</skos:definition>
        <skos:prefLabel xml:lang="en">gorge</skos:prefLabel>
        <skos:prefLabel xml:lang="fr">gorge</skos:prefLabel>
    </owl:NamedIndividual>
    


    <!-- http://data.ign.fr/id/codes/topo/typederelief/Grotte -->


    <owl:NamedIndividual rdf:about="http://data.ign.fr/id/codes/topo/typederelief/Grotte">
        <rdf:type rdf:resource="http://data.ign.fr/def/topo#TypeDeRelief"/>
        <rdf:type rdf:resource="http://www.w3.org/2004/02/skos/core#Concept"/>
        <skos:inScheme rdf:resource="http://data.ign.fr/id/codes/topo/typederelief/liste"/>
        <skos:inScheme rdf:resource="http://data.ign.fr/id/codes/topo/typedezai/liste"/>
        <skos:broader rdf:resource="http://data.ign.fr/id/codes/topo/typedezai/PAIOrographie"/>
        <skos:definition xml:lang="fr">Grotte naturelle ou excavation : aven, cave, gouffre, grotte.</skos:definition>
        <skos:definition xml:lang="en">Natural cave or excavation: aven, gulf, cave.</skos:definition>
        <skos:prefLabel xml:lang="en">cave</skos:prefLabel>
        <skos:prefLabel xml:lang="fr">grotte</skos:prefLabel>
    </owl:NamedIndividual>
    


    <!-- http://data.ign.fr/id/codes/topo/typederelief/Ile -->


    <owl:NamedIndividual rdf:about="http://data.ign.fr/id/codes/topo/typederelief/Ile">
        <rdf:type rdf:resource="http://data.ign.fr/def/topo#TypeDeRelief"/>
        <rdf:type rdf:resource="http://www.w3.org/2004/02/skos/core#Concept"/>
        <skos:inScheme rdf:resource="http://data.ign.fr/id/codes/topo/typederelief/liste"/>
        <skos:inScheme rdf:resource="http://data.ign.fr/id/codes/topo/typedezai/liste"/>
        <skos:broader rdf:resource="http://data.ign.fr/id/codes/topo/typedezai/PAIOrographie"/>
        <skos:definition xml:lang="en">Island or peninsula.</skos:definition>
        <skos:definition xml:lang="fr">Île, îlot ou presqu&apos;île.</skos:definition>
        <skos:prefLabel xml:lang="en">island</skos:prefLabel>
        <skos:prefLabel xml:lang="fr">île</skos:prefLabel>
    </owl:NamedIndividual>
    


    <!-- http://data.ign.fr/id/codes/topo/typederelief/Isthme -->


    <owl:NamedIndividual rdf:about="http://data.ign.fr/id/codes/topo/typederelief/Isthme">
        <rdf:type rdf:resource="http://data.ign.fr/def/topo#TypeDeRelief"/>
        <rdf:type rdf:resource="http://www.w3.org/2004/02/skos/core#Concept"/>
        <skos:inScheme rdf:resource="http://data.ign.fr/id/codes/topo/typederelief/liste"/>
        <skos:inScheme rdf:resource="http://data.ign.fr/id/codes/topo/typedezai/liste"/>
        <skos:broader rdf:resource="http://data.ign.fr/id/codes/topo/typedezai/PAIOrographie"/>
        <skos:definition xml:lang="en">A narrow strip of land between two seas, uniting two lands: coastal cord, isthmus.</skos:definition>
        <skos:definition xml:lang="fr">Bande de terre étroite entre deux mers, réunissant deux terres : cordon littoral, isthme.</skos:definition>
        <skos:prefLabel xml:lang="fr">isthme</skos:prefLabel>
        <skos:prefLabel xml:lang="en">isthmus</skos:prefLabel>
    </owl:NamedIndividual>
    


    <!-- http://data.ign.fr/id/codes/topo/typederelief/Levee -->


    <owl:NamedIndividual rdf:about="http://data.ign.fr/id/codes/topo/typederelief/Levee">
        <rdf:type rdf:resource="http://data.ign.fr/def/topo#TypeDeRelief"/>
        <rdf:type rdf:resource="http://www.w3.org/2004/02/skos/core#Concept"/>
        <skos:inScheme rdf:resource="http://data.ign.fr/id/codes/topo/typederelief/liste"/>
        <skos:definition xml:lang="fr">Digue en terre (levée de terre) ou en maçonnerie de faible largeur : crassier, levée de terre, digue en terre, remblai, terril.</skos:definition>
        <skos:definition xml:lang="en">Dike in earth (raised earth) or in masonry of small width: slag, raised earth, earth dam, embankment, heap.</skos:definition>
        <skos:prefLabel xml:lang="en">levee</skos:prefLabel>
        <skos:prefLabel xml:lang="fr">levée</skos:prefLabel>
    </owl:NamedIndividual>
    


    <!-- http://data.ign.fr/id/codes/topo/typederelief/Montagne -->


    <owl:NamedIndividual rdf:about="http://data.ign.fr/id/codes/topo/typederelief/Montagne">
        <rdf:type rdf:resource="http://data.ign.fr/def/topo#TypeDeRelief"/>
        <rdf:type rdf:resource="http://www.w3.org/2004/02/skos/core#Concept"/>
        <skos:inScheme rdf:resource="http://data.ign.fr/id/codes/topo/typederelief/liste"/>
        <skos:inScheme rdf:resource="http://data.ign.fr/id/codes/topo/typedezai/liste"/>
        <skos:broader rdf:resource="http://data.ign.fr/id/codes/topo/typedezai/PAIOrographie"/>
        <skos:definition xml:lang="en">Designates a mountain or a massif in a global way and not a particular summit (see summit).</skos:definition>
        <skos:definition xml:lang="fr">Désigne une montagne ou un massif de manière globale et non un sommet en particulier (voir sommet).</skos:definition>
        <skos:prefLabel xml:lang="fr">montagne</skos:prefLabel>
        <skos:prefLabel xml:lang="en">mountain</skos:prefLabel>
    </owl:NamedIndividual>
    


    <!-- http://data.ign.fr/id/codes/topo/typederelief/MurDeSoutenement -->


    <owl:NamedIndividual rdf:about="http://data.ign.fr/id/codes/topo/typederelief/MurDeSoutenement">
        <rdf:type rdf:resource="http://data.ign.fr/def/topo#TypeDeRelief"/>
        <rdf:type rdf:resource="http://www.w3.org/2004/02/skos/core#Concept"/>
        <skos:inScheme rdf:resource="http://data.ign.fr/id/codes/topo/typederelief/liste"/>
        <skos:definition xml:lang="fr">Mur épaulant un remblai, une terrasse.</skos:definition>
        <skos:definition xml:lang="en">Wall supporting an embankment, a terrace.</skos:definition>
        <skos:prefLabel xml:lang="fr">mur de soutènement</skos:prefLabel>
        <skos:prefLabel xml:lang="en">retaining wall</skos:prefLabel>
    </owl:NamedIndividual>
    


    <!-- http://data.ign.fr/id/codes/topo/typederelief/Pic -->


    <owl:NamedIndividual rdf:about="http://data.ign.fr/id/codes/topo/typederelief/Pic">
        <rdf:type rdf:resource="http://data.ign.fr/def/topo#TypeDeRelief"/>
        <rdf:type rdf:resource="http://www.w3.org/2004/02/skos/core#Concept"/>
        <skos:inScheme rdf:resource="http://data.ign.fr/id/codes/topo/typederelief/liste"/>
        <skos:inScheme rdf:resource="http://data.ign.fr/id/codes/topo/typedezai/liste"/>
        <skos:broader rdf:resource="http://data.ign.fr/id/codes/topo/typedezai/PAIOrographie"/>
        <skos:definition xml:lang="en">Sharp summit of a mountain: needle, peak.</skos:definition>
        <skos:definition xml:lang="fr">Sommet pointu d&apos;une montagne : aiguille, pic, piton.</skos:definition>
        <skos:prefLabel xml:lang="en">peak</skos:prefLabel>
        <skos:prefLabel xml:lang="fr">pic</skos:prefLabel>
    </owl:NamedIndividual>
    


    <!-- http://data.ign.fr/id/codes/topo/typederelief/Plage -->


    <owl:NamedIndividual rdf:about="http://data.ign.fr/id/codes/topo/typederelief/Plage">
        <rdf:type rdf:resource="http://data.ign.fr/def/topo#TypeDeRelief"/>
        <rdf:type rdf:resource="http://www.w3.org/2004/02/skos/core#Concept"/>
        <skos:inScheme rdf:resource="http://data.ign.fr/id/codes/topo/typederelief/liste"/>
        <skos:inScheme rdf:resource="http://data.ign.fr/id/codes/topo/typedezai/liste"/>
        <skos:broader rdf:resource="http://data.ign.fr/id/codes/topo/typedezai/PAIOrographie"/>
        <skos:definition xml:lang="en">Coastal zone marked by the ebb and flow of the tides: beach.</skos:definition>
        <skos:definition xml:lang="fr">Zone littorale marquée par le flux et le reflux des marées : grève, plage.</skos:definition>
        <skos:prefLabel xml:lang="en">beach</skos:prefLabel>
        <skos:prefLabel xml:lang="fr">plage</skos:prefLabel>
    </owl:NamedIndividual>
    


    <!-- http://data.ign.fr/id/codes/topo/typederelief/Plaine -->


    <owl:NamedIndividual rdf:about="http://data.ign.fr/id/codes/topo/typederelief/Plaine">
        <rdf:type rdf:resource="http://data.ign.fr/def/topo#TypeDeRelief"/>
        <rdf:type rdf:resource="http://www.w3.org/2004/02/skos/core#Concept"/>
        <skos:inScheme rdf:resource="http://data.ign.fr/id/codes/topo/typederelief/liste"/>
        <skos:inScheme rdf:resource="http://data.ign.fr/id/codes/topo/typedezai/liste"/>
        <skos:broader rdf:resource="http://data.ign.fr/id/codes/topo/typedezai/PAIOrographie"/>
        <skos:definition xml:lang="en">Land surface area characterized by relative flatness: plain, plateau.</skos:definition>
        <skos:definition xml:lang="fr">Zone de surface terrestre caractérisée par une relative planéité : plaine, plateau.</skos:definition>
        <skos:prefLabel xml:lang="en">plain</skos:prefLabel>
        <skos:prefLabel xml:lang="fr">plaine</skos:prefLabel>
    </owl:NamedIndividual>
    


    <!-- http://data.ign.fr/id/codes/topo/typederelief/Recif -->


    <owl:NamedIndividual rdf:about="http://data.ign.fr/id/codes/topo/typederelief/Recif">
        <rdf:type rdf:resource="http://data.ign.fr/def/topo#TypeDeRelief"/>
        <rdf:type rdf:resource="http://www.w3.org/2004/02/skos/core#Concept"/>
        <skos:inScheme rdf:resource="http://data.ign.fr/id/codes/topo/typederelief/liste"/>
        <skos:inScheme rdf:resource="http://data.ign.fr/id/codes/topo/typedezai/liste"/>
        <skos:broader rdf:resource="http://data.ign.fr/id/codes/topo/typedezai/PAIOrographie"/>
        <skos:definition xml:lang="fr">Rocher situé en mer ou dans un fleuve, mais dont une partie, faiblement émergée, peut constituer un obstacle ou un repère : brisant, récif, rocher marin.</skos:definition>
        <skos:definition xml:lang="en">Rock located in the sea or in a river, but part of which, slightly emerged, can constitute an obstacle or a landmark: breaking, reef, marine rock.</skos:definition>
        <skos:prefLabel xml:lang="en">reef</skos:prefLabel>
        <skos:prefLabel xml:lang="fr">récif</skos:prefLabel>
    </owl:NamedIndividual>
    


    <!-- http://data.ign.fr/id/codes/topo/typederelief/Rochers -->


    <owl:NamedIndividual rdf:about="http://data.ign.fr/id/codes/topo/typederelief/Rochers">
        <rdf:type rdf:resource="http://data.ign.fr/def/topo#TypeDeRelief"/>
        <rdf:type rdf:resource="http://www.w3.org/2004/02/skos/core#Concept"/>
        <skos:inScheme rdf:resource="http://data.ign.fr/id/codes/topo/typederelief/liste"/>
        <skos:inScheme rdf:resource="http://data.ign.fr/id/codes/topo/typedezai/liste"/>
        <skos:broader rdf:resource="http://data.ign.fr/id/codes/topo/typedezai/PAIOrographie"/>
        <skos:definition xml:lang="en">Zone or detail characterized by a rocky but not vertical nature: chaos, scree, rock.</skos:definition>
        <skos:definition xml:lang="fr">Zone ou détail caractérisé par une nature rocheuse mais non verticale : chaos, éboulis, pierrier, rocher.</skos:definition>
        <skos:prefLabel xml:lang="fr">rochers</skos:prefLabel>
        <skos:prefLabel xml:lang="en">rocks</skos:prefLabel>
    </owl:NamedIndividual>
    


    <!-- http://data.ign.fr/id/codes/topo/typederelief/Sommet -->


    <owl:NamedIndividual rdf:about="http://data.ign.fr/id/codes/topo/typederelief/Sommet">
        <rdf:type rdf:resource="http://data.ign.fr/def/topo#TypeDeRelief"/>
        <rdf:type rdf:resource="http://www.w3.org/2004/02/skos/core#Concept"/>
        <skos:inScheme rdf:resource="http://data.ign.fr/id/codes/topo/typederelief/liste"/>
        <skos:inScheme rdf:resource="http://data.ign.fr/id/codes/topo/typedezai/liste"/>
        <skos:broader rdf:resource="http://data.ign.fr/id/codes/topo/typedezai/PAIOrographie"/>
        <skos:definition xml:lang="en">High point of the relief not characterized by an abrupt profile (see the nature Pic): hill, nipple, mount, summit.</skos:definition>
        <skos:definition xml:lang="fr">Point haut du relief non caractérisé par un profil abrupt (voir la nature Pic) : colline, mamelon, mont, sommet.</skos:definition>
        <skos:prefLabel xml:lang="fr">sommet</skos:prefLabel>
        <skos:prefLabel xml:lang="en">summit</skos:prefLabel>
    </owl:NamedIndividual>
    


    <!-- http://data.ign.fr/id/codes/topo/typederelief/Talus -->


    <owl:NamedIndividual rdf:about="http://data.ign.fr/id/codes/topo/typederelief/Talus">
        <rdf:type rdf:resource="http://data.ign.fr/def/topo#TypeDeRelief"/>
        <rdf:type rdf:resource="http://www.w3.org/2004/02/skos/core#Concept"/>
        <skos:inScheme rdf:resource="http://data.ign.fr/id/codes/topo/typederelief/liste"/>
        <skos:definition xml:lang="fr">Ligne de rupture de pente : crassier, déblai, remblai, talus.</skos:definition>
        <skos:definition xml:lang="en">Slope breaking line: slag, excavation, embankment, embankment.</skos:definition>
        <skos:prefLabel xml:lang="en">slope</skos:prefLabel>
        <skos:prefLabel xml:lang="fr">talus</skos:prefLabel>
    </owl:NamedIndividual>
    


    <!-- http://data.ign.fr/id/codes/topo/typederelief/Vallee -->


    <owl:NamedIndividual rdf:about="http://data.ign.fr/id/codes/topo/typederelief/Vallee">
        <rdf:type rdf:resource="http://data.ign.fr/def/topo#TypeDeRelief"/>
        <rdf:type rdf:resource="http://www.w3.org/2004/02/skos/core#Concept"/>
        <skos:inScheme rdf:resource="http://data.ign.fr/id/codes/topo/typederelief/liste"/>
        <skos:inScheme rdf:resource="http://data.ign.fr/id/codes/topo/typedezai/liste"/>
        <skos:broader rdf:resource="http://data.ign.fr/id/codes/topo/typedezai/PAIOrographie"/>
        <skos:definition xml:lang="fr">Espace entre deux ou plusieurs montagnes. Forme définie par la convergence des versants et qui est, ou a été parcourue par un cours d&apos;eau : combe, ravin, val, vallée, vallon, thalweg.</skos:definition>
        <skos:definition xml:lang="en">Space between two or more mountains. Form defined by the convergence of slopes and which is, or has been traversed by a river: combe, ravine, val, valley, thalweg.</skos:definition>
        <skos:prefLabel xml:lang="en">valley</skos:prefLabel>
        <skos:prefLabel xml:lang="fr">vallée</skos:prefLabel>
    </owl:NamedIndividual>
    


    <!-- http://data.ign.fr/id/codes/topo/typederelief/Versant -->


    <owl:NamedIndividual rdf:about="http://data.ign.fr/id/codes/topo/typederelief/Versant">
        <rdf:type rdf:resource="http://data.ign.fr/def/topo#TypeDeRelief"/>
        <rdf:type rdf:resource="http://www.w3.org/2004/02/skos/core#Concept"/>
        <skos:inScheme rdf:resource="http://data.ign.fr/id/codes/topo/typederelief/liste"/>
        <skos:inScheme rdf:resource="http://data.ign.fr/id/codes/topo/typedezai/liste"/>
        <skos:broader rdf:resource="http://data.ign.fr/id/codes/topo/typedezai/PAIOrographie"/>
        <skos:definition xml:lang="en">Inclined plane joining a ridge line to a thalweg: hillside, slope.</skos:definition>
        <skos:definition xml:lang="fr">Plan incliné joignant une ligne de crête à un thalweg : coteau, versant.</skos:definition>
        <skos:prefLabel xml:lang="en">slope</skos:prefLabel>
        <skos:prefLabel xml:lang="fr">versant</skos:prefLabel>
    </owl:NamedIndividual>
    


    <!-- http://data.ign.fr/id/codes/topo/typederelief/Volcan -->


    <owl:NamedIndividual rdf:about="http://data.ign.fr/id/codes/topo/typederelief/Volcan">
        <rdf:type rdf:resource="http://data.ign.fr/def/topo#TypeDeRelief"/>
        <rdf:type rdf:resource="http://www.w3.org/2004/02/skos/core#Concept"/>
        <skos:inScheme rdf:resource="http://data.ign.fr/id/codes/topo/typederelief/liste"/>
        <skos:inScheme rdf:resource="http://data.ign.fr/id/codes/topo/typedezai/liste"/>
        <skos:broader rdf:resource="http://data.ign.fr/id/codes/topo/typedezai/PAIOrographie"/>
        <skos:definition xml:lang="en">Any form of relief testifying to volcanic activity: crater, volcano.</skos:definition>
        <skos:definition xml:lang="fr">Toute forme de relief témoignant d&apos;une activité volcanique : cratère, volcan.</skos:definition>
        <skos:prefLabel xml:lang="fr">volcan</skos:prefLabel>
        <skos:prefLabel xml:lang="en">volcano</skos:prefLabel>
    </owl:NamedIndividual>
    


    <!-- http://data.ign.fr/id/codes/topo/typederelief/liste -->


    <owl:NamedIndividual rdf:about="http://data.ign.fr/id/codes/topo/typederelief/liste">
        <rdf:type rdf:resource="http://www.w3.org/2004/02/skos/core#ConceptScheme"/>
        <rdfs:comment xml:lang="en">List of different types of terrain elements, represented as a hierarchy of SKOS concepts.</rdfs:comment>
        <rdfs:comment xml:lang="fr">Liste des différents types d&apos;éléments du relief, représentés comme une hiérarchie de concepts SKOS.</rdfs:comment>
        <rdfs:label xml:lang="fr">Type d&apos;élément du relief</rdfs:label>
        <rdfs:label xml:lang="en">Type of relief feature</rdfs:label>
    </owl:NamedIndividual>
    


    <!-- http://data.ign.fr/id/codes/topo/typedereservoir/ChateauDEau -->


    <owl:NamedIndividual rdf:about="http://data.ign.fr/id/codes/topo/typedereservoir/ChateauDEau">
        <rdf:type rdf:resource="http://data.ign.fr/def/topo#TypeDeReservoir"/>
        <rdf:type rdf:resource="http://www.w3.org/2004/02/skos/core#Concept"/>
        <skos:inScheme rdf:resource="http://data.ign.fr/id/codes/topo/typedereservoir/liste"/>
        <skos:definition xml:lang="fr">Réservoir d’eau construit en hauteur pour surélever le niveau de l’eau par rapport aux constructions.</skos:definition>
        <skos:definition xml:lang="en">Water tank built in height to raise the level of water compared to buildings.</skos:definition>
        <skos:prefLabel xml:lang="fr">château d&apos;eau</skos:prefLabel>
        <skos:prefLabel xml:lang="en">water tower</skos:prefLabel>
    </owl:NamedIndividual>
    


    <!-- http://data.ign.fr/id/codes/topo/typedereservoir/ReservoirDEau -->


    <owl:NamedIndividual rdf:about="http://data.ign.fr/id/codes/topo/typedereservoir/ReservoirDEau">
        <rdf:type rdf:resource="http://data.ign.fr/def/topo#TypeDeReservoir"/>
        <rdf:type rdf:resource="http://www.w3.org/2004/02/skos/core#Concept"/>
        <skos:inScheme rdf:resource="http://data.ign.fr/id/codes/topo/typedereservoir/liste"/>
        <skos:definition xml:lang="fr">Réservoirs d’eau et châteaux d’eau au sol dans lesquels la réserve d’eau est située au niveau du sol.</skos:definition>
        <skos:definition xml:lang="en">Water tanks and ground water towers in which the water supply is located at ground level.</skos:definition>
        <skos:prefLabel xml:lang="fr">réservoir d&apos;eau</skos:prefLabel>
        <skos:prefLabel xml:lang="en">water-tank</skos:prefLabel>
    </owl:NamedIndividual>
    


    <!-- http://data.ign.fr/id/codes/topo/typedereservoir/ReservoirIndustriel -->


    <owl:NamedIndividual rdf:about="http://data.ign.fr/id/codes/topo/typedereservoir/ReservoirIndustriel">
        <rdf:type rdf:resource="http://data.ign.fr/def/topo#TypeDeReservoir"/>
        <rdf:type rdf:resource="http://www.w3.org/2004/02/skos/core#Concept"/>
        <skos:inScheme rdf:resource="http://data.ign.fr/id/codes/topo/typedereservoir/liste"/>
        <skos:definition xml:lang="en">Industrial raw material tank: gasometer, hydrocarbon tank, building material tank, industrial tank.</skos:definition>
        <skos:definition xml:lang="fr">Réservoir de matière première industrielle : gazomètre, réservoir d’hydrocarbure, réservoir de matériaux de construction, réservoir industriel.</skos:definition>
        <skos:prefLabel xml:lang="fr">réservoir industriel</skos:prefLabel>
        <skos:prefLabel xml:lang="en">tank</skos:prefLabel>
    </owl:NamedIndividual>
    


    <!-- http://data.ign.fr/id/codes/topo/typedereservoir/liste -->


    <owl:NamedIndividual rdf:about="http://data.ign.fr/id/codes/topo/typedereservoir/liste">
        <rdf:type rdf:resource="http://www.w3.org/2004/02/skos/core#ConceptScheme"/>
        <rdfs:comment xml:lang="en">List of different types of tanks, represented as a hierarchy of SKOS concepts.</rdfs:comment>
        <rdfs:comment xml:lang="fr">Liste des différents types de réservoirs, représentés comme une hiérarchie de concepts SKOS.</rdfs:comment>
        <rdfs:label xml:lang="fr">Type de réservoirs</rdfs:label>
        <rdfs:label xml:lang="en">Type of tank</rdfs:label>
    </owl:NamedIndividual>
    


    <!-- http://data.ign.fr/id/codes/topo/typederoute/Autoroute -->


    <owl:NamedIndividual rdf:about="http://data.ign.fr/id/codes/topo/typederoute/Autoroute">
        <rdf:type rdf:resource="http://data.ign.fr/def/topo#TypeDeRoute"/>
        <rdf:type rdf:resource="http://www.w3.org/2004/02/skos/core#Concept"/>
        <skos:inScheme rdf:resource="http://data.ign.fr/id/codes/topo/typederoute/liste"/>
        <skos:definition xml:lang="en">Roads without junction, accessible only at designated points for this purpose and reserved for vehicles with mechanical propulsion. The classification in the category of highways is pronounced by decree of the council of state, taken after public inquiry.</skos:definition>
        <skos:definition xml:lang="fr">Routes sans croisement, accessibles seulement en des points aménagés à cet effet et réservées aux véhicules à propulsion mécanique. Le classement dans la catégorie des autoroutes est prononcé par décret du conseil d’état, pris après enquête publique.</skos:definition>
        <skos:prefLabel xml:lang="fr">autoroute</skos:prefLabel>
        <skos:prefLabel xml:lang="en">motorway</skos:prefLabel>
    </owl:NamedIndividual>
    


    <!-- http://data.ign.fr/id/codes/topo/typederoute/BacAuto -->


    <owl:NamedIndividual rdf:about="http://data.ign.fr/id/codes/topo/typederoute/BacAuto">
        <rdf:type rdf:resource="http://data.ign.fr/def/topo#TypeDeRoute"/>
        <rdf:type rdf:resource="http://www.w3.org/2004/02/skos/core#Concept"/>
        <skos:inScheme rdf:resource="http://data.ign.fr/id/codes/topo/typederoute/liste"/>
        <skos:definition xml:lang="en">Routes of the boat used to pass vehicles from one bank to the other of a watercourse or an arm of the sea.</skos:definition>
        <skos:definition xml:lang="fr">Trajets du bateau servant à passer des véhicules d’une rive à l’autre d’un cours d’eau ou d’un bras de mer.</skos:definition>
        <skos:prefLabel xml:lang="fr">bac auto</skos:prefLabel>
        <skos:prefLabel xml:lang="en">car ferry</skos:prefLabel>
    </owl:NamedIndividual>
    


    <!-- http://data.ign.fr/id/codes/topo/typederoute/BacPieton -->


    <owl:NamedIndividual rdf:about="http://data.ign.fr/id/codes/topo/typederoute/BacPieton">
        <rdf:type rdf:resource="http://data.ign.fr/def/topo#TypeDeRoute"/>
        <rdf:type rdf:resource="http://www.w3.org/2004/02/skos/core#Concept"/>
        <skos:inScheme rdf:resource="http://data.ign.fr/id/codes/topo/typederoute/liste"/>
        <skos:definition xml:lang="en">Routes of the boat used to cross pedestrians from one bank to the other of a watercourse or an arm of the sea.</skos:definition>
        <skos:definition xml:lang="fr">Trajets du bateau servant à passer des piétons d’une rive à l’autre d’un cours d’eau ou d’un bras de mer.</skos:definition>
        <skos:prefLabel xml:lang="fr">bac piéton</skos:prefLabel>
        <skos:prefLabel xml:lang="en">passenger ferry</skos:prefLabel>
    </owl:NamedIndividual>
    


    <!-- http://data.ign.fr/id/codes/topo/typederoute/Bretelle -->


    <owl:NamedIndividual rdf:about="http://data.ign.fr/id/codes/topo/typederoute/Bretelle">
        <rdf:type rdf:resource="http://data.ign.fr/def/topo#TypeDeRoute"/>
        <rdf:type rdf:resource="http://www.w3.org/2004/02/skos/core#Concept"/>
        <skos:inScheme rdf:resource="http://data.ign.fr/id/codes/topo/typederoute/liste"/>
        <skos:definition xml:lang="fr">Bretelles de liaison (ou d’échangeur) ou voies d’accès à une aire de service ou de repos.</skos:definition>
        <skos:definition xml:lang="en">Connecting braces (or interchange) or access routes to a service or rest area.</skos:definition>
        <skos:prefLabel xml:lang="fr">bretelle</skos:prefLabel>
        <skos:prefLabel xml:lang="en">ramp</skos:prefLabel>
    </owl:NamedIndividual>
    


    <!-- http://data.ign.fr/id/codes/topo/typederoute/Chemin -->


    <owl:NamedIndividual rdf:about="http://data.ign.fr/id/codes/topo/typederoute/Chemin">
        <rdf:type rdf:resource="http://data.ign.fr/def/topo#TypeDeRoute"/>
        <rdf:type rdf:resource="http://www.w3.org/2004/02/skos/core#Concept"/>
        <skos:inScheme rdf:resource="http://data.ign.fr/id/codes/topo/typederoute/liste"/>
        <skos:definition xml:lang="fr">Les chemins sont prévus pour la circulation de véhicules ou d’engins d’exploitation. Ils ne sont pas forcément carrossables pour tous les véhicules et par tout temps.</skos:definition>
        <skos:definition xml:lang="en">Roads are intended for the circulation of vehicles or machinery. They are not necessarily drivable for all vehicles and in any weather.</skos:definition>
        <skos:prefLabel xml:lang="fr">chemin</skos:prefLabel>
        <skos:prefLabel xml:lang="en">dirt road</skos:prefLabel>
    </owl:NamedIndividual>
    


    <!-- http://data.ign.fr/id/codes/topo/typederoute/Escalier -->


    <owl:NamedIndividual rdf:about="http://data.ign.fr/id/codes/topo/typederoute/Escalier">
        <rdf:type rdf:resource="http://data.ign.fr/def/topo#TypeDeRoute"/>
        <rdf:type rdf:resource="http://www.w3.org/2004/02/skos/core#Concept"/>
        <skos:inScheme rdf:resource="http://data.ign.fr/id/codes/topo/typederoute/liste"/>
        <skos:definition xml:lang="fr">Escaliers directement reliés au réseau routier, assurant la jonction entre deux voies de communication ou entre le réseau routier et un élément adressable.</skos:definition>
        <skos:definition xml:lang="en">Stairs directly connected to the road network, ensuring the junction between two communication channels or between the road network and an addressable element.</skos:definition>
        <skos:prefLabel xml:lang="fr">escalier</skos:prefLabel>
        <skos:prefLabel xml:lang="en">stair way street</skos:prefLabel>
    </owl:NamedIndividual>
    


    <!-- http://data.ign.fr/id/codes/topo/typederoute/PisteCyclable -->


    <owl:NamedIndividual rdf:about="http://data.ign.fr/id/codes/topo/typederoute/PisteCyclable">
        <rdf:type rdf:resource="http://data.ign.fr/def/topo#TypeDeRoute"/>
        <rdf:type rdf:resource="http://www.w3.org/2004/02/skos/core#Concept"/>
        <skos:inScheme rdf:resource="http://data.ign.fr/id/codes/topo/typederoute/liste"/>
        <skos:definition xml:lang="en">Segments of pavement in own site, reserved for bicycles. Bike lanes are excluded.</skos:definition>
        <skos:definition xml:lang="fr">Tronçons de chaussée en site propre, réservés aux cycles. Les bandes cyclables sont exclues.</skos:definition>
        <skos:prefLabel xml:lang="en">bicycle path</skos:prefLabel>
        <skos:prefLabel xml:lang="fr">piste cyclable</skos:prefLabel>
    </owl:NamedIndividual>
    


    <!-- http://data.ign.fr/id/codes/topo/typederoute/QuasiAutoroute -->


    <owl:NamedIndividual rdf:about="http://data.ign.fr/id/codes/topo/typederoute/QuasiAutoroute">
        <rdf:type rdf:resource="http://data.ign.fr/def/topo#TypeDeRoute"/>
        <rdf:type rdf:resource="http://www.w3.org/2004/02/skos/core#Concept"/>
        <skos:inScheme rdf:resource="http://data.ign.fr/id/codes/topo/typederoute/liste"/>
        <skos:definition xml:lang="fr">Routes de même définition que l’autoroute mais non classées officiellement dans cette catégorie. Ce sont des routes à chaussées séparées par un terre-plein central, qui ne possèdent pas de croisement à niveau avec le reste du réseau routier.</skos:definition>
        <skos:definition xml:lang="en">Routes of the same definition as the highway but not officially classified in this category. These are paved roads separated by a median strip, which do not have a level crossing with the rest of the road network.</skos:definition>
        <skos:prefLabel xml:lang="en">non-classified motorway</skos:prefLabel>
        <skos:prefLabel xml:lang="fr">quasi-autoroute</skos:prefLabel>
    </owl:NamedIndividual>
    


    <!-- http://data.ign.fr/id/codes/topo/typederoute/RouteADeuxChaussees -->


    <owl:NamedIndividual rdf:about="http://data.ign.fr/id/codes/topo/typederoute/RouteADeuxChaussees">
        <rdf:type rdf:resource="http://data.ign.fr/def/topo#TypeDeRoute"/>
        <rdf:type rdf:resource="http://www.w3.org/2004/02/skos/core#Concept"/>
        <skos:inScheme rdf:resource="http://data.ign.fr/id/codes/topo/typederoute/liste"/>
        <skos:definition xml:lang="en">Roads with 2 carriageways separated by a physical obstacle possibly open at intersections. They therefore have level crossings, which prevents them from being classified in the highway or near-highway category.</skos:definition>
        <skos:definition xml:lang="fr">Routes comportant 2 chaussées séparées par un obstacle physique éventuellement ouvert aux carrefours. Elles possèdent donc des croisements à niveau, ce qui leur interdit d&apos;être classées dans la catégorie autoroute ou quasi-autoroute.</skos:definition>
        <skos:prefLabel xml:lang="en">dual carriageway road</skos:prefLabel>
        <skos:prefLabel xml:lang="fr">route à deux chaussées</skos:prefLabel>
    </owl:NamedIndividual>
    


    <!-- http://data.ign.fr/id/codes/topo/typederoute/RouteAUneChaussee -->


    <owl:NamedIndividual rdf:about="http://data.ign.fr/id/codes/topo/typederoute/RouteAUneChaussee">
        <rdf:type rdf:resource="http://data.ign.fr/def/topo#TypeDeRoute"/>
        <rdf:type rdf:resource="http://www.w3.org/2004/02/skos/core#Concept"/>
        <skos:inScheme rdf:resource="http://data.ign.fr/id/codes/topo/typederoute/liste"/>
        <skos:definition xml:lang="en">Roads with 1 roadway. All tarmac roads that are not classified as 2-lane Road, Near-highway or Highway are included in this class.</skos:definition>
        <skos:definition xml:lang="fr">Routes comportant 1 chaussée. Toutes les routes goudronnées qui ne sont pas classées en Route à 2 chaussées, Quasi-autoroute ou Autoroute se retrouvent dans cette classe.</skos:definition>
        <skos:prefLabel xml:lang="fr">route à une chaussée</skos:prefLabel>
        <skos:prefLabel xml:lang="en">single carriageway road</skos:prefLabel>
    </owl:NamedIndividual>
    


    <!-- http://data.ign.fr/id/codes/topo/typederoute/RouteDepartementale -->


    <owl:NamedIndividual rdf:about="http://data.ign.fr/id/codes/topo/typederoute/RouteDepartementale">
        <rdf:type rdf:resource="http://data.ign.fr/def/topo#TypeDeRoute"/>
        <rdf:type rdf:resource="http://www.w3.org/2004/02/skos/core#Concept"/>
        <skos:inScheme rdf:resource="http://data.ign.fr/id/codes/topo/typederoute/liste"/>
        <skos:definition xml:lang="en">Road that is part of the public road departmental.</skos:definition>
        <skos:definition xml:lang="fr">Voie qui fait partie du domaine public routier départemental.</skos:definition>
        <skos:prefLabel xml:lang="fr">route départementale</skos:prefLabel>
        <skos:prefLabel xml:lang="en">secondary road</skos:prefLabel>
    </owl:NamedIndividual>
    


    <!-- http://data.ign.fr/id/codes/topo/typederoute/RouteEmpierree -->


    <owl:NamedIndividual rdf:about="http://data.ign.fr/id/codes/topo/typederoute/RouteEmpierree">
        <rdf:type rdf:resource="http://data.ign.fr/def/topo#TypeDeRoute"/>
        <rdf:type rdf:resource="http://www.w3.org/2004/02/skos/core#Concept"/>
        <skos:inScheme rdf:resource="http://data.ign.fr/id/codes/topo/typederoute/liste"/>
        <skos:definition xml:lang="en">Roads lightly surfaced (no surface coating or very degraded coating), but allowing the circulation of passenger cars all the time. All stone roads are included.</skos:definition>
        <skos:definition xml:lang="fr">Routes sommairement revêtues (pas de revêtement de surface ou revêtement très dégradé), mais permettant la circulation de véhicules automobiles de tourisme par tout temps. Toutes les routes empierrées sont incluses.</skos:definition>
        <skos:prefLabel xml:lang="en">gravel road</skos:prefLabel>
        <skos:prefLabel xml:lang="fr">route empierrée</skos:prefLabel>
    </owl:NamedIndividual>
    


    <!-- http://data.ign.fr/id/codes/topo/typederoute/RouteNationale -->


    <owl:NamedIndividual rdf:about="http://data.ign.fr/id/codes/topo/typederoute/RouteNationale">
        <rdf:type rdf:resource="http://data.ign.fr/def/topo#TypeDeRoute"/>
        <rdf:type rdf:resource="http://www.w3.org/2004/02/skos/core#Concept"/>
        <skos:inScheme rdf:resource="http://data.ign.fr/id/codes/topo/typederoute/liste"/>
        <skos:definition xml:lang="en">National public highway roadway other than motorways.</skos:definition>
        <skos:definition xml:lang="fr">Voie du domaine public routier national autre que les autoroutes.</skos:definition>
        <skos:prefLabel xml:lang="en">main road</skos:prefLabel>
        <skos:prefLabel xml:lang="fr">route nationale</skos:prefLabel>
    </owl:NamedIndividual>
    


    <!-- http://data.ign.fr/id/codes/topo/typederoute/Sentier -->


    <owl:NamedIndividual rdf:about="http://data.ign.fr/id/codes/topo/typederoute/Sentier">
        <rdf:type rdf:resource="http://data.ign.fr/def/topo#TypeDeRoute"/>
        <rdf:type rdf:resource="http://www.w3.org/2004/02/skos/core#Concept"/>
        <skos:inScheme rdf:resource="http://data.ign.fr/id/codes/topo/typederoute/liste"/>
        <skos:definition xml:lang="fr">Chemins étroits ne permettant pas le passage de véhicules. Seuls les principaux sentiers sont inclus. Passerelles supportant une allée, directement reliés au réseau routier. Les passerelles ont une position par rapport au sol supérieure à 0.</skos:definition>
        <skos:definition xml:lang="en">Narrow paths that do not allow the passage of vehicles. Only the main trails are included. Bridges supporting an alley, directly connected to the road network. The bridges have a position relative to the ground greater than 0.</skos:definition>
        <skos:prefLabel xml:lang="en">footpath</skos:prefLabel>
        <skos:prefLabel xml:lang="fr">sentier</skos:prefLabel>
    </owl:NamedIndividual>
    


    <!-- http://data.ign.fr/id/codes/topo/typederoute/liste -->


    <owl:NamedIndividual rdf:about="http://data.ign.fr/id/codes/topo/typederoute/liste">
        <rdf:type rdf:resource="http://www.w3.org/2004/02/skos/core#ConceptScheme"/>
        <rdfs:comment xml:lang="en">List of different road types, represented as a hierarchy of SKOS concepts.</rdfs:comment>
        <rdfs:comment xml:lang="fr">Liste des différents types de routes, représentés comme une hiérarchie de concepts SKOS.</rdfs:comment>
        <rdfs:label xml:lang="fr">Type de route</rdfs:label>
        <rdfs:label xml:lang="en">Type of road</rdfs:label>
    </owl:NamedIndividual>
    


    <!-- http://data.ign.fr/id/codes/topo/typedesource/AutreSource -->


    <owl:NamedIndividual rdf:about="http://data.ign.fr/id/codes/topo/typedesource/AutreSource">
        <rdf:type rdf:resource="http://www.w3.org/ns/prov#Entity"/>
        <rdfs:label xml:lang="fr">autre source de données</rdfs:label>
        <rdfs:label xml:lang="en">other data source</rdfs:label>
    </owl:NamedIndividual>
    


    <!-- http://data.ign.fr/id/codes/topo/typedesource/BdCarto -->


    <owl:NamedIndividual rdf:about="http://data.ign.fr/id/codes/topo/typedesource/BdCarto">
        <rdf:type rdf:resource="http://www.w3.org/ns/prov#Entity"/>
        <rdfs:label xml:lang="en">BD CARTO</rdfs:label>
        <rdfs:label xml:lang="fr">BD CARTO</rdfs:label>
        <foaf:homepage rdf:resource="http://professionnels.ign.fr/bdcarto"/>
    </owl:NamedIndividual>
    


    <!-- http://data.ign.fr/id/codes/topo/typedesource/BdNyme -->


    <owl:NamedIndividual rdf:about="http://data.ign.fr/id/codes/topo/typedesource/BdNyme">
        <rdf:type rdf:resource="http://www.w3.org/ns/prov#Entity"/>
        <rdfs:label xml:lang="en">BD NYME</rdfs:label>
        <rdfs:label xml:lang="fr">BD NYME</rdfs:label>
        <foaf:homepage rdf:resource="http://professionnels.ign.fr/bdnyme"/>
    </owl:NamedIndividual>
    


    <!-- http://data.ign.fr/id/codes/topo/typedesource/BdParcellaire -->


    <owl:NamedIndividual rdf:about="http://data.ign.fr/id/codes/topo/typedesource/BdParcellaire">
        <rdf:type rdf:resource="http://www.w3.org/ns/prov#Entity"/>
        <rdfs:label xml:lang="en">BD PARCELLAIRE</rdfs:label>
        <rdfs:label xml:lang="fr">BD PARCELLAIRE</rdfs:label>
        <foaf:homepage rdf:resource="http://professionnels.ign.fr/bdparcellaire"/>
    </owl:NamedIndividual>
    


    <!-- http://data.ign.fr/id/codes/topo/typedesource/BdTopo -->


    <owl:NamedIndividual rdf:about="http://data.ign.fr/id/codes/topo/typedesource/BdTopo">
        <rdf:type rdf:resource="http://www.w3.org/ns/prov#Entity"/>
        <rdfs:label xml:lang="en">BD TOPO</rdfs:label>
        <rdfs:label xml:lang="fr">BD TOPO</rdfs:label>
        <foaf:homepage rdf:resource="http://professionnels.ign.fr/bdtopo"/>
    </owl:NamedIndividual>
    


    <!-- http://data.ign.fr/id/codes/topo/typedesource/Cadastre -->


    <owl:NamedIndividual rdf:about="http://data.ign.fr/id/codes/topo/typedesource/Cadastre">
        <rdf:type rdf:resource="http://www.w3.org/ns/prov#Entity"/>
        <rdfs:label xml:lang="en">cadastre</rdfs:label>
        <rdfs:label xml:lang="fr">cadastre</rdfs:label>
    </owl:NamedIndividual>
    


    <!-- http://data.ign.fr/id/codes/topo/typedesource/Calcul -->


    <owl:NamedIndividual rdf:about="http://data.ign.fr/id/codes/topo/typedesource/Calcul">
        <rdf:type rdf:resource="http://www.w3.org/ns/prov#Entity"/>
        <rdfs:label xml:lang="fr">calcul</rdfs:label>
        <rdfs:label xml:lang="en">computation</rdfs:label>
    </owl:NamedIndividual>
    


    <!-- http://data.ign.fr/id/codes/topo/typedesource/Fichier -->


    <owl:NamedIndividual rdf:about="http://data.ign.fr/id/codes/topo/typedesource/Fichier">
        <rdf:type rdf:resource="http://www.w3.org/ns/prov#Entity"/>
        <rdfs:label xml:lang="fr">fichier</rdfs:label>
        <rdfs:label xml:lang="en">file</rdfs:label>
    </owl:NamedIndividual>
    


    <!-- http://data.ign.fr/id/codes/topo/typedesource/Georoute -->


    <owl:NamedIndividual rdf:about="http://data.ign.fr/id/codes/topo/typedesource/Georoute">
        <rdf:type rdf:resource="http://www.w3.org/ns/prov#Entity"/>
        <rdfs:label xml:lang="en">Georoute</rdfs:label>
        <rdfs:label xml:lang="fr">Géoroute</rdfs:label>
    </owl:NamedIndividual>
    


    <!-- http://data.ign.fr/id/codes/topo/typedesource/Orthophotographie -->


    <owl:NamedIndividual rdf:about="http://data.ign.fr/id/codes/topo/typedesource/Orthophotographie">
        <rdf:type rdf:resource="http://www.w3.org/ns/prov#Entity"/>
        <rdfs:label xml:lang="en">orthophotograph</rdfs:label>
        <rdfs:label xml:lang="fr">orthophotographie</rdfs:label>
    </owl:NamedIndividual>
    


    <!-- http://data.ign.fr/id/codes/topo/typedesource/Plan -->


    <owl:NamedIndividual rdf:about="http://data.ign.fr/id/codes/topo/typedesource/Plan">
        <rdf:type rdf:resource="http://www.w3.org/ns/prov#Entity"/>
        <rdfs:label xml:lang="en">plan</rdfs:label>
        <rdfs:label xml:lang="fr">plan</rdfs:label>
    </owl:NamedIndividual>
    


    <!-- http://data.ign.fr/id/codes/topo/typedesource/Scan25 -->


    <owl:NamedIndividual rdf:about="http://data.ign.fr/id/codes/topo/typedesource/Scan25">
        <rdf:type rdf:resource="http://www.w3.org/ns/prov#Entity"/>
        <rdfs:label xml:lang="en">Scan25</rdfs:label>
        <rdfs:label xml:lang="fr">Scan25</rdfs:label>
        <foaf:homepage rdf:resource="http://professionnels.ign.fr/scan25"/>
    </owl:NamedIndividual>
    


    <!-- http://data.ign.fr/id/codes/topo/typedesource/Terrain -->


    <owl:NamedIndividual rdf:about="http://data.ign.fr/id/codes/topo/typedesource/Terrain">
        <rdf:type rdf:resource="http://www.w3.org/ns/prov#Entity"/>
        <rdfs:label xml:lang="fr">relevé de terrain</rdfs:label>
        <rdfs:label xml:lang="en">topographic survey</rdfs:label>
    </owl:NamedIndividual>
    


    <!-- http://data.ign.fr/id/codes/topo/typedeterraindesport/BassinDeNatation -->


    <owl:NamedIndividual rdf:about="http://data.ign.fr/id/codes/topo/typedeterraindesport/BassinDeNatation">
        <rdf:type rdf:resource="http://data.ign.fr/def/topo#TypeDeTerrainDeSport"/>
        <rdf:type rdf:resource="http://www.w3.org/2004/02/skos/core#Concept"/>
        <skos:inScheme rdf:resource="http://data.ign.fr/id/codes/topo/typedeterraindesport/liste"/>
        <skos:broadMatch rdf:resource="http://data.ign.fr/id/codes/topo/typedezai/Piscine"/>
        <skos:definition xml:lang="fr">Bassin de natation d’une piscine découverte : bassin de natation, piscine (découverte).</skos:definition>
        <skos:definition xml:lang="en">Swimming pool of an outdoor swimming pool: swimming pool, swimming pool (discovery).</skos:definition>
        <skos:prefLabel xml:lang="fr">bassin de natation</skos:prefLabel>
        <skos:prefLabel xml:lang="en">swimming-pool</skos:prefLabel>
    </owl:NamedIndividual>
    


    <!-- http://data.ign.fr/id/codes/topo/typedeterraindesport/PisteDeSport -->


    <owl:NamedIndividual rdf:about="http://data.ign.fr/id/codes/topo/typedeterraindesport/PisteDeSport">
        <rdf:type rdf:resource="http://data.ign.fr/def/topo#TypeDeTerrainDeSport"/>
        <rdf:type rdf:resource="http://www.w3.org/2004/02/skos/core#Concept"/>
        <skos:inScheme rdf:resource="http://data.ign.fr/id/codes/topo/typedeterraindesport/liste"/>
        <skos:definition xml:lang="en">Large outdoor track reserved for the race: autodrome (track), automoto circuit (track), track (racetrack), racecourse (track), velodrome (track).</skos:definition>
        <skos:definition xml:lang="fr">Large piste en plein air réservée à la course : autodrome (piste), circuit automoto (piste), cynodrome (piste), hippodrome (piste), vélodrome (piste).</skos:definition>
        <skos:prefLabel xml:lang="fr">piste de sport</skos:prefLabel>
        <skos:prefLabel xml:lang="en">sports track</skos:prefLabel>
    </owl:NamedIndividual>
    


    <!-- http://data.ign.fr/id/codes/topo/typedeterraindesport/TerrainDeTennis -->


    <owl:NamedIndividual rdf:about="http://data.ign.fr/id/codes/topo/typedeterraindesport/TerrainDeTennis">
        <rdf:type rdf:resource="http://data.ign.fr/def/topo#TypeDeTerrainDeSport"/>
        <rdf:type rdf:resource="http://www.w3.org/2004/02/skos/core#Concept"/>
        <skos:inScheme rdf:resource="http://data.ign.fr/id/codes/topo/typedeterraindesport/liste"/>
        <skos:definition xml:lang="en">Specially landscaped grounds for playing tennis.</skos:definition>
        <skos:definition xml:lang="fr">Terrain spécialement aménagé pour la pratique du tennis.</skos:definition>
        <skos:prefLabel xml:lang="en">tennis court</skos:prefLabel>
        <skos:prefLabel xml:lang="fr">terrain de tennis</skos:prefLabel>
    </owl:NamedIndividual>
    


    <!-- http://data.ign.fr/id/codes/topo/typedeterraindesport/liste -->


    <owl:NamedIndividual rdf:about="http://data.ign.fr/id/codes/topo/typedeterraindesport/liste">
        <rdf:type rdf:resource="http://www.w3.org/2004/02/skos/core#ConceptScheme"/>
        <rdfs:comment xml:lang="en">List of different types of sports fields, represented as a hierarchy of SKOS concepts.</rdfs:comment>
        <rdfs:comment xml:lang="fr">Liste des différents types de terrains de sport, représentés comme une hiérarchie de concepts SKOS.</rdfs:comment>
        <rdfs:label xml:lang="fr">Type de terrain de sport</rdfs:label>
        <rdfs:label xml:lang="en">Type of sports ground</rdfs:label>
    </owl:NamedIndividual>
    


    <!-- http://data.ign.fr/id/codes/topo/typedetransportcable/CableTransporteur -->


    <owl:NamedIndividual rdf:about="http://data.ign.fr/id/codes/topo/typedetransportcable/CableTransporteur">
        <rdf:type rdf:resource="http://data.ign.fr/def/topo#TypeDeTransportCable"/>
        <rdf:type rdf:resource="http://www.w3.org/2004/02/skos/core#Concept"/>
        <skos:inScheme rdf:resource="http://data.ign.fr/id/codes/topo/typedetransportcable/liste"/>
        <skos:definition xml:lang="en">Means of transport consisting of one or more load-bearing cables used to transport equipment.</skos:definition>
        <skos:definition xml:lang="fr">Moyen de transport constitué d&apos;un ou de plusieurs câbles porteurs et servant à assurer le transport de matériel.</skos:definition>
        <skos:prefLabel xml:lang="en">cableway</skos:prefLabel>
        <skos:prefLabel xml:lang="fr">câble transporteur</skos:prefLabel>
    </owl:NamedIndividual>
    


    <!-- http://data.ign.fr/id/codes/topo/typedetransportcable/Telepherique -->


    <owl:NamedIndividual rdf:about="http://data.ign.fr/id/codes/topo/typedetransportcable/Telepherique">
        <rdf:type rdf:resource="http://data.ign.fr/def/topo#TypeDeTransportCable"/>
        <rdf:type rdf:resource="http://data.ign.fr/def/topo#TypeDeZAI"/>
        <rdf:type rdf:resource="http://www.w3.org/2004/02/skos/core#Concept"/>
        <skos:inScheme rdf:resource="http://data.ign.fr/id/codes/topo/typedetransportcable/liste"/>
        <skos:inScheme rdf:resource="http://data.ign.fr/id/codes/topo/typedezai/liste"/>
        <skos:broader rdf:resource="http://data.ign.fr/id/codes/topo/typedezai/PAITransport"/>
        <skos:definition xml:lang="en">Cable cars, including ski lifts, lifts, gondola lifts, ski lifts, telebens, chair lifts.</skos:definition>
        <skos:definition xml:lang="fr">Téléphériques, y compris les remonte-pentes, remontées mécaniques, télécabines, téléskis, télébennes, télésièges.</skos:definition>
        <skos:prefLabel xml:lang="en">aerial ropeway</skos:prefLabel>
        <skos:prefLabel xml:lang="fr">téléphérique</skos:prefLabel>
    </owl:NamedIndividual>
    


    <!-- http://data.ign.fr/id/codes/topo/typedetransportcable/liste -->


    <owl:NamedIndividual rdf:about="http://data.ign.fr/id/codes/topo/typedetransportcable/liste">
        <rdf:type rdf:resource="http://www.w3.org/2004/02/skos/core#ConceptScheme"/>
        <rdfs:comment xml:lang="en">List of different types of cable transport lines, represented as a hierarchy of SKOS concepts.</rdfs:comment>
        <rdfs:comment xml:lang="fr">Liste des différents types lignes de transport par câble, représentés comme une hiérarchie de concepts SKOS.</rdfs:comment>
        <rdfs:label xml:lang="fr">Type de ligne de transport par câble</rdfs:label>
        <rdfs:label xml:lang="en">Type of cableway transport line</rdfs:label>
    </owl:NamedIndividual>
    


    <!-- http://data.ign.fr/id/codes/topo/typedevegetation/Bananeraie -->


    <owl:NamedIndividual rdf:about="http://data.ign.fr/id/codes/topo/typedevegetation/Bananeraie">
        <rdf:type rdf:resource="http://data.ign.fr/def/topo#TypeDeVegetation"/>
        <rdf:type rdf:resource="http://www.w3.org/2004/02/skos/core#Concept"/>
        <skos:inScheme rdf:resource="http://data.ign.fr/id/codes/topo/typedevegetation/liste"/>
        <skos:broader rdf:resource="http://data.ign.fr/id/codes/topo/typedebatiment/ZoneArboree"/>
        <skos:definition xml:lang="en">Banana plantation.</skos:definition>
        <skos:definition xml:lang="fr">Plantation de bananiers.</skos:definition>
        <skos:prefLabel xml:lang="en">banana plantation</skos:prefLabel>
        <skos:prefLabel xml:lang="fr">bananeraie</skos:prefLabel>
    </owl:NamedIndividual>
    


    <!-- http://data.ign.fr/id/codes/topo/typedevegetation/Bois -->


    <owl:NamedIndividual rdf:about="http://data.ign.fr/id/codes/topo/typedevegetation/Bois">
        <rdf:type rdf:resource="http://data.ign.fr/def/topo#TypeDeVegetation"/>
        <rdf:type rdf:resource="http://www.w3.org/2004/02/skos/core#Concept"/>
        <skos:inScheme rdf:resource="http://data.ign.fr/id/codes/topo/typedevegetation/liste"/>
        <skos:inScheme rdf:resource="http://data.ign.fr/id/codes/topo/typedezai/liste"/>
        <skos:broader rdf:resource="http://data.ign.fr/id/codes/topo/typedebatiment/ZoneArboree"/>
        <skos:broader rdf:resource="http://data.ign.fr/id/codes/topo/typedezai/PAIEspaceNaturel"/>
        <skos:definition xml:lang="en">Area populated by forest trees covering at least 40% of the soil.</skos:definition>
        <skos:definition xml:lang="fr">Espace peuplé d’arbres forestiers couvrant au moins 40% du sol.</skos:definition>
        <skos:prefLabel xml:lang="fr">bois</skos:prefLabel>
        <skos:prefLabel xml:lang="en">wood</skos:prefLabel>
    </owl:NamedIndividual>
    


    <!-- http://data.ign.fr/id/codes/topo/typedevegetation/CanneASucre -->


    <owl:NamedIndividual rdf:about="http://data.ign.fr/id/codes/topo/typedevegetation/CanneASucre">
        <rdf:type rdf:resource="http://data.ign.fr/def/topo#TypeDeVegetation"/>
        <rdf:type rdf:resource="http://www.w3.org/2004/02/skos/core#Concept"/>
        <skos:inScheme rdf:resource="http://data.ign.fr/id/codes/topo/typedevegetation/liste"/>
        <skos:broader rdf:resource="http://data.ign.fr/id/codes/topo/typedebatiment/ZoneArboree"/>
        <skos:definition xml:lang="fr">Plantation de canne à sucre.</skos:definition>
        <skos:definition xml:lang="en">Plantation of sugar cane.</skos:definition>
        <skos:prefLabel xml:lang="fr">canne à sucre</skos:prefLabel>
        <skos:prefLabel xml:lang="en">sugarcane plantation</skos:prefLabel>
    </owl:NamedIndividual>
    


    <!-- http://data.ign.fr/id/codes/topo/typedevegetation/ForetFermeeConiferes -->


    <owl:NamedIndividual rdf:about="http://data.ign.fr/id/codes/topo/typedevegetation/ForetFermeeConiferes">
        <rdf:type rdf:resource="http://data.ign.fr/def/topo#TypeDeVegetation"/>
        <rdf:type rdf:resource="http://www.w3.org/2004/02/skos/core#Concept"/>
        <skos:inScheme rdf:resource="http://data.ign.fr/id/codes/topo/typedevegetation/liste"/>
        <skos:broader rdf:resource="http://data.ign.fr/id/codes/topo/typedebatiment/ZoneArboree"/>
        <skos:definition xml:lang="en">Area populated with forest trees covering at least 40% of the soil and composed mainly of conifers (ie a relative cover rate of more than 75%).</skos:definition>
        <skos:definition xml:lang="fr">Espace peuplé d’arbres forestiers couvrant au moins 40% du sol et composée essentiellement de conifères (soit un taux de couvert relatif de plus de 75%).</skos:definition>
        <skos:prefLabel xml:lang="en">closed softwood forest</skos:prefLabel>
        <skos:prefLabel xml:lang="fr">forêt fermée de conifères</skos:prefLabel>
    </owl:NamedIndividual>
    


    <!-- http://data.ign.fr/id/codes/topo/typedevegetation/ForetFermeeFeuillus -->


    <owl:NamedIndividual rdf:about="http://data.ign.fr/id/codes/topo/typedevegetation/ForetFermeeFeuillus">
        <rdf:type rdf:resource="http://data.ign.fr/def/topo#TypeDeVegetation"/>
        <rdf:type rdf:resource="http://www.w3.org/2004/02/skos/core#Concept"/>
        <skos:inScheme rdf:resource="http://data.ign.fr/id/codes/topo/typedevegetation/liste"/>
        <skos:broader rdf:resource="http://data.ign.fr/id/codes/topo/typedebatiment/ZoneArboree"/>
        <skos:definition xml:lang="en">Area populated with forest trees covering at least 40% of the soil, and composed of more than 75% of hardwoods (relative cover rate).</skos:definition>
        <skos:definition xml:lang="fr">Espace peuplé d’arbres forestiers couvrant au moins 40% du sol, et composée de plus de 75% de feuillus (taux de couvert relatif).</skos:definition>
        <skos:prefLabel xml:lang="en">closed hardwood forest</skos:prefLabel>
        <skos:prefLabel xml:lang="fr">forêt fermée de feuillus</skos:prefLabel>
    </owl:NamedIndividual>
    


    <!-- http://data.ign.fr/id/codes/topo/typedevegetation/ForetFermeeMixte -->


    <owl:NamedIndividual rdf:about="http://data.ign.fr/id/codes/topo/typedevegetation/ForetFermeeMixte">
        <rdf:type rdf:resource="http://data.ign.fr/def/topo#TypeDeVegetation"/>
        <rdf:type rdf:resource="http://www.w3.org/2004/02/skos/core#Concept"/>
        <skos:inScheme rdf:resource="http://data.ign.fr/id/codes/topo/typedevegetation/liste"/>
        <skos:broader rdf:resource="http://data.ign.fr/id/codes/topo/typedebatiment/ZoneArboree"/>
        <skos:definition xml:lang="en">Area populated with forest trees covering at least 40% of the soil, and composed of more than 25% and less than 75% of hardwoods (relative cover rate).</skos:definition>
        <skos:definition xml:lang="fr">Espace peuplé d’arbres forestiers couvrant au moins 40% du sol, et composée de plus de 25% et moins de 75% de feuillus (taux de couvert relatif).</skos:definition>
        <skos:prefLabel xml:lang="en">closed mixed forest</skos:prefLabel>
        <skos:prefLabel xml:lang="fr">forêt fermée mixte</skos:prefLabel>
    </owl:NamedIndividual>
    


    <!-- http://data.ign.fr/id/codes/topo/typedevegetation/ForetOuverte -->


    <owl:NamedIndividual rdf:about="http://data.ign.fr/id/codes/topo/typedevegetation/ForetOuverte">
        <rdf:type rdf:resource="http://data.ign.fr/def/topo#TypeDeVegetation"/>
        <rdf:type rdf:resource="http://www.w3.org/2004/02/skos/core#Concept"/>
        <skos:inScheme rdf:resource="http://data.ign.fr/id/codes/topo/typedevegetation/liste"/>
        <skos:broader rdf:resource="http://data.ign.fr/id/codes/topo/typedebatiment/ZoneArboree"/>
        <skos:definition xml:lang="en">Area populated with forest trees whose absolute cover is between 10% and 40%.</skos:definition>
        <skos:definition xml:lang="fr">Espace peuplé d’arbres forestiers dont le couvert absolu est compris entre 10% et 40%.</skos:definition>
        <skos:prefLabel xml:lang="fr">forêt ouverte</skos:prefLabel>
        <skos:prefLabel xml:lang="en">open forest</skos:prefLabel>
    </owl:NamedIndividual>
    


    <!-- http://data.ign.fr/id/codes/topo/typedevegetation/Haie -->


    <owl:NamedIndividual rdf:about="http://data.ign.fr/id/codes/topo/typedevegetation/Haie">
        <rdf:type rdf:resource="http://data.ign.fr/def/topo#TypeDeVegetation"/>
        <rdf:type rdf:resource="http://www.w3.org/2004/02/skos/core#Concept"/>
        <skos:inScheme rdf:resource="http://data.ign.fr/id/codes/topo/typedevegetation/liste"/>
        <skos:broader rdf:resource="http://data.ign.fr/id/codes/topo/typedebatiment/ZoneArboree"/>
        <skos:definition xml:lang="en">A natural fence made of trees, shrubs, thorns or branches that serves to limit or protect a field. Aligning trees or planting fruit trees less than 25 m wide.</skos:definition>
        <skos:definition xml:lang="fr">Clôture naturelle composée d’arbres, d’arbustes, d’épines ou de branchages et servant à limiter ou à protéger un champ. Alignement d’arbres ou plantation d’arbres fruitiers dont la largeur est inférieure à 25 m.</skos:definition>
        <skos:prefLabel xml:lang="fr">haie</skos:prefLabel>
        <skos:prefLabel xml:lang="en">hedge</skos:prefLabel>
    </owl:NamedIndividual>
    


    <!-- http://data.ign.fr/id/codes/topo/typedevegetation/LandeLigneuse -->


    <owl:NamedIndividual rdf:about="http://data.ign.fr/id/codes/topo/typedevegetation/LandeLigneuse">
        <rdf:type rdf:resource="http://data.ign.fr/def/topo#TypeDeVegetation"/>
        <rdf:type rdf:resource="http://www.w3.org/2004/02/skos/core#Concept"/>
        <skos:inScheme rdf:resource="http://data.ign.fr/id/codes/topo/typedevegetation/liste"/>
        <skos:broader rdf:resource="http://data.ign.fr/id/codes/topo/typedebatiment/ZoneArboree"/>
        <skos:definition xml:lang="en">Spontaneous vegetation that includes a significant proportion of woody plants (heather, broom, gorse, various thorny, etc.) and semi woody (ferns, phragmites ...) whose height does not exceed 5 meters. This woody vegetation has a vegetative cover of at least 25%.</skos:definition>
        <skos:definition xml:lang="fr">Végétation spontanée qui comprend une proportion importante de plantes ligneuses (bruyères, genêts, ajoncs, épineux divers, etc.) et semi ligneuses (fougères, phragmites…) dont la hauteur ne dépasse pas 5 mètres. Cette végétation ligneuse présente un couvert végétal d’au moins 25%.</skos:definition>
        <skos:prefLabel xml:lang="fr">lande ligneuse</skos:prefLabel>
        <skos:prefLabel xml:lang="en">woody heath</skos:prefLabel>
    </owl:NamedIndividual>
    


    <!-- http://data.ign.fr/id/codes/topo/typedevegetation/Mangrove -->


    <owl:NamedIndividual rdf:about="http://data.ign.fr/id/codes/topo/typedevegetation/Mangrove">
        <rdf:type rdf:resource="http://data.ign.fr/def/topo#TypeDeVegetation"/>
        <rdf:type rdf:resource="http://www.w3.org/2004/02/skos/core#Concept"/>
        <skos:inScheme rdf:resource="http://data.ign.fr/id/codes/topo/typedevegetation/liste"/>
        <skos:broader rdf:resource="http://data.ign.fr/id/codes/topo/typedebatiment/ZoneArboree"/>
        <skos:definition xml:lang="fr">Dans les régions côtières intertropicales,formation végétale caractérisée par des forêts impénétrables de palétuviers qui fixent leurs fortes racines dans les baies aux eaux calmes où se déposent boues et limons.</skos:definition>
        <skos:definition xml:lang="en">In the intertropical coastal regions, vegetation formation characterized by impenetrable forests of mangroves that fix their strong roots in the bays with calm waters where sludge and silt are deposited.</skos:definition>
        <skos:prefLabel xml:lang="fr">mangrove</skos:prefLabel>
        <skos:prefLabel xml:lang="en">mangrove forest</skos:prefLabel>
    </owl:NamedIndividual>
    


    <!-- http://data.ign.fr/id/codes/topo/typedevegetation/Peupleraie -->


    <owl:NamedIndividual rdf:about="http://data.ign.fr/id/codes/topo/typedevegetation/Peupleraie">
        <rdf:type rdf:resource="http://data.ign.fr/def/topo#TypeDeVegetation"/>
        <rdf:type rdf:resource="http://www.w3.org/2004/02/skos/core#Concept"/>
        <skos:inScheme rdf:resource="http://data.ign.fr/id/codes/topo/typedevegetation/liste"/>
        <skos:broader rdf:resource="http://data.ign.fr/id/codes/topo/typedebatiment/ZoneArboree"/>
        <skos:definition xml:lang="en">Area planted with poplars.</skos:definition>
        <skos:definition xml:lang="fr">Zone plantée de peupliers.</skos:definition>
        <skos:prefLabel xml:lang="fr">peupleraie</skos:prefLabel>
        <skos:prefLabel xml:lang="en">poplar plantation</skos:prefLabel>
    </owl:NamedIndividual>
    


    <!-- http://data.ign.fr/id/codes/topo/typedevegetation/Verger -->


    <owl:NamedIndividual rdf:about="http://data.ign.fr/id/codes/topo/typedevegetation/Verger">
        <rdf:type rdf:resource="http://data.ign.fr/def/topo#TypeDeVegetation"/>
        <rdf:type rdf:resource="http://www.w3.org/2004/02/skos/core#Concept"/>
        <skos:inScheme rdf:resource="http://data.ign.fr/id/codes/topo/typedevegetation/liste"/>
        <skos:broader rdf:resource="http://data.ign.fr/id/codes/topo/typedebatiment/ZoneArboree"/>
        <skos:definition xml:lang="en">Non-forest stand plantation area.</skos:definition>
        <skos:definition xml:lang="fr">Zone de plantation d’arbres hors peuplement forestier.</skos:definition>
        <skos:prefLabel xml:lang="en">orchard</skos:prefLabel>
        <skos:prefLabel xml:lang="fr">verger</skos:prefLabel>
    </owl:NamedIndividual>
    


    <!-- http://data.ign.fr/id/codes/topo/typedevegetation/Vigne -->


    <owl:NamedIndividual rdf:about="http://data.ign.fr/id/codes/topo/typedevegetation/Vigne">
        <rdf:type rdf:resource="http://data.ign.fr/def/topo#TypeDeVegetation"/>
        <rdf:type rdf:resource="http://www.w3.org/2004/02/skos/core#Concept"/>
        <skos:inScheme rdf:resource="http://data.ign.fr/id/codes/topo/typedevegetation/liste"/>
        <skos:broader rdf:resource="http://data.ign.fr/id/codes/topo/typedebatiment/ZoneArboree"/>
        <skos:definition xml:lang="en">Vineyard area.</skos:definition>
        <skos:definition xml:lang="fr">Zone de vignes.</skos:definition>
        <skos:prefLabel xml:lang="fr">vigne</skos:prefLabel>
        <skos:prefLabel xml:lang="en">vineyard</skos:prefLabel>
    </owl:NamedIndividual>
    


    <!-- http://data.ign.fr/id/codes/topo/typedevegetation/ZoneArboree -->


    <owl:NamedIndividual rdf:about="http://data.ign.fr/id/codes/topo/typedevegetation/ZoneArboree">
        <rdf:type rdf:resource="http://data.ign.fr/def/topo#TypeDeVegetation"/>
        <rdf:type rdf:resource="http://www.w3.org/2004/02/skos/core#Concept"/>
        <skos:inScheme rdf:resource="http://data.ign.fr/id/codes/topo/typedevegetation/liste"/>
        <skos:definition xml:lang="fr">Espace peuplé d’arbres d’essence quelconque.</skos:definition>
        <skos:definition xml:lang="en">Space populated with trees of any kind.</skos:definition>
        <skos:prefLabel xml:lang="en">wooded area</skos:prefLabel>
        <skos:prefLabel xml:lang="fr">zone arborée</skos:prefLabel>
    </owl:NamedIndividual>
    


    <!-- http://data.ign.fr/id/codes/topo/typedevegetation/liste -->


    <owl:NamedIndividual rdf:about="http://data.ign.fr/id/codes/topo/typedevegetation/liste">
        <rdf:type rdf:resource="http://www.w3.org/2004/02/skos/core#ConceptScheme"/>
        <rdfs:comment xml:lang="en">List of different types of vegetation, represented as a hierarchy of SKOS concepts.</rdfs:comment>
        <rdfs:comment xml:lang="fr">Liste des différents types de végétation, représentés comme une hiérarchie de concepts SKOS.</rdfs:comment>
        <rdfs:label xml:lang="fr">Type de végétation</rdfs:label>
        <rdfs:label xml:lang="en">Type of vegetation</rdfs:label>
        <skos:hasTopConcept rdf:resource="http://data.ign.fr/id/codes/topo/typedevegetation/ZoneArboree"/>
    </owl:NamedIndividual>
    


    <!-- http://data.ign.fr/id/codes/topo/typedevoieferree/Funiculaire -->


    <owl:NamedIndividual rdf:about="http://data.ign.fr/id/codes/topo/typedevoieferree/Funiculaire">
        <rdf:type rdf:resource="http://data.ign.fr/def/topo#TypeDeVoieFerree"/>
        <rdf:type rdf:resource="http://www.w3.org/2004/02/skos/core#Concept"/>
        <skos:inScheme rdf:resource="http://data.ign.fr/id/codes/topo/typedevoieferree/liste"/>
        <skos:altLabel xml:lang="en">rack-railway</skos:altLabel>
        <skos:altLabel xml:lang="fr">voie ferrée à crémaillère</skos:altLabel>
        <skos:definition xml:lang="fr">Funiculaire ou voie ferrée à crémaillère.</skos:definition>
        <skos:definition xml:lang="en">Funicular or cog railway.</skos:definition>
        <skos:prefLabel xml:lang="fr">Funiculaire</skos:prefLabel>
        <skos:prefLabel xml:lang="en">Funicular railway</skos:prefLabel>
    </owl:NamedIndividual>
    


    <!-- http://data.ign.fr/id/codes/topo/typedevoieferree/LGV -->


    <owl:NamedIndividual rdf:about="http://data.ign.fr/id/codes/topo/typedevoieferree/LGV">
        <rdf:type rdf:resource="http://data.ign.fr/def/topo#TypeDeVoieFerree"/>
        <rdf:type rdf:resource="http://www.w3.org/2004/02/skos/core#Concept"/>
        <skos:inScheme rdf:resource="http://data.ign.fr/id/codes/topo/typedevoieferree/liste"/>
        <skos:definition xml:lang="fr">Ligne ferroviaire réservée aux trains à grande vitesse.</skos:definition>
        <skos:definition xml:lang="en">Railway line reserved for high-speed trains.</skos:definition>
        <skos:prefLabel xml:lang="fr">ligne à grande vitesse</skos:prefLabel>
        <skos:prefLabel xml:lang="en">ultra-high speed railway</skos:prefLabel>
    </owl:NamedIndividual>
    


    <!-- http://data.ign.fr/id/codes/topo/typedevoieferree/VoieDeService -->


    <owl:NamedIndividual rdf:about="http://data.ign.fr/id/codes/topo/typedevoieferree/VoieDeService">
        <rdf:type rdf:resource="http://data.ign.fr/def/topo#TypeDeVoieFerree"/>
        <rdf:type rdf:resource="http://www.w3.org/2004/02/skos/core#Concept"/>
        <skos:inScheme rdf:resource="http://data.ign.fr/id/codes/topo/typedevoieferree/liste"/>
        <skos:definition xml:lang="fr">Les voies de service de moins de 200 m de long sont exclues, ainsi que les voies s’inscrivant dans un faisceau de voies ferrées de plus de 25 m de large (voir &lt;aire de triage&gt;) et les voies de service souterraines.</skos:definition>
        <skos:definition xml:lang="en">Service roads of less than 200 m in length are excluded, as well as tracks within a railway line of more than 25 m wide (see &lt;marshalling yard&gt;) and underground service roads.</skos:definition>
        <skos:prefLabel xml:lang="en">service track</skos:prefLabel>
        <skos:prefLabel xml:lang="fr">voie de service</skos:prefLabel>
    </owl:NamedIndividual>
    


    <!-- http://data.ign.fr/id/codes/topo/typedevoieferree/VoieNonExploitee -->


    <owl:NamedIndividual rdf:about="http://data.ign.fr/id/codes/topo/typedevoieferree/VoieNonExploitee">
        <rdf:type rdf:resource="http://data.ign.fr/def/topo#TypeDeVoieFerree"/>
        <rdf:type rdf:resource="http://www.w3.org/2004/02/skos/core#Concept"/>
        <skos:inScheme rdf:resource="http://data.ign.fr/id/codes/topo/typedevoieferree/liste"/>
        <skos:definition xml:lang="en">Decommissioned railway, railway closed to all traffic, neutralized railway.</skos:definition>
        <skos:definition xml:lang="fr">Voie ferrée déclassée, voie ferrée fermée à tout trafic, voie ferrée neutralisée.</skos:definition>
        <skos:prefLabel xml:lang="en">unused track</skos:prefLabel>
        <skos:prefLabel xml:lang="fr">voie non exploitée</skos:prefLabel>
    </owl:NamedIndividual>
    


    <!-- http://data.ign.fr/id/codes/topo/typedevoieferree/VoiePrincipale -->


    <owl:NamedIndividual rdf:about="http://data.ign.fr/id/codes/topo/typedevoieferree/VoiePrincipale">
        <rdf:type rdf:resource="http://data.ign.fr/def/topo#TypeDeVoieFerree"/>
        <rdf:type rdf:resource="http://www.w3.org/2004/02/skos/core#Concept"/>
        <skos:inScheme rdf:resource="http://data.ign.fr/id/codes/topo/typedevoieferree/liste"/>
        <skos:definition xml:lang="en">Railway line in operation used for the transport of passengers or goods. RER, railway line in operation, tourist railway, special branch line. All operating rail lines providing regular or seasonal service for the transport of passengers or goods. Metro lines and TGV lines are excluded.</skos:definition>
        <skos:definition xml:lang="fr">Voie ferrée en exploitation servant au transport des voyageurs ou des marchandises. RER, voie ferrée en exploitation, voie ferrée touristique, voie-mère d’embranchement particulier. Toutes les voies ferrées en exploitation assurant un service régulier ou saisonnier pour le transport des voyageurs ou des marchandises. Les lignes de métro et les lignes de TGV sont exclues.</skos:definition>
        <skos:prefLabel xml:lang="en">standard gauge railway</skos:prefLabel>
        <skos:prefLabel xml:lang="fr">voie ferrée principale</skos:prefLabel>
    </owl:NamedIndividual>
    


    <!-- http://data.ign.fr/id/codes/topo/typedevoieferree/VoieTransportUrbain -->


    <owl:NamedIndividual rdf:about="http://data.ign.fr/id/codes/topo/typedevoieferree/VoieTransportUrbain">
        <rdf:type rdf:resource="http://data.ign.fr/def/topo#TypeDeVoieFerree"/>
        <rdf:type rdf:resource="http://www.w3.org/2004/02/skos/core#Concept"/>
        <skos:inScheme rdf:resource="http://data.ign.fr/id/codes/topo/typedevoieferree/liste"/>
        <skos:definition xml:lang="en">Aerial metro or tram line.</skos:definition>
        <skos:definition xml:lang="fr">Ligne de métro aérien ou de tramway.</skos:definition>
        <skos:prefLabel xml:lang="en">urban transport railway</skos:prefLabel>
        <skos:prefLabel xml:lang="fr">voie de transport urbain</skos:prefLabel>
    </owl:NamedIndividual>
    


    <!-- http://data.ign.fr/id/codes/topo/typedevoieferree/liste -->


    <owl:NamedIndividual rdf:about="http://data.ign.fr/id/codes/topo/typedevoieferree/liste">
        <rdf:type rdf:resource="http://www.w3.org/2004/02/skos/core#ConceptScheme"/>
        <rdfs:comment xml:lang="en">List of different types of railways, represented as a hierarchy of SKOS concepts.</rdfs:comment>
        <rdfs:comment xml:lang="fr">Liste des différents types de voies ferrées, représentés comme une hiérarchie de concepts SKOS.</rdfs:comment>
        <rdfs:label xml:lang="fr">Type de voie ferrée</rdfs:label>
        <rdfs:label xml:lang="en">Type of railway track</rdfs:label>
    </owl:NamedIndividual>
    


    <!-- http://data.ign.fr/id/codes/topo/typedezai/Aerodrome -->


    <owl:NamedIndividual rdf:about="http://data.ign.fr/id/codes/topo/typedezai/Aerodrome">
        <rdf:type rdf:resource="http://data.ign.fr/def/topo#TypeDeZAI"/>
        <rdf:type rdf:resource="http://www.w3.org/2004/02/skos/core#Concept"/>
        <skos:inScheme rdf:resource="http://data.ign.fr/id/codes/topo/typedezai/liste"/>
        <skos:broader rdf:resource="http://data.ign.fr/id/codes/topo/typedezai/PAITransport"/>
        <skos:definition xml:lang="en">Any land or body of water specially designed for the landing, take-off and maneuvering of aircraft, including ancillary facilities it may include for the purposes of traffic and the service of aircraft: military aerodrome, military heliport. not taken into account the flying clubs, the gliding grounds, the ULM tracks.</skos:definition>
        <skos:definition xml:lang="fr">Tout terrain ou plan d&apos;eau spécialement aménagé pour l&apos;atterrissage, le décollage et les manoeuvres des aéronefs y compris les installations annexes qu&apos;il peut comporter pour les besoins du trafic et le service des aéronefs : aérodrome militaire, héliport militaire.Ne sont pas pris en compte les aéro-clubs, les terrains de vol à voile, les pistes d&apos;ULM.</skos:definition>
        <skos:prefLabel xml:lang="en">aerodrome</skos:prefLabel>
        <skos:prefLabel xml:lang="fr">aérodrome</skos:prefLabel>
    </owl:NamedIndividual>
    


    <!-- http://data.ign.fr/id/codes/topo/typedezai/AeroportInternational -->


    <owl:NamedIndividual rdf:about="http://data.ign.fr/id/codes/topo/typedezai/AeroportInternational">
        <rdf:type rdf:resource="http://data.ign.fr/def/topo#TypeDeZAI"/>
        <rdf:type rdf:resource="http://www.w3.org/2004/02/skos/core#Concept"/>
        <skos:inScheme rdf:resource="http://data.ign.fr/id/codes/topo/typedezai/liste"/>
        <skos:broader rdf:resource="http://data.ign.fr/id/codes/topo/typedezai/PAITransport"/>
        <skos:definition xml:lang="en">Aerodrome of international status on which facilities have been provided for the shelter, maintenance or distribution of aircraft, and for the reception, loading and unloading of passengers, the loading and unloading of merchandise.</skos:definition>
        <skos:definition xml:lang="fr">Aérodrome de statut international sur lequel ont été prévues des installations en vue de l&apos;abri, de l&apos;entretien ou de la répartition des aéronefs, ainsi que pour la réception, l&apos;embarquement et le débarquement des passagers, le chargement et le déchargement des marchandises.</skos:definition>
        <skos:prefLabel xml:lang="fr">aéroport international</skos:prefLabel>
        <skos:prefLabel xml:lang="en">international airport</skos:prefLabel>
    </owl:NamedIndividual>
    


    <!-- http://data.ign.fr/id/codes/topo/typedezai/AeroportQuelconque -->


    <owl:NamedIndividual rdf:about="http://data.ign.fr/id/codes/topo/typedezai/AeroportQuelconque">
        <rdf:type rdf:resource="http://data.ign.fr/def/topo#TypeDeZAI"/>
        <rdf:type rdf:resource="http://www.w3.org/2004/02/skos/core#Concept"/>
        <skos:inScheme rdf:resource="http://data.ign.fr/id/codes/topo/typedezai/liste"/>
        <skos:broader rdf:resource="http://data.ign.fr/id/codes/topo/typedezai/PAITransport"/>
        <skos:definition xml:lang="en">Aerodrome on which facilities have been provided for the purpose of sheltering, maintaining or distributing aircraft, and for receiving, loading and unloading passengers, loading and unloading of goods.</skos:definition>
        <skos:definition xml:lang="fr">Aérodrome sur lequel ont été prévues des installations en vue de l&apos;abri, de l&apos;entretien ou de la répartition des aéronefs, ainsi que pour la réception, l&apos;embarquement et le débarquement des passagers, le chargement et le déchargement des marchandises.</skos:definition>
        <skos:prefLabel xml:lang="en">airport</skos:prefLabel>
        <skos:prefLabel xml:lang="fr">aéroport</skos:prefLabel>
    </owl:NamedIndividual>
    


    <!-- http://data.ign.fr/id/codes/topo/typedezai/AireDeRepos -->


    <owl:NamedIndividual rdf:about="http://data.ign.fr/id/codes/topo/typedezai/AireDeRepos">
        <rdf:type rdf:resource="http://data.ign.fr/def/topo#TypeDeZAI"/>
        <rdf:type rdf:resource="http://www.w3.org/2004/02/skos/core#Concept"/>
        <skos:inScheme rdf:resource="http://data.ign.fr/id/codes/topo/typedezai/liste"/>
        <skos:broader rdf:resource="http://data.ign.fr/id/codes/topo/typedezai/PAITransport"/>
        <skos:definition xml:lang="en">Developed space (presence of a compulsory water point) away from the roadways, especially highways, to allow users to stop and rest.Emprise of the area. The contours of the surface never rest on sections of road that represent the axis of pavements.</skos:definition>
        <skos:definition xml:lang="fr">Espace aménagé (présence d&apos;un point d&apos;eau obligatoire) à l &apos;écart des chaussées, notamment des autoroutes, pour permettre aux usagers de s&apos;arrêter et de se reposer.Emprise de l&apos;aire. Les contours de la surface ne s&apos;appuient jamais sur des tronçons de route qui représentent l&apos;axe des chaussées.</skos:definition>
        <skos:prefLabel xml:lang="fr">aire de repos</skos:prefLabel>
        <skos:prefLabel xml:lang="en">rest area</skos:prefLabel>
    </owl:NamedIndividual>
    


    <!-- http://data.ign.fr/id/codes/topo/typedezai/AireDeService -->


    <owl:NamedIndividual rdf:about="http://data.ign.fr/id/codes/topo/typedezai/AireDeService">
        <rdf:type rdf:resource="http://data.ign.fr/def/topo#TypeDeZAI"/>
        <rdf:type rdf:resource="http://www.w3.org/2004/02/skos/core#Concept"/>
        <skos:inScheme rdf:resource="http://data.ign.fr/id/codes/topo/typedezai/liste"/>
        <skos:broader rdf:resource="http://data.ign.fr/id/codes/topo/typedezai/PAITransport"/>
        <skos:definition xml:lang="fr">Espace aménagé à l&apos;écart des chaussées, notamment des autoroutes, pour permettre aux usagers de se ravitailler en carburant. Emprise de l&apos;aire. Les contours de la surface ne s&apos;appuient jamais sur des tronçons de route (qui représentent l&apos;axe des chaussées).</skos:definition>
        <skos:definition xml:lang="en">Space arranged away from roads, especially highways, to allow users to refuel. Emprise of the area. The contours of the surface never rest on sections of road (which represent the axis of pavements).</skos:definition>
        <skos:prefLabel xml:lang="fr">aire de service</skos:prefLabel>
        <skos:prefLabel xml:lang="en">service area</skos:prefLabel>
    </owl:NamedIndividual>
    


    <!-- http://data.ign.fr/id/codes/topo/typedezai/Amer -->


    <owl:NamedIndividual rdf:about="http://data.ign.fr/id/codes/topo/typedezai/Amer">
        <rdf:type rdf:resource="http://data.ign.fr/def/topo#TypeDeZAI"/>
        <rdf:type rdf:resource="http://www.w3.org/2004/02/skos/core#Concept"/>
        <skos:inScheme rdf:resource="http://data.ign.fr/id/codes/topo/typedezai/liste"/>
        <skos:broader rdf:resource="http://data.ign.fr/id/codes/topo/typedezai/PAIHydrographie"/>
        <skos:definition xml:lang="fr">Point de repère visible de la mer : amer, bouée, balise, phare, feu, tourelle.</skos:definition>
        <skos:definition xml:lang="en">Visible landmark of the sea: bitter, buoy, beacon, lighthouse, fire, turret.</skos:definition>
        <skos:prefLabel xml:lang="fr">amer</skos:prefLabel>
        <skos:prefLabel xml:lang="en">seamark</skos:prefLabel>
    </owl:NamedIndividual>
    


    <!-- http://data.ign.fr/id/codes/topo/typedezai/Aquaculture -->


    <owl:NamedIndividual rdf:about="http://data.ign.fr/id/codes/topo/typedezai/Aquaculture">
        <rdf:type rdf:resource="http://data.ign.fr/def/topo#TypeDeZAI"/>
        <rdf:type rdf:resource="http://www.w3.org/2004/02/skos/core#Concept"/>
        <skos:inScheme rdf:resource="http://data.ign.fr/id/codes/topo/typedezai/liste"/>
        <skos:broader rdf:resource="http://data.ign.fr/id/codes/topo/typedezai/PAIIndustrielCommercial"/>
        <skos:definition xml:lang="fr">Site aménagé pour l&apos;élevage piscicole ou la culture d&apos;espèces animales marines (coques, coquilles Saint-Jacques, huîtres, moules, palourdes,etc.) : bouchot, parc à huîtres, zone conchylicole, zone mytilicole, zone ostréicole. Toutes les zones de plus de 3 ha possédant des installations fixes de pêche et délimitées par des alignements de pieux, les parcs à huîtres, les bassins. Les installations de pêche au carrelet sont exclues.</skos:definition>
        <skos:definition xml:lang="en">Site developed for fish farming or the cultivation of marine animal species (hulls, scallops, oysters, mussels, clams, etc.): bouchot, oyster beds, shellfish growing area, mussel zone, oyster farming area. All areas of more than 3 ha with fixed fishing facilities and defined by pile alignments, oyster beds, ponds. The plaice fishing facilities are excluded.</skos:definition>
        <skos:prefLabel xml:lang="en">aquaculture facilities</skos:prefLabel>
        <skos:prefLabel xml:lang="fr">installation d&apos;aquaculture</skos:prefLabel>
    </owl:NamedIndividual>
    


    <!-- http://data.ign.fr/id/codes/topo/typedezai/Arbre -->


    <owl:NamedIndividual rdf:about="http://data.ign.fr/id/codes/topo/typedezai/Arbre">
        <rdf:type rdf:resource="http://data.ign.fr/def/topo#TypeDeZAI"/>
        <rdf:type rdf:resource="http://www.w3.org/2004/02/skos/core#Concept"/>
        <skos:inScheme rdf:resource="http://data.ign.fr/id/codes/topo/typedezai/liste"/>
        <skos:broader rdf:resource="http://data.ign.fr/id/codes/topo/typedezai/PAIEspaceNaturel"/>
        <skos:definition xml:lang="fr">Arbre nommé isolé, arbre remarquable.</skos:definition>
        <skos:definition xml:lang="en">Isolated named tree, remarkable tree.</skos:definition>
        <skos:prefLabel xml:lang="fr">arbre</skos:prefLabel>
        <skos:prefLabel xml:lang="en">tree</skos:prefLabel>
    </owl:NamedIndividual>
    


    <!-- http://data.ign.fr/id/codes/topo/typedezai/Baie -->


    <owl:NamedIndividual rdf:about="http://data.ign.fr/id/codes/topo/typedezai/Baie">
        <rdf:type rdf:resource="http://data.ign.fr/def/topo#TypeDeZAI"/>
        <rdf:type rdf:resource="http://www.w3.org/2004/02/skos/core#Concept"/>
        <skos:inScheme rdf:resource="http://data.ign.fr/id/codes/topo/typedezai/liste"/>
        <skos:broader rdf:resource="http://data.ign.fr/id/codes/topo/typedezai/PAIHydrographie"/>
        <skos:definition xml:lang="fr">Espace marin pénétrant entre les terres : anse, baie, calanque, crique, golfe.</skos:definition>
        <skos:definition xml:lang="en">Marine space penetrating between the grounds: cove, bay, cove, cove, gulf.</skos:definition>
        <skos:prefLabel xml:lang="fr">baie</skos:prefLabel>
        <skos:prefLabel xml:lang="en">bay</skos:prefLabel>
    </owl:NamedIndividual>
    


    <!-- http://data.ign.fr/id/codes/topo/typedezai/Banc -->


    <owl:NamedIndividual rdf:about="http://data.ign.fr/id/codes/topo/typedezai/Banc">
        <rdf:type rdf:resource="http://data.ign.fr/def/topo#TypeDeZAI"/>
        <rdf:type rdf:resource="http://www.w3.org/2004/02/skos/core#Concept"/>
        <skos:inScheme rdf:resource="http://data.ign.fr/id/codes/topo/typedezai/liste"/>
        <skos:broader rdf:resource="http://data.ign.fr/id/codes/topo/typedezai/PAIHydrographie"/>
        <skos:definition xml:lang="en">At sea or on a river, non-rocky underwater relief representing a potential danger for navigation: benches, shoals.</skos:definition>
        <skos:definition xml:lang="fr">En mer ou sur un fleuve, relief sous-marin non rocheux représentant un danger potentiel pour la navigation: bancs, hauts-fonds.</skos:definition>
        <skos:prefLabel xml:lang="fr">banc</skos:prefLabel>
        <skos:prefLabel xml:lang="en">bank</skos:prefLabel>
    </owl:NamedIndividual>
    


    <!-- http://data.ign.fr/id/codes/topo/typedezai/Barrage -->


    <owl:NamedIndividual rdf:about="http://data.ign.fr/id/codes/topo/typedezai/Barrage">
        <rdf:type rdf:resource="http://data.ign.fr/def/topo#TypeDeZAI"/>
        <rdf:type rdf:resource="http://www.w3.org/2004/02/skos/core#Concept"/>
        <skos:inScheme rdf:resource="http://data.ign.fr/id/codes/topo/typedezai/liste"/>
        <skos:broader rdf:resource="http://data.ign.fr/id/codes/topo/typedezai/PAITransport"/>
        <skos:definition xml:lang="en">Artificial obstacle placed across a watercourse: dam, lock, valve.</skos:definition>
        <skos:definition xml:lang="fr">Obstacle artificiel placé en travers d&apos;un cours d&apos;eau : barrage, écluse, vanne.</skos:definition>
        <skos:narrowMatch rdf:resource="http://data.ign.fr/id/codes/topo/typedebatiment/Barrage"/>
        <skos:narrowMatch rdf:resource="http://data.ign.fr/id/codes/topo/typedebatiment/Ecluse"/>
        <skos:prefLabel xml:lang="en">barrage</skos:prefLabel>
        <skos:prefLabel xml:lang="fr">barrage</skos:prefLabel>
    </owl:NamedIndividual>
    


    <!-- http://data.ign.fr/id/codes/topo/typedezai/BarriereDePeage -->


    <owl:NamedIndividual rdf:about="http://data.ign.fr/id/codes/topo/typedezai/BarriereDePeage">
        <rdf:type rdf:resource="http://data.ign.fr/def/topo#TypeDeZAI"/>
        <rdf:type rdf:resource="http://www.w3.org/2004/02/skos/core#Concept"/>
        <skos:inScheme rdf:resource="http://data.ign.fr/id/codes/topo/typedezai/liste"/>
        <skos:broader rdf:resource="http://data.ign.fr/id/codes/topo/typedezai/PAITransport"/>
        <skos:definition xml:lang="fr">Barrière de péage. Toutes les barrières de péage sont représentées, qu&apos;elles soient ou non accompagnées d&apos;un élargissement de la chaussée ou d&apos;un bâtiment : péage d&apos;autoroute, de pont, de route.</skos:definition>
        <skos:definition xml:lang="en">Toll barrier. All toll barriers are represented, whether or not accompanied by a widening of the roadway or a building: highway toll, bridge, road.</skos:definition>
        <skos:prefLabel xml:lang="fr">barrière de péage</skos:prefLabel>
        <skos:prefLabel xml:lang="en">toll-gate</skos:prefLabel>
        <skos:relatedMatch rdf:resource="http://data.ign.fr/id/codes/topo/typedebatiment/Peage"/>
    </owl:NamedIndividual>
    


    <!-- http://data.ign.fr/id/codes/topo/typedezai/Borne -->


    <owl:NamedIndividual rdf:about="http://data.ign.fr/id/codes/topo/typedezai/Borne">
        <rdf:type rdf:resource="http://data.ign.fr/def/topo#TypeDeZAI"/>
        <rdf:type rdf:resource="http://www.w3.org/2004/02/skos/core#Concept"/>
        <skos:inScheme rdf:resource="http://data.ign.fr/id/codes/topo/typedezai/liste"/>
        <skos:broader rdf:resource="http://data.ign.fr/id/codes/topo/typedezai/PAIAdministratifOuMilitaire"/>
        <skos:definition xml:lang="fr">Borne nommée : borne frontière, point de triangulation, point frontière.</skos:definition>
        <skos:definition xml:lang="en">Named terminal: boundary marker, triangulation point, boundary point.</skos:definition>
        <skos:prefLabel xml:lang="fr">borne</skos:prefLabel>
        <skos:prefLabel xml:lang="en">marker</skos:prefLabel>
    </owl:NamedIndividual>
    


    <!-- http://data.ign.fr/id/codes/topo/typedezai/BureauDePoste -->


    <owl:NamedIndividual rdf:about="http://data.ign.fr/id/codes/topo/typedezai/BureauDePoste">
        <rdf:type rdf:resource="http://data.ign.fr/def/topo#TypeDeZAI"/>
        <rdf:type rdf:resource="http://www.w3.org/2004/02/skos/core#Concept"/>
        <skos:inScheme rdf:resource="http://data.ign.fr/id/codes/topo/typedezai/liste"/>
        <skos:altLabel xml:lang="en">general post office</skos:altLabel>
        <skos:altLabel xml:lang="fr">hôtel des postes</skos:altLabel>
        <skos:broader rdf:resource="http://data.ign.fr/id/codes/topo/typedezai/PAIAdministratifOuMilitaire"/>
        <skos:definition xml:lang="fr">Bureau de poste ouvert au public : Bureau de poste, hôtel des postes. Seuls les bureaux de poste ouverts en permanence sont inclus. En général, dans les agglomérations, seules les postes centrales sont incluses.</skos:definition>
        <skos:definition xml:lang="en">Post Office open to the public: Post Office, Post Office. Only permanently open post offices are included. In general, in the agglomerations, only the central stations are included.</skos:definition>
        <skos:prefLabel xml:lang="fr">bureau de poste</skos:prefLabel>
        <skos:prefLabel xml:lang="en">post office</skos:prefLabel>
    </owl:NamedIndividual>
    


    <!-- http://data.ign.fr/id/codes/topo/typedezai/Camping -->


    <owl:NamedIndividual rdf:about="http://data.ign.fr/id/codes/topo/typedezai/Camping">
        <rdf:type rdf:resource="http://data.ign.fr/def/topo#TypeDeZAI"/>
        <rdf:type rdf:resource="http://www.w3.org/2004/02/skos/core#Concept"/>
        <skos:inScheme rdf:resource="http://data.ign.fr/id/codes/topo/typedezai/liste"/>
        <skos:broader rdf:resource="http://data.ign.fr/id/codes/topo/typedezai/PAICultureLoisirs"/>
        <skos:definition xml:lang="fr">Emplacement aménagé pour la pratique du camping d&apos;une superficie de plus de 2 ha.</skos:definition>
        <skos:definition xml:lang="en">Site arranged for the practice of the camping of an area of more than 2 ha.</skos:definition>
        <skos:prefLabel xml:lang="fr">camping</skos:prefLabel>
        <skos:prefLabel xml:lang="en">camping grounds</skos:prefLabel>
    </owl:NamedIndividual>
    


    <!-- http://data.ign.fr/id/codes/topo/typedezai/Canal -->


    <owl:NamedIndividual rdf:about="http://data.ign.fr/id/codes/topo/typedezai/Canal">
        <rdf:type rdf:resource="http://data.ign.fr/def/topo#TypeDeZAI"/>
        <rdf:type rdf:resource="http://www.w3.org/2004/02/skos/core#Concept"/>
        <skos:inScheme rdf:resource="http://data.ign.fr/id/codes/topo/typedezai/liste"/>
        <skos:broader rdf:resource="http://data.ign.fr/id/codes/topo/typedezai/PAIHydrographie"/>
        <skos:definition xml:lang="en">Artificial water course: old canal, reach, canal, ditch, channel.</skos:definition>
        <skos:definition xml:lang="fr">Cours d&apos;eau artificiel : ancien canal, bief, canal, fossé, rigole.</skos:definition>
        <skos:prefLabel xml:lang="fr">canal</skos:prefLabel>
        <skos:prefLabel xml:lang="en">channel</skos:prefLabel>
    </owl:NamedIndividual>
    


    <!-- http://data.ign.fr/id/codes/topo/typedezai/Carrefour -->


    <owl:NamedIndividual rdf:about="http://data.ign.fr/id/codes/topo/typedezai/Carrefour">
        <rdf:type rdf:resource="http://data.ign.fr/def/topo#TypeDeZAI"/>
        <rdf:type rdf:resource="http://www.w3.org/2004/02/skos/core#Concept"/>
        <skos:inScheme rdf:resource="http://data.ign.fr/id/codes/topo/typedezai/liste"/>
        <skos:broader rdf:resource="http://data.ign.fr/id/codes/topo/typedezai/PAITransport"/>
        <skos:definition xml:lang="en">Node of the road network: road junction, interchange, roundabout.</skos:definition>
        <skos:definition xml:lang="fr">Noeud du réseau routier : carrefour routier, échangeur, rond-point.</skos:definition>
        <skos:prefLabel xml:lang="fr">carrefour</skos:prefLabel>
        <skos:prefLabel xml:lang="en">crossroads</skos:prefLabel>
    </owl:NamedIndividual>
    


    <!-- http://data.ign.fr/id/codes/topo/typedezai/CaserneDePompiers -->


    <owl:NamedIndividual rdf:about="http://data.ign.fr/id/codes/topo/typedezai/CaserneDePompiers">
        <rdf:type rdf:resource="http://data.ign.fr/def/topo#TypeDeZAI"/>
        <rdf:type rdf:resource="http://www.w3.org/2004/02/skos/core#Concept"/>
        <skos:inScheme rdf:resource="http://data.ign.fr/id/codes/topo/typedezai/liste"/>
        <skos:broader rdf:resource="http://data.ign.fr/id/codes/topo/typedezai/PAIAdministratifOuMilitaire"/>
        <skos:definition xml:lang="en">Building with or without an office or a permanence and which is entirely concerned by the activity of the body of the Fire-fighters.</skos:definition>
        <skos:definition xml:lang="fr">Bâtiment ayant ou non un bureau ou une permanence et qui est entièment concerné par l&apos;activité du corps des Sapeurs-Pompiers.</skos:definition>
        <skos:prefLabel xml:lang="fr">caserne de pompiers</skos:prefLabel>
        <skos:prefLabel xml:lang="en">fire station</skos:prefLabel>
    </owl:NamedIndividual>
    


    <!-- http://data.ign.fr/id/codes/topo/typedezai/CentraleElectrique -->


    <owl:NamedIndividual rdf:about="http://data.ign.fr/id/codes/topo/typedezai/CentraleElectrique">
        <rdf:type rdf:resource="http://data.ign.fr/def/topo#TypeDeZAI"/>
        <rdf:type rdf:resource="http://www.w3.org/2004/02/skos/core#Concept"/>
        <skos:inScheme rdf:resource="http://data.ign.fr/id/codes/topo/typedezai/liste"/>
        <skos:broader rdf:resource="http://data.ign.fr/id/codes/topo/typedezai/PAIIndustrielCommercial"/>
        <skos:definition xml:lang="en">Plant where electric power is produced: hydroelectric plant, thermal power station, nuclear power station. Underground power plants are excluded.</skos:definition>
        <skos:definition xml:lang="fr">Usine où l&apos;on produit de l&apos;énergie électrique : centrale hydroélectrique, centrale thermique, centrale nucléaire. Les centrales électriques souterraines sont exclues.</skos:definition>
        <skos:prefLabel xml:lang="fr">centrale électrique</skos:prefLabel>
        <skos:prefLabel xml:lang="en">power station</skos:prefLabel>
    </owl:NamedIndividual>
    


    <!-- http://data.ign.fr/id/codes/topo/typedezai/Chemin -->


    <owl:NamedIndividual rdf:about="http://data.ign.fr/id/codes/topo/typedezai/Chemin">
        <rdf:type rdf:resource="http://data.ign.fr/def/topo#TypeDeZAI"/>
        <rdf:type rdf:resource="http://www.w3.org/2004/02/skos/core#Concept"/>
        <skos:inScheme rdf:resource="http://data.ign.fr/id/codes/topo/typedezai/liste"/>
        <skos:broader rdf:resource="http://data.ign.fr/id/codes/topo/typedezai/PAITransport"/>
        <skos:definition xml:lang="en">Non-road communication path: driveway, path, forest laie, path.</skos:definition>
        <skos:definition xml:lang="fr">Voie de communication non routière : allée, chemin, laie forestière, sentier.</skos:definition>
        <skos:prefLabel xml:lang="fr">chemin</skos:prefLabel>
        <skos:prefLabel xml:lang="en">trail</skos:prefLabel>
    </owl:NamedIndividual>
    


    <!-- http://data.ign.fr/id/codes/topo/typedezai/Construction -->


    <owl:NamedIndividual rdf:about="http://data.ign.fr/id/codes/topo/typedezai/Construction">
        <rdf:type rdf:resource="http://data.ign.fr/def/topo#TypeDeZAI"/>
        <rdf:type rdf:resource="http://www.w3.org/2004/02/skos/core#Concept"/>
        <skos:inScheme rdf:resource="http://data.ign.fr/id/codes/topo/typedezai/liste"/>
        <skos:broader rdf:resource="http://data.ign.fr/id/codes/topo/typedezai/PAICultureLoisirs"/>
        <skos:definition xml:lang="en">Construction named inhabited or associated with a group of houses: various construction, dovecote, windmill.</skos:definition>
        <skos:definition xml:lang="fr">Construction nommée habitée ou associée à un groupe d&apos;habitations : construction diverse, pigeonnier, moulin à vent.</skos:definition>
        <skos:prefLabel xml:lang="fr">construction nommée</skos:prefLabel>
        <skos:prefLabel xml:lang="en">named building</skos:prefLabel>
    </owl:NamedIndividual>
    


    <!-- http://data.ign.fr/id/codes/topo/typedezai/Croix -->


    <owl:NamedIndividual rdf:about="http://data.ign.fr/id/codes/topo/typedezai/Croix">
        <rdf:type rdf:resource="http://data.ign.fr/def/topo#TypeDeZAI"/>
        <rdf:type rdf:resource="http://www.w3.org/2004/02/skos/core#Concept"/>
        <skos:inScheme rdf:resource="http://data.ign.fr/id/codes/topo/typedezai/liste"/>
        <skos:broader rdf:resource="http://data.ign.fr/id/codes/topo/typedezai/PAIReligieux"/>
        <skos:definition xml:lang="fr">Monument religieux : croix, calvaire, vierge, statue religieuse.</skos:definition>
        <skos:definition xml:lang="en">Religious monument: cross, calvary, virgin, religious statue.</skos:definition>
        <skos:prefLabel xml:lang="fr">croix</skos:prefLabel>
        <skos:prefLabel xml:lang="en">cross</skos:prefLabel>
    </owl:NamedIndividual>
    


    <!-- http://data.ign.fr/id/codes/topo/typedezai/CulteCatholiqueOuOrthodoxe -->


    <owl:NamedIndividual rdf:about="http://data.ign.fr/id/codes/topo/typedezai/CulteCatholiqueOuOrthodoxe">
        <rdf:type rdf:resource="http://data.ign.fr/def/topo#TypeDeZAI"/>
        <rdf:type rdf:resource="http://www.w3.org/2004/02/skos/core#Concept"/>
        <skos:inScheme rdf:resource="http://data.ign.fr/id/codes/topo/typedezai/liste"/>
        <skos:broader rdf:resource="http://data.ign.fr/id/codes/topo/typedezai/PAIReligieux"/>
        <skos:definition xml:lang="en">Building reserved for the exercise of Catholic or Orthodox worship: church, cathedral, basilica, chapel, abbey, oratory.</skos:definition>
        <skos:definition xml:lang="fr">Bâtiment réservé à l&apos;exercice du culte catholique ou orthodoxe : église, cathédrale, basilique, chapelle, abbaye, oratoire.</skos:definition>
        <skos:prefLabel xml:lang="en">catholic or orthodox building</skos:prefLabel>
        <skos:prefLabel xml:lang="fr">édifice religieux catholique ou orthodoxe</skos:prefLabel>
    </owl:NamedIndividual>
    


    <!-- http://data.ign.fr/id/codes/topo/typedezai/CulteDivers -->


    <owl:NamedIndividual rdf:about="http://data.ign.fr/id/codes/topo/typedezai/CulteDivers">
        <rdf:type rdf:resource="http://data.ign.fr/def/topo#TypeDeZAI"/>
        <rdf:type rdf:resource="http://www.w3.org/2004/02/skos/core#Concept"/>
        <skos:inScheme rdf:resource="http://data.ign.fr/id/codes/topo/typedezai/liste"/>
        <skos:broader rdf:resource="http://data.ign.fr/id/codes/topo/typedezai/PAIReligieux"/>
        <skos:definition xml:lang="en">Building reserved for religious worship other than Christian, Islamic or Jewish: Buddhist temple, Hindu temple.</skos:definition>
        <skos:definition xml:lang="fr">Bâtiment réservé à l&apos;exercice d&apos;un culte religieux autre que chrétien, islamique ou israélite : temple bouddhiste, temple hindouiste.</skos:definition>
        <skos:prefLabel xml:lang="en">other religious building</skos:prefLabel>
        <skos:prefLabel xml:lang="fr">édifice religieux divers</skos:prefLabel>
    </owl:NamedIndividual>
    


    <!-- http://data.ign.fr/id/codes/topo/typedezai/CulteIslamique -->


    <owl:NamedIndividual rdf:about="http://data.ign.fr/id/codes/topo/typedezai/CulteIslamique">
        <rdf:type rdf:resource="http://data.ign.fr/def/topo#TypeDeZAI"/>
        <rdf:type rdf:resource="http://www.w3.org/2004/02/skos/core#Concept"/>
        <skos:inScheme rdf:resource="http://data.ign.fr/id/codes/topo/typedezai/liste"/>
        <skos:broader rdf:resource="http://data.ign.fr/id/codes/topo/typedezai/PAIReligieux"/>
        <skos:definition xml:lang="en">Building reserved for the exercise of Islamic worship: mosque.</skos:definition>
        <skos:definition xml:lang="fr">Bâtiment réservé à l&apos;exercice du culte islamique : mosquée.</skos:definition>
        <skos:prefLabel xml:lang="en">moslem religious building</skos:prefLabel>
        <skos:prefLabel xml:lang="fr">édifice religieux islamique</skos:prefLabel>
    </owl:NamedIndividual>
    


    <!-- http://data.ign.fr/id/codes/topo/typedezai/CulteIsraelite -->


    <owl:NamedIndividual rdf:about="http://data.ign.fr/id/codes/topo/typedezai/CulteIsraelite">
        <rdf:type rdf:resource="http://data.ign.fr/def/topo#TypeDeZAI"/>
        <rdf:type rdf:resource="http://www.w3.org/2004/02/skos/core#Concept"/>
        <skos:inScheme rdf:resource="http://data.ign.fr/id/codes/topo/typedezai/liste"/>
        <skos:broader rdf:resource="http://data.ign.fr/id/codes/topo/typedezai/PAIReligieux"/>
        <skos:definition xml:lang="en">Building reserved for the exercise of Jewish worship: synagogue.</skos:definition>
        <skos:definition xml:lang="fr">Bâtiment réservé à l&apos;exercice du culte israélite : synagogue.</skos:definition>
        <skos:prefLabel xml:lang="en">jewish religious building</skos:prefLabel>
        <skos:prefLabel xml:lang="fr">édifice religieux israélite</skos:prefLabel>
    </owl:NamedIndividual>
    


    <!-- http://data.ign.fr/id/codes/topo/typedezai/CulteProtestant -->


    <owl:NamedIndividual rdf:about="http://data.ign.fr/id/codes/topo/typedezai/CulteProtestant">
        <rdf:type rdf:resource="http://data.ign.fr/def/topo#TypeDeZAI"/>
        <rdf:type rdf:resource="http://www.w3.org/2004/02/skos/core#Concept"/>
        <skos:inScheme rdf:resource="http://data.ign.fr/id/codes/topo/typedezai/liste"/>
        <skos:broader rdf:resource="http://data.ign.fr/id/codes/topo/typedezai/PAIReligieux"/>
        <skos:definition xml:lang="en">Building reserved for the practice of Protestant worship: temple (Protestant), Reformed church.</skos:definition>
        <skos:definition xml:lang="fr">Bâtiment réservé à l&apos;exercice du culte protestant : temple (protestant), église réformée.</skos:definition>
        <skos:prefLabel xml:lang="en">protestant building</skos:prefLabel>
        <skos:prefLabel xml:lang="fr">édifice religieux protestant</skos:prefLabel>
    </owl:NamedIndividual>
    


    <!-- http://data.ign.fr/id/codes/topo/typedezai/Digue -->


    <owl:NamedIndividual rdf:about="http://data.ign.fr/id/codes/topo/typedezai/Digue">
        <rdf:type rdf:resource="http://data.ign.fr/def/topo#TypeDeZAI"/>
        <rdf:type rdf:resource="http://www.w3.org/2004/02/skos/core#Concept"/>
        <skos:inScheme rdf:resource="http://data.ign.fr/id/codes/topo/typedezai/liste"/>
        <skos:broader rdf:resource="http://data.ign.fr/id/codes/topo/typedezai/PAICultureLoisirs"/>
        <skos:definition xml:lang="fr">Digue, môle, jetée.</skos:definition>
        <skos:definition xml:lang="en">Dike, breakwater, jetty.</skos:definition>
        <skos:prefLabel xml:lang="fr">digue</skos:prefLabel>
        <skos:prefLabel xml:lang="en">dike</skos:prefLabel>
    </owl:NamedIndividual>
    


    <!-- http://data.ign.fr/id/codes/topo/typedezai/Dolmen -->


    <owl:NamedIndividual rdf:about="http://data.ign.fr/id/codes/topo/typedezai/Dolmen">
        <rdf:type rdf:resource="http://data.ign.fr/def/topo#TypeDeZAI"/>
        <rdf:type rdf:resource="http://www.w3.org/2004/02/skos/core#Concept"/>
        <skos:inScheme rdf:resource="http://data.ign.fr/id/codes/topo/typedezai/liste"/>
        <skos:broader rdf:resource="http://data.ign.fr/id/codes/topo/typedezai/PAICultureLoisirs"/>
        <skos:definition xml:lang="en">Megalithic monument formed by a large flat stone resting on other vertically standing stones. Covered walkways are included.</skos:definition>
        <skos:definition xml:lang="fr">Monument mégalithique formé d&apos;une grande pierre plate posée sur d&apos;autres pierres dressées verticalement. Les allées couvertes sont incluses.</skos:definition>
        <skos:prefLabel xml:lang="en">dolmen</skos:prefLabel>
        <skos:prefLabel xml:lang="fr">dolmen</skos:prefLabel>
    </owl:NamedIndividual>
    


    <!-- http://data.ign.fr/id/codes/topo/typedezai/Echangeur -->


    <owl:NamedIndividual rdf:about="http://data.ign.fr/id/codes/topo/typedezai/Echangeur">
        <rdf:type rdf:resource="http://data.ign.fr/def/topo#TypeDeZAI"/>
        <rdf:type rdf:resource="http://www.w3.org/2004/02/skos/core#Concept"/>
        <skos:inScheme rdf:resource="http://data.ign.fr/id/codes/topo/typedezai/liste"/>
        <skos:broader rdf:resource="http://data.ign.fr/id/codes/topo/typedezai/PAITransport"/>
        <skos:definition xml:lang="en">Node of the divided road network. Motorway interchange bearing a name.</skos:definition>
        <skos:definition xml:lang="fr">Noeud du réseau routier à chaussées séparées. Échangeur autoroutier portant un nom.</skos:definition>
        <skos:prefLabel xml:lang="en">interchange</skos:prefLabel>
        <skos:prefLabel xml:lang="fr">échangeur</skos:prefLabel>
    </owl:NamedIndividual>
    


    <!-- http://data.ign.fr/id/codes/topo/typedezai/Embouchure -->


    <owl:NamedIndividual rdf:about="http://data.ign.fr/id/codes/topo/typedezai/Embouchure">
        <rdf:type rdf:resource="http://data.ign.fr/def/topo#TypeDeZAI"/>
        <rdf:type rdf:resource="http://www.w3.org/2004/02/skos/core#Concept"/>
        <skos:inScheme rdf:resource="http://data.ign.fr/id/codes/topo/typedezai/liste"/>
        <skos:broader rdf:resource="http://data.ign.fr/id/codes/topo/typedezai/PAIHydrographie"/>
        <skos:definition xml:lang="fr">Embouchure d&apos;un fleuve : delta, embouchure, estuaire.</skos:definition>
        <skos:definition xml:lang="en">Mouth of a river: delta, mouth, estuary.</skos:definition>
        <skos:prefLabel xml:lang="fr">embouchure</skos:prefLabel>
        <skos:prefLabel xml:lang="en">mouth</skos:prefLabel>
    </owl:NamedIndividual>
    


    <!-- http://data.ign.fr/id/codes/topo/typedezai/EnceinteMilitaire -->


    <owl:NamedIndividual rdf:about="http://data.ign.fr/id/codes/topo/typedezai/EnceinteMilitaire">
        <rdf:type rdf:resource="http://data.ign.fr/def/topo#TypeDeZAI"/>
        <rdf:type rdf:resource="http://www.w3.org/2004/02/skos/core#Concept"/>
        <skos:inScheme rdf:resource="http://data.ign.fr/id/codes/topo/typedezai/liste"/>
        <skos:broader rdf:resource="http://data.ign.fr/id/codes/topo/typedezai/PAIAdministratifOuMilitaire"/>
        <skos:definition xml:lang="en">Area permanently reserved for troop gatherings of all arms, either for maneuvers, exercises (training camp), or for tests, studies: base, camp, barracks, deposit of equipment, permanent ground of training, barracks of CRS, barracks of mobile gendarmes, ... The ranges are excluded as well as the properties of the army which are not indicated in any way on the ground (neither fences, barriers, nor signs,. ..) and not subject to any particular restriction.</skos:definition>
        <skos:definition xml:lang="fr">Zone en permanence réservée pour les rassemblements de troupes de toutes les armes, soit pour des manoeuvres, des exercices (camp d&apos;instruction), soit pour des essais, des études: base, camp, caserne, dépôt de matériels, terrain permanent d&apos;entrainement, caserne de CRS, caserne de gendarmes mobiles, ... Les champs de tir sont exclus ainsi que les propriétés de l&apos;armée qui ne sont indiquées d&apos;aucune manière sur le terrain (ni clôtures, ni barrières, ni pancartes, ...) et ne faisant l&apos;objet d&apos;aucune restriction particulière.</skos:definition>
        <skos:prefLabel xml:lang="fr">enceinte militaire</skos:prefLabel>
        <skos:prefLabel xml:lang="en">military area</skos:prefLabel>
    </owl:NamedIndividual>
    


    <!-- http://data.ign.fr/id/codes/topo/typedezai/EnseignementPrimaire -->


    <owl:NamedIndividual rdf:about="http://data.ign.fr/id/codes/topo/typedezai/EnseignementPrimaire">
        <rdf:type rdf:resource="http://data.ign.fr/def/topo#TypeDeZAI"/>
        <rdf:type rdf:resource="http://www.w3.org/2004/02/skos/core#Concept"/>
        <skos:inScheme rdf:resource="http://data.ign.fr/id/codes/topo/typedezai/liste"/>
        <skos:broader rdf:resource="http://data.ign.fr/id/codes/topo/typedezai/PAIScienceEnseignement"/>
        <skos:definition xml:lang="en">Institution devoted to nursery and primary education: primary school, nursery school, school group, Institut Médico-Pédagogique (I.M.P.). All primary schools, public, religious or private, having a simple contract or association with the State are included. The nurseries are excluded.</skos:definition>
        <skos:definition xml:lang="fr">Établissement consacré à l&apos;enseignement maternel et primaire : école primaire, école maternelle, groupe scolaire, Institut Médico-Pédagogique (I.M.P.). Tous les établissements d&apos;enseignement primaire, publics, confessionnels ou privés, ayant un contrat simple ou d&apos;association avec l&apos;État sont inclus. Les crèches sont exclues.</skos:definition>
        <skos:prefLabel xml:lang="en">nursery or elementary school</skos:prefLabel>
        <skos:prefLabel xml:lang="fr">établissement d&apos;enseignement maternel ou primaire</skos:prefLabel>
    </owl:NamedIndividual>
    


    <!-- http://data.ign.fr/id/codes/topo/typedezai/EnseignementSecondaire -->


    <owl:NamedIndividual rdf:about="http://data.ign.fr/id/codes/topo/typedezai/EnseignementSecondaire">
        <rdf:type rdf:resource="http://data.ign.fr/def/topo#TypeDeZAI"/>
        <rdf:type rdf:resource="http://www.w3.org/2004/02/skos/core#Concept"/>
        <skos:inScheme rdf:resource="http://data.ign.fr/id/codes/topo/typedezai/liste"/>
        <skos:broader rdf:resource="http://data.ign.fr/id/codes/topo/typedezai/PAIScienceEnseignement"/>
        <skos:definition xml:lang="en">Establishment devoted to secondary education: middle school, high school, Center for Help by Work (C.A.T.), Professional Training of Adults (F.P.A.), Medical-Professional Institute (I.M.Pro.). All public, religious or private secondary schools with a simple contract or association with the state are included.</skos:definition>
        <skos:definition xml:lang="fr">Établissement consacré à l&apos;enseignement secondaire : collège, lycée, Centre d&apos;Aide par le Travail (C.A.T.), Formation Professionnelle des Adultes (F.P.A.), Institut Médico-Professionnel (I.M.Pro.). Tous les établissements d&apos;enseignement secondaire publics, confessionnels ou privés, ayant un contrat simple ou d&apos;association avec l&apos;État sont inclus.</skos:definition>
        <skos:prefLabel xml:lang="en">secondary education school</skos:prefLabel>
        <skos:prefLabel xml:lang="fr">établissement d&apos;enseignement secondaire</skos:prefLabel>
    </owl:NamedIndividual>
    


    <!-- http://data.ign.fr/id/codes/topo/typedezai/EnseignementSuperieur -->


    <owl:NamedIndividual rdf:about="http://data.ign.fr/id/codes/topo/typedezai/EnseignementSuperieur">
        <rdf:type rdf:resource="http://data.ign.fr/def/topo#TypeDeZAI"/>
        <rdf:type rdf:resource="http://www.w3.org/2004/02/skos/core#Concept"/>
        <skos:inScheme rdf:resource="http://data.ign.fr/id/codes/topo/typedezai/liste"/>
        <skos:broader rdf:resource="http://data.ign.fr/id/codes/topo/typedezai/PAIScienceEnseignement"/>
        <skos:definition xml:lang="en">Institution devoted to higher education: faculty, university center, institute, grande école, etc. All public, religious or private higher education institutions with a simple contract or association with the state are included. Evening classes, cities and university restaurants are excluded.</skos:definition>
        <skos:definition xml:lang="fr">Établissement consacré à l&apos;enseignement supérieur : faculté, centre universitaire, institut, grande école,etc. Tous les établissements d&apos;enseignement supérieur publics, confessionnels ou privés, ayant un contrat simple ou d&apos;association avec l&apos;État sont inclus. Les cours du soir, les cités et les restaurants universitaires sont exclus.</skos:definition>
        <skos:prefLabel xml:lang="en">postsecondary education school</skos:prefLabel>
        <skos:prefLabel xml:lang="fr">établissement d&apos;enseignement supérieur</skos:prefLabel>
    </owl:NamedIndividual>
    


    <!-- http://data.ign.fr/id/codes/topo/typedezai/EspaceMaritime -->


    <owl:NamedIndividual rdf:about="http://data.ign.fr/id/codes/topo/typedezai/EspaceMaritime">
        <rdf:type rdf:resource="http://data.ign.fr/def/topo#TypeDeZAI"/>
        <rdf:type rdf:resource="http://www.w3.org/2004/02/skos/core#Concept"/>
        <skos:inScheme rdf:resource="http://data.ign.fr/id/codes/topo/typedezai/liste"/>
        <skos:broader rdf:resource="http://data.ign.fr/id/codes/topo/typedezai/PAIHydrographie"/>
        <skos:definition xml:lang="fr">Espace maritime, mer, océan, passe.</skos:definition>
        <skos:definition xml:lang="en">Maritime area, sea, ocean, pass.</skos:definition>
        <skos:prefLabel xml:lang="fr">espace maritime</skos:prefLabel>
        <skos:prefLabel xml:lang="en">maritime feature</skos:prefLabel>
    </owl:NamedIndividual>
    


    <!-- http://data.ign.fr/id/codes/topo/typedezai/EspacePublic -->


    <owl:NamedIndividual rdf:about="http://data.ign.fr/id/codes/topo/typedezai/EspacePublic">
        <rdf:type rdf:resource="http://data.ign.fr/def/topo#TypeDeZAI"/>
        <rdf:type rdf:resource="http://www.w3.org/2004/02/skos/core#Concept"/>
        <skos:inScheme rdf:resource="http://data.ign.fr/id/codes/topo/typedezai/liste"/>
        <skos:broader rdf:resource="http://data.ign.fr/id/codes/topo/typedezai/PAICultureLoisirs"/>
        <skos:definition xml:lang="fr">Large espace découvert urbain désigné par un toponyme où aboutissent plusieurs rues, fermé à la circulation automobile, constituant un lieu remarquable : place, square, jardin, parc, parc communal, parc intercommunal, parc départemental, parc interdépartemental. Seuls les espaces publics possédant un toponyme sont retenus. Les parcs à vocation commerciale sont exclus (voir la valeur &apos;Parc de loisirs&apos;), de même que les parcs naturels (réserves, parcs nationaux, parcs naturels régionaux) qui sont traités en PAI_ESPACE_NATUREL.</skos:definition>
        <skos:definition xml:lang="en">Large open space urban designated by a toponym where end several streets, closed to traffic, constituting a remarkable place: square, square, garden, park, communal park, intercommunal park, departmental park, interdepartmental park. Only public spaces with a toponym are retained. The commercial parks are excluded (see the value &apos;Leisure park&apos;), as well as the natural parks (reserves, national parks, regional natural parks) which are treated in PAI_ESPACE_NATUREL.</skos:definition>
        <skos:prefLabel xml:lang="fr">espace public nommé</skos:prefLabel>
        <skos:prefLabel xml:lang="en">named public area</skos:prefLabel>
    </owl:NamedIndividual>
    


    <!-- http://data.ign.fr/id/codes/topo/typedezai/EtablissementHospitalier -->


    <owl:NamedIndividual rdf:about="http://data.ign.fr/id/codes/topo/typedezai/EtablissementHospitalier">
        <rdf:type rdf:resource="http://data.ign.fr/def/topo#TypeDeZAI"/>
        <rdf:type rdf:resource="http://www.w3.org/2004/02/skos/core#Concept"/>
        <skos:inScheme rdf:resource="http://data.ign.fr/id/codes/topo/typedezai/liste"/>
        <skos:broader rdf:resource="http://data.ign.fr/id/codes/topo/typedezai/PAISante"/>
        <skos:definition xml:lang="en">Public or private institution that receives or deals for a limited time the sick, wounded and women in childbirth: hospital, sanatorium, hospice, health center, dispensary, day hospital, psychiatric hospital, etc. All facilities providing care and accommodation or care only are included. Retirement homes that do not have a health center are excluded.</skos:definition>
        <skos:definition xml:lang="fr">Établissement public ou privé qui reçoit ou traite pendant un temps limité les malades, les blessés et les femmes en couches : hôpital, sanatorium, hospice, centre de soins, dispensaire, hôpital de jour, hôpital psychiatrique, etc. Tous les établissements assurant les soins et l&apos;hébergement ou les soins seulement sont inclus. Les maisons de retraite ne possédant pas de centre de soins sont exclues.</skos:definition>
        <skos:prefLabel xml:lang="en">healthcare facility</skos:prefLabel>
        <skos:prefLabel xml:lang="fr">établissement hospitalier</skos:prefLabel>
    </owl:NamedIndividual>
    


    <!-- http://data.ign.fr/id/codes/topo/typedezai/EtablissementPenitenciaire -->


    <owl:NamedIndividual rdf:about="http://data.ign.fr/id/codes/topo/typedezai/EtablissementPenitenciaire">
        <rdf:type rdf:resource="http://data.ign.fr/def/topo#TypeDeZAI"/>
        <rdf:type rdf:resource="http://www.w3.org/2004/02/skos/core#Concept"/>
        <skos:inScheme rdf:resource="http://data.ign.fr/id/codes/topo/typedezai/liste"/>
        <skos:broader rdf:resource="http://data.ign.fr/id/codes/topo/typedezai/PAIAdministratifOuMilitaire"/>
        <skos:definition xml:lang="en">Enclosed institution equipped to receive offenders sentenced to deprivation of liberty or inmates awaiting trial: prison. The annexes are excluded.</skos:definition>
        <skos:definition xml:lang="fr">Établissement clos aménagé pour recevoir des délinquants condamnés à une peine privative de liberté ou des détenus en instance de jugement: maison d&apos;arrêt, prison. Les annexes sont exclues.</skos:definition>
        <skos:prefLabel xml:lang="en">penitentiary</skos:prefLabel>
        <skos:prefLabel xml:lang="fr">établissement pénitenciaire</skos:prefLabel>
    </owl:NamedIndividual>
    


    <!-- http://data.ign.fr/id/codes/topo/typedezai/EtablissementThermal -->


    <owl:NamedIndividual rdf:about="http://data.ign.fr/id/codes/topo/typedezai/EtablissementThermal">
        <rdf:type rdf:resource="http://data.ign.fr/def/topo#TypeDeZAI"/>
        <rdf:type rdf:resource="http://www.w3.org/2004/02/skos/core#Concept"/>
        <skos:inScheme rdf:resource="http://data.ign.fr/id/codes/topo/typedezai/liste"/>
        <skos:broader rdf:resource="http://data.ign.fr/id/codes/topo/typedezai/PAISante"/>
        <skos:definition xml:lang="en">Establishment where medicinal waters are used (mineral waters, hot or not): thermal establishment, thalassotherapy center. Only establishments approved by the Social Security are included.</skos:definition>
        <skos:definition xml:lang="fr">Établissement où l&apos;on utilise les eaux médicinales (eaux minérales, chaudes ou non) : établissement thermal, centre de thalassothérapie. Seuls sont inclus les établissements agréés par la Sécurité Sociale.</skos:definition>
        <skos:prefLabel xml:lang="en">health resort</skos:prefLabel>
        <skos:prefLabel xml:lang="fr">établissement thermal</skos:prefLabel>
    </owl:NamedIndividual>
    


    <!-- http://data.ign.fr/id/codes/topo/typedezai/GareFretUniquement -->


    <owl:NamedIndividual rdf:about="http://data.ign.fr/id/codes/topo/typedezai/GareFretUniquement">
        <rdf:type rdf:resource="http://data.ign.fr/def/topo#TypeDeZAI"/>
        <rdf:type rdf:resource="http://www.w3.org/2004/02/skos/core#Concept"/>
        <skos:inScheme rdf:resource="http://data.ign.fr/id/codes/topo/typedezai/liste"/>
        <skos:broader rdf:resource="http://data.ign.fr/id/codes/topo/typedezai/PAITransport"/>
        <skos:definition xml:lang="en">Railway establishment providing a commercial merchandise service: freight station, service point. Air or sea freight is excluded.</skos:definition>
        <skos:definition xml:lang="fr">Établissement ferroviaire assurant un service commercial de marchandises : gare de fret, point de desserte. Le fret aérien ou maritime est exclu.</skos:definition>
        <skos:prefLabel xml:lang="fr">gare de fret</skos:prefLabel>
        <skos:prefLabel xml:lang="en">goods station</skos:prefLabel>
    </owl:NamedIndividual>
    


    <!-- http://data.ign.fr/id/codes/topo/typedezai/GareRoutiere -->


    <owl:NamedIndividual rdf:about="http://data.ign.fr/id/codes/topo/typedezai/GareRoutiere">
        <rdf:type rdf:resource="http://data.ign.fr/def/topo#TypeDeZAI"/>
        <rdf:type rdf:resource="http://www.w3.org/2004/02/skos/core#Concept"/>
        <skos:inScheme rdf:resource="http://data.ign.fr/id/codes/topo/typedezai/liste"/>
        <skos:broader rdf:resource="http://data.ign.fr/id/codes/topo/typedezai/PAITransport"/>
        <skos:definition xml:lang="en">All facilities intended for the loading and unloading of passengers by bus or bus at a specific point. The bus stations of city buses, school buses, RATP and bus depots are not included.</skos:definition>
        <skos:definition xml:lang="fr">Ensemble des installations destinées à l&apos;embarquement et au débarquement de voyageurs en car ou en bus en un point déterminé. Ne sont pas retenues les gares routières des bus de ville, des bus scolaires, de la RATP et les dépôts de bus.</skos:definition>
        <skos:prefLabel xml:lang="en">bus station</skos:prefLabel>
        <skos:prefLabel xml:lang="fr">gare routière</skos:prefLabel>
    </owl:NamedIndividual>
    


    <!-- http://data.ign.fr/id/codes/topo/typedezai/GareVoyageursEtFret -->


    <owl:NamedIndividual rdf:about="http://data.ign.fr/id/codes/topo/typedezai/GareVoyageursEtFret">
        <rdf:type rdf:resource="http://data.ign.fr/def/topo#TypeDeZAI"/>
        <rdf:type rdf:resource="http://www.w3.org/2004/02/skos/core#Concept"/>
        <skos:inScheme rdf:resource="http://data.ign.fr/id/codes/topo/typedezai/liste"/>
        <skos:broader rdf:resource="http://data.ign.fr/id/codes/topo/typedezai/PAITransport"/>
        <skos:definition xml:lang="en">Railway establishment providing a commercial service for passengers and goods (Only the main building open to the public)</skos:definition>
        <skos:definition xml:lang="fr">Établissement ferroviaire assurant un service commercial de voyageurs et de marchandises.(Uniquement le bâtiment principal ouvert au public.)</skos:definition>
        <skos:prefLabel xml:lang="fr">gare de voyageurs et fret</skos:prefLabel>
        <skos:prefLabel xml:lang="en">passengers and goods station</skos:prefLabel>
    </owl:NamedIndividual>
    


    <!-- http://data.ign.fr/id/codes/topo/typedezai/GareVoyageursUniquement -->


    <owl:NamedIndividual rdf:about="http://data.ign.fr/id/codes/topo/typedezai/GareVoyageursUniquement">
        <rdf:type rdf:resource="http://data.ign.fr/def/topo#TypeDeZAI"/>
        <rdf:type rdf:resource="http://www.w3.org/2004/02/skos/core#Concept"/>
        <skos:inScheme rdf:resource="http://data.ign.fr/id/codes/topo/typedezai/liste"/>
        <skos:broader rdf:resource="http://data.ign.fr/id/codes/topo/typedezai/PAITransport"/>
        <skos:definition xml:lang="en">Railway or cable transport establishment with or without a commercial passenger service: station, station, stopping point, urban railway station, cable car station. All stations and railway stops in use are included.</skos:definition>
        <skos:definition xml:lang="fr">Établissement ferroviaire ou de transport par câble assurant avec ou sans personnel un service commercial de voyageurs : gare, station, point d&apos;arrêt, station réseau ferré urbain, gare téléphérique. Toutes les gares et arrêts ferroviaires en service sont inclus.</skos:definition>
        <skos:prefLabel xml:lang="fr">gare de voyageurs</skos:prefLabel>
        <skos:prefLabel xml:lang="en">passengers station</skos:prefLabel>
    </owl:NamedIndividual>
    


    <!-- http://data.ign.fr/id/codes/topo/typedezai/Gendarmerie -->


    <owl:NamedIndividual rdf:about="http://data.ign.fr/id/codes/topo/typedezai/Gendarmerie">
        <rdf:type rdf:resource="http://data.ign.fr/def/topo#TypeDeZAI"/>
        <rdf:type rdf:resource="http://www.w3.org/2004/02/skos/core#Concept"/>
        <skos:inScheme rdf:resource="http://data.ign.fr/id/codes/topo/typedezai/liste"/>
        <skos:broader rdf:resource="http://data.ign.fr/id/codes/topo/typedezai/PAIAdministratifOuMilitaire"/>
        <skos:definition xml:lang="en">Barracks where the gendarmes are lodged; offices where they fulfill their administrative functions: gendarmerie, highway police. Definition of the footprint of the site: area of the entire barracks, usually delimited by a fence and including housing and offices.</skos:definition>
        <skos:definition xml:lang="fr">Caserne où les gendarmes sont logés ; bureaux où ils remplissent leurs fonctions administratives : gendarmerie, gendarmerie d&apos;autoroute. Définition de l&apos;emprise du site : surface de l&apos;ensemble de la caserne, généralement délimitée par une clôture et incluant logements et bureaux.</skos:definition>
        <skos:prefLabel xml:lang="en">gendarmerie</skos:prefLabel>
        <skos:prefLabel xml:lang="fr">gendarmerie</skos:prefLabel>
    </owl:NamedIndividual>
    


    <!-- http://data.ign.fr/id/codes/topo/typedezai/Glacier -->


    <owl:NamedIndividual rdf:about="http://data.ign.fr/id/codes/topo/typedezai/Glacier">
        <rdf:type rdf:resource="http://data.ign.fr/def/topo#TypeDeZAI"/>
        <rdf:type rdf:resource="http://www.w3.org/2004/02/skos/core#Concept"/>
        <skos:inScheme rdf:resource="http://data.ign.fr/id/codes/topo/typedezai/liste"/>
        <skos:broader rdf:resource="http://data.ign.fr/id/codes/topo/typedezai/PAIHydrographie"/>
        <skos:definition xml:lang="en">Name of a glacier or a detail related to a glacier: crevasse, glacier, moraine, firn, serac.</skos:definition>
        <skos:definition xml:lang="fr">Nom d&apos;un glacier ou d&apos;un détail relatif à un glacier : crevasse, glacier, moraine, névé, sérac.</skos:definition>
        <skos:prefLabel xml:lang="en">glacier</skos:prefLabel>
        <skos:prefLabel xml:lang="fr">glacier</skos:prefLabel>
    </owl:NamedIndividual>
    


    <!-- http://data.ign.fr/id/codes/topo/typedezai/Golf -->


    <owl:NamedIndividual rdf:about="http://data.ign.fr/id/codes/topo/typedezai/Golf">
        <rdf:type rdf:resource="http://data.ign.fr/def/topo#TypeDeZAI"/>
        <rdf:type rdf:resource="http://www.w3.org/2004/02/skos/core#Concept"/>
        <skos:inScheme rdf:resource="http://data.ign.fr/id/codes/topo/typedezai/liste"/>
        <skos:broader rdf:resource="http://data.ign.fr/id/codes/topo/typedezai/PAISport"/>
        <skos:definition xml:lang="en">Land open to the public and dedicated to the practice of golf. Less than 9 holes and minigolfs are excluded.</skos:definition>
        <skos:definition xml:lang="fr">Terrain ouvert au public et consacré à la pratique du golf. Les terrains de moins de 9 trous et les minigolfs sont exclus.</skos:definition>
        <skos:prefLabel xml:lang="fr">golf</skos:prefLabel>
        <skos:prefLabel xml:lang="en">golf course</skos:prefLabel>
    </owl:NamedIndividual>
    


    <!-- http://data.ign.fr/id/codes/topo/typedezai/Grange -->


    <owl:NamedIndividual rdf:about="http://data.ign.fr/id/codes/topo/typedezai/Grange">
        <rdf:type rdf:resource="http://data.ign.fr/def/topo#TypeDeZAI"/>
        <rdf:type rdf:resource="http://www.w3.org/2004/02/skos/core#Concept"/>
        <skos:inScheme rdf:resource="http://data.ign.fr/id/codes/topo/typedezai/liste"/>
        <skos:broader rdf:resource="http://data.ign.fr/id/codes/topo/typedezai/PAIZoneHabitation"/>
        <skos:definition xml:lang="fr">Construction légère : abri, baraquement, cabane, grange, hangar.</skos:definition>
        <skos:definition xml:lang="en">Light construction: shelter, barracks, hut, barn, shed.</skos:definition>
        <skos:prefLabel xml:lang="en">barn</skos:prefLabel>
        <skos:prefLabel xml:lang="fr">grange</skos:prefLabel>
    </owl:NamedIndividual>
    


    <!-- http://data.ign.fr/id/codes/topo/typedezai/HabitationTroglodytique -->


    <owl:NamedIndividual rdf:about="http://data.ign.fr/id/codes/topo/typedezai/HabitationTroglodytique">
        <rdf:type rdf:resource="http://data.ign.fr/def/topo#TypeDeZAI"/>
        <rdf:type rdf:resource="http://www.w3.org/2004/02/skos/core#Concept"/>
        <skos:inScheme rdf:resource="http://data.ign.fr/id/codes/topo/typedezai/liste"/>
        <skos:broader rdf:resource="http://data.ign.fr/id/codes/topo/typedezai/PAICultureLoisirs"/>
        <skos:definition xml:lang="fr">Excavation naturelle ou creusée dans le roc (caverne, grotte), habitée ou anciennement habitée.</skos:definition>
        <skos:definition xml:lang="en">Natural excavation or excavated in the rock (cavern, cave), inhabited or formerly inhabited.</skos:definition>
        <skos:prefLabel xml:lang="en">cliff dwelling</skos:prefLabel>
        <skos:prefLabel xml:lang="fr">habitation troglodytique</skos:prefLabel>
    </owl:NamedIndividual>
    


    <!-- http://data.ign.fr/id/codes/topo/typedezai/HarasNational -->


    <owl:NamedIndividual rdf:about="http://data.ign.fr/id/codes/topo/typedezai/HarasNational">
        <rdf:type rdf:resource="http://data.ign.fr/def/topo#TypeDeZAI"/>
        <rdf:type rdf:resource="http://www.w3.org/2004/02/skos/core#Concept"/>
        <skos:inScheme rdf:resource="http://data.ign.fr/id/codes/topo/typedezai/liste"/>
        <skos:broader rdf:resource="http://data.ign.fr/id/codes/topo/typedezai/PAIIndustrielCommercial"/>
        <skos:definition xml:lang="fr">Lieu ou établissement destiné à la reproduction de l&apos;espèce chevaline, à l&apos;amélioration des races de chevaux par la sélection des étalons. Tous les haras nationaux sont inclus. L&apos;enceinte comprend l&apos;ensemble des installations (manège, écuries, piste d&apos;entraînement,etc.).</skos:definition>
        <skos:definition xml:lang="en">Place or establishment intended for the reproduction of the horse species, for the improvement of the breeds of horses by the selection of the stallions. All national stud farms are included. The enclosure includes all the facilities (carousel, stables, training track, etc.).</skos:definition>
        <skos:prefLabel xml:lang="fr">haras national</skos:prefLabel>
        <skos:prefLabel xml:lang="en">ranch</skos:prefLabel>
    </owl:NamedIndividual>
    


    <!-- http://data.ign.fr/id/codes/topo/typedezai/Hippodrome -->


    <owl:NamedIndividual rdf:about="http://data.ign.fr/id/codes/topo/typedezai/Hippodrome">
        <rdf:type rdf:resource="http://data.ign.fr/def/topo#TypeDeZAI"/>
        <rdf:type rdf:resource="http://www.w3.org/2004/02/skos/core#Concept"/>
        <skos:inScheme rdf:resource="http://data.ign.fr/id/codes/topo/typedezai/liste"/>
        <skos:broader rdf:resource="http://data.ign.fr/id/codes/topo/typedezai/PAISport"/>
        <skos:definition xml:lang="fr">Lieu ouvert au public et consacré aux courses de chevaux. Seuls les hippodromes possédant des aménagements conséquents (tribunes, bâtiments spécifiques) sont inclus.</skos:definition>
        <skos:definition xml:lang="en">Open to the public and dedicated to horse racing. Only racetracks with significant amenities (stands, specific buildings) are included.</skos:definition>
        <skos:prefLabel xml:lang="fr">hippodrome</skos:prefLabel>
        <skos:prefLabel xml:lang="en">racecourse</skos:prefLabel>
    </owl:NamedIndividual>
    


    <!-- http://data.ign.fr/id/codes/topo/typedezai/Hopital -->


    <owl:NamedIndividual rdf:about="http://data.ign.fr/id/codes/topo/typedezai/Hopital">
        <rdf:type rdf:resource="http://data.ign.fr/def/topo#TypeDeZAI"/>
        <rdf:type rdf:resource="http://www.w3.org/2004/02/skos/core#Concept"/>
        <skos:inScheme rdf:resource="http://data.ign.fr/id/codes/topo/typedezai/liste"/>
        <skos:broader rdf:resource="http://data.ign.fr/id/codes/topo/typedezai/PAISante"/>
        <skos:definition xml:lang="en">Public or private institution, where all the medical and surgical heavy and / or long-term care, as well as deliveries are carried out: hospital, university hospital, military hospital, clinic.</skos:definition>
        <skos:definition xml:lang="fr">Établissement public ou privé, où sont effectués tous les soins médicaux et chirurgicaux lourds et/ou de longue durée, ainsi que les accouchements : hôpital, CHU, hôpital militaire, clinique.</skos:definition>
        <skos:prefLabel xml:lang="en">hospital</skos:prefLabel>
        <skos:prefLabel xml:lang="fr">hôpital</skos:prefLabel>
    </owl:NamedIndividual>
    


    <!-- http://data.ign.fr/id/codes/topo/typedezai/HotelDeDepartement -->


    <owl:NamedIndividual rdf:about="http://data.ign.fr/id/codes/topo/typedezai/HotelDeDepartement">
        <rdf:type rdf:resource="http://data.ign.fr/def/topo#TypeDeZAI"/>
        <rdf:type rdf:resource="http://www.w3.org/2004/02/skos/core#Concept"/>
        <skos:inScheme rdf:resource="http://data.ign.fr/id/codes/topo/typedezai/liste"/>
        <skos:broader rdf:resource="http://data.ign.fr/id/codes/topo/typedezai/PAIAdministratifOuMilitaire"/>
        <skos:definition xml:lang="en">Building where the General Council sits. Only the main building is included. The annexes are not, except possibly an annex located in another agglomeration when it has a function close to that of the headquarters.</skos:definition>
        <skos:definition xml:lang="fr">Bâtiment où siège le conseil général. Seul le bâtiment principal est inclus. Les annexes ne le sont pas, sauf éventuellement une annexe située dans une autre agglomération lorsqu&apos;elle a une fonction proche de celle du siège.</skos:definition>
        <skos:prefLabel xml:lang="en">departmental administration building</skos:prefLabel>
        <skos:prefLabel xml:lang="fr">hôtel de département</skos:prefLabel>
    </owl:NamedIndividual>
    


    <!-- http://data.ign.fr/id/codes/topo/typedezai/HotelDeRegion -->


    <owl:NamedIndividual rdf:about="http://data.ign.fr/id/codes/topo/typedezai/HotelDeRegion">
        <rdf:type rdf:resource="http://data.ign.fr/def/topo#TypeDeZAI"/>
        <rdf:type rdf:resource="http://www.w3.org/2004/02/skos/core#Concept"/>
        <skos:inScheme rdf:resource="http://data.ign.fr/id/codes/topo/typedezai/liste"/>
        <skos:broader rdf:resource="http://data.ign.fr/id/codes/topo/typedezai/PAIAdministratifOuMilitaire"/>
        <skos:definition xml:lang="en">Building where the regional council sits. Only the main building is included. The annexes are not, except possibly an annex located in another agglomeration when it has a function close to that of the headquarters.</skos:definition>
        <skos:definition xml:lang="fr">Bâtiment où siège le conseil régional. Seul le bâtiment principal est inclus. Les annexes ne le sont pas, sauf éventuellement une annexe située dans une autre agglomération lorsqu&apos;elle a une fonction proche de celle du siège.</skos:definition>
        <skos:prefLabel xml:lang="fr">hôtel de région</skos:prefLabel>
        <skos:prefLabel xml:lang="en">regional administration building</skos:prefLabel>
    </owl:NamedIndividual>
    


    <!-- http://data.ign.fr/id/codes/topo/typedezai/InfrastructureRoutiere -->


    <owl:NamedIndividual rdf:about="http://data.ign.fr/id/codes/topo/typedezai/InfrastructureRoutiere">
        <rdf:type rdf:resource="http://data.ign.fr/def/topo#TypeDeZAI"/>
        <rdf:type rdf:resource="http://www.w3.org/2004/02/skos/core#Concept"/>
        <skos:inScheme rdf:resource="http://data.ign.fr/id/codes/topo/typedezai/liste"/>
        <skos:broader rdf:resource="http://data.ign.fr/id/codes/topo/typedezai/PAITransport"/>
        <skos:definition xml:lang="en">A road network element that is neither an attribute of a &apos;road segment&apos; object nor the &apos;crossroad&apos; attribute value: road, toll area, rest area.</skos:definition>
        <skos:definition xml:lang="fr">Élément du réseau routier ne figurant ni en attribut d&apos;un objet &apos;tronçon de route&apos; ni avec la valeur d&apos;attribut &apos;carrefour&apos; : route, aire de péage, aire de repos.</skos:definition>
        <skos:prefLabel xml:lang="fr">infrastructure routière</skos:prefLabel>
        <skos:prefLabel xml:lang="en">road transport infrastructure</skos:prefLabel>
    </owl:NamedIndividual>
    


    <!-- http://data.ign.fr/id/codes/topo/typedezai/Lac -->


    <owl:NamedIndividual rdf:about="http://data.ign.fr/id/codes/topo/typedezai/Lac">
        <rdf:type rdf:resource="http://data.ign.fr/def/topo#TypeDeZAI"/>
        <rdf:type rdf:resource="http://www.w3.org/2004/02/skos/core#Concept"/>
        <skos:inScheme rdf:resource="http://data.ign.fr/id/codes/topo/typedezai/liste"/>
        <skos:broader rdf:resource="http://data.ign.fr/id/codes/topo/typedezai/PAIHydrographie"/>
        <skos:definition xml:lang="en">Body of water: pond, pond, lake, pond.</skos:definition>
        <skos:definition xml:lang="fr">Étendue d&apos;eau terrestre : bassin, étang, lac, mare.</skos:definition>
        <skos:prefLabel xml:lang="fr">lac</skos:prefLabel>
        <skos:prefLabel xml:lang="en">lake</skos:prefLabel>
    </owl:NamedIndividual>
    


    <!-- http://data.ign.fr/id/codes/topo/typedezai/LieuDitHabite -->


    <owl:NamedIndividual rdf:about="http://data.ign.fr/id/codes/topo/typedezai/LieuDitHabite">
        <rdf:type rdf:resource="http://data.ign.fr/def/topo#TypeDeZAI"/>
        <rdf:type rdf:resource="http://www.w3.org/2004/02/skos/core#Concept"/>
        <skos:inScheme rdf:resource="http://data.ign.fr/id/codes/topo/typedezai/liste"/>
        <skos:broader rdf:resource="http://data.ign.fr/id/codes/topo/typedezai/PAIZoneHabitation"/>
        <skos:definition xml:lang="en">Inhabited locality characterized by a name.</skos:definition>
        <skos:definition xml:lang="fr">Lieu-dit habité caractérisé par un nom.</skos:definition>
        <skos:prefLabel xml:lang="en">inhabited local placename</skos:prefLabel>
        <skos:prefLabel xml:lang="fr">lieu-dit habité</skos:prefLabel>
    </owl:NamedIndividual>
    


    <!-- http://data.ign.fr/id/codes/topo/typedezai/LieuDitNonHabite -->


    <owl:NamedIndividual rdf:about="http://data.ign.fr/id/codes/topo/typedezai/LieuDitNonHabite">
        <rdf:type rdf:resource="http://data.ign.fr/def/topo#TypeDeZAI"/>
        <rdf:type rdf:resource="http://www.w3.org/2004/02/skos/core#Concept"/>
        <skos:inScheme rdf:resource="http://data.ign.fr/id/codes/topo/typedezai/liste"/>
        <skos:broader rdf:resource="http://data.ign.fr/id/codes/topo/typedezai/PAIEspaceNaturel"/>
        <skos:definition xml:lang="en">Any locality, whose name is generally attached to land: uninhabited locality, plantation, cultivated area.</skos:definition>
        <skos:definition xml:lang="fr">Lieu-dit quelconque, dont le nom est généralement attaché à des terres : lieu-dit non habité, plantation, espace cultivé.</skos:definition>
        <skos:prefLabel xml:lang="fr">lieu-dit non habité</skos:prefLabel>
        <skos:prefLabel xml:lang="en">non inhabited local placename</skos:prefLabel>
    </owl:NamedIndividual>
    


    <!-- http://data.ign.fr/id/codes/topo/typedezai/MaisonDuParc -->


    <owl:NamedIndividual rdf:about="http://data.ign.fr/id/codes/topo/typedezai/MaisonDuParc">
        <rdf:type rdf:resource="http://data.ign.fr/def/topo#TypeDeZAI"/>
        <rdf:type rdf:resource="http://www.w3.org/2004/02/skos/core#Concept"/>
        <skos:inScheme rdf:resource="http://data.ign.fr/id/codes/topo/typedezai/liste"/>
        <skos:broader rdf:resource="http://data.ign.fr/id/codes/topo/typedezai/PAICultureLoisirs"/>
        <skos:definition xml:lang="en">Building open to the public and managed by a National or Regional Park.</skos:definition>
        <skos:definition xml:lang="fr">Bâtiment ouvert au public et géré par un Parc National ou Régional.</skos:definition>
        <skos:prefLabel xml:lang="fr">maison du parc</skos:prefLabel>
        <skos:prefLabel xml:lang="en">park center</skos:prefLabel>
    </owl:NamedIndividual>
    


    <!-- http://data.ign.fr/id/codes/topo/typedezai/MaisonForestiere -->


    <owl:NamedIndividual rdf:about="http://data.ign.fr/id/codes/topo/typedezai/MaisonForestiere">
        <rdf:type rdf:resource="http://data.ign.fr/def/topo#TypeDeZAI"/>
        <rdf:type rdf:resource="http://www.w3.org/2004/02/skos/core#Concept"/>
        <skos:inScheme rdf:resource="http://data.ign.fr/id/codes/topo/typedezai/liste"/>
        <skos:broader rdf:resource="http://data.ign.fr/id/codes/topo/typedezai/PAIAdministratifOuMilitaire"/>
        <skos:definition xml:lang="en">House managed by the National Forest Office. Guard houses occupied by at least one NFB agent are included. The offices of the NFB, the homes of agents also used as offices, are excluded when they are not located in a forest house.</skos:definition>
        <skos:definition xml:lang="fr">Maison gérée par l&apos;office national des forêts. Les maisons de garde occupées par au moins un agent de l&apos;ONF sont incluses. Les bureaux de l&apos;ONF, les domiciles d&apos;agents servant aussi de bureau, sont exclus lorsqu&apos;ils ne sont pas situés dans une maison forestière.</skos:definition>
        <skos:prefLabel xml:lang="en">forest house</skos:prefLabel>
        <skos:prefLabel xml:lang="fr">maison forestière</skos:prefLabel>
    </owl:NamedIndividual>
    


    <!-- http://data.ign.fr/id/codes/topo/typedezai/Marais -->


    <owl:NamedIndividual rdf:about="http://data.ign.fr/id/codes/topo/typedezai/Marais">
        <rdf:type rdf:resource="http://data.ign.fr/def/topo#TypeDeZAI"/>
        <rdf:type rdf:resource="http://www.w3.org/2004/02/skos/core#Concept"/>
        <skos:inScheme rdf:resource="http://data.ign.fr/id/codes/topo/typedezai/liste"/>
        <skos:broader rdf:resource="http://data.ign.fr/id/codes/topo/typedezai/PAIHydrographie"/>
        <skos:definition xml:lang="en">Wetland: marsh, swamp, saline.</skos:definition>
        <skos:definition xml:lang="fr">Zone humide : marais, marécage, saline.</skos:definition>
        <skos:prefLabel xml:lang="fr">marais</skos:prefLabel>
        <skos:prefLabel xml:lang="en">marsh</skos:prefLabel>
    </owl:NamedIndividual>
    


    <!-- http://data.ign.fr/id/codes/topo/typedezai/MaraisSalants -->


    <owl:NamedIndividual rdf:about="http://data.ign.fr/id/codes/topo/typedezai/MaraisSalants">
        <rdf:type rdf:resource="http://data.ign.fr/def/topo#TypeDeZAI"/>
        <rdf:type rdf:resource="http://www.w3.org/2004/02/skos/core#Concept"/>
        <skos:inScheme rdf:resource="http://data.ign.fr/id/codes/topo/typedezai/liste"/>
        <skos:broader rdf:resource="http://data.ign.fr/id/codes/topo/typedezai/PAIIndustrielCommercial"/>
        <skos:definition xml:lang="en">Area consisting of basins dug near the coasts to extract salt from seawater by evaporation. Areas of salt marshes less than 3 ha are excluded. Old salt marshes that are no longer active are excluded.</skos:definition>
        <skos:definition xml:lang="fr">Zone constituée de bassins creusés à proximité des côtes pour extraire le sel de l&apos;eau de mer par évaporation. Les zones de marais salants de moins de 3 ha sont exclues. Les anciens marais salants qui ne sont plus en activité sont exclus.</skos:definition>
        <skos:prefLabel xml:lang="fr">marais salants</skos:prefLabel>
        <skos:prefLabel xml:lang="en">salt evaporator</skos:prefLabel>
    </owl:NamedIndividual>
    


    <!-- http://data.ign.fr/id/codes/topo/typedezai/Marche -->


    <owl:NamedIndividual rdf:about="http://data.ign.fr/id/codes/topo/typedezai/Marche">
        <rdf:type rdf:resource="http://data.ign.fr/def/topo#TypeDeZAI"/>
        <rdf:type rdf:resource="http://www.w3.org/2004/02/skos/core#Concept"/>
        <skos:inScheme rdf:resource="http://data.ign.fr/id/codes/topo/typedezai/liste"/>
        <skos:broader rdf:resource="http://data.ign.fr/id/codes/topo/typedezai/PAIIndustrielCommercial"/>
        <skos:definition xml:lang="en">Any building built for the purpose of marketing wholesale or retail foodstuffs: covered market, national interest market, regional interest market, hall, fair, permanent exhibition area, covered auction.</skos:definition>
        <skos:definition xml:lang="fr">Tout ensemble construit dont la finalité est la commercialisation de gros ou de détail de denrées alimentaires : marché couvert, marché d&apos;intérêt national, marché d&apos;intérêt régional, halle, foire, zone d&apos;exposition à caractère permanent, criée couverte.</skos:definition>
        <skos:prefLabel xml:lang="fr">marché</skos:prefLabel>
        <skos:prefLabel xml:lang="en">market</skos:prefLabel>
    </owl:NamedIndividual>
    


    <!-- http://data.ign.fr/id/codes/topo/typedezai/Menhir -->


    <owl:NamedIndividual rdf:about="http://data.ign.fr/id/codes/topo/typedezai/Menhir">
        <rdf:type rdf:resource="http://data.ign.fr/def/topo#TypeDeZAI"/>
        <rdf:type rdf:resource="http://www.w3.org/2004/02/skos/core#Concept"/>
        <skos:inScheme rdf:resource="http://data.ign.fr/id/codes/topo/typedezai/liste"/>
        <skos:broader rdf:resource="http://data.ign.fr/id/codes/topo/typedezai/PAICultureLoisirs"/>
        <skos:definition xml:lang="en">Elongated stone, erected vertically. The alignments in cromlech are included.</skos:definition>
        <skos:definition xml:lang="fr">Pierre allongée, dressée verticalement. Les alignements en cromlech sont inclus.</skos:definition>
        <skos:prefLabel xml:lang="en">menhir</skos:prefLabel>
        <skos:prefLabel xml:lang="fr">menhir</skos:prefLabel>
    </owl:NamedIndividual>
    


    <!-- http://data.ign.fr/id/codes/topo/typedezai/Mine -->


    <owl:NamedIndividual rdf:about="http://data.ign.fr/id/codes/topo/typedezai/Mine">
        <rdf:type rdf:resource="http://data.ign.fr/def/topo#TypeDeZAI"/>
        <rdf:type rdf:resource="http://www.w3.org/2004/02/skos/core#Concept"/>
        <skos:inScheme rdf:resource="http://data.ign.fr/id/codes/topo/typedezai/liste"/>
        <skos:broader rdf:resource="http://data.ign.fr/id/codes/topo/typedezai/PAIIndustrielCommercial"/>
        <skos:definition xml:lang="fr">Lieu d&apos;où l&apos;on extrait des minerais : mine de houille, mine de lignite, crassier, entrée de mine, terril. Les mines à ciel ouvert de plus de 10 ha sont incluses. Les mines souterraines sont exclues.</skos:definition>
        <skos:definition xml:lang="en">Location from which minerals are mined: coal mine, lignite mine, slag pit, mine entrance, slag heap. Open pit mines of more than 10 ha are included. Underground mines are excluded.</skos:definition>
        <skos:prefLabel xml:lang="en">mine</skos:prefLabel>
        <skos:prefLabel xml:lang="fr">mine</skos:prefLabel>
    </owl:NamedIndividual>
    


    <!-- http://data.ign.fr/id/codes/topo/typedezai/Moulin -->


    <owl:NamedIndividual rdf:about="http://data.ign.fr/id/codes/topo/typedezai/Moulin">
        <rdf:type rdf:resource="http://data.ign.fr/def/topo#TypeDeZAI"/>
        <rdf:type rdf:resource="http://www.w3.org/2004/02/skos/core#Concept"/>
        <skos:inScheme rdf:resource="http://data.ign.fr/id/codes/topo/typedezai/liste"/>
        <skos:broader rdf:resource="http://data.ign.fr/id/codes/topo/typedezai/PAIZoneHabitation"/>
        <skos:definition xml:lang="en">Mill or old water mill.</skos:definition>
        <skos:definition xml:lang="fr">Moulin ou ancien moulin à eau.</skos:definition>
        <skos:prefLabel xml:lang="en">mill</skos:prefLabel>
        <skos:prefLabel xml:lang="fr">moulin</skos:prefLabel>
    </owl:NamedIndividual>
    


    <!-- http://data.ign.fr/id/codes/topo/typedezai/Musee -->


    <owl:NamedIndividual rdf:about="http://data.ign.fr/id/codes/topo/typedezai/Musee">
        <rdf:type rdf:resource="http://data.ign.fr/def/topo#TypeDeZAI"/>
        <rdf:type rdf:resource="http://www.w3.org/2004/02/skos/core#Concept"/>
        <skos:inScheme rdf:resource="http://data.ign.fr/id/codes/topo/typedezai/liste"/>
        <skos:broader rdf:resource="http://data.ign.fr/id/codes/topo/typedezai/PAICultureLoisirs"/>
        <skos:definition xml:lang="en">Open to the public with a large collection of art and science objects, documents, etc. that can be used in their history. Included: all museums controlled or supervised by the Ministry of Culture (national museums, classified, controlled, etc.), museums under certain technical ministries or public assistance (Army Museum, Navy Museum ), private museums or associations with high notoriety, ecomuseums.</skos:definition>
        <skos:definition xml:lang="fr">Établissement ouvert au public exposant une grande collection d&apos;objets, de documents, etc., relatifs aux arts et aux sciences et pouvant servir à leur histoire. Sont inclus : tous les musées controlés ou supervisés par le ministère de la Culture (musées nationaux, classés, controlés,etc.), les musées relevant de certains ministères techniques ou de l&apos;assistance publique (musée de l&apos;armée, de la marine), les musées privés ou associatifs ayant une grande notoriété, les écomusées.</skos:definition>
        <skos:prefLabel xml:lang="en">museum</skos:prefLabel>
        <skos:prefLabel xml:lang="fr">musée</skos:prefLabel>
    </owl:NamedIndividual>
    


    <!-- http://data.ign.fr/id/codes/topo/typedezai/OuvrageMilitaire -->


    <owl:NamedIndividual rdf:about="http://data.ign.fr/id/codes/topo/typedezai/OuvrageMilitaire">
        <rdf:type rdf:resource="http://data.ign.fr/def/topo#TypeDeZAI"/>
        <rdf:type rdf:resource="http://www.w3.org/2004/02/skos/core#Concept"/>
        <skos:inScheme rdf:resource="http://data.ign.fr/id/codes/topo/typedezai/liste"/>
        <skos:broader rdf:resource="http://data.ign.fr/id/codes/topo/typedezai/PAIAdministratifOuMilitaire"/>
        <skos:definition xml:lang="en">Military works or installations.</skos:definition>
        <skos:definition xml:lang="fr">Ouvrages ou installations militaires.</skos:definition>
        <skos:prefLabel xml:lang="en">defence work</skos:prefLabel>
        <skos:prefLabel xml:lang="fr">ouvrage militaire</skos:prefLabel>
    </owl:NamedIndividual>
    


    <!-- http://data.ign.fr/id/codes/topo/typedezai/PAIAdministratifOuMilitaire -->


    <owl:NamedIndividual rdf:about="http://data.ign.fr/id/codes/topo/typedezai/PAIAdministratifOuMilitaire">
        <rdf:type rdf:resource="http://data.ign.fr/def/topo#TypeDeZAI"/>
        <rdf:type rdf:resource="http://www.w3.org/2004/02/skos/core#Concept"/>
        <skos:inScheme rdf:resource="http://data.ign.fr/id/codes/topo/typedezai/liste"/>
        <skos:definition xml:lang="en">Designation of an establishment, site or area of public, administrative or military character.</skos:definition>
        <skos:definition xml:lang="fr">Désignation d&apos;un établissement, site ou zone ayant un caractère public, administratif ou militaire.</skos:definition>
        <skos:prefLabel xml:lang="fr">PAI administratif ou militaire</skos:prefLabel>
        <skos:prefLabel xml:lang="en">administrative or military POI</skos:prefLabel>
    </owl:NamedIndividual>
    


    <!-- http://data.ign.fr/id/codes/topo/typedezai/PAICultureLoisirs -->


    <owl:NamedIndividual rdf:about="http://data.ign.fr/id/codes/topo/typedezai/PAICultureLoisirs">
        <rdf:type rdf:resource="http://data.ign.fr/def/topo#TypeDeZAI"/>
        <rdf:type rdf:resource="http://www.w3.org/2004/02/skos/core#Concept"/>
        <skos:inScheme rdf:resource="http://data.ign.fr/id/codes/topo/typedezai/liste"/>
        <skos:definition xml:lang="en">Designation of an establishment or place specially equipped for a cultural, tourist or leisure activity.</skos:definition>
        <skos:definition xml:lang="fr">Désignation d&apos;un établissement ou lieu spécialement aménagé pour une activité culturelle, touristique ou de loisirs.</skos:definition>
        <skos:prefLabel xml:lang="fr">PAI culture ou loisirs</skos:prefLabel>
        <skos:prefLabel xml:lang="en">culture or leasure POI</skos:prefLabel>
    </owl:NamedIndividual>
    


    <!-- http://data.ign.fr/id/codes/topo/typedezai/PAIEspaceNaturel -->


    <owl:NamedIndividual rdf:about="http://data.ign.fr/id/codes/topo/typedezai/PAIEspaceNaturel">
        <rdf:type rdf:resource="http://data.ign.fr/def/topo#TypeDeZAI"/>
        <rdf:type rdf:resource="http://www.w3.org/2004/02/skos/core#Concept"/>
        <skos:inScheme rdf:resource="http://data.ign.fr/id/codes/topo/typedezai/liste"/>
        <skos:definition xml:lang="en">Designation of an uninhabited locality whose name does not relate to an orographic detail or a hydrographic detail.</skos:definition>
        <skos:definition xml:lang="fr">Désignation d&apos;un lieu-dit non habité dont le nom ne se rapporte ni à un détail orographique ni à un détail hydrographique.</skos:definition>
        <skos:prefLabel xml:lang="fr">PAI espace naturel</skos:prefLabel>
        <skos:prefLabel xml:lang="en">natural POI</skos:prefLabel>
    </owl:NamedIndividual>
    


    <!-- http://data.ign.fr/id/codes/topo/typedezai/PAIGestionEaux -->


    <owl:NamedIndividual rdf:about="http://data.ign.fr/id/codes/topo/typedezai/PAIGestionEaux">
        <rdf:type rdf:resource="http://data.ign.fr/def/topo#TypeDeZAI"/>
        <rdf:type rdf:resource="http://www.w3.org/2004/02/skos/core#Concept"/>
        <skos:inScheme rdf:resource="http://data.ign.fr/id/codes/topo/typedezai/liste"/>
        <skos:definition xml:lang="en">Designation of a construction or site related to the supply, treatment of water for different needs (agricultural, industrial, consumption) or sewage treatment before release into the wild.</skos:definition>
        <skos:definition xml:lang="fr">Désignation d&apos;une construction ou site liés à l&apos;approvisionnement, au traitement de l&apos;eau pour différents besoins (agricole, industriel, consommation) ou à l&apos;épuration des eaux usées avant rejet dans la nature.</skos:definition>
        <skos:prefLabel xml:lang="fr">PAI gestion des eaux</skos:prefLabel>
        <skos:prefLabel xml:lang="en">water treatment POI</skos:prefLabel>
    </owl:NamedIndividual>
    


    <!-- http://data.ign.fr/id/codes/topo/typedezai/PAIHydrographie -->


    <owl:NamedIndividual rdf:about="http://data.ign.fr/id/codes/topo/typedezai/PAIHydrographie">
        <rdf:type rdf:resource="http://data.ign.fr/def/topo#TypeDeZAI"/>
        <rdf:type rdf:resource="http://www.w3.org/2004/02/skos/core#Concept"/>
        <skos:inScheme rdf:resource="http://data.ign.fr/id/codes/topo/typedezai/liste"/>
        <skos:definition xml:lang="en">Designation relating to a hydrographic detail.</skos:definition>
        <skos:definition xml:lang="fr">Désignation se rapportant à un détail hydrographique.</skos:definition>
        <skos:prefLabel xml:lang="fr">PAI hydrographie</skos:prefLabel>
        <skos:prefLabel xml:lang="en">hydrographic POI</skos:prefLabel>
    </owl:NamedIndividual>
    


    <!-- http://data.ign.fr/id/codes/topo/typedezai/PAIIndustrielCommercial -->


    <owl:NamedIndividual rdf:about="http://data.ign.fr/id/codes/topo/typedezai/PAIIndustrielCommercial">
        <rdf:type rdf:resource="http://data.ign.fr/def/topo#TypeDeZAI"/>
        <rdf:type rdf:resource="http://www.w3.org/2004/02/skos/core#Concept"/>
        <skos:inScheme rdf:resource="http://data.ign.fr/id/codes/topo/typedezai/liste"/>
        <skos:definition xml:lang="en">Designation of a building, site or zone of an industrial or commercial nature.</skos:definition>
        <skos:definition xml:lang="fr">Désignation d&apos;un bâtiment, site ou zone à caractère industriel ou commercial.</skos:definition>
        <skos:prefLabel xml:lang="fr">PAI industriel ou commercial</skos:prefLabel>
        <skos:prefLabel xml:lang="en">industrial or commercial POI</skos:prefLabel>
    </owl:NamedIndividual>
    


    <!-- http://data.ign.fr/id/codes/topo/typedezai/PAIOrographie -->


    <owl:NamedIndividual rdf:about="http://data.ign.fr/id/codes/topo/typedezai/PAIOrographie">
        <rdf:type rdf:resource="http://data.ign.fr/def/topo#TypeDeZAI"/>
        <rdf:type rdf:resource="http://www.w3.org/2004/02/skos/core#Concept"/>
        <skos:inScheme rdf:resource="http://data.ign.fr/id/codes/topo/typedezai/liste"/>
        <skos:definition xml:lang="en">Designation of a relief detail.</skos:definition>
        <skos:definition xml:lang="fr">Désignation d&apos;un détail du relief.</skos:definition>
        <skos:prefLabel xml:lang="fr">PAI orographie</skos:prefLabel>
        <skos:prefLabel xml:lang="en">relief POI</skos:prefLabel>
    </owl:NamedIndividual>
    


    <!-- http://data.ign.fr/id/codes/topo/typedezai/PAIReligieux -->


    <owl:NamedIndividual rdf:about="http://data.ign.fr/id/codes/topo/typedezai/PAIReligieux">
        <rdf:type rdf:resource="http://data.ign.fr/def/topo#TypeDeZAI"/>
        <rdf:type rdf:resource="http://www.w3.org/2004/02/skos/core#Concept"/>
        <skos:inScheme rdf:resource="http://data.ign.fr/id/codes/topo/typedezai/liste"/>
        <skos:definition xml:lang="en">Designation of a building reserved for the practice of a religion.</skos:definition>
        <skos:definition xml:lang="fr">Désignation d&apos;un bâtiment réservé à la pratique d&apos;une religion.</skos:definition>
        <skos:prefLabel xml:lang="fr">PAI religieux</skos:prefLabel>
        <skos:prefLabel xml:lang="en">religious POI</skos:prefLabel>
    </owl:NamedIndividual>
    


    <!-- http://data.ign.fr/id/codes/topo/typedezai/PAISante -->


    <owl:NamedIndividual rdf:about="http://data.ign.fr/id/codes/topo/typedezai/PAISante">
        <rdf:type rdf:resource="http://data.ign.fr/def/topo#TypeDeZAI"/>
        <rdf:type rdf:resource="http://www.w3.org/2004/02/skos/core#Concept"/>
        <skos:inScheme rdf:resource="http://data.ign.fr/id/codes/topo/typedezai/liste"/>
        <skos:definition xml:lang="en">Designation of a thermal or hospital type establishment.</skos:definition>
        <skos:definition xml:lang="fr">Désignation d&apos;un établissement thermal ou de type hospitalier.</skos:definition>
        <skos:prefLabel xml:lang="fr">PAI santé</skos:prefLabel>
        <skos:prefLabel xml:lang="en">healthcare POI</skos:prefLabel>
    </owl:NamedIndividual>
    


    <!-- http://data.ign.fr/id/codes/topo/typedezai/PAIScienceEnseignement -->


    <owl:NamedIndividual rdf:about="http://data.ign.fr/id/codes/topo/typedezai/PAIScienceEnseignement">
        <rdf:type rdf:resource="http://data.ign.fr/def/topo#TypeDeZAI"/>
        <rdf:type rdf:resource="http://www.w3.org/2004/02/skos/core#Concept"/>
        <skos:inScheme rdf:resource="http://data.ign.fr/id/codes/topo/typedezai/liste"/>
        <skos:definition xml:lang="en">Designation of an educational or research institution.</skos:definition>
        <skos:definition xml:lang="fr">Désignation d&apos;un établissement d&apos;enseignement ou de recherche.</skos:definition>
        <skos:prefLabel xml:lang="fr">PAI science ou enseignement</skos:prefLabel>
        <skos:prefLabel xml:lang="en">science or education POI</skos:prefLabel>
    </owl:NamedIndividual>
    


    <!-- http://data.ign.fr/id/codes/topo/typedezai/PAISport -->


    <owl:NamedIndividual rdf:about="http://data.ign.fr/id/codes/topo/typedezai/PAISport">
        <rdf:type rdf:resource="http://data.ign.fr/def/topo#TypeDeZAI"/>
        <rdf:type rdf:resource="http://www.w3.org/2004/02/skos/core#Concept"/>
        <skos:inScheme rdf:resource="http://data.ign.fr/id/codes/topo/typedezai/liste"/>
        <skos:definition xml:lang="fr">Désignation d&apos;un établissement ou lieu spécialement aménagé pour la pratique d&apos;une ou plusieurs activités sportives.</skos:definition>
        <skos:prefLabel xml:lang="fr">PAI sport</skos:prefLabel>
        <skos:prefLabel xml:lang="en">sports POI</skos:prefLabel>
    </owl:NamedIndividual>
    


    <!-- http://data.ign.fr/id/codes/topo/typedezai/PAITransport -->


    <owl:NamedIndividual rdf:about="http://data.ign.fr/id/codes/topo/typedezai/PAITransport">
        <rdf:type rdf:resource="http://data.ign.fr/def/topo#TypeDeZAI"/>
        <rdf:type rdf:resource="http://www.w3.org/2004/02/skos/core#Concept"/>
        <skos:inScheme rdf:resource="http://data.ign.fr/id/codes/topo/typedezai/liste"/>
        <skos:definition xml:lang="en">Designation of an establishment or place specially equipped for the practice of one or more sports activities.</skos:definition>
        <skos:definition xml:lang="fr">Désignation d&apos;un bâtiment ou site lié à une activité de transport routier, ferré ou aérien.</skos:definition>
        <skos:prefLabel xml:lang="fr">PAI transport</skos:prefLabel>
        <skos:prefLabel xml:lang="en">transport POI</skos:prefLabel>
    </owl:NamedIndividual>
    


    <!-- http://data.ign.fr/id/codes/topo/typedezai/PAIZoneHabitation -->


    <owl:NamedIndividual rdf:about="http://data.ign.fr/id/codes/topo/typedezai/PAIZoneHabitation">
        <rdf:type rdf:resource="http://data.ign.fr/def/topo#TypeDeZAI"/>
        <rdf:type rdf:resource="http://www.w3.org/2004/02/skos/core#Concept"/>
        <skos:inScheme rdf:resource="http://data.ign.fr/id/codes/topo/typedezai/liste"/>
        <skos:definition xml:lang="en">Designation of an inhabited locality characterized by a name.</skos:definition>
        <skos:definition xml:lang="fr">Désignation d&apos;un lieu-dit habité caractérisé par un nom.</skos:definition>
        <skos:prefLabel xml:lang="fr">PAI zone d&apos;habitation</skos:prefLabel>
        <skos:prefLabel xml:lang="en">dwellings zone POI</skos:prefLabel>
    </owl:NamedIndividual>
    


    <!-- http://data.ign.fr/id/codes/topo/typedezai/PalaisDeJustice -->


    <owl:NamedIndividual rdf:about="http://data.ign.fr/id/codes/topo/typedezai/PalaisDeJustice">
        <rdf:type rdf:resource="http://data.ign.fr/def/topo#TypeDeZAI"/>
        <rdf:type rdf:resource="http://www.w3.org/2004/02/skos/core#Concept"/>
        <skos:inScheme rdf:resource="http://data.ign.fr/id/codes/topo/typedezai/liste"/>
        <skos:broader rdf:resource="http://data.ign.fr/id/codes/topo/typedezai/PAIAdministratifOuMilitaire"/>
        <skos:definition xml:lang="en">Building where justice is done: courthouse, court. Only criminal justice is treated. Administrative tribunals are excluded.</skos:definition>
        <skos:definition xml:lang="fr">Bâtiment où l&apos;on rend la justice : palais de justice, tribunal. Seule la justice pénale est traitée. Les tribunaux administratifs sont exclus.</skos:definition>
        <skos:prefLabel xml:lang="en">law-courts</skos:prefLabel>
        <skos:prefLabel xml:lang="fr">palais de justice</skos:prefLabel>
    </owl:NamedIndividual>
    


    <!-- http://data.ign.fr/id/codes/topo/typedezai/Parc -->


    <owl:NamedIndividual rdf:about="http://data.ign.fr/id/codes/topo/typedezai/Parc">
        <rdf:type rdf:resource="http://data.ign.fr/def/topo#TypeDeZAI"/>
        <rdf:type rdf:resource="http://www.w3.org/2004/02/skos/core#Concept"/>
        <skos:inScheme rdf:resource="http://data.ign.fr/id/codes/topo/typedezai/liste"/>
        <skos:broader rdf:resource="http://data.ign.fr/id/codes/topo/typedezai/PAIEspaceNaturel"/>
        <skos:definition xml:lang="fr">Espace réglementé, généralement libre d&apos;accès pour le public et où la nature fait l&apos;objet d&apos;une protection spéciale : jardin, parc municipal, parc intercommunal, parc départemental, parc interdépartemental, parc naturel régional, parc national, réserve naturelle, parc marin. Les parcs à vocation commerciale ne sont pas pris en compte.</skos:definition>
        <skos:definition xml:lang="en">Regulated area, generally free for the public and where nature is the subject of special protection: garden, municipal park, intercommunal park, departmental park, interdepartmental park, regional nature park, national park, nature reserve, park marine. Commercial parks are not taken into account.</skos:definition>
        <skos:prefLabel xml:lang="fr">parc</skos:prefLabel>
        <skos:prefLabel xml:lang="en">park</skos:prefLabel>
    </owl:NamedIndividual>
    


    <!-- http://data.ign.fr/id/codes/topo/typedezai/ParcDeLoisirs -->


    <owl:NamedIndividual rdf:about="http://data.ign.fr/id/codes/topo/typedezai/ParcDeLoisirs">
        <rdf:type rdf:resource="http://data.ign.fr/def/topo#TypeDeZAI"/>
        <rdf:type rdf:resource="http://www.w3.org/2004/02/skos/core#Concept"/>
        <skos:inScheme rdf:resource="http://data.ign.fr/id/codes/topo/typedezai/liste"/>
        <skos:broader rdf:resource="http://data.ign.fr/id/codes/topo/typedezai/PAICultureLoisirs"/>
        <skos:definition xml:lang="en">Commercial park specially designed for recreation: permanent games center, amusement park, relaxation park, leisure center. Only parks with an area exceeding 10 ha and equipped with substantial equipment are included. Public parks (gardens, municipal parks, departmental parks) are excluded (see the value &apos;public space&apos;).</skos:definition>
        <skos:definition xml:lang="fr">Parc à caractère commercial spécialement aménagé pour les loisirs : centre permanent de jeux, parc d&apos;attractions, parc de détente, centre de loisirs. Seuls les parcs dont la superficie excède 10 ha et dotés d&apos;équipements conséquents sont inclus. Les parcs publics (jardins, parcs communaux, départementaux) sont exclus (voir la valeur &apos;espace public&apos;).</skos:definition>
        <skos:prefLabel xml:lang="en">leisure park</skos:prefLabel>
        <skos:prefLabel xml:lang="fr">parc de loisirs</skos:prefLabel>
    </owl:NamedIndividual>
    


    <!-- http://data.ign.fr/id/codes/topo/typedezai/ParcDesExpositions -->


    <owl:NamedIndividual rdf:about="http://data.ign.fr/id/codes/topo/typedezai/ParcDesExpositions">
        <rdf:type rdf:resource="http://data.ign.fr/def/topo#TypeDeZAI"/>
        <rdf:type rdf:resource="http://www.w3.org/2004/02/skos/core#Concept"/>
        <skos:inScheme rdf:resource="http://data.ign.fr/id/codes/topo/typedezai/liste"/>
        <skos:broader rdf:resource="http://data.ign.fr/id/codes/topo/typedezai/PAICultureLoisirs"/>
        <skos:definition xml:lang="fr">Lieu d&apos;exposition ou de culture : centre culturel, parc des expositions.</skos:definition>
        <skos:definition xml:lang="en">Place of exhibition or culture: cultural center, exhibition center.</skos:definition>
        <skos:prefLabel xml:lang="en">fairground</skos:prefLabel>
        <skos:prefLabel xml:lang="fr">parc des expositions</skos:prefLabel>
    </owl:NamedIndividual>
    


    <!-- http://data.ign.fr/id/codes/topo/typedezai/ParcZoologique -->


    <owl:NamedIndividual rdf:about="http://data.ign.fr/id/codes/topo/typedezai/ParcZoologique">
        <rdf:type rdf:resource="http://data.ign.fr/def/topo#TypeDeZAI"/>
        <rdf:type rdf:resource="http://www.w3.org/2004/02/skos/core#Concept"/>
        <skos:inScheme rdf:resource="http://data.ign.fr/id/codes/topo/typedezai/liste"/>
        <skos:broader rdf:resource="http://data.ign.fr/id/codes/topo/typedezai/PAICultureLoisirs"/>
        <skos:definition xml:lang="fr">Parc ouvert au public, où il est possible de voir des animaux sauvages vivant en captivité ou en semi-liberté. Tous les parcs ouverts au public sont inclus.</skos:definition>
        <skos:definition xml:lang="en">Park open to the public, where it is possible to see wild animals living in captivity or semi-freedom. All parks open to the public are included.</skos:definition>
        <skos:prefLabel xml:lang="fr">parc zoologique</skos:prefLabel>
        <skos:prefLabel xml:lang="en">zoological park</skos:prefLabel>
    </owl:NamedIndividual>
    


    <!-- http://data.ign.fr/id/codes/topo/typedezai/PareFeu -->


    <owl:NamedIndividual rdf:about="http://data.ign.fr/id/codes/topo/typedezai/PareFeu">
        <rdf:type rdf:resource="http://data.ign.fr/def/topo#TypeDeZAI"/>
        <rdf:type rdf:resource="http://www.w3.org/2004/02/skos/core#Concept"/>
        <skos:inScheme rdf:resource="http://data.ign.fr/id/codes/topo/typedezai/liste"/>
        <skos:broader rdf:resource="http://data.ign.fr/id/codes/topo/typedezai/PAIEspaceNaturel"/>
        <skos:definition xml:lang="en">Device designed to prevent the spread of a fire (usually opening in the endangered forest).</skos:definition>
        <skos:definition xml:lang="fr">Dispositif destiné à empêcher la propagation d&apos;un incendie (généralement, ouverture pratiquée dans le massif forestier menacé).</skos:definition>
        <skos:prefLabel xml:lang="en">fire-break</skos:prefLabel>
        <skos:prefLabel xml:lang="fr">pare-feu</skos:prefLabel>
    </owl:NamedIndividual>
    


    <!-- http://data.ign.fr/id/codes/topo/typedezai/Parking -->


    <owl:NamedIndividual rdf:about="http://data.ign.fr/id/codes/topo/typedezai/Parking">
        <rdf:type rdf:resource="http://data.ign.fr/def/topo#TypeDeZAI"/>
        <rdf:type rdf:resource="http://www.w3.org/2004/02/skos/core#Concept"/>
        <skos:inScheme rdf:resource="http://data.ign.fr/id/codes/topo/typedezai/liste"/>
        <skos:broader rdf:resource="http://data.ign.fr/id/codes/topo/typedezai/PAITransport"/>
        <skos:definition xml:lang="en">A parking area or parking area is a parking area for vehicles: parking, parking, underground parking, parking. All public car parks with more than 25 spaces are included, whether underground or air (eg municipal car parks), Car parks with more than 25 spaces associated with transport services (train stations, airports) are retained even if they do not have a proper name. Parking spaces at rest or service areas are not retained (see &apos;Rest Area&apos; and &apos;Service Area&apos; values). Car parks belonging to purely commercial establishments (eg supermarket car park) are excluded (for these, see also the &apos;Road surface&apos; class). Parking is a one-off object located in the center of the parking area, or at the entrance for underground car parks. It is generally associated with a surface area for car parks over 5 ha.</skos:definition>
        <skos:definition xml:lang="fr">Une aire de stationnement ou parking est une zone aménagée pour le stationnement des véhicules : aire de stationnement, parking, parking souterrain, parking à étages. Tous les parkings publics nommés de plus de 25 places sont inclus qu&apos;ils soient souterrains ou aériens (ex. parkings municipaux), Les parkings de plus de 25 places associés à des services de transport (gares, aéroports) sont retenus même s&apos;ils n&apos;ont pas de nom propre. Les parkings d&apos;aires de repos ou de service ne sont pas retenus (voir les valeur &apos;Aire de repos&apos; et &apos;Aire de service&apos;). Le parkings appartenant à des établissements purement commerciaux (ex. parking de supermarché) sont exclus (pour ces derniers, voir aussi la classe &apos;Surface de route&apos;). Un Parking est un objet ponctuel situé au centre de l&apos;aire de stationnement, ou à l&apos;entrée pour les parkings souterrains. Il est généralement associé à une surface pour des parkings aériens de plus de 5 ha.</skos:definition>
        <skos:prefLabel xml:lang="en">car park</skos:prefLabel>
        <skos:prefLabel xml:lang="fr">parking</skos:prefLabel>
    </owl:NamedIndividual>
    


    <!-- http://data.ign.fr/id/codes/topo/typedezai/Pecherie -->


    <owl:NamedIndividual rdf:about="http://data.ign.fr/id/codes/topo/typedezai/Pecherie">
        <rdf:type rdf:resource="http://data.ign.fr/def/topo#TypeDeZAI"/>
        <rdf:type rdf:resource="http://www.w3.org/2004/02/skos/core#Concept"/>
        <skos:inScheme rdf:resource="http://data.ign.fr/id/codes/topo/typedezai/liste"/>
        <skos:broader rdf:resource="http://data.ign.fr/id/codes/topo/typedezai/PAIHydrographie"/>
        <skos:definition xml:lang="en">Aquaculture activity area: bouchot, oyster farm, fishery.</skos:definition>
        <skos:definition xml:lang="fr">Zone d&apos;activité aquacole : bouchot, parc à huîtres, pêcherie.</skos:definition>
        <skos:prefLabel xml:lang="en">aquaculture area</skos:prefLabel>
        <skos:prefLabel xml:lang="fr">pêcherie</skos:prefLabel>
    </owl:NamedIndividual>
    


    <!-- http://data.ign.fr/id/codes/topo/typedezai/Perte -->


    <owl:NamedIndividual rdf:about="http://data.ign.fr/id/codes/topo/typedezai/Perte">
        <rdf:type rdf:resource="http://data.ign.fr/def/topo#TypeDeZAI"/>
        <rdf:type rdf:resource="http://www.w3.org/2004/02/skos/core#Concept"/>
        <skos:inScheme rdf:resource="http://data.ign.fr/id/codes/topo/typedezai/liste"/>
        <skos:broader rdf:resource="http://data.ign.fr/id/codes/topo/typedezai/PAIHydrographie"/>
        <skos:definition xml:lang="fr">Lieu où disparaît, où se perd un cours d&apos;eau, qui réapparaît ensuite, en formant une résurgence, après avoir effectué un trajet souterrain.</skos:definition>
        <skos:definition xml:lang="en">Place where disappears, where a stream is lost, which reappears then, forming a resurgence, after having made an underground trip.</skos:definition>
        <skos:prefLabel xml:lang="en">loss</skos:prefLabel>
        <skos:prefLabel xml:lang="fr">perte</skos:prefLabel>
    </owl:NamedIndividual>
    


    <!-- http://data.ign.fr/id/codes/topo/typedezai/Piscine -->


    <owl:NamedIndividual rdf:about="http://data.ign.fr/id/codes/topo/typedezai/Piscine">
        <rdf:type rdf:resource="http://data.ign.fr/def/topo#TypeDeZAI"/>
        <rdf:type rdf:resource="http://www.w3.org/2004/02/skos/core#Concept"/>
        <skos:inScheme rdf:resource="http://data.ign.fr/id/codes/topo/typedezai/liste"/>
        <skos:broader rdf:resource="http://data.ign.fr/id/codes/topo/typedezai/PAISport"/>
        <skos:definition xml:lang="fr">Grand bassin de natation, et ensemble des installations qui l&apos;entourent : piscine couverte, piscine découverte. Toutes les piscines ouvertes au public et ayant un bassin au moins de 25 m ou plus sont incluses. Les piscines des centres de vacances ou des hôtels sont exclues (voir la classe TERRAIN_SPORT).</skos:definition>
        <skos:definition xml:lang="en">Large swimming pool, and all the facilities that surround it: indoor pool, outdoor pool. All pools open to the public and having a pool of at least 25 m or more are included. Pools at holiday centers or hotels are excluded (see the TERRAIN_SPORT class).</skos:definition>
        <skos:narrowMatch rdf:resource="http://data.ign.fr/id/codes/topo/typedebatiment/BassinDeNatation"/>
        <skos:prefLabel xml:lang="fr">piscine</skos:prefLabel>
        <skos:prefLabel xml:lang="en">swimming-pool</skos:prefLabel>
    </owl:NamedIndividual>
    


    <!-- http://data.ign.fr/id/codes/topo/typedezai/PointDEau -->


    <owl:NamedIndividual rdf:about="http://data.ign.fr/id/codes/topo/typedezai/PointDEau">
        <rdf:type rdf:resource="http://data.ign.fr/def/topo#TypeDeZAI"/>
        <rdf:type rdf:resource="http://www.w3.org/2004/02/skos/core#Concept"/>
        <skos:inScheme rdf:resource="http://data.ign.fr/id/codes/topo/typedezai/liste"/>
        <skos:broader rdf:resource="http://data.ign.fr/id/codes/topo/typedezai/PAIHydrographie"/>
        <skos:definition xml:lang="en">Any natural or artificial water point: catchment, cistern, fountain, well, resurgence, source.</skos:definition>
        <skos:definition xml:lang="fr">Tout point d&apos;eau naturel ou artificiel : captage, citerne, fontaine, puits, résurgence, source.</skos:definition>
        <skos:prefLabel xml:lang="fr">point d&apos;eau</skos:prefLabel>
        <skos:prefLabel xml:lang="en">waterhole</skos:prefLabel>
    </owl:NamedIndividual>
    


    <!-- http://data.ign.fr/id/codes/topo/typedezai/PointDeVue -->


    <owl:NamedIndividual rdf:about="http://data.ign.fr/id/codes/topo/typedezai/PointDeVue">
        <rdf:type rdf:resource="http://data.ign.fr/def/topo#TypeDeZAI"/>
        <rdf:type rdf:resource="http://www.w3.org/2004/02/skos/core#Concept"/>
        <skos:inScheme rdf:resource="http://data.ign.fr/id/codes/topo/typedezai/liste"/>
        <skos:broader rdf:resource="http://data.ign.fr/id/codes/topo/typedezai/PAIEspaceNaturel"/>
        <skos:definition xml:lang="fr">Endroit d&apos;où l&apos;on jouit d&apos;une vue pittoresque : point de vue, table d&apos;orientation, belvédè. Seuls les points de vue aménagés (table d&apos;orientation, bancs,etc.) sont inclus.</skos:definition>
        <skos:definition xml:lang="en">Place from where one enjoys a picturesque sight: point of view, orientation table, belvede. Only the points of view (orientation table, benches, etc.) are included.</skos:definition>
        <skos:prefLabel xml:lang="fr">point de vue</skos:prefLabel>
        <skos:prefLabel xml:lang="en">viewpoint</skos:prefLabel>
    </owl:NamedIndividual>
    


    <!-- http://data.ign.fr/id/codes/topo/typedezai/Port -->


    <owl:NamedIndividual rdf:about="http://data.ign.fr/id/codes/topo/typedezai/Port">
        <rdf:type rdf:resource="http://data.ign.fr/def/topo#TypeDeZAI"/>
        <rdf:type rdf:resource="http://www.w3.org/2004/02/skos/core#Concept"/>
        <skos:inScheme rdf:resource="http://data.ign.fr/id/codes/topo/typedezai/liste"/>
        <skos:broader rdf:resource="http://data.ign.fr/id/codes/topo/typedezai/PAITransport"/>
        <skos:definition xml:lang="fr">Abri naturel ou artificiel aménagé pour recevoir les navires, pour l&apos;embarquement et le débarquement de leur chargement : port de plaisance, port de pêche, port national, port privé, port international, port militaire.</skos:definition>
        <skos:definition xml:lang="en">Natural or artificial shelter fitted out to receive the ships, for loading and unloading of their load: marina, fishing port, national port, private port, international port, military port.</skos:definition>
        <skos:prefLabel xml:lang="en">harbor</skos:prefLabel>
        <skos:prefLabel xml:lang="fr">port</skos:prefLabel>
    </owl:NamedIndividual>
    


    <!-- http://data.ign.fr/id/codes/topo/typedezai/PosteDePolice -->


    <owl:NamedIndividual rdf:about="http://data.ign.fr/id/codes/topo/typedezai/PosteDePolice">
        <rdf:type rdf:resource="http://data.ign.fr/def/topo#TypeDeZAI"/>
        <rdf:type rdf:resource="http://www.w3.org/2004/02/skos/core#Concept"/>
        <skos:inScheme rdf:resource="http://data.ign.fr/id/codes/topo/typedezai/liste"/>
        <skos:altLabel xml:lang="fr">hôtel de police</skos:altLabel>
        <skos:altLabel xml:lang="en">police station</skos:altLabel>
        <skos:broader rdf:resource="http://data.ign.fr/id/codes/topo/typedezai/PAIAdministratifOuMilitaire"/>
        <skos:definition xml:lang="en">Establishment occupied by a police commissioner (judicial police officer responsible for enforcing police regulations and ensuring the maintenance of public peace): national police station, police station, highway, port or airport CRS. Buildings housing only the municipal police are excluded. The barracks of CRS and mobile gendarmes take the value &apos;military enclosure&apos; and the gendarmeries the value &apos;gendarmerie&apos;.</skos:definition>
        <skos:definition xml:lang="fr">Établissement occupé par un commissaire de police (officier de police judiciaire chargé de faire observer les règlements de police et de veiller au maintien de la paix publique) : hôtel de police nationale, commissariat, CRS d&apos;autoroute, de port ou d&apos;aéroport. Les bâtiments hébergeant uniquement la police municipale sont exclus. Les casernes de CRS et de gendarmes mobiles prennent la valeur &apos;enceinte militaire&apos; et les gendarmeries la valeur &apos;gendarmerie&apos;.</skos:definition>
        <skos:prefLabel xml:lang="en">police post</skos:prefLabel>
        <skos:prefLabel xml:lang="fr">poste de police</skos:prefLabel>
    </owl:NamedIndividual>
    


    <!-- http://data.ign.fr/id/codes/topo/typedezai/PrefectureDeRegion -->


    <owl:NamedIndividual rdf:about="http://data.ign.fr/id/codes/topo/typedezai/PrefectureDeRegion">
        <rdf:type rdf:resource="http://data.ign.fr/def/topo#TypeDeZAI"/>
        <rdf:type rdf:resource="http://www.w3.org/2004/02/skos/core#Concept"/>
        <skos:inScheme rdf:resource="http://data.ign.fr/id/codes/topo/typedezai/liste"/>
        <skos:broader rdf:resource="http://data.ign.fr/id/codes/topo/typedezai/PAIAdministratifOuMilitaire"/>
        <skos:definition xml:lang="en">Establishment which houses the headquarters of the civil administration of the region. The annexes are excluded.</skos:definition>
        <skos:definition xml:lang="fr">Établissement qui abrite le siège de l&apos;administration civile de la région. Les annexes sont exclues.</skos:definition>
        <skos:prefLabel xml:lang="fr">préfecture de région</skos:prefLabel>
        <skos:prefLabel xml:lang="en">regional prefecture</skos:prefLabel>
    </owl:NamedIndividual>
    


    <!-- http://data.ign.fr/id/codes/topo/typedezai/Quartier -->


    <owl:NamedIndividual rdf:about="http://data.ign.fr/id/codes/topo/typedezai/Quartier">
        <rdf:type rdf:resource="http://data.ign.fr/def/topo#TypeDeZAI"/>
        <rdf:type rdf:resource="http://www.w3.org/2004/02/skos/core#Concept"/>
        <skos:inScheme rdf:resource="http://data.ign.fr/id/codes/topo/typedezai/liste"/>
        <skos:broader rdf:resource="http://data.ign.fr/id/codes/topo/typedezai/PAIZoneHabitation"/>
        <skos:definition xml:lang="en">Neighborhood named: city, suburb, housing estate.</skos:definition>
        <skos:definition xml:lang="fr">Quartier nommé : cité, faubourg, lotissement.</skos:definition>
        <skos:prefLabel xml:lang="en">district</skos:prefLabel>
        <skos:prefLabel xml:lang="fr">quartier</skos:prefLabel>
    </owl:NamedIndividual>
    


    <!-- http://data.ign.fr/id/codes/topo/typedezai/Refuge -->


    <owl:NamedIndividual rdf:about="http://data.ign.fr/id/codes/topo/typedezai/Refuge">
        <rdf:type rdf:resource="http://data.ign.fr/def/topo#TypeDeZAI"/>
        <rdf:type rdf:resource="http://www.w3.org/2004/02/skos/core#Concept"/>
        <skos:inScheme rdf:resource="http://data.ign.fr/id/codes/topo/typedezai/liste"/>
        <skos:broader rdf:resource="http://data.ign.fr/id/codes/topo/typedezai/PAICultureLoisirs"/>
        <skos:definition xml:lang="fr">Refuge, refuge gardé, abri de montagne nommé.</skos:definition>
        <skos:definition xml:lang="en">Refuge, sheltered refuge, named mountain shelter.</skos:definition>
        <skos:prefLabel xml:lang="fr">refuge</skos:prefLabel>
        <skos:prefLabel xml:lang="en">shelter</skos:prefLabel>
    </owl:NamedIndividual>
    


    <!-- http://data.ign.fr/id/codes/topo/typedezai/Riviere -->


    <owl:NamedIndividual rdf:about="http://data.ign.fr/id/codes/topo/typedezai/Riviere">
        <rdf:type rdf:resource="http://data.ign.fr/def/topo#TypeDeZAI"/>
        <rdf:type rdf:resource="http://www.w3.org/2004/02/skos/core#Concept"/>
        <skos:inScheme rdf:resource="http://data.ign.fr/id/codes/topo/typedezai/liste"/>
        <skos:broader rdf:resource="http://data.ign.fr/id/codes/topo/typedezai/PAIHydrographie"/>
        <skos:definition xml:lang="fr">Cours d&apos;eau: fleuve, rivière, ruisseau, torrent.</skos:definition>
        <skos:definition xml:lang="en">Stream: river, stream.</skos:definition>
        <skos:prefLabel xml:lang="en">river</skos:prefLabel>
        <skos:prefLabel xml:lang="fr">rivière</skos:prefLabel>
    </owl:NamedIndividual>
    


    <!-- http://data.ign.fr/id/codes/topo/typedezai/RondPoint -->


    <owl:NamedIndividual rdf:about="http://data.ign.fr/id/codes/topo/typedezai/RondPoint">
        <rdf:type rdf:resource="http://data.ign.fr/def/topo#TypeDeZAI"/>
        <rdf:type rdf:resource="http://www.w3.org/2004/02/skos/core#Concept"/>
        <skos:inScheme rdf:resource="http://data.ign.fr/id/codes/topo/typedezai/liste"/>
        <skos:broader rdf:resource="http://data.ign.fr/id/codes/topo/typedezai/PAITransport"/>
        <skos:definition xml:lang="fr">Rond-point, place de forme circulaire, ovale ou semi-circulaire, ou carrefour giratoire. Un giratoire est formé d&apos;un anneau central qui permet aux usagers de prendre n&apos;importe quelle direction, y compris de faire un demi-tour. Seuls les ronds-points nommés sont retenus.</skos:definition>
        <skos:definition xml:lang="en">Roundabout, circular, oval or semicircular square, or roundabout. A roundabout consists of a central ring that allows users to take any direction, including making a U-turn. Only the roundabouts named are retained.</skos:definition>
        <skos:prefLabel xml:lang="fr">rond-point</skos:prefLabel>
        <skos:prefLabel xml:lang="en">roundabout</skos:prefLabel>
    </owl:NamedIndividual>
    


    <!-- http://data.ign.fr/id/codes/topo/typedezai/Science -->


    <owl:NamedIndividual rdf:about="http://data.ign.fr/id/codes/topo/typedezai/Science">
        <rdf:type rdf:resource="http://data.ign.fr/def/topo#TypeDeZAI"/>
        <rdf:type rdf:resource="http://www.w3.org/2004/02/skos/core#Concept"/>
        <skos:inScheme rdf:resource="http://data.ign.fr/id/codes/topo/typedezai/liste"/>
        <skos:broader rdf:resource="http://data.ign.fr/id/codes/topo/typedezai/PAIScienceEnseignement"/>
        <skos:definition xml:lang="en">Scientific or technical institution named: research center, laboratory, observatory, scientific station.</skos:definition>
        <skos:definition xml:lang="fr">Établissement scientifique ou technique nommé: centre de recherche, laboratoire, observatoire, station scientifique.</skos:definition>
        <skos:prefLabel xml:lang="en">scientific or technological center</skos:prefLabel>
        <skos:prefLabel xml:lang="fr">établissement scientifique ou technique</skos:prefLabel>
    </owl:NamedIndividual>
    


    <!-- http://data.ign.fr/id/codes/topo/typedezai/Stade -->


    <owl:NamedIndividual rdf:about="http://data.ign.fr/id/codes/topo/typedezai/Stade">
        <rdf:type rdf:resource="http://data.ign.fr/def/topo#TypeDeZAI"/>
        <rdf:type rdf:resource="http://www.w3.org/2004/02/skos/core#Concept"/>
        <skos:inScheme rdf:resource="http://data.ign.fr/id/codes/topo/typedezai/liste"/>
        <skos:broader rdf:resource="http://data.ign.fr/id/codes/topo/typedezai/PAISport"/>
        <skos:definition xml:lang="fr">Grande enceinte, terrain aménagé pour la pratique des sports, et le plus souvent entouré de gradins, de tribunes : stade, terrain de sports, vélodrome découvert, circuit auto-moto, complexe sportif pluridisciplinaire. Seules les enceintes incluant des aménagements conséquents (piste &apos;construite&apos;, tribunes,etc.) sont incluses. Les terrains d&apos;entraînement incluant seulement 2 ou 3 terrains de football et de petits vestiaires sont exclus (voir aussi la classe TERRAIN_SPORT).</skos:definition>
        <skos:definition xml:lang="en">Large enclosure, ground arranged for the practice of the sports, and most often surrounded by bleachers, tribunes: stadium, ground of sports, velodrome discovered, circuit auto-moto, sport complex multidisciplinary. Only enclosures including substantial amenities (track &apos;built&apos;, stands, etc.) are included. Training grounds with only 2 or 3 football pitches and locker rooms are excluded (see also TERRAIN_SPORT class).</skos:definition>
        <skos:prefLabel xml:lang="fr">stade</skos:prefLabel>
        <skos:prefLabel xml:lang="en">stadium</skos:prefLabel>
    </owl:NamedIndividual>
    


    <!-- http://data.ign.fr/id/codes/topo/typedezai/StationDeMetro -->


    <owl:NamedIndividual rdf:about="http://data.ign.fr/id/codes/topo/typedezai/StationDeMetro">
        <rdf:type rdf:resource="http://data.ign.fr/def/topo#TypeDeZAI"/>
        <rdf:type rdf:resource="http://www.w3.org/2004/02/skos/core#Concept"/>
        <skos:inScheme rdf:resource="http://data.ign.fr/id/codes/topo/typedezai/liste"/>
        <skos:broader rdf:resource="http://data.ign.fr/id/codes/topo/typedezai/PAITransport"/>
        <skos:definition xml:lang="fr">Station où il est possible d&apos;accéder au réseau du métro. On saisit un seul objet &apos;Station de métro&apos; même s&apos;il y a plusieurs entrées distinctes, éventuellement plusieurs ponctuels &apos;Station de métro&apos; pour les correspondances importantes (ex : Bastille) mais un seul ponctuel pour une station de métro qui n&apos;est pas une correspondance.</skos:definition>
        <skos:definition xml:lang="en">Station where it is possible to access the metro network. One seize only one object &apos;Metro Station&apos; even if there are several separate entrances, possibly several punctual &apos;Metro Station&apos; for important connections (eg Bastille) but only one punctual for a metro station that is not not a match.</skos:definition>
        <skos:prefLabel xml:lang="fr">station de métro</skos:prefLabel>
        <skos:prefLabel xml:lang="en">underground station</skos:prefLabel>
    </owl:NamedIndividual>
    


    <!-- http://data.ign.fr/id/codes/topo/typedezai/Tombeau -->


    <owl:NamedIndividual rdf:about="http://data.ign.fr/id/codes/topo/typedezai/Tombeau">
        <rdf:type rdf:resource="http://data.ign.fr/def/topo#TypeDeZAI"/>
        <rdf:type rdf:resource="http://www.w3.org/2004/02/skos/core#Concept"/>
        <skos:inScheme rdf:resource="http://data.ign.fr/id/codes/topo/typedezai/liste"/>
        <skos:broader rdf:resource="http://data.ign.fr/id/codes/topo/typedezai/PAIReligieux"/>
        <skos:definition xml:lang="en">Cemetery, grave or tomb named: cemetery, tomb, tomb, ossuary, funeral parlor.</skos:definition>
        <skos:definition xml:lang="fr">Cimetière, tombe ou tombeau nommé : cimetière, tombe, tombeau, ossuaire, funérarium.</skos:definition>
        <skos:prefLabel xml:lang="en">tomb</skos:prefLabel>
        <skos:prefLabel xml:lang="fr">tombeau</skos:prefLabel>
    </owl:NamedIndividual>
    


    <!-- http://data.ign.fr/id/codes/topo/typedezai/Usine -->


    <owl:NamedIndividual rdf:about="http://data.ign.fr/id/codes/topo/typedezai/Usine">
        <rdf:type rdf:resource="http://data.ign.fr/def/topo#TypeDeZAI"/>
        <rdf:type rdf:resource="http://www.w3.org/2004/02/skos/core#Concept"/>
        <skos:inScheme rdf:resource="http://data.ign.fr/id/codes/topo/typedezai/liste"/>
        <skos:broader rdf:resource="http://data.ign.fr/id/codes/topo/typedezai/PAIIndustrielCommercial"/>
        <skos:definition xml:lang="en">Establishment dominated by an industrial activity (manufacture of objects or products, transformation or conservation of raw materials): workshop, factory, manufacture, mine with built infrastructure, factory, sawmill. Sites with an area of less than 5 ha are generally excluded.</skos:definition>
        <skos:definition xml:lang="fr">Établissement dominé par une activité industrielle (fabrication d&apos;objets ou de produits, transformation ou conservation de matières premières) : atelier, fabrique, manufacture, mine avec infrastructure bâtie, usine, scierie. Les sites dont la superficie est inférieure à 5 ha sont généralement exclus.</skos:definition>
        <skos:prefLabel xml:lang="en">factory</skos:prefLabel>
        <skos:prefLabel xml:lang="fr">usine</skos:prefLabel>
    </owl:NamedIndividual>
    


    <!-- http://data.ign.fr/id/codes/topo/typedezai/UsineDeTraitementDesEaux -->


    <owl:NamedIndividual rdf:about="http://data.ign.fr/id/codes/topo/typedezai/UsineDeTraitementDesEaux">
        <rdf:type rdf:resource="http://data.ign.fr/def/topo#TypeDeZAI"/>
        <rdf:type rdf:resource="http://www.w3.org/2004/02/skos/core#Concept"/>
        <skos:inScheme rdf:resource="http://data.ign.fr/id/codes/topo/typedezai/liste"/>
        <skos:broader rdf:resource="http://data.ign.fr/id/codes/topo/typedezai/PAIGestionEaux"/>
        <skos:definition xml:lang="en">Establishment with facilities to make water clean for consumption (water treatment plant) or to purify wastewater before discharge into the natural environment (sewage treatment plants, lagooning plants): water treatment plant, station purification plant, lagooning station. Treatment and lagooning plants are included. Stations treating water to make it fit for consumption are included when they include significant facilities (factories including basins, filtering, mechanical treatments). Stations are excluded when it concerns only a secondary chemical treatment carried out at the level of a catchment or a reservoir. Bearing stations are also excluded.</skos:definition>
        <skos:definition xml:lang="fr">Établissement comprenant des installations destinées à rendre l&apos;eau propre à la consommation (usine de traitement des eaux) ou à épurer des eaux usées avant leur rejet dans la nature (stations d&apos;épuration, de lagunage) : usine de traitement des eaux, station d&apos;épuration, station de lagunage. Les stations d&apos;épuration et de lagunage sont incluses. Les stations traitant l&apos;eau afin de la rendre propre à la consommation sont incluses lorsqu&apos;elles comprennent des installations conséquentes (usines comprenant bassins, filtrages, traitements mécaniques). Sont exclues les stations lorsqu&apos;il s&apos;agit uniquement d&apos;un traitement chimique d&apos;appoint effectué au niveau d&apos;un captage ou d&apos;un réservoir. Les stations de relèvement sont également exclues.</skos:definition>
        <skos:prefLabel xml:lang="fr">usine de traitement des eaux</skos:prefLabel>
        <skos:prefLabel xml:lang="en">water treatment plant</skos:prefLabel>
    </owl:NamedIndividual>
    


    <!-- http://data.ign.fr/id/codes/topo/typedezai/Vestiges -->


    <owl:NamedIndividual rdf:about="http://data.ign.fr/id/codes/topo/typedezai/Vestiges">
        <rdf:type rdf:resource="http://data.ign.fr/def/topo#TypeDeZAI"/>
        <rdf:type rdf:resource="http://www.w3.org/2004/02/skos/core#Concept"/>
        <skos:inScheme rdf:resource="http://data.ign.fr/id/codes/topo/typedezai/liste"/>
        <skos:broader rdf:resource="http://data.ign.fr/id/codes/topo/typedezai/PAICultureLoisirs"/>
        <skos:definition xml:lang="en">Archaeological remains, excavations, burial mounds, oppidum.</skos:definition>
        <skos:definition xml:lang="fr">Vestiges archéologiques, fouilles, tumulus, oppidum.</skos:definition>
        <skos:prefLabel xml:lang="en">archeological ruins</skos:prefLabel>
        <skos:prefLabel xml:lang="fr">vestiges archéologiques</skos:prefLabel>
    </owl:NamedIndividual>
    


    <!-- http://data.ign.fr/id/codes/topo/typedezai/VillageDeVacances -->


    <owl:NamedIndividual rdf:about="http://data.ign.fr/id/codes/topo/typedezai/VillageDeVacances">
        <rdf:type rdf:resource="http://data.ign.fr/def/topo#TypeDeZAI"/>
        <rdf:type rdf:resource="http://www.w3.org/2004/02/skos/core#Concept"/>
        <skos:inScheme rdf:resource="http://data.ign.fr/id/codes/topo/typedezai/liste"/>
        <skos:broader rdf:resource="http://data.ign.fr/id/codes/topo/typedezai/PAICultureLoisirs"/>
        <skos:definition xml:lang="en">Establishment of holidays including sports facilities or substantial relaxation of which the manager is private or public: village of vacanaces, colony of holidays. Hotels and &apos;holiday camps&apos; are excluded, as well as establishments with a carrying capacity of less than 300 people.</skos:definition>
        <skos:definition xml:lang="fr">Établissement de vacances comprenant des équipements sportifs ou de détente conséquents dont le gestionnaire est privé ou public: village de vacanaces, colonie de vacances. Les hôtels et les &apos;camps de vacances&apos; sont exclus, ainsi que les établissements dont la capacité de rpise en charge est inférieure à 300 personnes.</skos:definition>
        <skos:prefLabel xml:lang="en">holiday village</skos:prefLabel>
        <skos:prefLabel xml:lang="fr">village de vacances</skos:prefLabel>
    </owl:NamedIndividual>
    


    <!-- http://data.ign.fr/id/codes/topo/typedezai/VoieFerree -->


    <owl:NamedIndividual rdf:about="http://data.ign.fr/id/codes/topo/typedezai/VoieFerree">
        <rdf:type rdf:resource="http://data.ign.fr/def/topo#TypeDeZAI"/>
        <rdf:type rdf:resource="http://www.w3.org/2004/02/skos/core#Concept"/>
        <skos:inScheme rdf:resource="http://data.ign.fr/id/codes/topo/typedezai/liste"/>
        <skos:broader rdf:resource="http://data.ign.fr/id/codes/topo/typedezai/PAITransport"/>
        <skos:definition xml:lang="en">Railroad name</skos:definition>
        <skos:definition xml:lang="fr">Voie ferrée nommée</skos:definition>
        <skos:prefLabel xml:lang="en">railway line</skos:prefLabel>
        <skos:prefLabel xml:lang="fr">voie ferrée</skos:prefLabel>
    </owl:NamedIndividual>
    


    <!-- http://data.ign.fr/id/codes/topo/typedezai/ZoneIndustrielle -->


    <owl:NamedIndividual rdf:about="http://data.ign.fr/id/codes/topo/typedezai/ZoneIndustrielle">
        <rdf:type rdf:resource="http://data.ign.fr/def/topo#TypeDeZAI"/>
        <rdf:type rdf:resource="http://www.w3.org/2004/02/skos/core#Concept"/>
        <skos:inScheme rdf:resource="http://data.ign.fr/id/codes/topo/typedezai/liste"/>
        <skos:broader rdf:resource="http://data.ign.fr/id/codes/topo/typedezai/PAIIndustrielCommercial"/>
        <skos:definition xml:lang="en">Grouping of production activities on the initiative of local authorities or parastatals (chambers of commerce and industry) and bearing a name: artisanal zone, industrial zone. Sites with an area of less than 5 ha are generally excluded.</skos:definition>
        <skos:definition xml:lang="fr">Regroupement d&apos;activités de production sur l&apos;initiative des collectivités locales ou d&apos;organismes parapublics (chambres de commerce et d&apos;industrie) et portant un nom : zone artisanale, zone industrielle. Les sites dont la superficie est inférieure à 5 ha sont généralement exclus.</skos:definition>
        <skos:prefLabel xml:lang="en">industrial area</skos:prefLabel>
        <skos:prefLabel xml:lang="fr">zone industrielle</skos:prefLabel>
    </owl:NamedIndividual>
    


    <!-- http://data.ign.fr/id/codes/topo/typedezai/liste -->


    <owl:NamedIndividual rdf:about="http://data.ign.fr/id/codes/topo/typedezai/liste">
        <rdf:type rdf:resource="http://www.w3.org/2004/02/skos/core#ConceptScheme"/>
        <rdfs:comment xml:lang="en">List of different types of activity areas and interests, represented as a hierarchy of SKOS concepts.</rdfs:comment>
        <rdfs:comment xml:lang="fr">Liste des différents types de zones d&apos;activité et d&apos;intérêt, représentés comme une hiérarchie de concepts SKOS.</rdfs:comment>
        <rdfs:label xml:lang="fr">Type de ZAI</rdfs:label>
        <rdfs:label xml:lang="en">Type of AOI</rdfs:label>
        <skos:hasTopConcept rdf:resource="http://data.ign.fr/id/codes/topo/typedezai/PAIAdministratifOuMilitaire"/>
        <skos:hasTopConcept rdf:resource="http://data.ign.fr/id/codes/topo/typedezai/PAICultureLoisirs"/>
        <skos:hasTopConcept rdf:resource="http://data.ign.fr/id/codes/topo/typedezai/PAIEspaceNaturel"/>
        <skos:hasTopConcept rdf:resource="http://data.ign.fr/id/codes/topo/typedezai/PAIGestionEaux"/>
        <skos:hasTopConcept rdf:resource="http://data.ign.fr/id/codes/topo/typedezai/PAIHydrographie"/>
        <skos:hasTopConcept rdf:resource="http://data.ign.fr/id/codes/topo/typedezai/PAIIndustrielCommercial"/>
        <skos:hasTopConcept rdf:resource="http://data.ign.fr/id/codes/topo/typedezai/PAIOrographie"/>
        <skos:hasTopConcept rdf:resource="http://data.ign.fr/id/codes/topo/typedezai/PAIReligieux"/>
        <skos:hasTopConcept rdf:resource="http://data.ign.fr/id/codes/topo/typedezai/PAISante"/>
        <skos:hasTopConcept rdf:resource="http://data.ign.fr/id/codes/topo/typedezai/PAIScienceEnseignement"/>
        <skos:hasTopConcept rdf:resource="http://data.ign.fr/id/codes/topo/typedezai/PAISport"/>
        <skos:hasTopConcept rdf:resource="http://data.ign.fr/id/codes/topo/typedezai/PAITransport"/>
        <skos:hasTopConcept rdf:resource="http://data.ign.fr/id/codes/topo/typedezai/PAIZoneHabitation"/>
    </owl:NamedIndividual>
    


    <!-- http://purl.org/dc/terms/ -->


    <rdf:Description rdf:about="http://purl.org/dc/terms/">
        <terms:modified rdf:datatype="http://www.w3.org/2001/XMLSchema#date">2012-06-14</terms:modified>
        <terms:title xml:lang="en">DCMI Metadata Terms - other</terms:title>
        <terms:publisher rdf:resource="http://purl.org/dc/aboutdcmi#DCMI"/>
    </rdf:Description>
    


    <!-- http://purl.org/dc/terms/Agent -->


    <rdf:Description rdf:about="http://purl.org/dc/terms/Agent">
        <rdf:type rdf:resource="http://purl.org/dc/terms/AgentClass"/>
        <terms:issued rdf:datatype="http://www.w3.org/2001/XMLSchema#date">2008-01-14</terms:issued>
    </rdf:Description>
    


    <!-- http://purl.org/dc/terms/AgentClass -->


    <rdf:Description rdf:about="http://purl.org/dc/terms/AgentClass">
        <terms:issued rdf:datatype="http://www.w3.org/2001/XMLSchema#date">2008-01-14</terms:issued>
    </rdf:Description>
    


    <!-- http://purl.org/dc/terms/BibliographicResource -->


    <rdf:Description rdf:about="http://purl.org/dc/terms/BibliographicResource">
        <terms:issued rdf:datatype="http://www.w3.org/2001/XMLSchema#date">2008-01-14</terms:issued>
    </rdf:Description>
    


    <!-- http://purl.org/dc/terms/Box -->


    <rdf:Description rdf:about="http://purl.org/dc/terms/Box">
        <terms:issued rdf:datatype="http://www.w3.org/2001/XMLSchema#date">2000-07-11</terms:issued>
    </rdf:Description>
    


    <!-- http://purl.org/dc/terms/DCMIType -->


    <rdf:Description rdf:about="http://purl.org/dc/terms/DCMIType">
        <rdf:type rdf:resource="http://purl.org/dc/dcam/VocabularyEncodingScheme"/>
        <terms:issued rdf:datatype="http://www.w3.org/2001/XMLSchema#date">2000-07-11</terms:issued>
        <rdfs:comment xml:lang="en">The set of classes specified by the DCMI Type Vocabulary, used to categorize the nature or genre of the resource.</rdfs:comment>
        <rdfs:isDefinedBy rdf:resource="http://purl.org/dc/terms/"/>
        <rdfs:label xml:lang="en">DCMI Type Vocabulary</rdfs:label>
        <rdfs:seeAlso rdf:resource="http://purl.org/dc/dcmitype/"/>
    </rdf:Description>
    


    <!-- http://purl.org/dc/terms/DDC -->


    <rdf:Description rdf:about="http://purl.org/dc/terms/DDC">
        <rdf:type rdf:resource="http://purl.org/dc/dcam/VocabularyEncodingScheme"/>
        <terms:issued rdf:datatype="http://www.w3.org/2001/XMLSchema#date">2000-07-11</terms:issued>
        <rdfs:comment xml:lang="en">The set of conceptual resources specified by the Dewey Decimal Classification.</rdfs:comment>
        <rdfs:isDefinedBy rdf:resource="http://purl.org/dc/terms/"/>
        <rdfs:label xml:lang="en">DDC</rdfs:label>
        <rdfs:seeAlso rdf:resource="http://www.oclc.org/dewey/"/>
    </rdf:Description>
    


    <!-- http://purl.org/dc/terms/FileFormat -->


    <rdf:Description rdf:about="http://purl.org/dc/terms/FileFormat">
        <terms:issued rdf:datatype="http://www.w3.org/2001/XMLSchema#date">2008-01-14</terms:issued>
    </rdf:Description>
    


    <!-- http://purl.org/dc/terms/Frequency -->


    <rdf:Description rdf:about="http://purl.org/dc/terms/Frequency">
        <terms:issued rdf:datatype="http://www.w3.org/2001/XMLSchema#date">2008-01-14</terms:issued>
    </rdf:Description>
    


    <!-- http://purl.org/dc/terms/IMT -->


    <rdf:Description rdf:about="http://purl.org/dc/terms/IMT">
        <rdf:type rdf:resource="http://purl.org/dc/dcam/VocabularyEncodingScheme"/>
        <terms:issued rdf:datatype="http://www.w3.org/2001/XMLSchema#date">2000-07-11</terms:issued>
        <rdfs:comment xml:lang="en">The set of media types specified by the Internet Assigned Numbers Authority.</rdfs:comment>
        <rdfs:isDefinedBy rdf:resource="http://purl.org/dc/terms/"/>
        <rdfs:label xml:lang="en">IMT</rdfs:label>
        <rdfs:seeAlso rdf:resource="http://www.iana.org/assignments/media-types/"/>
    </rdf:Description>
    


    <!-- http://purl.org/dc/terms/ISO3166 -->


    <rdf:Description rdf:about="http://purl.org/dc/terms/ISO3166">
        <terms:issued rdf:datatype="http://www.w3.org/2001/XMLSchema#date">2000-07-11</terms:issued>
    </rdf:Description>
    


    <!-- http://purl.org/dc/terms/ISO639-2 -->


    <rdf:Description rdf:about="http://purl.org/dc/terms/ISO639-2">
        <terms:issued rdf:datatype="http://www.w3.org/2001/XMLSchema#date">2000-07-11</terms:issued>
    </rdf:Description>
    


    <!-- http://purl.org/dc/terms/ISO639-3 -->


    <rdf:Description rdf:about="http://purl.org/dc/terms/ISO639-3">
        <terms:issued rdf:datatype="http://www.w3.org/2001/XMLSchema#date">2008-01-14</terms:issued>
    </rdf:Description>
    


    <!-- http://purl.org/dc/terms/Jurisdiction -->


    <rdf:Description rdf:about="http://purl.org/dc/terms/Jurisdiction">
        <terms:issued rdf:datatype="http://www.w3.org/2001/XMLSchema#date">2008-01-14</terms:issued>
    </rdf:Description>
    


    <!-- http://purl.org/dc/terms/LCC -->


    <rdf:Description rdf:about="http://purl.org/dc/terms/LCC">
        <rdf:type rdf:resource="http://purl.org/dc/dcam/VocabularyEncodingScheme"/>
        <terms:issued rdf:datatype="http://www.w3.org/2001/XMLSchema#date">2000-07-11</terms:issued>
        <rdfs:comment xml:lang="en">The set of conceptual resources specified by the Library of Congress Classification.</rdfs:comment>
        <rdfs:isDefinedBy rdf:resource="http://purl.org/dc/terms/"/>
        <rdfs:label xml:lang="en">LCC</rdfs:label>
        <rdfs:seeAlso rdf:resource="http://lcweb.loc.gov/catdir/cpso/lcco/lcco.html"/>
    </rdf:Description>
    


    <!-- http://purl.org/dc/terms/LCSH -->


    <rdf:Description rdf:about="http://purl.org/dc/terms/LCSH">
        <rdf:type rdf:resource="http://purl.org/dc/dcam/VocabularyEncodingScheme"/>
        <terms:issued rdf:datatype="http://www.w3.org/2001/XMLSchema#date">2000-07-11</terms:issued>
        <rdfs:comment xml:lang="en">The set of labeled concepts specified by the Library of Congress Subject Headings.</rdfs:comment>
        <rdfs:isDefinedBy rdf:resource="http://purl.org/dc/terms/"/>
        <rdfs:label xml:lang="en">LCSH</rdfs:label>
    </rdf:Description>
    


    <!-- http://purl.org/dc/terms/LicenseDocument -->


    <rdf:Description rdf:about="http://purl.org/dc/terms/LicenseDocument">
        <terms:issued rdf:datatype="http://www.w3.org/2001/XMLSchema#date">2008-01-14</terms:issued>
    </rdf:Description>
    


    <!-- http://purl.org/dc/terms/LinguisticSystem -->


    <rdf:Description rdf:about="http://purl.org/dc/terms/LinguisticSystem">
        <terms:issued rdf:datatype="http://www.w3.org/2001/XMLSchema#date">2008-01-14</terms:issued>
    </rdf:Description>
    


    <!-- http://purl.org/dc/terms/Location -->


    <rdf:Description rdf:about="http://purl.org/dc/terms/Location">
        <terms:issued rdf:datatype="http://www.w3.org/2001/XMLSchema#date">2008-01-14</terms:issued>
    </rdf:Description>
    


    <!-- http://purl.org/dc/terms/LocationPeriodOrJurisdiction -->


    <rdf:Description rdf:about="http://purl.org/dc/terms/LocationPeriodOrJurisdiction">
        <terms:issued rdf:datatype="http://www.w3.org/2001/XMLSchema#date">2008-01-14</terms:issued>
    </rdf:Description>
    


    <!-- http://purl.org/dc/terms/MESH -->


    <rdf:Description rdf:about="http://purl.org/dc/terms/MESH">
        <rdf:type rdf:resource="http://purl.org/dc/dcam/VocabularyEncodingScheme"/>
        <terms:issued rdf:datatype="http://www.w3.org/2001/XMLSchema#date">2000-07-11</terms:issued>
        <rdfs:comment xml:lang="en">The set of labeled concepts specified by the Medical Subject Headings.</rdfs:comment>
        <rdfs:isDefinedBy rdf:resource="http://purl.org/dc/terms/"/>
        <rdfs:label xml:lang="en">MeSH</rdfs:label>
        <rdfs:seeAlso rdf:resource="http://www.nlm.nih.gov/mesh/meshhome.html"/>
    </rdf:Description>
    


    <!-- http://purl.org/dc/terms/MediaType -->


    <rdf:Description rdf:about="http://purl.org/dc/terms/MediaType">
        <terms:issued rdf:datatype="http://www.w3.org/2001/XMLSchema#date">2008-01-14</terms:issued>
    </rdf:Description>
    


    <!-- http://purl.org/dc/terms/MediaTypeOrExtent -->


    <rdf:Description rdf:about="http://purl.org/dc/terms/MediaTypeOrExtent">
        <terms:issued rdf:datatype="http://www.w3.org/2001/XMLSchema#date">2008-01-14</terms:issued>
    </rdf:Description>
    


    <!-- http://purl.org/dc/terms/MethodOfAccrual -->


    <rdf:Description rdf:about="http://purl.org/dc/terms/MethodOfAccrual">
        <terms:issued rdf:datatype="http://www.w3.org/2001/XMLSchema#date">2008-01-14</terms:issued>
    </rdf:Description>
    


    <!-- http://purl.org/dc/terms/MethodOfInstruction -->


    <rdf:Description rdf:about="http://purl.org/dc/terms/MethodOfInstruction">
        <terms:issued rdf:datatype="http://www.w3.org/2001/XMLSchema#date">2008-01-14</terms:issued>
    </rdf:Description>
    


    <!-- http://purl.org/dc/terms/NLM -->


    <rdf:Description rdf:about="http://purl.org/dc/terms/NLM">
        <rdf:type rdf:resource="http://purl.org/dc/dcam/VocabularyEncodingScheme"/>
        <terms:issued rdf:datatype="http://www.w3.org/2001/XMLSchema#date">2005-06-13</terms:issued>
        <rdfs:comment xml:lang="en">The set of conceptual resources specified by the National Library of Medicine Classification.</rdfs:comment>
        <rdfs:isDefinedBy rdf:resource="http://purl.org/dc/terms/"/>
        <rdfs:label xml:lang="en">NLM</rdfs:label>
        <rdfs:seeAlso rdf:resource="http://wwwcf.nlm.nih.gov/class/"/>
    </rdf:Description>
    


    <!-- http://purl.org/dc/terms/Period -->


    <rdf:Description rdf:about="http://purl.org/dc/terms/Period">
        <terms:issued rdf:datatype="http://www.w3.org/2001/XMLSchema#date">2000-07-11</terms:issued>
    </rdf:Description>
    


    <!-- http://purl.org/dc/terms/PeriodOfTime -->


    <rdf:Description rdf:about="http://purl.org/dc/terms/PeriodOfTime">
        <terms:issued rdf:datatype="http://www.w3.org/2001/XMLSchema#date">2008-01-14</terms:issued>
    </rdf:Description>
    


    <!-- http://purl.org/dc/terms/PhysicalMedium -->


    <rdf:Description rdf:about="http://purl.org/dc/terms/PhysicalMedium">
        <terms:issued rdf:datatype="http://www.w3.org/2001/XMLSchema#date">2008-01-14</terms:issued>
    </rdf:Description>
    


    <!-- http://purl.org/dc/terms/PhysicalResource -->


    <rdf:Description rdf:about="http://purl.org/dc/terms/PhysicalResource">
        <terms:issued rdf:datatype="http://www.w3.org/2001/XMLSchema#date">2008-01-14</terms:issued>
    </rdf:Description>
    


    <!-- http://purl.org/dc/terms/Point -->


    <rdf:Description rdf:about="http://purl.org/dc/terms/Point">
        <terms:issued rdf:datatype="http://www.w3.org/2001/XMLSchema#date">2000-07-11</terms:issued>
    </rdf:Description>
    


    <!-- http://purl.org/dc/terms/Policy -->


    <rdf:Description rdf:about="http://purl.org/dc/terms/Policy">
        <terms:issued rdf:datatype="http://www.w3.org/2001/XMLSchema#date">2008-01-14</terms:issued>
    </rdf:Description>
    


    <!-- http://purl.org/dc/terms/ProvenanceStatement -->


    <rdf:Description rdf:about="http://purl.org/dc/terms/ProvenanceStatement">
        <terms:issued rdf:datatype="http://www.w3.org/2001/XMLSchema#date">2008-01-14</terms:issued>
    </rdf:Description>
    


    <!-- http://purl.org/dc/terms/RFC1766 -->


    <rdf:Description rdf:about="http://purl.org/dc/terms/RFC1766">
        <terms:issued rdf:datatype="http://www.w3.org/2001/XMLSchema#date">2000-07-11</terms:issued>
    </rdf:Description>
    


    <!-- http://purl.org/dc/terms/RFC3066 -->


    <rdf:Description rdf:about="http://purl.org/dc/terms/RFC3066">
        <terms:issued rdf:datatype="http://www.w3.org/2001/XMLSchema#date">2002-07-13</terms:issued>
    </rdf:Description>
    


    <!-- http://purl.org/dc/terms/RFC4646 -->


    <rdf:Description rdf:about="http://purl.org/dc/terms/RFC4646">
        <terms:issued rdf:datatype="http://www.w3.org/2001/XMLSchema#date">2008-01-14</terms:issued>
    </rdf:Description>
    


    <!-- http://purl.org/dc/terms/RFC5646 -->


    <rdf:Description rdf:about="http://purl.org/dc/terms/RFC5646">
        <terms:issued rdf:datatype="http://www.w3.org/2001/XMLSchema#date">2010-10-11</terms:issued>
    </rdf:Description>
    


    <!-- http://purl.org/dc/terms/RightsStatement -->


    <rdf:Description rdf:about="http://purl.org/dc/terms/RightsStatement">
        <terms:issued rdf:datatype="http://www.w3.org/2001/XMLSchema#date">2008-01-14</terms:issued>
    </rdf:Description>
    


    <!-- http://purl.org/dc/terms/SizeOrDuration -->


    <rdf:Description rdf:about="http://purl.org/dc/terms/SizeOrDuration">
        <terms:issued rdf:datatype="http://www.w3.org/2001/XMLSchema#date">2008-01-14</terms:issued>
    </rdf:Description>
    


    <!-- http://purl.org/dc/terms/Standard -->


    <rdf:Description rdf:about="http://purl.org/dc/terms/Standard">
        <terms:issued rdf:datatype="http://www.w3.org/2001/XMLSchema#date">2008-01-14</terms:issued>
    </rdf:Description>
    


    <!-- http://purl.org/dc/terms/TGN -->


    <rdf:Description rdf:about="http://purl.org/dc/terms/TGN">
        <rdf:type rdf:resource="http://purl.org/dc/dcam/VocabularyEncodingScheme"/>
        <terms:issued rdf:datatype="http://www.w3.org/2001/XMLSchema#date">2000-07-11</terms:issued>
        <rdfs:comment xml:lang="en">The set of places specified by the Getty Thesaurus of Geographic Names.</rdfs:comment>
        <rdfs:isDefinedBy rdf:resource="http://purl.org/dc/terms/"/>
        <rdfs:label xml:lang="en">TGN</rdfs:label>
        <rdfs:seeAlso rdf:resource="http://www.getty.edu/research/tools/vocabulary/tgn/index.html"/>
    </rdf:Description>
    


    <!-- http://purl.org/dc/terms/UDC -->


    <rdf:Description rdf:about="http://purl.org/dc/terms/UDC">
        <rdf:type rdf:resource="http://purl.org/dc/dcam/VocabularyEncodingScheme"/>
        <terms:issued rdf:datatype="http://www.w3.org/2001/XMLSchema#date">2000-07-11</terms:issued>
        <rdfs:comment xml:lang="en">The set of conceptual resources specified by the Universal Decimal Classification.</rdfs:comment>
        <rdfs:isDefinedBy rdf:resource="http://purl.org/dc/terms/"/>
        <rdfs:label xml:lang="en">UDC</rdfs:label>
        <rdfs:seeAlso rdf:resource="http://www.udcc.org/"/>
    </rdf:Description>
    


    <!-- http://purl.org/dc/terms/URI -->


    <rdf:Description rdf:about="http://purl.org/dc/terms/URI">
        <terms:issued rdf:datatype="http://www.w3.org/2001/XMLSchema#date">2000-07-11</terms:issued>
    </rdf:Description>
    


    <!-- http://purl.org/dc/terms/W3CDTF -->


    <rdf:Description rdf:about="http://purl.org/dc/terms/W3CDTF">
        <terms:issued rdf:datatype="http://www.w3.org/2001/XMLSchema#date">2000-07-11</terms:issued>
    </rdf:Description>
    


    <!-- http://purl.org/dc/terms/abstract -->


    <rdf:Description rdf:about="http://purl.org/dc/terms/abstract">
        <terms:issued rdf:datatype="http://www.w3.org/2001/XMLSchema#date">2000-07-11</terms:issued>
    </rdf:Description>
    


    <!-- http://purl.org/dc/terms/accessRights -->


    <rdf:Description rdf:about="http://purl.org/dc/terms/accessRights">
        <terms:issued rdf:datatype="http://www.w3.org/2001/XMLSchema#date">2003-02-15</terms:issued>
    </rdf:Description>
    


    <!-- http://purl.org/dc/terms/accrualMethod -->


    <rdf:Description rdf:about="http://purl.org/dc/terms/accrualMethod">
        <terms:issued rdf:datatype="http://www.w3.org/2001/XMLSchema#date">2005-06-13</terms:issued>
    </rdf:Description>
    


    <!-- http://purl.org/dc/terms/accrualPeriodicity -->


    <rdf:Description rdf:about="http://purl.org/dc/terms/accrualPeriodicity">
        <terms:issued rdf:datatype="http://www.w3.org/2001/XMLSchema#date">2005-06-13</terms:issued>
    </rdf:Description>
    


    <!-- http://purl.org/dc/terms/accrualPolicy -->


    <rdf:Description rdf:about="http://purl.org/dc/terms/accrualPolicy">
        <terms:issued rdf:datatype="http://www.w3.org/2001/XMLSchema#date">2005-06-13</terms:issued>
    </rdf:Description>
    


    <!-- http://purl.org/dc/terms/alternative -->


    <rdf:Description rdf:about="http://purl.org/dc/terms/alternative">
        <terms:issued rdf:datatype="http://www.w3.org/2001/XMLSchema#date">2000-07-11</terms:issued>
    </rdf:Description>
    


    <!-- http://purl.org/dc/terms/audience -->


    <rdf:Description rdf:about="http://purl.org/dc/terms/audience">
        <terms:issued rdf:datatype="http://www.w3.org/2001/XMLSchema#date">2001-05-21</terms:issued>
    </rdf:Description>
    


    <!-- http://purl.org/dc/terms/available -->


    <rdf:Description rdf:about="http://purl.org/dc/terms/available">
        <terms:issued rdf:datatype="http://www.w3.org/2001/XMLSchema#date">2000-07-11</terms:issued>
    </rdf:Description>
    


    <!-- http://purl.org/dc/terms/bibliographicCitation -->


    <rdf:Description rdf:about="http://purl.org/dc/terms/bibliographicCitation">
        <terms:issued rdf:datatype="http://www.w3.org/2001/XMLSchema#date">2003-02-15</terms:issued>
    </rdf:Description>
    


    <!-- http://purl.org/dc/terms/conformsTo -->


    <rdf:Description rdf:about="http://purl.org/dc/terms/conformsTo">
        <terms:issued rdf:datatype="http://www.w3.org/2001/XMLSchema#date">2001-05-21</terms:issued>
    </rdf:Description>
    


    <!-- http://purl.org/dc/terms/contributor -->


    <rdf:Description rdf:about="http://purl.org/dc/terms/contributor">
        <terms:issued rdf:datatype="http://www.w3.org/2001/XMLSchema#date">2008-01-14</terms:issued>
    </rdf:Description>
    


    <!-- http://purl.org/dc/terms/coverage -->


    <rdf:Description rdf:about="http://purl.org/dc/terms/coverage">
        <terms:issued rdf:datatype="http://www.w3.org/2001/XMLSchema#date">2008-01-14</terms:issued>
    </rdf:Description>
    


    <!-- http://purl.org/dc/terms/created -->


    <rdf:Description rdf:about="http://purl.org/dc/terms/created">
        <terms:issued rdf:datatype="http://www.w3.org/2001/XMLSchema#date">2000-07-11</terms:issued>
    </rdf:Description>
    


    <!-- http://purl.org/dc/terms/creator -->


    <rdf:Description rdf:about="http://purl.org/dc/terms/creator">
        <terms:issued rdf:datatype="http://www.w3.org/2001/XMLSchema#date">2008-01-14</terms:issued>
    </rdf:Description>
    


    <!-- http://purl.org/dc/terms/date -->


    <rdf:Description rdf:about="http://purl.org/dc/terms/date">
        <terms:issued rdf:datatype="http://www.w3.org/2001/XMLSchema#date">2008-01-14</terms:issued>
    </rdf:Description>
    


    <!-- http://purl.org/dc/terms/dateAccepted -->


    <rdf:Description rdf:about="http://purl.org/dc/terms/dateAccepted">
        <terms:issued rdf:datatype="http://www.w3.org/2001/XMLSchema#date">2002-07-13</terms:issued>
    </rdf:Description>
    


    <!-- http://purl.org/dc/terms/dateCopyrighted -->


    <rdf:Description rdf:about="http://purl.org/dc/terms/dateCopyrighted">
        <terms:issued rdf:datatype="http://www.w3.org/2001/XMLSchema#date">2002-07-13</terms:issued>
    </rdf:Description>
    


    <!-- http://purl.org/dc/terms/dateSubmitted -->


    <rdf:Description rdf:about="http://purl.org/dc/terms/dateSubmitted">
        <terms:issued rdf:datatype="http://www.w3.org/2001/XMLSchema#date">2002-07-13</terms:issued>
    </rdf:Description>
    


    <!-- http://purl.org/dc/terms/description -->


    <rdf:Description rdf:about="http://purl.org/dc/terms/description">
        <terms:issued rdf:datatype="http://www.w3.org/2001/XMLSchema#date">2008-01-14</terms:issued>
    </rdf:Description>
    


    <!-- http://purl.org/dc/terms/educationLevel -->


    <rdf:Description rdf:about="http://purl.org/dc/terms/educationLevel">
        <terms:issued rdf:datatype="http://www.w3.org/2001/XMLSchema#date">2002-07-13</terms:issued>
    </rdf:Description>
    


    <!-- http://purl.org/dc/terms/extent -->


    <rdf:Description rdf:about="http://purl.org/dc/terms/extent">
        <terms:issued rdf:datatype="http://www.w3.org/2001/XMLSchema#date">2000-07-11</terms:issued>
    </rdf:Description>
    


    <!-- http://purl.org/dc/terms/format -->


    <rdf:Description rdf:about="http://purl.org/dc/terms/format">
        <terms:issued rdf:datatype="http://www.w3.org/2001/XMLSchema#date">2008-01-14</terms:issued>
    </rdf:Description>
    


    <!-- http://purl.org/dc/terms/hasFormat -->


    <rdf:Description rdf:about="http://purl.org/dc/terms/hasFormat">
        <terms:issued rdf:datatype="http://www.w3.org/2001/XMLSchema#date">2000-07-11</terms:issued>
    </rdf:Description>
    


    <!-- http://purl.org/dc/terms/hasPart -->


    <rdf:Description rdf:about="http://purl.org/dc/terms/hasPart">
        <terms:issued rdf:datatype="http://www.w3.org/2001/XMLSchema#date">2000-07-11</terms:issued>
    </rdf:Description>
    


    <!-- http://purl.org/dc/terms/hasVersion -->


    <rdf:Description rdf:about="http://purl.org/dc/terms/hasVersion">
        <terms:issued rdf:datatype="http://www.w3.org/2001/XMLSchema#date">2000-07-11</terms:issued>
    </rdf:Description>
    


    <!-- http://purl.org/dc/terms/identifier -->


    <rdf:Description rdf:about="http://purl.org/dc/terms/identifier">
        <terms:issued rdf:datatype="http://www.w3.org/2001/XMLSchema#date">2008-01-14</terms:issued>
    </rdf:Description>
    


    <!-- http://purl.org/dc/terms/instructionalMethod -->


    <rdf:Description rdf:about="http://purl.org/dc/terms/instructionalMethod">
        <terms:issued rdf:datatype="http://www.w3.org/2001/XMLSchema#date">2005-06-13</terms:issued>
        <dcam:rangeIncludes rdf:resource="http://purl.org/dc/terms/MethodOfInstruction"/>
        <terms:description xml:lang="en">Instructional Method typically includes ways of presenting instructional materials or conducting instructional activities, patterns of learner-to-learner and learner-to-instructor interactions, and mechanisms by which group and individual levels of learning are measured.  Instructional methods include all aspects of the instruction and learning processes from planning and implementation through evaluation and feedback.</terms:description>
        <rdfs:comment xml:lang="en">A process, used to engender knowledge, attitudes and skills, that the described resource is designed to support.</rdfs:comment>
        <rdfs:isDefinedBy rdf:resource="http://purl.org/dc/terms/"/>
        <rdfs:label xml:lang="en">Instructional Method</rdfs:label>
    </rdf:Description>
    


    <!-- http://purl.org/dc/terms/isFormatOf -->


    <rdf:Description rdf:about="http://purl.org/dc/terms/isFormatOf">
        <terms:issued rdf:datatype="http://www.w3.org/2001/XMLSchema#date">2000-07-11</terms:issued>
    </rdf:Description>
    


    <!-- http://purl.org/dc/terms/isPartOf -->


    <rdf:Description rdf:about="http://purl.org/dc/terms/isPartOf">
        <terms:issued rdf:datatype="http://www.w3.org/2001/XMLSchema#date">2000-07-11</terms:issued>
    </rdf:Description>
    


    <!-- http://purl.org/dc/terms/isReferencedBy -->


    <rdf:Description rdf:about="http://purl.org/dc/terms/isReferencedBy">
        <terms:issued rdf:datatype="http://www.w3.org/2001/XMLSchema#date">2000-07-11</terms:issued>
    </rdf:Description>
    


    <!-- http://purl.org/dc/terms/isReplacedBy -->


    <rdf:Description rdf:about="http://purl.org/dc/terms/isReplacedBy">
        <terms:issued rdf:datatype="http://www.w3.org/2001/XMLSchema#date">2000-07-11</terms:issued>
    </rdf:Description>
    


    <!-- http://purl.org/dc/terms/isRequiredBy -->


    <rdf:Description rdf:about="http://purl.org/dc/terms/isRequiredBy">
        <terms:issued rdf:datatype="http://www.w3.org/2001/XMLSchema#date">2000-07-11</terms:issued>
    </rdf:Description>
    


    <!-- http://purl.org/dc/terms/isVersionOf -->


    <rdf:Description rdf:about="http://purl.org/dc/terms/isVersionOf">
        <terms:issued rdf:datatype="http://www.w3.org/2001/XMLSchema#date">2000-07-11</terms:issued>
    </rdf:Description>
    


    <!-- http://purl.org/dc/terms/issued -->


    <rdf:Description rdf:about="http://purl.org/dc/terms/issued">
        <terms:issued rdf:datatype="http://www.w3.org/2001/XMLSchema#date">2000-07-11</terms:issued>
    </rdf:Description>
    


    <!-- http://purl.org/dc/terms/language -->


    <rdf:Description rdf:about="http://purl.org/dc/terms/language">
        <terms:issued rdf:datatype="http://www.w3.org/2001/XMLSchema#date">2008-01-14</terms:issued>
    </rdf:Description>
    


    <!-- http://purl.org/dc/terms/license -->


    <rdf:Description rdf:about="http://purl.org/dc/terms/license">
        <terms:issued rdf:datatype="http://www.w3.org/2001/XMLSchema#date">2004-06-14</terms:issued>
    </rdf:Description>
    


    <!-- http://purl.org/dc/terms/mediator -->


    <rdf:Description rdf:about="http://purl.org/dc/terms/mediator">
        <terms:issued rdf:datatype="http://www.w3.org/2001/XMLSchema#date">2001-05-21</terms:issued>
    </rdf:Description>
    


    <!-- http://purl.org/dc/terms/medium -->


    <rdf:Description rdf:about="http://purl.org/dc/terms/medium">
        <terms:issued rdf:datatype="http://www.w3.org/2001/XMLSchema#date">2000-07-11</terms:issued>
    </rdf:Description>
    


    <!-- http://purl.org/dc/terms/modified -->


    <rdf:Description rdf:about="http://purl.org/dc/terms/modified">
        <terms:issued rdf:datatype="http://www.w3.org/2001/XMLSchema#date">2000-07-11</terms:issued>
    </rdf:Description>
    


    <!-- http://purl.org/dc/terms/provenance -->


    <rdf:Description rdf:about="http://purl.org/dc/terms/provenance">
        <terms:issued rdf:datatype="http://www.w3.org/2001/XMLSchema#date">2004-09-20</terms:issued>
        <dcam:rangeIncludes rdf:resource="http://purl.org/dc/terms/ProvenanceStatement"/>
        <terms:description xml:lang="en">The statement may include a description of any changes successive custodians made to the resource.</terms:description>
        <rdfs:comment xml:lang="en">A statement of any changes in ownership and custody of the resource since its creation that are significant for its authenticity, integrity, and interpretation.</rdfs:comment>
        <rdfs:isDefinedBy rdf:resource="http://purl.org/dc/terms/"/>
        <rdfs:label xml:lang="en">Provenance</rdfs:label>
    </rdf:Description>
    


    <!-- http://purl.org/dc/terms/publisher -->


    <rdf:Description rdf:about="http://purl.org/dc/terms/publisher">
        <terms:issued rdf:datatype="http://www.w3.org/2001/XMLSchema#date">2008-01-14</terms:issued>
    </rdf:Description>
    


    <!-- http://purl.org/dc/terms/references -->


    <rdf:Description rdf:about="http://purl.org/dc/terms/references">
        <terms:issued rdf:datatype="http://www.w3.org/2001/XMLSchema#date">2000-07-11</terms:issued>
    </rdf:Description>
    


    <!-- http://purl.org/dc/terms/relation -->


    <rdf:Description rdf:about="http://purl.org/dc/terms/relation">
        <terms:issued rdf:datatype="http://www.w3.org/2001/XMLSchema#date">2008-01-14</terms:issued>
    </rdf:Description>
    


    <!-- http://purl.org/dc/terms/replaces -->


    <rdf:Description rdf:about="http://purl.org/dc/terms/replaces">
        <terms:issued rdf:datatype="http://www.w3.org/2001/XMLSchema#date">2000-07-11</terms:issued>
    </rdf:Description>
    


    <!-- http://purl.org/dc/terms/requires -->


    <rdf:Description rdf:about="http://purl.org/dc/terms/requires">
        <terms:issued rdf:datatype="http://www.w3.org/2001/XMLSchema#date">2000-07-11</terms:issued>
    </rdf:Description>
    


    <!-- http://purl.org/dc/terms/rights -->


    <rdf:Description rdf:about="http://purl.org/dc/terms/rights">
        <terms:issued rdf:datatype="http://www.w3.org/2001/XMLSchema#date">2008-01-14</terms:issued>
    </rdf:Description>
    


    <!-- http://purl.org/dc/terms/rightsHolder -->


    <rdf:Description rdf:about="http://purl.org/dc/terms/rightsHolder">
        <terms:issued rdf:datatype="http://www.w3.org/2001/XMLSchema#date">2004-06-14</terms:issued>
        <dcam:rangeIncludes rdf:resource="http://purl.org/dc/terms/Agent"/>
        <terms:description xml:lang="en">Recommended practice is to refer to the rights holder with a URI. If this is not possible or feasible, a literal value that identifies the rights holder may be provided.</terms:description>
        <rdfs:comment xml:lang="en">A person or organization owning or managing rights over the resource.</rdfs:comment>
        <rdfs:isDefinedBy rdf:resource="http://purl.org/dc/terms/"/>
        <rdfs:label xml:lang="en">Rights Holder</rdfs:label>
    </rdf:Description>
    


    <!-- http://purl.org/dc/terms/source -->


    <rdf:Description rdf:about="http://purl.org/dc/terms/source">
        <terms:issued rdf:datatype="http://www.w3.org/2001/XMLSchema#date">2008-01-14</terms:issued>
    </rdf:Description>
    


    <!-- http://purl.org/dc/terms/spatial -->


    <rdf:Description rdf:about="http://purl.org/dc/terms/spatial">
        <terms:issued rdf:datatype="http://www.w3.org/2001/XMLSchema#date">2000-07-11</terms:issued>
    </rdf:Description>
    


    <!-- http://purl.org/dc/terms/subject -->


    <rdf:Description rdf:about="http://purl.org/dc/terms/subject">
        <terms:issued rdf:datatype="http://www.w3.org/2001/XMLSchema#date">2008-01-14</terms:issued>
    </rdf:Description>
    


    <!-- http://purl.org/dc/terms/tableOfContents -->


    <rdf:Description rdf:about="http://purl.org/dc/terms/tableOfContents">
        <terms:issued rdf:datatype="http://www.w3.org/2001/XMLSchema#date">2000-07-11</terms:issued>
    </rdf:Description>
    


    <!-- http://purl.org/dc/terms/temporal -->


    <rdf:Description rdf:about="http://purl.org/dc/terms/temporal">
        <terms:issued rdf:datatype="http://www.w3.org/2001/XMLSchema#date">2000-07-11</terms:issued>
    </rdf:Description>
    


    <!-- http://purl.org/dc/terms/title -->


    <rdf:Description rdf:about="http://purl.org/dc/terms/title">
        <terms:issued rdf:datatype="http://www.w3.org/2001/XMLSchema#date">2008-01-14</terms:issued>
    </rdf:Description>
    


    <!-- http://purl.org/dc/terms/type -->


    <rdf:Description rdf:about="http://purl.org/dc/terms/type">
        <terms:issued rdf:datatype="http://www.w3.org/2001/XMLSchema#date">2008-01-14</terms:issued>
    </rdf:Description>
    


    <!-- http://purl.org/dc/terms/valid -->


    <rdf:Description rdf:about="http://purl.org/dc/terms/valid">
        <terms:issued rdf:datatype="http://www.w3.org/2001/XMLSchema#date">2000-07-11</terms:issued>
    </rdf:Description>
    


    <!-- http://www.eurecom.fr/~atemezin/ -->


    <owl:NamedIndividual rdf:about="http://www.eurecom.fr/~atemezin/">
        <rdf:type rdf:resource="http://xmlns.com/foaf/0.1/Person"/>
    </owl:NamedIndividual>
    


    <!-- http://www.semanticweb.org/bbucher/ontologies/2025/9/geodata#amraimond -->


    <owl:NamedIndividual rdf:about="http://www.semanticweb.org/bbucher/ontologies/2025/9/geodata#amraimond">
        <rdf:type rdf:resource="http://www.w3.org/ns/prov#Agent"/>
        <rdf:type rdf:resource="http://www.w3.org/ns/prov#Person"/>
        <rdf:type rdf:resource="http://xmlns.com/foaf/0.1/Person"/>
        <prov:actedOnBehalfOf rdf:resource="http://www.semanticweb.org/bbucher/ontologies/2025/9/geodata#geodata-paris"/>
        <foaf:family_name>Olteanu-Raimond</foaf:family_name>
        <foaf:givenname>Ana-Maria</foaf:givenname>
        <foaf:member rdf:resource="http://www.semanticweb.org/bbucher/ontologies/2025/9/geodata#geodata-paris"/>
        <foaf:name>Ana-Maria Olteanu-Raimond</foaf:name>
        <foaf:title>Mme.</foaf:title>
    </owl:NamedIndividual>
    


    <!-- http://www.semanticweb.org/bbucher/ontologies/2025/9/geodata#bbucher -->


    <owl:NamedIndividual rdf:about="http://www.semanticweb.org/bbucher/ontologies/2025/9/geodata#bbucher">
        <rdf:type rdf:resource="http://www.w3.org/ns/prov#Agent"/>
        <rdf:type rdf:resource="http://www.w3.org/ns/prov#Person"/>
        <rdf:type rdf:resource="http://xmlns.com/foaf/0.1/Person"/>
        <prov:actedOnBehalfOf rdf:resource="http://www.semanticweb.org/bbucher/ontologies/2025/9/geodata#geodata-paris"/>
        <foaf:family_name>Bucher</foaf:family_name>
        <foaf:givenname>Bénédicte</foaf:givenname>
        <foaf:member rdf:resource="http://www.semanticweb.org/bbucher/ontologies/2025/9/geodata#geodata-paris"/>
        <foaf:name>Bénédicte Bucher</foaf:name>
        <foaf:title>Mme.</foaf:title>
    </owl:NamedIndividual>
    


    <!-- http://www.semanticweb.org/bbucher/ontologies/2025/9/geodata#geodata-paris -->


    <owl:NamedIndividual rdf:about="http://www.semanticweb.org/bbucher/ontologies/2025/9/geodata#geodata-paris">
        <rdf:type rdf:resource="http://www.w3.org/ns/prov#Agent"/>
        <rdf:type rdf:resource="http://www.w3.org/ns/prov#Organization"/>
        <rdf:type rdf:resource="http://xmlns.com/foaf/0.1/Organization"/>
        <foaf:homepage rdf:resource="https://geodata-paris.fr"/>
        <foaf:name>Géodata Paris</foaf:name>
    </owl:NamedIndividual>
    


    <!-- http://www.semanticweb.org/bbucher/ontologies/2025/9/geodata#mdvandamme -->


    <owl:NamedIndividual rdf:about="http://www.semanticweb.org/bbucher/ontologies/2025/9/geodata#mdvandamme">
        <rdf:type rdf:resource="http://www.w3.org/ns/prov#Agent"/>
        <rdf:type rdf:resource="http://www.w3.org/ns/prov#Person"/>
        <rdf:type rdf:resource="http://xmlns.com/foaf/0.1/Person"/>
        <prov:actedOnBehalfOf rdf:resource="http://www.semanticweb.org/bbucher/ontologies/2025/9/geodata#geodata-paris"/>
        <foaf:family_name>Van Damme</foaf:family_name>
        <foaf:givenname>Marie-Dominique</foaf:givenname>
        <foaf:member rdf:resource="http://www.semanticweb.org/bbucher/ontologies/2025/9/geodata#geodata-paris"/>
        <foaf:name>Marie-Dominique Van Damme</foaf:name>
        <foaf:title>Mme.</foaf:title>
        <foaf:workInfoHomepage>https://www.umr-lastig.fr/mdvandamme/</foaf:workInfoHomepage>
    </owl:NamedIndividual>
    


    <!-- http://www.w3.org/ns/dcat -->


    <rdf:Description rdf:about="http://www.w3.org/ns/dcat">
        <dcat:hasCurrentVersion rdf:resource="http://www.w3.org/ns/dcat3"/>
        <dcat:hasVersion rdf:resource="http://www.w3.org/ns/dcat2"/>
        <dcat:hasVersion rdf:resource="http://www.w3.org/ns/dcat2014"/>
        <dcat:hasVersion rdf:resource="http://www.w3.org/ns/dcat3"/>
        <dcat:previousVersion rdf:resource="http://www.w3.org/ns/dcat2"/>
        <terms:created rdf:datatype="http://www.w3.org/2001/XMLSchema#date">2020-12-17</terms:created>
        <terms:modified rdf:datatype="http://www.w3.org/2001/XMLSchema#date">2020-11-30</terms:modified>
        <terms:modified rdf:datatype="http://www.w3.org/2001/XMLSchema#date">2021-03-09</terms:modified>
        <terms:modified rdf:datatype="http://www.w3.org/2001/XMLSchema#date">2021-04-08</terms:modified>
        <terms:modified rdf:datatype="http://www.w3.org/2001/XMLSchema#date">2021-06-23</terms:modified>
        <terms:modified rdf:datatype="http://www.w3.org/2001/XMLSchema#date">2021-09-27</terms:modified>
        <terms:modified rdf:datatype="http://www.w3.org/2001/XMLSchema#date">2022-03-22</terms:modified>
        <terms:modified rdf:datatype="http://www.w3.org/2001/XMLSchema#date">2022-05-23</terms:modified>
        <terms:modified rdf:datatype="http://www.w3.org/2001/XMLSchema#date">2023-01-05</terms:modified>
        <dcat:version>3</dcat:version>
    </rdf:Description>
    


    <!-- https://geodata-paris.fr -->


    <owl:NamedIndividual rdf:about="https://geodata-paris.fr"/>
    <rdf:Description>
        <rdf:type rdf:resource="http://xmlns.com/foaf/0.1/Person"/>
        <foaf:name>David Browning</foaf:name>
    </rdf:Description>
    <rdf:Description rdf:nodeID="genid93">
        <rdf:type rdf:resource="http://xmlns.com/foaf/0.1/Person"/>
        <foaf:homepage rdf:resource="https://jakub.klímek.com/"/>
        <rdfs:seeAlso rdf:resource="https://jakub.klímek.com/#me"/>
        <foaf:name>Jakub Klímek</foaf:name>
    </rdf:Description>
    <rdf:Description>
        <rdf:type rdf:resource="http://xmlns.com/foaf/0.1/Person"/>
        <foaf:name>Peter Winstanley</foaf:name>
    </rdf:Description>
    <rdf:Description rdf:nodeID="genid95">
        <rdf:type rdf:resource="http://www.w3.org/ns/org#Organization"/>
        <foaf:homepage rdf:resource="https://www.w3.org/"/>
        <rdfs:seeAlso rdf:resource="https://www.wikidata.org/entity/Q37033"/>
        <foaf:name>World Wide Web Consortium (W3C)</foaf:name>
    </rdf:Description>
    <rdf:Description rdf:nodeID="genid96">
        <rdf:type rdf:resource="http://xmlns.com/foaf/0.1/Person"/>
        <rdfs:seeAlso rdf:resource="https://orcid.org/0000-0002-3884-3420"/>
        <org:memberOf rdf:nodeID="genid97"/>
        <foaf:name>Simon J D Cox</foaf:name>
        <foaf:workInfoHomepage rdf:resource="http://people.csiro.au/Simon-Cox"/>
    </rdf:Description>
    <rdf:Description rdf:nodeID="genid97">
        <foaf:homepage rdf:resource="https://www.csiro.au"/>
        <foaf:name>Commonwealth Scientific and Industrial Research Organisation</foaf:name>
    </rdf:Description>
    <rdf:Description rdf:nodeID="genid98">
        <rdf:type rdf:resource="http://xmlns.com/foaf/0.1/Person"/>
        <rdfs:seeAlso rdf:resource="https://orcid.org/0000-0001-9300-2694"/>
        <foaf:name>Andrea Perego</foaf:name>
    </rdf:Description>
    <rdf:Description rdf:nodeID="genid99">
        <rdf:type rdf:resource="http://xmlns.com/foaf/0.1/Person"/>
        <foaf:homepage rdf:resource="https://w3id.org/people/ralbertoni/"/>
        <rdfs:seeAlso rdf:resource="https://orcid.org/0000-0001-5648-2713"/>
        <foaf:name>Riccardo Albertoni</foaf:name>
    </rdf:Description>
    <rdf:Description rdf:nodeID="genid100">
        <rdf:type rdf:resource="http://xmlns.com/foaf/0.1/Person"/>
        <foaf:homepage rdf:resource="https://agbeltran.github.io"/>
        <rdfs:seeAlso rdf:resource="https://orcid.org/0000-0003-3499-8262"/>
        <org:memberOf rdf:nodeID="genid101"/>
        <foaf:name>Alejandra Gonzalez-Beltran</foaf:name>
    </rdf:Description>
    <rdf:Description rdf:nodeID="genid101">
        <foaf:homepage rdf:resource="http://stfc.ac.uk"/>
        <foaf:name>Science and Technology Facilities Council, UK</foaf:name>
    </rdf:Description>
    <rdf:Description>
        <rdf:type rdf:resource="http://xmlns.com/foaf/0.1/Person"/>
        <foaf:name>Anna Odgaard Ingram</foaf:name>
    </rdf:Description>
    <rdf:Description rdf:nodeID="genid103">
        <rdf:type rdf:resource="http://xmlns.com/foaf/0.1/Person"/>
        <org:memberOf rdf:nodeID="genid104"/>
        <foaf:name>Vassilios Peristeras</foaf:name>
    </rdf:Description>
    <rdf:Description rdf:nodeID="genid104">
        <foaf:homepage rdf:resource="http://ec.europa.eu/dgs/informatics/"/>
        <foaf:name>European Commission, DG DIGIT</foaf:name>
    </rdf:Description>
    <rdf:Description rdf:nodeID="genid105">
        <rdf:type rdf:resource="http://xmlns.com/foaf/0.1/Person"/>
        <org:memberOf rdf:nodeID="genid106"/>
        <foaf:name>Fadi Maali</foaf:name>
    </rdf:Description>
    <rdf:Description rdf:nodeID="genid106">
        <foaf:homepage rdf:resource="http://www.deri.ie/"/>
        <foaf:name>DERI, NUI Galway</foaf:name>
    </rdf:Description>
    <rdf:Description rdf:nodeID="genid107">
        <rdf:type rdf:resource="http://xmlns.com/foaf/0.1/Person"/>
        <foaf:homepage rdf:resource="http://makxdekkers.com/"/>
        <rdfs:seeAlso rdf:resource="http://makxdekkers.com/makxdekkers.rdf#me"/>
        <foaf:name>Makx Dekkers</foaf:name>
    </rdf:Description>
    <rdf:Description rdf:nodeID="genid108">
        <rdf:type rdf:resource="http://xmlns.com/foaf/0.1/Person"/>
        <foaf:homepage rdf:resource="http://www.asahi-net.or.jp/~ax2s-kmtn/"/>
        <foaf:name>Shuji Kamitsuna</foaf:name>
    </rdf:Description>
    <rdf:Description rdf:nodeID="genid109">
        <rdf:type rdf:resource="http://xmlns.com/foaf/0.1/Person"/>
        <org:hasMembership rdf:nodeID="genid110"/>
        <foaf:family_name>Abadie</foaf:family_name>
        <foaf:firstName>Nathalie</foaf:firstName>
        <foaf:mbox rdf:resource="mailto:nathalie-f.abadie@ign.fr"/>
        <foaf:name>Nathalie Abadie</foaf:name>
        <foaf:workInfoHomepage rdf:resource="http://recherche.ign.fr/labos/cogit/cv.php?prenom=Nathalie&amp;nom=Abadie"/>
    </rdf:Description>
    <rdf:Description rdf:nodeID="genid110">
        <rdf:type rdf:resource="http://www.w3.org/ns/org#Membership"/>
        <org:memberDuring rdf:nodeID="genid111"/>
        <org:organization rdf:resource="http://recherche.ign.fr/"/>
        <org:organization rdf:resource="http://www.ign.fr/"/>
        <org:role rdf:nodeID="genid113"/>
    </rdf:Description>
    <rdf:Description rdf:nodeID="genid111">
        <rdf:type rdf:resource="http://www.w3.org/2006/time#Interval"/>
        <time:hasBeginning rdf:nodeID="genid112"/>
    </rdf:Description>
    <rdf:Description rdf:nodeID="genid113">
        <rdf:type rdf:resource="http://www.w3.org/ns/org#Role"/>
        <rdfs:label xml:lang="fr">Chargée de recherche</rdfs:label>
        <rdfs:label xml:lang="en">Survey engineer and Scientist</rdfs:label>
    </rdf:Description>
    <rdf:Description rdf:nodeID="genid112">
        <rdf:type rdf:resource="http://www.w3.org/2006/time#Instant"/>
        <time:inXSDDateTimeStamp rdf:datatype="http://www.w3.org/2001/XMLSchema#dateTimeStamp">2005-09-09</time:inXSDDateTimeStamp>
    </rdf:Description>
    <rdf:Description rdf:nodeID="genid114">
        <rdf:type rdf:resource="http://xmlns.com/foaf/0.1/Person"/>
        <org:hasMembership rdf:nodeID="genid115"/>
        <foaf:family_name>McGibbney</foaf:family_name>
        <foaf:firstName>Lewis J</foaf:firstName>
        <foaf:mbox rdf:resource="mailto:lewis.j.mcgibbney@jpl.nasa.gov"/>
        <foaf:name>Lewis John McGibbney</foaf:name>
    </rdf:Description>
    <rdf:Description rdf:nodeID="genid115">
        <rdf:type rdf:resource="http://www.w3.org/ns/org#Membership"/>
        <org:memberDuring rdf:nodeID="genid116"/>
        <org:organization rdf:resource="http://dbpedia.org/resource/JPL"/>
        <org:organization rdf:resource="https://www.jpl.nasa.gov"/>
        <org:role rdf:nodeID="genid118"/>
    </rdf:Description>
    <rdf:Description rdf:nodeID="genid116">
        <rdf:type rdf:resource="http://www.w3.org/2006/time#Interval"/>
        <time:hasBeginning rdf:nodeID="genid117"/>
    </rdf:Description>
    <rdf:Description rdf:nodeID="genid118">
        <rdf:type rdf:resource="http://www.w3.org/ns/org#Role"/>
        <rdfs:label>Data Scientist</rdfs:label>
    </rdf:Description>
    <rdf:Description rdf:nodeID="genid117">
        <rdf:type rdf:resource="http://www.w3.org/2006/time#Instant"/>
        <time:inXSDDateTimeStamp rdf:datatype="http://www.w3.org/2001/XMLSchema#dateTimeStamp">2014-04-01T00:00:00+08:00</time:inXSDDateTimeStamp>
    </rdf:Description>
    


    <!-- 
    ///////////////////////////////////////////////////////////////////////////////////////
    //
    // Annotations
    //
    ///////////////////////////////////////////////////////////////////////////////////////
     -->


    <rdf:Description rdf:about="http://purl.org/dc/terms/Agent">
        <rdfs:comment xml:lang="en">A resource that acts or has the power to act.</rdfs:comment>
        <rdfs:isDefinedBy rdf:resource="http://purl.org/dc/terms/"/>
        <rdfs:label xml:lang="en">Agent</rdfs:label>
    </rdf:Description>
    <rdf:Description rdf:about="http://purl.org/dc/terms/AgentClass">
        <rdfs:comment xml:lang="en">A group of agents.</rdfs:comment>
        <rdfs:isDefinedBy rdf:resource="http://purl.org/dc/terms/"/>
        <rdfs:label xml:lang="en">Agent Class</rdfs:label>
    </rdf:Description>
    <rdf:Description rdf:about="http://purl.org/dc/terms/BibliographicResource">
        <rdfs:comment xml:lang="en">A book, article, or other documentary resource.</rdfs:comment>
        <rdfs:isDefinedBy rdf:resource="http://purl.org/dc/terms/"/>
        <rdfs:label xml:lang="en">Bibliographic Resource</rdfs:label>
    </rdf:Description>
    <rdf:Description rdf:about="http://purl.org/dc/terms/Box">
        <rdfs:comment xml:lang="en">The set of regions in space defined by their geographic coordinates according to the DCMI Box Encoding Scheme.</rdfs:comment>
        <rdfs:isDefinedBy rdf:resource="http://purl.org/dc/terms/"/>
        <rdfs:label xml:lang="en">DCMI Box</rdfs:label>
        <rdfs:seeAlso rdf:resource="https://www.dublincore.org/specifications/dublin-core/dcmi-box/"/>
    </rdf:Description>
    <rdf:Description rdf:about="http://purl.org/dc/terms/FileFormat">
        <rdfs:comment xml:lang="en">A digital resource format.</rdfs:comment>
        <rdfs:isDefinedBy rdf:resource="http://purl.org/dc/terms/"/>
        <rdfs:label xml:lang="en">File Format</rdfs:label>
    </rdf:Description>
    <rdf:Description rdf:about="http://purl.org/dc/terms/Frequency">
        <rdfs:comment xml:lang="en">A rate at which something recurs.</rdfs:comment>
        <rdfs:isDefinedBy rdf:resource="http://purl.org/dc/terms/"/>
        <rdfs:label xml:lang="en">Frequency</rdfs:label>
    </rdf:Description>
    <rdf:Description rdf:about="http://purl.org/dc/terms/ISO3166">
        <rdfs:comment xml:lang="en">The set of codes listed in ISO 3166-1 for the representation of names of countries.</rdfs:comment>
        <rdfs:isDefinedBy rdf:resource="http://purl.org/dc/terms/"/>
        <rdfs:label xml:lang="en">ISO 3166</rdfs:label>
        <rdfs:seeAlso rdf:resource="https://www.iso.org/obp/ui/#search"/>
    </rdf:Description>
    <rdf:Description rdf:about="http://purl.org/dc/terms/ISO639-2">
        <rdfs:comment xml:lang="en">The three-letter alphabetic codes listed in ISO639-2 for the representation of names of languages.</rdfs:comment>
        <rdfs:isDefinedBy rdf:resource="http://purl.org/dc/terms/"/>
        <rdfs:label xml:lang="en">ISO 639-2</rdfs:label>
        <rdfs:seeAlso rdf:resource="http://lcweb.loc.gov/standards/iso639-2/langhome.html"/>
    </rdf:Description>
    <rdf:Description rdf:about="http://purl.org/dc/terms/ISO639-3">
        <rdfs:comment xml:lang="en">The set of three-letter codes listed in ISO 639-3 for the representation of names of languages.</rdfs:comment>
        <rdfs:isDefinedBy rdf:resource="http://purl.org/dc/terms/"/>
        <rdfs:label xml:lang="en">ISO 639-3</rdfs:label>
        <rdfs:seeAlso rdf:resource="http://www.sil.org/iso639-3/"/>
    </rdf:Description>
    <rdf:Description rdf:about="http://purl.org/dc/terms/Jurisdiction">
        <rdfs:comment xml:lang="en">The extent or range of judicial, law enforcement, or other authority.</rdfs:comment>
        <rdfs:isDefinedBy rdf:resource="http://purl.org/dc/terms/"/>
        <rdfs:label xml:lang="en">Jurisdiction</rdfs:label>
    </rdf:Description>
    <rdf:Description rdf:about="http://purl.org/dc/terms/LicenseDocument">
        <rdfs:comment xml:lang="en">A legal document giving official permission to do something with a resource.</rdfs:comment>
        <rdfs:isDefinedBy rdf:resource="http://purl.org/dc/terms/"/>
        <rdfs:label xml:lang="en">License Document</rdfs:label>
    </rdf:Description>
    <rdf:Description rdf:about="http://purl.org/dc/terms/LinguisticSystem">
        <terms:description xml:lang="en">Written, spoken, sign, and computer languages are linguistic systems.</terms:description>
        <rdfs:comment xml:lang="en">A system of signs, symbols, sounds, gestures, or rules used in communication.</rdfs:comment>
        <rdfs:isDefinedBy rdf:resource="http://purl.org/dc/terms/"/>
        <rdfs:label xml:lang="en">Linguistic System</rdfs:label>
    </rdf:Description>
    <rdf:Description rdf:about="http://purl.org/dc/terms/Location">
        <rdfs:comment xml:lang="en">A spatial region or named place.</rdfs:comment>
        <rdfs:isDefinedBy rdf:resource="http://purl.org/dc/terms/"/>
        <rdfs:label xml:lang="en">Location</rdfs:label>
    </rdf:Description>
    <rdf:Description rdf:about="http://purl.org/dc/terms/LocationPeriodOrJurisdiction">
        <rdfs:comment xml:lang="en">A location, period of time, or jurisdiction.</rdfs:comment>
        <rdfs:isDefinedBy rdf:resource="http://purl.org/dc/terms/"/>
        <rdfs:label xml:lang="en">Location, Period, or Jurisdiction</rdfs:label>
    </rdf:Description>
    <rdf:Description rdf:about="http://purl.org/dc/terms/MediaType">
        <rdfs:comment xml:lang="en">A file format or physical medium.</rdfs:comment>
        <rdfs:isDefinedBy rdf:resource="http://purl.org/dc/terms/"/>
        <rdfs:label xml:lang="en">Media Type</rdfs:label>
    </rdf:Description>
    <rdf:Description rdf:about="http://purl.org/dc/terms/MediaTypeOrExtent">
        <rdfs:comment xml:lang="en">A media type or extent.</rdfs:comment>
        <rdfs:isDefinedBy rdf:resource="http://purl.org/dc/terms/"/>
        <rdfs:label xml:lang="en">Media Type or Extent</rdfs:label>
    </rdf:Description>
    <rdf:Description rdf:about="http://purl.org/dc/terms/MethodOfAccrual">
        <rdfs:comment xml:lang="en">A method by which resources are added to a collection.</rdfs:comment>
        <rdfs:isDefinedBy rdf:resource="http://purl.org/dc/terms/"/>
        <rdfs:label xml:lang="en">Method of Accrual</rdfs:label>
    </rdf:Description>
    <rdf:Description rdf:about="http://purl.org/dc/terms/MethodOfInstruction">
        <rdfs:comment xml:lang="en">A process that is used to engender knowledge, attitudes, and skills.</rdfs:comment>
        <rdfs:isDefinedBy rdf:resource="http://purl.org/dc/terms/"/>
        <rdfs:label xml:lang="en">Method of Instruction</rdfs:label>
    </rdf:Description>
    <rdf:Description rdf:about="http://purl.org/dc/terms/Period">
        <rdfs:comment xml:lang="en">The set of time intervals defined by their limits according to the DCMI Period Encoding Scheme.</rdfs:comment>
        <rdfs:isDefinedBy rdf:resource="http://purl.org/dc/terms/"/>
        <rdfs:label xml:lang="en">DCMI Period</rdfs:label>
        <rdfs:seeAlso rdf:resource="https://www.dublincore.org/specifications/dublin-core/dcmi-period/"/>
    </rdf:Description>
    <rdf:Description rdf:about="http://purl.org/dc/terms/PeriodOfTime">
        <rdfs:comment xml:lang="en">An interval of time that is named or defined by its start and end dates.</rdfs:comment>
        <rdfs:isDefinedBy rdf:resource="http://purl.org/dc/terms/"/>
        <rdfs:label xml:lang="en">Period of Time</rdfs:label>
    </rdf:Description>
    <rdf:Description rdf:about="http://purl.org/dc/terms/PhysicalMedium">
        <terms:description xml:lang="en">Examples include paper, canvas, or DVD.</terms:description>
        <rdfs:comment xml:lang="en">A physical material or carrier.</rdfs:comment>
        <rdfs:isDefinedBy rdf:resource="http://purl.org/dc/terms/"/>
        <rdfs:label xml:lang="en">Physical Medium</rdfs:label>
    </rdf:Description>
    <rdf:Description rdf:about="http://purl.org/dc/terms/PhysicalResource">
        <rdfs:comment xml:lang="en">A material thing.</rdfs:comment>
        <rdfs:isDefinedBy rdf:resource="http://purl.org/dc/terms/"/>
        <rdfs:label xml:lang="en">Physical Resource</rdfs:label>
    </rdf:Description>
    <rdf:Description rdf:about="http://purl.org/dc/terms/Point">
        <rdfs:comment xml:lang="en">The set of points in space defined by their geographic coordinates according to the DCMI Point Encoding Scheme.</rdfs:comment>
        <rdfs:isDefinedBy rdf:resource="http://purl.org/dc/terms/"/>
        <rdfs:label xml:lang="en">DCMI Point</rdfs:label>
        <rdfs:seeAlso rdf:resource="https://www.dublincore.org/specifications/dublin-core/dcmi-point/"/>
    </rdf:Description>
    <rdf:Description rdf:about="http://purl.org/dc/terms/Policy">
        <rdfs:comment xml:lang="en">A plan or course of action by an authority, intended to influence and determine decisions, actions, and other matters.</rdfs:comment>
        <rdfs:isDefinedBy rdf:resource="http://purl.org/dc/terms/"/>
        <rdfs:label xml:lang="en">Policy</rdfs:label>
    </rdf:Description>
    <rdf:Description rdf:about="http://purl.org/dc/terms/ProvenanceStatement">
        <rdfs:comment xml:lang="en">Any changes in ownership and custody of a resource since its creation that are significant for its authenticity, integrity, and interpretation.</rdfs:comment>
        <rdfs:isDefinedBy rdf:resource="http://purl.org/dc/terms/"/>
        <rdfs:label xml:lang="en">Provenance Statement</rdfs:label>
    </rdf:Description>
    <rdf:Description rdf:about="http://purl.org/dc/terms/RFC1766">
        <rdfs:comment xml:lang="en">The set of tags, constructed according to RFC 1766, for the identification of languages.</rdfs:comment>
        <rdfs:isDefinedBy rdf:resource="http://purl.org/dc/terms/"/>
        <rdfs:label xml:lang="en">RFC 1766</rdfs:label>
        <rdfs:seeAlso rdf:resource="http://www.ietf.org/rfc/rfc1766.txt"/>
    </rdf:Description>
    <rdf:Description rdf:about="http://purl.org/dc/terms/RFC3066">
        <terms:description xml:lang="en">RFC 3066 has been obsoleted by RFC 4646.</terms:description>
        <rdfs:comment xml:lang="en">The set of tags constructed according to RFC 3066 for the identification of languages.</rdfs:comment>
        <rdfs:isDefinedBy rdf:resource="http://purl.org/dc/terms/"/>
        <rdfs:label xml:lang="en">RFC 3066</rdfs:label>
        <rdfs:seeAlso rdf:resource="http://www.ietf.org/rfc/rfc3066.txt"/>
    </rdf:Description>
    <rdf:Description rdf:about="http://purl.org/dc/terms/RFC4646">
        <terms:description xml:lang="en">RFC 4646 obsoletes RFC 3066.</terms:description>
        <rdfs:comment xml:lang="en">The set of tags constructed according to RFC 4646 for the identification of languages.</rdfs:comment>
        <rdfs:isDefinedBy rdf:resource="http://purl.org/dc/terms/"/>
        <rdfs:label xml:lang="en">RFC 4646</rdfs:label>
        <rdfs:seeAlso rdf:resource="http://www.ietf.org/rfc/rfc4646.txt"/>
    </rdf:Description>
    <rdf:Description rdf:about="http://purl.org/dc/terms/RFC5646">
        <terms:description xml:lang="en">RFC 5646 obsoletes RFC 4646.</terms:description>
        <rdfs:comment xml:lang="en">The set of tags constructed according to RFC 5646 for the identification of languages.</rdfs:comment>
        <rdfs:isDefinedBy rdf:resource="http://purl.org/dc/terms/"/>
        <rdfs:label xml:lang="en">RFC 5646</rdfs:label>
        <rdfs:seeAlso rdf:resource="http://www.ietf.org/rfc/rfc5646.txt"/>
    </rdf:Description>
    <rdf:Description rdf:about="http://purl.org/dc/terms/RightsStatement">
        <rdfs:comment xml:lang="en">A statement about the intellectual property rights (IPR) held in or over a resource, a legal document giving official permission to do something with a resource, or a statement about access rights.</rdfs:comment>
        <rdfs:isDefinedBy rdf:resource="http://purl.org/dc/terms/"/>
        <rdfs:label xml:lang="en">Rights Statement</rdfs:label>
    </rdf:Description>
    <rdf:Description rdf:about="http://purl.org/dc/terms/SizeOrDuration">
        <terms:description xml:lang="en">Examples include a number of pages, a specification of length, width, and breadth, or a period in hours, minutes, and seconds.</terms:description>
        <rdfs:comment xml:lang="en">A dimension or extent, or a time taken to play or execute.</rdfs:comment>
        <rdfs:isDefinedBy rdf:resource="http://purl.org/dc/terms/"/>
        <rdfs:label xml:lang="en">Size or Duration</rdfs:label>
    </rdf:Description>
    <rdf:Description rdf:about="http://purl.org/dc/terms/Standard">
        <rdfs:comment xml:lang="en">A reference point against which other things can be evaluated or compared.</rdfs:comment>
        <rdfs:isDefinedBy rdf:resource="http://purl.org/dc/terms/"/>
        <rdfs:label xml:lang="en">Standard</rdfs:label>
    </rdf:Description>
    <rdf:Description rdf:about="http://purl.org/dc/terms/URI">
        <rdfs:comment xml:lang="en">The set of identifiers constructed according to the generic syntax for Uniform Resource Identifiers as specified by the Internet Engineering Task Force.</rdfs:comment>
        <rdfs:isDefinedBy rdf:resource="http://purl.org/dc/terms/"/>
        <rdfs:label xml:lang="en">URI</rdfs:label>
        <rdfs:seeAlso rdf:resource="http://www.ietf.org/rfc/rfc3986.txt"/>
    </rdf:Description>
    <rdf:Description rdf:about="http://purl.org/dc/terms/W3CDTF">
        <rdfs:comment xml:lang="en">The set of dates and times constructed according to the W3C Date and Time Formats Specification.</rdfs:comment>
        <rdfs:isDefinedBy rdf:resource="http://purl.org/dc/terms/"/>
        <rdfs:label xml:lang="en">W3C-DTF</rdfs:label>
        <rdfs:seeAlso rdf:resource="http://www.w3.org/TR/NOTE-datetime"/>
    </rdf:Description>
    <rdf:Description rdf:about="http://purl.org/dc/terms/abstract">
        <rdfs:comment xml:lang="en">A summary of the resource.</rdfs:comment>
        <rdfs:isDefinedBy rdf:resource="http://purl.org/dc/terms/"/>
        <rdfs:label xml:lang="en">Abstract</rdfs:label>
    </rdf:Description>
    <rdf:Description rdf:about="http://purl.org/dc/terms/accessRights">
        <dcam:rangeIncludes rdf:resource="http://purl.org/dc/terms/RightsStatement"/>
        <terms:description xml:lang="en">Access Rights may include information regarding access or restrictions based on privacy, security, or other policies.</terms:description>
        <rdfs:comment xml:lang="en">Information about who access the resource or an indication of its security status.</rdfs:comment>
        <rdfs:isDefinedBy rdf:resource="http://purl.org/dc/terms/"/>
        <rdfs:label xml:lang="en">Access Rights</rdfs:label>
    </rdf:Description>
    <rdf:Description rdf:about="http://purl.org/dc/terms/accrualMethod">
        <dcam:rangeIncludes rdf:resource="http://purl.org/dc/terms/MethodOfAccrual"/>
        <terms:description xml:lang="en">Recommended practice is to use a value from the Collection Description Accrual Method Vocabulary [[DCMI-ACCRUALMETHOD](https://dublincore.org/groups/collections/accrual-method/)].</terms:description>
        <rdfs:comment xml:lang="en">The method by which items are added to a collection.</rdfs:comment>
        <rdfs:isDefinedBy rdf:resource="http://purl.org/dc/terms/"/>
        <rdfs:label xml:lang="en">Accrual Method</rdfs:label>
    </rdf:Description>
    <rdf:Description rdf:about="http://purl.org/dc/terms/accrualPeriodicity">
        <dcam:rangeIncludes rdf:resource="http://purl.org/dc/terms/Frequency"/>
        <terms:description xml:lang="en">Recommended practice is to use a value from the Collection Description Frequency Vocabulary [[DCMI-COLLFREQ](https://dublincore.org/groups/collections/frequency/)].</terms:description>
        <rdfs:comment xml:lang="en">The frequency with which items are added to a collection.</rdfs:comment>
        <rdfs:isDefinedBy rdf:resource="http://purl.org/dc/terms/"/>
        <rdfs:label xml:lang="en">Accrual Periodicity</rdfs:label>
    </rdf:Description>
    <rdf:Description rdf:about="http://purl.org/dc/terms/accrualPolicy">
        <dcam:rangeIncludes rdf:resource="http://purl.org/dc/terms/Policy"/>
        <terms:description xml:lang="en">Recommended practice is to use a value from the Collection Description Accrual Policy Vocabulary [[DCMI-ACCRUALPOLICY](https://dublincore.org/groups/collections/accrual-policy/)].</terms:description>
        <rdfs:comment xml:lang="en">The policy governing the addition of items to a collection.</rdfs:comment>
        <rdfs:isDefinedBy rdf:resource="http://purl.org/dc/terms/"/>
        <rdfs:label xml:lang="en">Accrual Policy</rdfs:label>
    </rdf:Description>
    <rdf:Description rdf:about="http://purl.org/dc/terms/alternative">
        <terms:description xml:lang="en">The distinction between titles and alternative titles is application-specific.</terms:description>
        <rdfs:comment xml:lang="en">An alternative name for the resource.</rdfs:comment>
        <rdfs:isDefinedBy rdf:resource="http://purl.org/dc/terms/"/>
        <rdfs:label xml:lang="en">Alternative Title</rdfs:label>
    </rdf:Description>
    <rdf:Description rdf:about="http://purl.org/dc/terms/audience">
        <dcam:rangeIncludes rdf:resource="http://purl.org/dc/terms/AgentClass"/>
        <terms:description xml:lang="en">Recommended practice is to use this property with non-literal values from a vocabulary of audience types.</terms:description>
        <rdfs:comment xml:lang="en">A class of agents for whom the resource is intended or useful.</rdfs:comment>
        <rdfs:isDefinedBy rdf:resource="http://purl.org/dc/terms/"/>
        <rdfs:label xml:lang="en">Audience</rdfs:label>
    </rdf:Description>
    <rdf:Description rdf:about="http://purl.org/dc/terms/available">
        <terms:description xml:lang="en">Recommended practice is to describe the date, date/time, or period of time as recommended for the property Date, of which this is a subproperty.</terms:description>
        <rdfs:comment xml:lang="en">Date that the resource became or will become available.</rdfs:comment>
        <rdfs:isDefinedBy rdf:resource="http://purl.org/dc/terms/"/>
        <rdfs:label xml:lang="en">Date Available</rdfs:label>
    </rdf:Description>
    <rdf:Description rdf:about="http://purl.org/dc/terms/bibliographicCitation">
        <terms:description xml:lang="en">Recommended practice is to include sufficient bibliographic detail to identify the resource as unambiguously as possible.</terms:description>
        <rdfs:comment xml:lang="en">A bibliographic reference for the resource.</rdfs:comment>
        <rdfs:isDefinedBy rdf:resource="http://purl.org/dc/terms/"/>
        <rdfs:label xml:lang="en">Bibliographic Citation</rdfs:label>
    </rdf:Description>
    <rdf:Description rdf:about="http://purl.org/dc/terms/conformsTo">
        <dcam:rangeIncludes rdf:resource="http://purl.org/dc/terms/Standard"/>
        <rdfs:comment xml:lang="en">An established standard to which the described resource conforms.</rdfs:comment>
        <rdfs:isDefinedBy rdf:resource="http://purl.org/dc/terms/"/>
        <rdfs:label xml:lang="en">Conforms To</rdfs:label>
    </rdf:Description>
    <rdf:Description rdf:about="http://purl.org/dc/terms/contributor">
        <dcam:rangeIncludes rdf:resource="http://purl.org/dc/terms/Agent"/>
        <terms:description xml:lang="en">The guidelines for using names of persons or organizations as creators apply to contributors.</terms:description>
        <rdfs:comment xml:lang="en">An entity responsible for making contributions to the resource.</rdfs:comment>
        <rdfs:isDefinedBy rdf:resource="http://purl.org/dc/terms/"/>
        <rdfs:label xml:lang="en">Contributor</rdfs:label>
    </rdf:Description>
    <rdf:Description rdf:about="http://purl.org/dc/terms/coverage">
        <dcam:rangeIncludes rdf:resource="http://purl.org/dc/terms/Jurisdiction"/>
        <dcam:rangeIncludes rdf:resource="http://purl.org/dc/terms/Location"/>
        <dcam:rangeIncludes rdf:resource="http://purl.org/dc/terms/Period"/>
        <terms:description xml:lang="en">Spatial topic and spatial applicability may be a named place or a location specified by its geographic coordinates. Temporal topic may be a named period, date, or date range. A jurisdiction may be a named administrative entity or a geographic place to which the resource applies. Recommended practice is to use a controlled vocabulary such as the Getty Thesaurus of Geographic Names [[TGN](https://www.getty.edu/research/tools/vocabulary/tgn/index.html)]. Where appropriate, named places or time periods may be used in preference to numeric identifiers such as sets of coordinates or date ranges.  Because coverage is so broadly defined, it is preferable to use the more specific subproperties Temporal Coverage and Spatial Coverage.</terms:description>
        <rdfs:comment xml:lang="en">The spatial or temporal topic of the resource, spatial applicability of the resource, or jurisdiction under which the resource is relevant.</rdfs:comment>
        <rdfs:isDefinedBy rdf:resource="http://purl.org/dc/terms/"/>
        <rdfs:label xml:lang="en">Coverage</rdfs:label>
    </rdf:Description>
    <rdf:Description rdf:about="http://purl.org/dc/terms/created">
        <terms:description xml:lang="en">Recommended practice is to describe the date, date/time, or period of time as recommended for the property Date, of which this is a subproperty.</terms:description>
        <rdfs:comment xml:lang="en">Date of creation of the resource.</rdfs:comment>
        <rdfs:isDefinedBy rdf:resource="http://purl.org/dc/terms/"/>
        <rdfs:label xml:lang="en">Date Created</rdfs:label>
    </rdf:Description>
    <rdf:Description rdf:about="http://purl.org/dc/terms/creator">
        <dcam:rangeIncludes rdf:resource="http://purl.org/dc/terms/Agent"/>
        <terms:description xml:lang="en">Recommended practice is to identify the creator with a URI.  If this is not possible or feasible, a literal value that identifies the creator may be provided.</terms:description>
        <rdfs:comment xml:lang="en">An entity responsible for making the resource.</rdfs:comment>
        <rdfs:isDefinedBy rdf:resource="http://purl.org/dc/terms/"/>
        <rdfs:label xml:lang="en">Creator</rdfs:label>
    </rdf:Description>
    <rdf:Description rdf:about="http://purl.org/dc/terms/date">
        <terms:description xml:lang="en">Date may be used to express temporal information at any level of granularity.  Recommended practice is to express the date, date/time, or period of time according to ISO 8601-1 [[ISO 8601-1](https://www.iso.org/iso-8601-date-and-time-format.html)] or a published profile of the ISO standard, such as the W3C Note on Date and Time Formats [[W3CDTF](https://www.w3.org/TR/NOTE-datetime)] or the Extended Date/Time Format Specification [[EDTF](http://www.loc.gov/standards/datetime/)].  If the full date is unknown, month and year (YYYY-MM) or just year (YYYY) may be used. Date ranges may be specified using ISO 8601 period of time specification in which start and end dates are separated by a &apos;/&apos; (slash) character.  Either the start or end date may be missing.</terms:description>
        <rdfs:comment xml:lang="en">A point or period of time associated with an event in the lifecycle of the resource.</rdfs:comment>
        <rdfs:isDefinedBy rdf:resource="http://purl.org/dc/terms/"/>
        <rdfs:label xml:lang="en">Date</rdfs:label>
    </rdf:Description>
    <rdf:Description rdf:about="http://purl.org/dc/terms/dateAccepted">
        <terms:description xml:lang="en">Recommended practice is to describe the date, date/time, or period of time as recommended for the property Date, of which this is a subproperty.  Examples of resources to which a date of acceptance may be relevant are a thesis (accepted by a university department) or an article (accepted by a journal).</terms:description>
        <rdfs:comment xml:lang="en">Date of acceptance of the resource.</rdfs:comment>
        <rdfs:isDefinedBy rdf:resource="http://purl.org/dc/terms/"/>
        <rdfs:label xml:lang="en">Date Accepted</rdfs:label>
    </rdf:Description>
    <rdf:Description rdf:about="http://purl.org/dc/terms/dateCopyrighted">
        <terms:description xml:lang="en">Typically a year.  Recommended practice is to describe the date, date/time, or period of time as recommended for the property Date, of which this is a subproperty.</terms:description>
        <rdfs:comment xml:lang="en">Date of copyright of the resource.</rdfs:comment>
        <rdfs:isDefinedBy rdf:resource="http://purl.org/dc/terms/"/>
        <rdfs:label xml:lang="en">Date Copyrighted</rdfs:label>
    </rdf:Description>
    <rdf:Description rdf:about="http://purl.org/dc/terms/dateSubmitted">
        <terms:description xml:lang="en">Recommended practice is to describe the date, date/time, or period of time as recommended for the property Date, of which this is a subproperty.  Examples of resources to which a &apos;Date Submitted&apos; may be relevant include a thesis (submitted to a university department) or an article (submitted to a journal).</terms:description>
        <rdfs:comment xml:lang="en">Date of submission of the resource.</rdfs:comment>
        <rdfs:isDefinedBy rdf:resource="http://purl.org/dc/terms/"/>
        <rdfs:label xml:lang="en">Date Submitted</rdfs:label>
    </rdf:Description>
    <rdf:Description rdf:about="http://purl.org/dc/terms/description">
        <terms:description xml:lang="en">Description may include but is not limited to: an abstract, a table of contents, a graphical representation, or a free-text account of the resource.</terms:description>
        <rdfs:comment xml:lang="en">An account of the resource.</rdfs:comment>
        <rdfs:isDefinedBy rdf:resource="http://purl.org/dc/terms/"/>
        <rdfs:label xml:lang="en">Description</rdfs:label>
    </rdf:Description>
    <rdf:Description rdf:about="http://purl.org/dc/terms/educationLevel">
        <dcam:rangeIncludes rdf:resource="http://purl.org/dc/terms/AgentClass"/>
        <rdfs:comment xml:lang="en">A class of agents, defined in terms of progression through an educational or training context, for which the described resource is intended.</rdfs:comment>
        <rdfs:isDefinedBy rdf:resource="http://purl.org/dc/terms/"/>
        <rdfs:label xml:lang="en">Audience Education Level</rdfs:label>
    </rdf:Description>
    <rdf:Description rdf:about="http://purl.org/dc/terms/extent">
        <dcam:rangeIncludes rdf:resource="http://purl.org/dc/terms/SizeOrDuration"/>
        <terms:description xml:lang="en">Recommended practice is to specify the file size in megabytes and duration in ISO 8601 format.</terms:description>
        <rdfs:comment xml:lang="en">The size or duration of the resource.</rdfs:comment>
        <rdfs:isDefinedBy rdf:resource="http://purl.org/dc/terms/"/>
        <rdfs:label xml:lang="en">Extent</rdfs:label>
    </rdf:Description>
    <rdf:Description rdf:about="http://purl.org/dc/terms/format">
        <dcam:rangeIncludes rdf:resource="http://purl.org/dc/terms/Extent"/>
        <dcam:rangeIncludes rdf:resource="http://purl.org/dc/terms/MediaType"/>
        <terms:description xml:lang="en">Recommended practice is to use a controlled vocabulary where available. For example, for file formats one could use the list of Internet Media Types [[MIME](https://www.iana.org/assignments/media-types/media-types.xhtml)].  Examples of dimensions include size and duration.</terms:description>
        <rdfs:comment xml:lang="en">The file format, physical medium, or dimensions of the resource.</rdfs:comment>
        <rdfs:isDefinedBy rdf:resource="http://purl.org/dc/terms/"/>
        <rdfs:label xml:lang="en">Format</rdfs:label>
    </rdf:Description>
    <rdf:Description rdf:about="http://purl.org/dc/terms/hasFormat">
        <terms:description xml:lang="en">This property is intended to be used with non-literal values. This property is an inverse property of Is Format Of.</terms:description>
        <rdfs:comment xml:lang="en">A related resource that is substantially the same as the pre-existing described resource, but in another format.</rdfs:comment>
        <rdfs:isDefinedBy rdf:resource="http://purl.org/dc/terms/"/>
        <rdfs:label xml:lang="en">Has Format</rdfs:label>
    </rdf:Description>
    <rdf:Description rdf:about="http://purl.org/dc/terms/hasPart">
        <terms:description xml:lang="en">This property is intended to be used with non-literal values. This property is an inverse property of Is Part Of.</terms:description>
        <rdfs:comment xml:lang="en">A related resource that is included either physically or logically in the described resource.</rdfs:comment>
        <rdfs:isDefinedBy rdf:resource="http://purl.org/dc/terms/"/>
        <rdfs:label xml:lang="en">Has Part</rdfs:label>
    </rdf:Description>
    <rdf:Description rdf:about="http://purl.org/dc/terms/hasVersion">
        <terms:description xml:lang="en">Changes in version imply substantive changes in content rather than differences in format. This property is intended to be used with non-literal values. This property is an inverse property of Is Version Of.</terms:description>
        <rdfs:comment xml:lang="en">A related resource that is a version, edition, or adaptation of the described resource.</rdfs:comment>
        <rdfs:isDefinedBy rdf:resource="http://purl.org/dc/terms/"/>
        <rdfs:label xml:lang="en">Has Version</rdfs:label>
    </rdf:Description>
    <rdf:Description rdf:about="http://purl.org/dc/terms/identifier">
        <terms:description xml:lang="en">Recommended practice is to identify the resource by means of a string conforming to an identification system. Examples include International Standard Book Number (ISBN), Digital Object Identifier (DOI), and Uniform Resource Name (URN).  Persistent identifiers should be provided as HTTP URIs.</terms:description>
        <rdfs:comment xml:lang="en">An unambiguous reference to the resource within a given context.</rdfs:comment>
        <rdfs:isDefinedBy rdf:resource="http://purl.org/dc/terms/"/>
        <rdfs:label xml:lang="en">Identifier</rdfs:label>
    </rdf:Description>
    <rdf:Description rdf:about="http://purl.org/dc/terms/isFormatOf">
        <terms:description xml:lang="en">This property is intended to be used with non-literal values. This property is an inverse property of Has Format.</terms:description>
        <rdfs:comment xml:lang="en">A pre-existing related resource that is substantially the same as the described resource, but in another format.</rdfs:comment>
        <rdfs:isDefinedBy rdf:resource="http://purl.org/dc/terms/"/>
        <rdfs:label xml:lang="en">Is Format Of</rdfs:label>
    </rdf:Description>
    <rdf:Description rdf:about="http://purl.org/dc/terms/isPartOf">
        <terms:description xml:lang="en">This property is intended to be used with non-literal values. This property is an inverse property of Has Part.</terms:description>
        <rdfs:comment xml:lang="en">A related resource in which the described resource is physically or logically included.</rdfs:comment>
        <rdfs:isDefinedBy rdf:resource="http://purl.org/dc/terms/"/>
        <rdfs:label xml:lang="en">Is Part Of</rdfs:label>
    </rdf:Description>
    <rdf:Description rdf:about="http://purl.org/dc/terms/isReferencedBy">
        <terms:description xml:lang="en">This property is intended to be used with non-literal values. This property is an inverse property of References.</terms:description>
        <rdfs:comment xml:lang="en">A related resource that references, cites, or otherwise points to the described resource.</rdfs:comment>
        <rdfs:isDefinedBy rdf:resource="http://purl.org/dc/terms/"/>
        <rdfs:label xml:lang="en">Is Referenced By</rdfs:label>
    </rdf:Description>
    <rdf:Description rdf:about="http://purl.org/dc/terms/isReplacedBy">
        <terms:description xml:lang="en">This property is intended to be used with non-literal values. This property is an inverse property of Replaces.</terms:description>
        <rdfs:comment xml:lang="en">A related resource that supplants, displaces, or supersedes the described resource.</rdfs:comment>
        <rdfs:isDefinedBy rdf:resource="http://purl.org/dc/terms/"/>
        <rdfs:label xml:lang="en">Is Replaced By</rdfs:label>
    </rdf:Description>
    <rdf:Description rdf:about="http://purl.org/dc/terms/isRequiredBy">
        <terms:description xml:lang="en">This property is intended to be used with non-literal values. This property is an inverse property of Requires.</terms:description>
        <rdfs:comment xml:lang="en">A related resource that requires the described resource to support its function, delivery, or coherence.</rdfs:comment>
        <rdfs:isDefinedBy rdf:resource="http://purl.org/dc/terms/"/>
        <rdfs:label xml:lang="en">Is Required By</rdfs:label>
    </rdf:Description>
    <rdf:Description rdf:about="http://purl.org/dc/terms/isVersionOf">
        <terms:description xml:lang="en">Changes in version imply substantive changes in content rather than differences in format. This property is intended to be used with non-literal values. This property is an inverse property of Has Version.</terms:description>
        <rdfs:comment xml:lang="en">A related resource of which the described resource is a version, edition, or adaptation.</rdfs:comment>
        <rdfs:isDefinedBy rdf:resource="http://purl.org/dc/terms/"/>
        <rdfs:label xml:lang="en">Is Version Of</rdfs:label>
    </rdf:Description>
    <rdf:Description rdf:about="http://purl.org/dc/terms/issued">
        <terms:description xml:lang="en">Recommended practice is to describe the date, date/time, or period of time as recommended for the property Date, of which this is a subproperty.</terms:description>
        <rdfs:comment xml:lang="en">Date of formal issuance of the resource.</rdfs:comment>
        <rdfs:isDefinedBy rdf:resource="http://purl.org/dc/terms/"/>
        <rdfs:label xml:lang="en">Date Issued</rdfs:label>
    </rdf:Description>
    <rdf:Description rdf:about="http://purl.org/dc/terms/language">
        <dcam:rangeIncludes rdf:resource="http://purl.org/dc/terms/LinguisticSystem"/>
        <terms:description xml:lang="en">Recommended practice is to use either a non-literal value representing a language from a controlled vocabulary such as ISO 639-2 or ISO 639-3, or a literal value consisting of an IETF Best Current Practice 47 [[IETF-BCP47](https://tools.ietf.org/html/bcp47)] language tag.</terms:description>
        <rdfs:comment xml:lang="en">A language of the resource.</rdfs:comment>
        <rdfs:isDefinedBy rdf:resource="http://purl.org/dc/terms/"/>
        <rdfs:label xml:lang="en">Language</rdfs:label>
    </rdf:Description>
    <rdf:Description rdf:about="http://purl.org/dc/terms/license">
        <dcam:rangeIncludes rdf:resource="http://purl.org/dc/terms/LicenseDocument"/>
        <terms:description xml:lang="en">Recommended practice is to identify the license document with a URI. If this is not possible or feasible, a literal value that identifies the license may be provided.</terms:description>
        <rdfs:comment xml:lang="en">A legal document giving official permission to do something with the resource.</rdfs:comment>
        <rdfs:isDefinedBy rdf:resource="http://purl.org/dc/terms/"/>
        <rdfs:label xml:lang="en">License</rdfs:label>
    </rdf:Description>
    <rdf:Description rdf:about="http://purl.org/dc/terms/mediator">
        <dcam:rangeIncludes rdf:resource="http://purl.org/dc/terms/AgentClass"/>
        <terms:description xml:lang="en">In an educational context, a mediator might be a parent, teacher, teaching assistant, or care-giver.</terms:description>
        <rdfs:comment xml:lang="en">An entity that mediates access to the resource.</rdfs:comment>
        <rdfs:isDefinedBy rdf:resource="http://purl.org/dc/terms/"/>
        <rdfs:label xml:lang="en">Mediator</rdfs:label>
    </rdf:Description>
    <rdf:Description rdf:about="http://purl.org/dc/terms/medium">
        <dcam:domainIncludes rdf:resource="http://purl.org/dc/terms/PhysicalResource"/>
        <dcam:rangeIncludes rdf:resource="http://purl.org/dc/terms/PhysicalMedium"/>
        <rdfs:comment xml:lang="en">The material or physical carrier of the resource.</rdfs:comment>
        <rdfs:isDefinedBy rdf:resource="http://purl.org/dc/terms/"/>
        <rdfs:label xml:lang="en">Medium</rdfs:label>
    </rdf:Description>
    <rdf:Description rdf:about="http://purl.org/dc/terms/modified">
        <terms:description xml:lang="en">Recommended practice is to describe the date, date/time, or period of time as recommended for the property Date, of which this is a subproperty.</terms:description>
        <rdfs:comment xml:lang="en">Date on which the resource was changed.</rdfs:comment>
        <rdfs:isDefinedBy rdf:resource="http://purl.org/dc/terms/"/>
        <rdfs:label xml:lang="en">Date Modified</rdfs:label>
    </rdf:Description>
    <rdf:Description rdf:about="http://purl.org/dc/terms/publisher">
        <dcam:rangeIncludes rdf:resource="http://purl.org/dc/terms/Agent"/>
        <rdfs:comment xml:lang="en">An entity responsible for making the resource available.</rdfs:comment>
        <rdfs:isDefinedBy rdf:resource="http://purl.org/dc/terms/"/>
        <rdfs:label xml:lang="en">Publisher</rdfs:label>
    </rdf:Description>
    <rdf:Description rdf:about="http://purl.org/dc/terms/references">
        <terms:description xml:lang="en">This property is intended to be used with non-literal values. This property is an inverse property of Is Referenced By.</terms:description>
        <rdfs:comment xml:lang="en">A related resource that is referenced, cited, or otherwise pointed to by the described resource.</rdfs:comment>
        <rdfs:isDefinedBy rdf:resource="http://purl.org/dc/terms/"/>
        <rdfs:label xml:lang="en">References</rdfs:label>
    </rdf:Description>
    <rdf:Description rdf:about="http://purl.org/dc/terms/relation">
        <terms:description xml:lang="en">Recommended practice is to identify the related resource by means of a URI.  If this is not possible or feasible, a string conforming to a formal identification system may be provided.</terms:description>
        <rdfs:comment xml:lang="en">A related resource.</rdfs:comment>
        <rdfs:isDefinedBy rdf:resource="http://purl.org/dc/terms/"/>
        <rdfs:label xml:lang="en">Relation</rdfs:label>
    </rdf:Description>
    <rdf:Description rdf:about="http://purl.org/dc/terms/replaces">
        <terms:description xml:lang="en">This property is intended to be used with non-literal values. This property is an inverse property of Is Replaced By.</terms:description>
        <rdfs:comment xml:lang="en">A related resource that is supplanted, displaced, or superseded by the described resource.</rdfs:comment>
        <rdfs:isDefinedBy rdf:resource="http://purl.org/dc/terms/"/>
        <rdfs:label xml:lang="en">Replaces</rdfs:label>
    </rdf:Description>
    <rdf:Description rdf:about="http://purl.org/dc/terms/requires">
        <terms:description xml:lang="en">This property is intended to be used with non-literal values. This property is an inverse property of Is Required By.</terms:description>
        <rdfs:comment xml:lang="en">A related resource that is required by the described resource to support its function, delivery, or coherence.</rdfs:comment>
        <rdfs:isDefinedBy rdf:resource="http://purl.org/dc/terms/"/>
        <rdfs:label xml:lang="en">Requires</rdfs:label>
    </rdf:Description>
    <rdf:Description rdf:about="http://purl.org/dc/terms/rights">
        <dcam:rangeIncludes rdf:resource="http://purl.org/dc/terms/RightsStatement"/>
        <terms:description xml:lang="en">Typically, rights information includes a statement about various property rights associated with the resource, including intellectual property rights.  Recommended practice is to refer to a rights statement with a URI.  If this is not possible or feasible, a literal value (name, label, or short text) may be provided.</terms:description>
        <rdfs:comment xml:lang="en">Information about rights held in and over the resource.</rdfs:comment>
        <rdfs:isDefinedBy rdf:resource="http://purl.org/dc/terms/"/>
        <rdfs:label xml:lang="en">Rights</rdfs:label>
    </rdf:Description>
    <rdf:Description rdf:about="http://purl.org/dc/terms/source">
        <terms:description xml:lang="en">This property is intended to be used with non-literal values. The described resource may be derived from the related resource in whole or in part. Best practice is to identify the related resource by means of a URI or a string conforming to a formal identification system.</terms:description>
        <rdfs:comment xml:lang="en">A related resource from which the described resource is derived.</rdfs:comment>
        <rdfs:isDefinedBy rdf:resource="http://purl.org/dc/terms/"/>
        <rdfs:label xml:lang="en">Source</rdfs:label>
    </rdf:Description>
    <rdf:Description rdf:about="http://purl.org/dc/terms/spatial">
        <dcam:rangeIncludes rdf:resource="http://purl.org/dc/terms/Location"/>
        <rdfs:comment xml:lang="en">Spatial characteristics of the resource.</rdfs:comment>
        <rdfs:isDefinedBy rdf:resource="http://purl.org/dc/terms/"/>
        <rdfs:label xml:lang="en">Spatial Coverage</rdfs:label>
    </rdf:Description>
    <rdf:Description rdf:about="http://purl.org/dc/terms/subject">
        <terms:description xml:lang="en">Recommended practice is to refer to the subject with a URI. If this is not possible or feasible, a literal value that identifies the subject may be provided. Both should preferably refer to a subject in a controlled vocabulary.</terms:description>
        <rdfs:comment xml:lang="en">A topic of the resource.</rdfs:comment>
        <rdfs:isDefinedBy rdf:resource="http://purl.org/dc/terms/"/>
        <rdfs:label xml:lang="en">Subject</rdfs:label>
    </rdf:Description>
    <rdf:Description rdf:about="http://purl.org/dc/terms/tableOfContents">
        <rdfs:comment xml:lang="en">A list of subunits of the resource.</rdfs:comment>
        <rdfs:isDefinedBy rdf:resource="http://purl.org/dc/terms/"/>
        <rdfs:label xml:lang="en">Table Of Contents</rdfs:label>
    </rdf:Description>
    <rdf:Description rdf:about="http://purl.org/dc/terms/temporal">
        <dcam:rangeIncludes rdf:resource="http://purl.org/dc/terms/PeriodOfTime"/>
        <rdfs:comment xml:lang="en">Temporal characteristics of the resource.</rdfs:comment>
        <rdfs:isDefinedBy rdf:resource="http://purl.org/dc/terms/"/>
        <rdfs:label xml:lang="en">Temporal Coverage</rdfs:label>
    </rdf:Description>
    <rdf:Description rdf:about="http://purl.org/dc/terms/title">
        <rdfs:comment xml:lang="en">A name given to the resource.</rdfs:comment>
        <rdfs:isDefinedBy rdf:resource="http://purl.org/dc/terms/"/>
        <rdfs:label xml:lang="en">Title</rdfs:label>
    </rdf:Description>
    <rdf:Description rdf:about="http://purl.org/dc/terms/type">
        <terms:description xml:lang="en">Recommended practice is to use a controlled vocabulary such as the DCMI Type Vocabulary [[DCMI-TYPE](http://dublincore.org/documents/dcmi-type-vocabulary/)]. To describe the file format, physical medium, or dimensions of the resource, use the property Format.</terms:description>
        <rdfs:comment xml:lang="en">The nature or genre of the resource.</rdfs:comment>
        <rdfs:isDefinedBy rdf:resource="http://purl.org/dc/terms/"/>
        <rdfs:label xml:lang="en">Type</rdfs:label>
    </rdf:Description>
    <rdf:Description rdf:about="http://purl.org/dc/terms/valid">
        <terms:description xml:lang="en">Recommended practice is to describe the date, date/time, or period of time as recommended for the property Date, of which this is a subproperty.</terms:description>
        <rdfs:comment xml:lang="en">Date (often a range) of validity of a resource.</rdfs:comment>
        <rdfs:isDefinedBy rdf:resource="http://purl.org/dc/terms/"/>
        <rdfs:label xml:lang="en">Date Valid</rdfs:label>
    </rdf:Description>
    <rdf:Description rdf:about="http://www.w3.org/2004/02/skos/core#broadMatch">
        <rdfs:isDefinedBy rdf:resource="http://www.w3.org/2004/02/skos/core"/>
        <rdfs:label xml:lang="en">has broader match</rdfs:label>
        <skos:definition xml:lang="en">skos:broadMatch is used to state a hierarchical mapping link between two conceptual resources in different concept schemes.</skos:definition>
    </rdf:Description>
    <rdf:Description rdf:about="http://www.w3.org/2004/02/skos/core#broader">
        <rdfs:comment xml:lang="en">Broader concepts are typically rendered as parents in a concept hierarchy (tree).</rdfs:comment>
        <rdfs:isDefinedBy rdf:resource="http://www.w3.org/2004/02/skos/core"/>
        <rdfs:label xml:lang="en">has broader</rdfs:label>
        <skos:definition xml:lang="en">Relates a concept to a concept that is more general in meaning.</skos:definition>
        <skos:scopeNote xml:lang="en">By convention, skos:broader is only used to assert an immediate (i.e. direct) hierarchical link between two conceptual resources.</skos:scopeNote>
    </rdf:Description>
    <rdf:Description rdf:about="http://www.w3.org/2004/02/skos/core#hasTopConcept">
        <rdfs:isDefinedBy rdf:resource="http://www.w3.org/2004/02/skos/core"/>
        <rdfs:label xml:lang="en">has top concept</rdfs:label>
        <skos:definition xml:lang="en">Relates, by convention, a concept scheme to a concept which is topmost in the broader/narrower concept hierarchies for that scheme, providing an entry point to these hierarchies.</skos:definition>
    </rdf:Description>
    <rdf:Description rdf:about="http://www.w3.org/2004/02/skos/core#narrowMatch">
        <rdfs:isDefinedBy rdf:resource="http://www.w3.org/2004/02/skos/core"/>
        <rdfs:label xml:lang="en">has narrower match</rdfs:label>
        <skos:definition xml:lang="en">skos:narrowMatch is used to state a hierarchical mapping link between two conceptual resources in different concept schemes.</skos:definition>
    </rdf:Description>
    <rdf:Description rdf:about="http://www.w3.org/2004/02/skos/core#relatedMatch">
        <rdfs:isDefinedBy rdf:resource="http://www.w3.org/2004/02/skos/core"/>
        <rdfs:label xml:lang="en">has related match</rdfs:label>
        <skos:definition xml:lang="en">skos:relatedMatch is used to state an associative mapping link between two conceptual resources in different concept schemes.</skos:definition>
    </rdf:Description>
    <rdf:Description rdf:about="http://www.w3.org/ns/dcat#distribution">
        <rdfs:comment xml:lang="en">An available distribution of the dataset.</rdfs:comment>
        <rdfs:comment xml:lang="fr">Connecte un jeu de données à des distributions disponibles.</rdfs:comment>
        <rdfs:comment xml:lang="cs">Dostupná distribuce datové sady.</rdfs:comment>
        <rdfs:comment xml:lang="da">En tilgængelig repræsentation af datasættet.</rdfs:comment>
        <rdfs:comment xml:lang="es">Una distribución disponible del conjunto de datos.</rdfs:comment>
        <rdfs:comment xml:lang="it">Una distribuzione disponibile per il set di dati.</rdfs:comment>
        <rdfs:comment xml:lang="el">Συνδέει ένα σύνολο δεδομένων με μία από τις διαθέσιμες διανομές του.</rdfs:comment>
        <rdfs:comment xml:lang="ar">تربط قائمة البيانات بطريقة أو بشكل يسمح  الوصول الى البيانات</rdfs:comment>
        <rdfs:comment xml:lang="ja">データセットを、その利用可能な配信に接続します。</rdfs:comment>
        <rdfs:isDefinedBy rdf:resource="http://www.w3.org/TR/vocab-dcat/"/>
        <rdfs:label xml:lang="cs">distribuce</rdfs:label>
        <rdfs:label xml:lang="es">distribución</rdfs:label>
        <rdfs:label xml:lang="da">distribution</rdfs:label>
        <rdfs:label xml:lang="en">distribution</rdfs:label>
        <rdfs:label xml:lang="fr">distribution</rdfs:label>
        <rdfs:label xml:lang="it">distribuzione</rdfs:label>
        <rdfs:label xml:lang="el">διανομή</rdfs:label>
        <rdfs:label xml:lang="ar">توزيع</rdfs:label>
        <rdfs:label xml:lang="ja">データセット配信</rdfs:label>
        <skos:altLabel xml:lang="da">har distribution</skos:altLabel>
        <skos:altLabel xml:lang="en">has distribution</skos:altLabel>
        <skos:definition xml:lang="en">An available distribution of the dataset.</skos:definition>
        <skos:definition xml:lang="fr">Connecte un jeu de données à des distributions disponibles.</skos:definition>
        <skos:definition xml:lang="cs">Dostupná distribuce datové sady.</skos:definition>
        <skos:definition xml:lang="da">En tilgængelig repræsentation af datasættet.</skos:definition>
        <skos:definition xml:lang="es">Una distribución disponible del conjunto de datos.</skos:definition>
        <skos:definition xml:lang="it">Una distribuzione disponibile per il set di dati.</skos:definition>
        <skos:definition xml:lang="el">Συνδέει ένα σύνολο δεδομένων με μία από τις διαθέσιμες διανομές του.</skos:definition>
        <skos:definition xml:lang="ar">تربط قائمة البيانات بطريقة أو بشكل يسمح  الوصول الى البيانات</skos:definition>
        <skos:definition xml:lang="ja">データセットを、その利用可能な配信に接続します。</skos:definition>
        <skos:editorialNote xml:lang="en">Status: English Definition text modified by DCAT revision team, translations pending (except for Italian, Spanish and Czech).</skos:editorialNote>
    </rdf:Description>
    <rdf:Description rdf:about="http://www.w3.org/ns/dcat#hasCurrentVersion">
        <rdfs:comment xml:lang="es">Este recurso es más específico y versionado con contenido equivalente [PAV].</rdfs:comment>
        <rdfs:comment xml:lang="it">Per questa risorsa esiste una risorsa più specifica e versionata, ma con lo stesso contenuto.</rdfs:comment>
        <rdfs:comment xml:lang="en">This resource has a more specific, versioned resource with equivalent content [PAV].</rdfs:comment>
        <rdfs:isDefinedBy rdf:resource="https://www.w3.org/TR/vocab-dcat-3/"/>
        <rdfs:label xml:lang="it">ha versione attuale</rdfs:label>
        <rdfs:label xml:lang="en">has current version</rdfs:label>
        <rdfs:label xml:lang="es">tiene versión actual</rdfs:label>
        <skos:changeNote xml:lang="en">New property added in DCAT 3.</skos:changeNote>
        <skos:changeNote xml:lang="cs">Nová vlastnost přidaná ve verzi DCAT 3.</skos:changeNote>
        <skos:changeNote xml:lang="es">Nueva propiedad agregada in DCAT 3.</skos:changeNote>
        <skos:changeNote xml:lang="it">Nuova proprietà aggiunta in DCAT 3.</skos:changeNote>
        <skos:changeNote xml:lang="da">Ny egenskab tilføjet i DCAT 3.</skos:changeNote>
        <skos:definition xml:lang="es">Este recurso es más específico y versionado con contenido equivalente [PAV].</skos:definition>
        <skos:definition xml:lang="it">Per questa risorsa esiste una risorsa più specifica e versionata, ma con lo stesso contenuto.</skos:definition>
        <skos:definition xml:lang="en">This resource has a more specific, versioned resource with equivalent content [PAV].</skos:definition>
        <skos:scopeNote xml:lang="es">Esta propepiedad está destinada a relacionar un recurso no versionado o abstracto con una versión instantánea que puede usarse como un enlace permanente a la versión actual del recurso [PAV].</skos:scopeNote>
        <skos:scopeNote xml:lang="es">La noción de versión que se usa en esta propiedad está limitada a las versiones que resultan de revisiones de un recurso como parte de su ciclo de vida.</skos:scopeNote>
        <skos:scopeNote xml:lang="it">La nozione di versione usata da questa proprietà è limitata a versioni risultanti da revisioni a cui una risorsa è soggetta nel suo ciclo di vita.</skos:scopeNote>
        <skos:scopeNote xml:lang="it">Questa proprietà è usata per correlare una risorsa non versionata o astratta a un suo specifico snapshot che può essere usato come permalink per indicare la versione attuale del suo contenuto.</skos:scopeNote>
        <skos:scopeNote xml:lang="en">The notion of version used by this property is limited to versions resulting from revisions occurring to a resource as part of its life-cycle.</skos:scopeNote>
        <skos:scopeNote xml:lang="en">This property is intended for relating a non-versioned or abstract resource to a single snapshot that can be used as a permalink to indicate the current version of the content [PAV].</skos:scopeNote>
    </rdf:Description>
    <rdf:Description rdf:about="http://www.w3.org/ns/dcat#last">
        <rdfs:comment xml:lang="es">El último recurso en una colección ordenada o serie de recursos, al que el recurso pertenece.</rdfs:comment>
        <rdfs:comment xml:lang="it">L&apos;ultima risorsa in una collezione ordinata o in una serie di risorse, di cui la risorsa fa parte.</rdfs:comment>
        <rdfs:comment xml:lang="en">The last resource in an ordered collection or series of resources, to which the current resource belongs.</rdfs:comment>
        <rdfs:isDefinedBy rdf:resource="https://www.w3.org/TR/vocab-dcat-3/"/>
        <rdfs:label xml:lang="en">last</rdfs:label>
        <rdfs:label xml:lang="it">ultimo</rdfs:label>
        <rdfs:label xml:lang="es">último</rdfs:label>
        <skos:changeNote xml:lang="en">New property added in DCAT 3.</skos:changeNote>
        <skos:changeNote xml:lang="cs">Nová vlastnost přidaná ve verzi DCAT 3.</skos:changeNote>
        <skos:changeNote xml:lang="es">Nueva propiedad agregada in DCAT 3.</skos:changeNote>
        <skos:changeNote xml:lang="it">Nuova proprietà aggiunta in DCAT 3.</skos:changeNote>
        <skos:changeNote xml:lang="da">Ny egenskab tilføjet i DCAT 3.</skos:changeNote>
        <skos:definition xml:lang="es">El último recurso en una colección ordenada o serie de recursos, al que el recurso pertenece.</skos:definition>
        <skos:definition xml:lang="it">L&apos;ultima risorsa in una collezione ordinata o in una serie di risorse, di cui la risorsa fa parte.</skos:definition>
        <skos:definition xml:lang="en">The last resource in an ordered collection or series of resources, to which the current resource belongs.</skos:definition>
        <skos:scopeNote xml:lang="es">En DCAT esta propiedad se usa para recursos que pertenecen a una dcat:DatasetSeries.</skos:scopeNote>
        <skos:scopeNote xml:lang="it">In DCAT questa proprietà è usata per risorse che fanno parte di una dcat:DatasetSeries.</skos:scopeNote>
        <skos:scopeNote xml:lang="en">In DCAT this property is used for resources belonging to a dcat:DatasetSeries.</skos:scopeNote>
    </rdf:Description>
    <rdf:Description rdf:about="http://xmlns.com/foaf/0.1/homepage">
        <rdfs:comment xml:lang="es">Este axioma se necesita de manera que Protege cargue DCAT3 sin problemas.</rdfs:comment>
        <rdfs:comment xml:lang="en">This axiom needed so that Protege loads DCAT 3 without errors.</rdfs:comment>
    </rdf:Description>
</rdf:RDF>



<!-- Generated by the OWL API (version 5.1.18) https://github.com/owlcs/owlapi/ -->


